<?xml version="1.0" encoding="utf-8"?>
<rdf:RDF
   xmlns:dc="http://purl.org/dc/elements/1.1/"
   xmlns:dct="http://purl.org/dc/terms/"
   xmlns:rdf="http://www.w3.org/1999/02/22-rdf-syntax-ns#"
   xmlns:schema="https://schema.org/"
   xmlns:skos="http://www.w3.org/2004/02/skos/core#"
>
  <rdf:Description rdf:about="https://doi.org/10.6069/uwlswd.2skv-5f55#v">
    <rdf:type rdf:resource="http://www.w3.org/2004/02/skos/core#Concept"/>
    <skos:inScheme rdf:resource="https://doi.org/10.6069/uwlswd.2skv-5f55"/>
    <skos:prefLabel xml:lang="en">8x10 in. or 21x26 cm. transparency</skos:prefLabel>
    <skos:definition xml:lang="en">Dimensions of the transparency are either 8x10 in. or 21x26
         cm.</skos:definition>
    <skos:notation xml:lang="en">v</skos:notation>
  </rdf:Description>
  <rdf:Description rdf:about="https://doi.org/10.6069/uwlswd.2skv-5f55#a">
    <rdf:type rdf:resource="http://www.w3.org/2004/02/skos/core#Concept"/>
    <skos:inScheme rdf:resource="https://doi.org/10.6069/uwlswd.2skv-5f55"/>
    <skos:prefLabel xml:lang="en">standard 8 mm. film width</skos:prefLabel>
    <skos:definition xml:lang="en">Width of the film is standard 8 mm.</skos:definition>
    <skos:scopeNote xml:lang="en">Includes film termed Mauer 8 mm.</skos:scopeNote>
    <skos:notation xml:lang="en">a</skos:notation>
  </rdf:Description>
  <rdf:Description rdf:about="https://doi.org/10.6069/uwlswd.2skv-5f55#f">
    <rdf:type rdf:resource="http://www.w3.org/2004/02/skos/core#Concept"/>
    <skos:inScheme rdf:resource="https://doi.org/10.6069/uwlswd.2skv-5f55"/>
    <skos:prefLabel xml:lang="en">35 mm. film width</skos:prefLabel>
    <skos:definition xml:lang="en">Width of the film is 35 mm.</skos:definition>
    <skos:notation xml:lang="en">f</skos:notation>
  </rdf:Description>
  <rdf:Description rdf:about="https://doi.org/10.6069/uwlswd.2skv-5f55#y">
    <rdf:type rdf:resource="http://www.w3.org/2004/02/skos/core#Concept"/>
    <skos:inScheme rdf:resource="https://doi.org/10.6069/uwlswd.2skv-5f55"/>
    <skos:prefLabel xml:lang="en">7x7 in. or 18x18 cm. transparency</skos:prefLabel>
    <skos:definition xml:lang="en">Dimensions of the transparency are either 7x7 in. or 18x18
         cm.</skos:definition>
    <skos:notation xml:lang="en">y</skos:notation>
  </rdf:Description>
  <rdf:Description rdf:about="https://doi.org/10.6069/uwlswd.2skv-5f55#d">
    <rdf:type rdf:resource="http://www.w3.org/2004/02/skos/core#Concept"/>
    <skos:inScheme rdf:resource="https://doi.org/10.6069/uwlswd.2skv-5f55"/>
    <skos:prefLabel xml:lang="en">16 mm. film width</skos:prefLabel>
    <skos:definition xml:lang="en">Width of the film is 16 mm.</skos:definition>
    <skos:notation xml:lang="en">d</skos:notation>
  </rdf:Description>
  <rdf:Description rdf:about="https://doi.org/10.6069/uwlswd.2skv-5f55#ux">
    <rdf:type rdf:resource="http://www.w3.org/2004/02/skos/core#Concept"/>
    <skos:inScheme rdf:resource="https://doi.org/10.6069/uwlswd.2skv-5f55"/>
    <skos:prefLabel xml:lang="en">7x7 in. or 18x18 cm. [obsolete]</skos:prefLabel>
    <skos:notation xml:lang="en">u</skos:notation>
  </rdf:Description>
  <rdf:Description rdf:about="https://doi.org/10.6069/uwlswd.2skv-5f55#s">
    <rdf:type rdf:resource="http://www.w3.org/2004/02/skos/core#Concept"/>
    <skos:inScheme rdf:resource="https://doi.org/10.6069/uwlswd.2skv-5f55"/>
    <skos:prefLabel xml:lang="en">4x5 in. or 10x13 cm. transparency</skos:prefLabel>
    <skos:definition xml:lang="en">Dimensions of the transparency are either 4x5 in. or 10x13
         cm.</skos:definition>
    <skos:notation xml:lang="en">s</skos:notation>
  </rdf:Description>
  <rdf:Description rdf:about="https://doi.org/10.6069/uwlswd.2skv-5f55">
    <rdf:type rdf:resource="http://www.w3.org/2004/02/skos/core#ConceptScheme"/>
    <dct:type rdf:resource="http://purl.org/dc/dcmitype/Dataset"/>
    <dct:title xml:lang="en">Projected graphic: dimensions</dct:title>
    <dct:alternative xml:lang="en">MARC21 007/07 values for projected graphics expressed using
         RDF</dct:alternative>
    <dct:description xml:lang="en">Width or dimensions of the projected graphic item. Width is
         given for filmstrips. Height and width are given for slides and
         transparencies.</dct:description>
    <schema:disambiguatingDescription>SKOS Concept Scheme for MARC 00X
         Values</schema:disambiguatingDescription>
    <dct:publisher rdf:resource="http://viaf.org/viaf/139541794"/>
    <dct:source rdf:resource="https://www.loc.gov/marc/bibliographic/bd007.html"/>
    <dct:source rdf:resource="http://marc21rdf.info"/>
    <dct:provenance rdf:resource="https://doi.org/10.6069/uwlswd.2e2b-y833"/>
    <dct:creator rdf:resource="http://viaf.org/viaf/139541794"/>
    <dct:contributor rdf:resource="http://viaf.org/viaf/151962300"/>
    <dct:issued>2024</dct:issued>
    <dc:contributor xml:lang="en">Metadata Management Associates</dc:contributor>
    <dc:language>en</dc:language>
    <dct:license rdf:resource="http://creativecommons.org/publicdomain/zero/1.0"/>
    <schema:version>1-0-0</schema:version>
    <dct:format rdf:resource="http://www.w3.org/ns/formats/RDF_XML"/>
  </rdf:Description>
  <rdf:Description rdf:about="https://doi.org/10.6069/uwlswd.2skv-5f55#b">
    <rdf:type rdf:resource="http://www.w3.org/2004/02/skos/core#Concept"/>
    <skos:inScheme rdf:resource="https://doi.org/10.6069/uwlswd.2skv-5f55"/>
    <skos:prefLabel xml:lang="en">super 8 mm./single 8 mm. film width</skos:prefLabel>
    <skos:definition xml:lang="en">Width of the film is super 8 mm.</skos:definition>
    <skos:scopeNote xml:lang="en">Single 8 mm. film is a Japanese equivalent of super 8 mm.
         film.</skos:scopeNote>
    <skos:notation xml:lang="en">b</skos:notation>
  </rdf:Description>
  <rdf:Description rdf:about="https://doi.org/10.6069/uwlswd.2skv-5f55#e">
    <rdf:type rdf:resource="http://www.w3.org/2004/02/skos/core#Concept"/>
    <skos:inScheme rdf:resource="https://doi.org/10.6069/uwlswd.2skv-5f55"/>
    <skos:prefLabel xml:lang="en">28 mm. film width</skos:prefLabel>
    <skos:definition xml:lang="en">Width of the film is 28 mm.</skos:definition>
    <skos:notation xml:lang="en">e</skos:notation>
  </rdf:Description>
  <rdf:Description rdf:about="https://doi.org/10.6069/uwlswd.2skv-5f55#w">
    <rdf:type rdf:resource="http://www.w3.org/2004/02/skos/core#Concept"/>
    <skos:inScheme rdf:resource="https://doi.org/10.6069/uwlswd.2skv-5f55"/>
    <skos:prefLabel xml:lang="en">9x9 in. or 23x23 cm. transparency</skos:prefLabel>
    <skos:definition xml:lang="en">Dimensions of the transparency are either 9x9 in. or 23x23
         cm.</skos:definition>
    <skos:notation xml:lang="en">w</skos:notation>
  </rdf:Description>
  <rdf:Description rdf:about="https://doi.org/10.6069/uwlswd.2skv-5f55#k">
    <rdf:type rdf:resource="http://www.w3.org/2004/02/skos/core#Concept"/>
    <skos:inScheme rdf:resource="https://doi.org/10.6069/uwlswd.2skv-5f55"/>
    <skos:prefLabel xml:lang="en">2 1/4 x 2 1/4 in. or 6x6 cm. slide</skos:prefLabel>
    <skos:definition xml:lang="en">Dimensions of the slide in its mounting are either 2 1/4 x 2
         1/4 in. or 6x6 cm.</skos:definition>
    <skos:notation xml:lang="en">k</skos:notation>
  </rdf:Description>
  <rdf:Description rdf:about="https://doi.org/10.6069/uwlswd.2skv-5f55#g">
    <rdf:type rdf:resource="http://www.w3.org/2004/02/skos/core#Concept"/>
    <skos:inScheme rdf:resource="https://doi.org/10.6069/uwlswd.2skv-5f55"/>
    <skos:prefLabel xml:lang="en">70 mm. film width</skos:prefLabel>
    <skos:definition xml:lang="en">Width of the film is 70 mm.</skos:definition>
    <skos:notation xml:lang="en">g</skos:notation>
  </rdf:Description>
  <rdf:Description rdf:about="https://doi.org/10.6069/uwlswd.2skv-5f55#t">
    <rdf:type rdf:resource="http://www.w3.org/2004/02/skos/core#Concept"/>
    <skos:inScheme rdf:resource="https://doi.org/10.6069/uwlswd.2skv-5f55"/>
    <skos:prefLabel xml:lang="en">5x7 in. or 13x18 cm. transparency</skos:prefLabel>
    <skos:definition xml:lang="en">Dimensions of the transparency are either 5x7 in. or 13x18
         cm.</skos:definition>
    <skos:notation xml:lang="en">t</skos:notation>
  </rdf:Description>
  <rdf:Description rdf:about="https://doi.org/10.6069/uwlswd.2skv-5f55#x">
    <rdf:type rdf:resource="http://www.w3.org/2004/02/skos/core#Concept"/>
    <skos:inScheme rdf:resource="https://doi.org/10.6069/uwlswd.2skv-5f55"/>
    <skos:prefLabel xml:lang="en">10x10 in. or 26x26 cm. transparency</skos:prefLabel>
    <skos:definition xml:lang="en">Dimensions of the transparency are either 10x10 in. or 26x26
         cm.</skos:definition>
    <skos:notation xml:lang="en">x</skos:notation>
  </rdf:Description>
  <rdf:Description rdf:about="https://doi.org/10.6069/uwlswd.2skv-5f55#j">
    <rdf:type rdf:resource="http://www.w3.org/2004/02/skos/core#Concept"/>
    <skos:inScheme rdf:resource="https://doi.org/10.6069/uwlswd.2skv-5f55"/>
    <skos:prefLabel xml:lang="en">2x2 in. or 5x5 cm. slide</skos:prefLabel>
    <skos:definition xml:lang="en">Dimensions of the slide in its mounting are either 2x2 in. or
         5x5 cm.</skos:definition>
    <skos:notation xml:lang="en">j</skos:notation>
  </rdf:Description>
  <rdf:Description rdf:about="https://doi.org/10.6069/uwlswd.2skv-5f55#u">
    <rdf:type rdf:resource="http://www.w3.org/2004/02/skos/core#Concept"/>
    <skos:inScheme rdf:resource="https://doi.org/10.6069/uwlswd.2skv-5f55"/>
    <skos:prefLabel xml:lang="en">unknown</skos:prefLabel>
    <skos:definition xml:lang="en">Dimensions are not known.</skos:definition>
    <skos:notation xml:lang="en">u</skos:notation>
  </rdf:Description>
  <rdf:Description rdf:about="https://doi.org/10.6069/uwlswd.2skv-5f55#z">
    <rdf:type rdf:resource="http://www.w3.org/2004/02/skos/core#Concept"/>
    <skos:inScheme rdf:resource="https://doi.org/10.6069/uwlswd.2skv-5f55"/>
    <skos:prefLabel xml:lang="en">other</skos:prefLabel>
    <skos:definition xml:lang="en">Dimensions other than standard 8 mm. film width, super 8
         mm./single 8 mm. film width, 9.5 mm. film width, 16 mm. film width, 28 mm. film width, 35
         mm. film width, 70 mm. film width, 2x2 in. or 5x5 cm. slide, 2 1/4 x 2 1/4 in. or 6x6 cm.
         slide, 4x5 in. or 10x13 cm. transparency, 5x7 in. or 13x18 cm. transparency, 8x10 in. or
         21x26 cm. transparency, 9x9 in. or 23x23 cm. transparency, 10x10 in. or 26x26 cm.
         transparency, or 7x7 in. or 18x18 cm. transparency.</skos:definition>
    <skos:notation xml:lang="en">z</skos:notation>
  </rdf:Description>
  <rdf:Description rdf:about="https://doi.org/10.6069/uwlswd.2skv-5f55#yx">
    <rdf:type rdf:resource="http://www.w3.org/2004/02/skos/core#Concept"/>
    <skos:inScheme rdf:resource="https://doi.org/10.6069/uwlswd.2skv-5f55"/>
    <skos:prefLabel xml:lang="en">unknown [obsolete]</skos:prefLabel>
    <skos:notation xml:lang="en">y</skos:notation>
  </rdf:Description>
  <rdf:Description rdf:about="https://doi.org/10.6069/uwlswd.2skv-5f55#c">
    <rdf:type rdf:resource="http://www.w3.org/2004/02/skos/core#Concept"/>
    <skos:inScheme rdf:resource="https://doi.org/10.6069/uwlswd.2skv-5f55"/>
    <skos:prefLabel xml:lang="en">9.5 mm. film width</skos:prefLabel>
    <skos:definition xml:lang="en">Width of the film is 9.5 mm.</skos:definition>
    <skos:notation xml:lang="en">c</skos:notation>
  </rdf:Description>
</rdf:RDF>
