@prefix dc: <http://purl.org/dc/elements/1.1/> .
@prefix dct: <http://purl.org/dc/terms/> .
@prefix schema: <https://schema.org/> .
@prefix skos: <http://www.w3.org/2004/02/skos/core#> .

<https://doi.org/10.6069/uwlswd.2skv-5f55#a> a skos:Concept ;
    skos:definition "Width of the film is standard 8 mm."@en ;
    skos:inScheme <https://doi.org/10.6069/uwlswd.2skv-5f55> ;
    skos:notation "a" ;
    skos:prefLabel "standard 8 mm. film width"@en ;
    skos:scopeNote "Includes film termed Mauer 8 mm."@en .

<https://doi.org/10.6069/uwlswd.2skv-5f55#b> a skos:Concept ;
    skos:definition "Width of the film is super 8 mm."@en ;
    skos:inScheme <https://doi.org/10.6069/uwlswd.2skv-5f55> ;
    skos:notation "b" ;
    skos:prefLabel "super 8 mm./single 8 mm. film width"@en ;
    skos:scopeNote """Single 8 mm. film is a Japanese equivalent of super 8 mm.
         film."""@en .

<https://doi.org/10.6069/uwlswd.2skv-5f55#c> a skos:Concept ;
    skos:definition "Width of the film is 9.5 mm."@en ;
    skos:inScheme <https://doi.org/10.6069/uwlswd.2skv-5f55> ;
    skos:notation "c" ;
    skos:prefLabel "9.5 mm. film width"@en .

<https://doi.org/10.6069/uwlswd.2skv-5f55#d> a skos:Concept ;
    skos:definition "Width of the film is 16 mm."@en ;
    skos:inScheme <https://doi.org/10.6069/uwlswd.2skv-5f55> ;
    skos:notation "d" ;
    skos:prefLabel "16 mm. film width"@en .

<https://doi.org/10.6069/uwlswd.2skv-5f55#e> a skos:Concept ;
    skos:definition "Width of the film is 28 mm."@en ;
    skos:inScheme <https://doi.org/10.6069/uwlswd.2skv-5f55> ;
    skos:notation "e" ;
    skos:prefLabel "28 mm. film width"@en .

<https://doi.org/10.6069/uwlswd.2skv-5f55#f> a skos:Concept ;
    skos:definition "Width of the film is 35 mm."@en ;
    skos:inScheme <https://doi.org/10.6069/uwlswd.2skv-5f55> ;
    skos:notation "f" ;
    skos:prefLabel "35 mm. film width"@en .

<https://doi.org/10.6069/uwlswd.2skv-5f55#g> a skos:Concept ;
    skos:definition "Width of the film is 70 mm."@en ;
    skos:inScheme <https://doi.org/10.6069/uwlswd.2skv-5f55> ;
    skos:notation "g" ;
    skos:prefLabel "70 mm. film width"@en .

<https://doi.org/10.6069/uwlswd.2skv-5f55#j> a skos:Concept ;
    skos:definition """Dimensions of the slide in its mounting are either 2x2 in. or
         5x5 cm."""@en ;
    skos:inScheme <https://doi.org/10.6069/uwlswd.2skv-5f55> ;
    skos:notation "j" ;
    skos:prefLabel "2x2 in. or 5x5 cm. slide"@en .

<https://doi.org/10.6069/uwlswd.2skv-5f55#k> a skos:Concept ;
    skos:definition """Dimensions of the slide in its mounting are either 2 1/4 x 2
         1/4 in. or 6x6 cm."""@en ;
    skos:inScheme <https://doi.org/10.6069/uwlswd.2skv-5f55> ;
    skos:notation "k" ;
    skos:prefLabel "2 1/4 x 2 1/4 in. or 6x6 cm. slide"@en .

<https://doi.org/10.6069/uwlswd.2skv-5f55#s> a skos:Concept ;
    skos:definition """Dimensions of the transparency are either 4x5 in. or 10x13
         cm."""@en ;
    skos:inScheme <https://doi.org/10.6069/uwlswd.2skv-5f55> ;
    skos:notation "s" ;
    skos:prefLabel "4x5 in. or 10x13 cm. transparency"@en .

<https://doi.org/10.6069/uwlswd.2skv-5f55#t> a skos:Concept ;
    skos:definition """Dimensions of the transparency are either 5x7 in. or 13x18
         cm."""@en ;
    skos:inScheme <https://doi.org/10.6069/uwlswd.2skv-5f55> ;
    skos:notation "t" ;
    skos:prefLabel "5x7 in. or 13x18 cm. transparency"@en .

<https://doi.org/10.6069/uwlswd.2skv-5f55#u> a skos:Concept ;
    skos:definition "Dimensions are not known."@en ;
    skos:inScheme <https://doi.org/10.6069/uwlswd.2skv-5f55> ;
    skos:notation "u" ;
    skos:prefLabel "unknown"@en .

<https://doi.org/10.6069/uwlswd.2skv-5f55#ux> a skos:Concept ;
    skos:inScheme <https://doi.org/10.6069/uwlswd.2skv-5f55> ;
    skos:notation "u" ;
    skos:prefLabel "7x7 in. or 18x18 cm. [obsolete]"@en .

<https://doi.org/10.6069/uwlswd.2skv-5f55#v> a skos:Concept ;
    skos:definition """Dimensions of the transparency are either 8x10 in. or 21x26
         cm."""@en ;
    skos:inScheme <https://doi.org/10.6069/uwlswd.2skv-5f55> ;
    skos:notation "v" ;
    skos:prefLabel "8x10 in. or 21x26 cm. transparency"@en .

<https://doi.org/10.6069/uwlswd.2skv-5f55#w> a skos:Concept ;
    skos:definition """Dimensions of the transparency are either 9x9 in. or 23x23
         cm."""@en ;
    skos:inScheme <https://doi.org/10.6069/uwlswd.2skv-5f55> ;
    skos:notation "w" ;
    skos:prefLabel "9x9 in. or 23x23 cm. transparency"@en .

<https://doi.org/10.6069/uwlswd.2skv-5f55#x> a skos:Concept ;
    skos:definition """Dimensions of the transparency are either 10x10 in. or 26x26
         cm."""@en ;
    skos:inScheme <https://doi.org/10.6069/uwlswd.2skv-5f55> ;
    skos:notation "x" ;
    skos:prefLabel "10x10 in. or 26x26 cm. transparency"@en .

<https://doi.org/10.6069/uwlswd.2skv-5f55#y> a skos:Concept ;
    skos:definition """Dimensions of the transparency are either 7x7 in. or 18x18
         cm."""@en ;
    skos:inScheme <https://doi.org/10.6069/uwlswd.2skv-5f55> ;
    skos:notation "y" ;
    skos:prefLabel "7x7 in. or 18x18 cm. transparency"@en .

<https://doi.org/10.6069/uwlswd.2skv-5f55#yx> a skos:Concept ;
    skos:inScheme <https://doi.org/10.6069/uwlswd.2skv-5f55> ;
    skos:notation "y" ;
    skos:prefLabel "unknown [obsolete]"@en .

<https://doi.org/10.6069/uwlswd.2skv-5f55#z> a skos:Concept ;
    skos:definition """Dimensions other than standard 8 mm. film width, super 8
         mm./single 8 mm. film width, 9.5 mm. film width, 16 mm. film width, 28 mm. film width, 35
         mm. film width, 70 mm. film width, 2x2 in. or 5x5 cm. slide, 2 1/4 x 2 1/4 in. or 6x6 cm.
         slide, 4x5 in. or 10x13 cm. transparency, 5x7 in. or 13x18 cm. transparency, 8x10 in. or
         21x26 cm. transparency, 9x9 in. or 23x23 cm. transparency, 10x10 in. or 26x26 cm.
         transparency, or 7x7 in. or 18x18 cm. transparency."""@en ;
    skos:inScheme <https://doi.org/10.6069/uwlswd.2skv-5f55> ;
    skos:notation "z" ;
    skos:prefLabel "other"@en .

<https://doi.org/10.6069/uwlswd.2skv-5f55> a skos:ConceptScheme ;
    dc:contributor "Metadata Management Associates"@en ;
    dc:language "en" ;
    dct:alternative """MARC21 007/07 values for projected graphics expressed using
         RDF"""@en ;
    dct:contributor <http://viaf.org/viaf/151962300> ;
    dct:creator <http://viaf.org/viaf/139541794> ;
    dct:description """Width or dimensions of the projected graphic item. Width is
         given for filmstrips. Height and width are given for slides and
         transparencies."""@en ;
    dct:format <http://www.w3.org/ns/formats/Turtle> ;
    dct:hasFormat <https://uwlib-cams.github.io/uwlswd_vocabs_marc_007/projected_graphic_dimensions/projected_graphic_dimensions.html>,
        <https://uwlib-cams.github.io/uwlswd_vocabs_marc_007/projected_graphic_dimensions/projected_graphic_dimensions.jsonld>,
        <https://uwlib-cams.github.io/uwlswd_vocabs_marc_007/projected_graphic_dimensions/projected_graphic_dimensions.nt>,
        <https://uwlib-cams.github.io/uwlswd_vocabs_marc_007/projected_graphic_dimensions/projected_graphic_dimensions.rdf> ;
    dct:issued "2024" ;
    dct:license <http://creativecommons.org/publicdomain/zero/1.0> ;
    dct:provenance <https://doi.org/10.6069/uwlswd.2e2b-y833#marc00Xvalues> ;
    dct:publisher <http://viaf.org/viaf/139541794> ;
    dct:source <http://marc21rdf.info>,
        <https://www.loc.gov/marc/bibliographic/bd007.html> ;
    dct:title "Projected graphic: dimensions"@en ;
    dct:type <http://purl.org/dc/dcmitype/Dataset> ;
    schema:disambiguatingDescription """SKOS Concept Scheme for MARC 00X
         Values"""@en ;
    schema:version "1-0-0" .

