@prefix dc: <http://purl.org/dc/elements/1.1/> .
@prefix dct: <http://purl.org/dc/terms/> .
@prefix schema: <https://schema.org/> .
@prefix skos: <http://www.w3.org/2004/02/skos/core#> .

<https://doi.org/10.6069/uwlswd.pm5s-5m12#h> a skos:Concept ;
    skos:definition """Vertical cutting, with no lateral information intended for
         reproduction."""@en ;
    skos:inScheme <https://doi.org/10.6069/uwlswd.pm5s-5m12> ;
    skos:notation "h" ;
    skos:prefLabel "hill-and-dale cutting"@en ;
    skos:scopeNote """All cylinders and some early discs have this
         cutting."""@en .

<https://doi.org/10.6069/uwlswd.pm5s-5m12#l> a skos:Concept ;
    skos:definition """Cutting containing lateral information intended for
         reproduction. Such discs may also have vertical components intended for
         reproduction."""@en ;
    skos:inScheme <https://doi.org/10.6069/uwlswd.pm5s-5m12> ;
    skos:notation "l" ;
    skos:prefLabel "lateral or combined cutting"@en ;
    skos:scopeNote """Most contemporary discs (i.e., all quadraphonic discs and nearly
         all stereophonic discs) contain both vertical and laterial information. Monographic discs
         are normally lateral only."""@en .

<https://doi.org/10.6069/uwlswd.pm5s-5m12#n> a skos:Concept ;
    skos:definition "Item is not a disc or a cylinder."@en ;
    skos:inScheme <https://doi.org/10.6069/uwlswd.pm5s-5m12> ;
    skos:notation "n" ;
    skos:prefLabel "not applicable"@en ;
    skos:scopeNote """Includes compact audio discs as they are pitted rather than
         cut."""@en .

<https://doi.org/10.6069/uwlswd.pm5s-5m12#u> a skos:Concept ;
    skos:definition "Kind of cutting is not known."@en ;
    skos:inScheme <https://doi.org/10.6069/uwlswd.pm5s-5m12> ;
    skos:notation "u" ;
    skos:prefLabel "unknown"@en .

<https://doi.org/10.6069/uwlswd.pm5s-5m12> a skos:ConceptScheme ;
    dc:contributor "Metadata Management Associates"@en ;
    dc:language "en" ;
    dct:alternative """MARC21 007/11 values for sound recordings expressed using
         RDF"""@en ;
    dct:contributor <http://viaf.org/viaf/151962300> ;
    dct:creator <http://viaf.org/viaf/139541794> ;
    dct:description """Kind of cutting of the grooves used on a
         disc."""@en ;
    dct:format <http://www.w3.org/ns/formats/Turtle> ;
    dct:hasFormat <https://uwlib-cams.github.io/uwlswd_vocabs_marc_007/sound_recording_kind_of_cutting/sound_recording_kind_of_cutting.html>,
        <https://uwlib-cams.github.io/uwlswd_vocabs_marc_007/sound_recording_kind_of_cutting/sound_recording_kind_of_cutting.jsonld>,
        <https://uwlib-cams.github.io/uwlswd_vocabs_marc_007/sound_recording_kind_of_cutting/sound_recording_kind_of_cutting.nt>,
        <https://uwlib-cams.github.io/uwlswd_vocabs_marc_007/sound_recording_kind_of_cutting/sound_recording_kind_of_cutting.rdf> ;
    dct:issued "2024" ;
    dct:license <http://creativecommons.org/publicdomain/zero/1.0> ;
    dct:provenance <https://doi.org/10.6069/uwlswd.2e2b-y833#marc00Xvalues> ;
    dct:publisher <http://viaf.org/viaf/139541794> ;
    dct:source <http://marc21rdf.info>,
        <https://www.loc.gov/marc/bibliographic/bd007.html> ;
    dct:title "Sound recording: kind of cutting"@en ;
    dct:type <http://purl.org/dc/dcmitype/Dataset> ;
    schema:disambiguatingDescription """SKOS Concept Scheme for MARC 00X
         Values"""@en ;
    schema:version "1-0-0" .

