@prefix dc: <http://purl.org/dc/elements/1.1/> .
@prefix dct: <http://purl.org/dc/terms/> .
@prefix schema: <https://schema.org/> .
@prefix skos: <http://www.w3.org/2004/02/skos/core#> .

<https://doi.org/10.6069/uwlswd.ry8c-5814#a> a skos:Concept ;
    skos:definition """Eye-readable print with braille interleaved or
         embossed."""@en ;
    skos:inScheme <https://doi.org/10.6069/uwlswd.ry8c-5814> ;
    skos:notation "a" ;
    skos:prefLabel "print/braille"@en .

<https://doi.org/10.6069/uwlswd.ry8c-5814#b> a skos:Concept ;
    skos:definition """Item is jumbo or enlarged braille, which is used for braille
         students and braille readers with reduced tactile sensitivity."""@en ;
    skos:inScheme <https://doi.org/10.6069/uwlswd.ry8c-5814> ;
    skos:notation "b" ;
    skos:prefLabel "jumbo or enlarged braille"@en .

<https://doi.org/10.6069/uwlswd.ry8c-5814#n> a skos:Concept ;
    skos:definition "Not braille."@en ;
    skos:inScheme <https://doi.org/10.6069/uwlswd.ry8c-5814> ;
    skos:notation "n" ;
    skos:prefLabel "not applicable"@en .

<https://doi.org/10.6069/uwlswd.ry8c-5814#u> a skos:Concept ;
    skos:definition """Special physical characteristics are not
         known."""@en ;
    skos:inScheme <https://doi.org/10.6069/uwlswd.ry8c-5814> ;
    skos:notation "u" ;
    skos:prefLabel "unknown"@en .

<https://doi.org/10.6069/uwlswd.ry8c-5814#z> a skos:Concept ;
    skos:definition """Specific physical characteristics other than print/braille, or
         jumbo or enlarged braille."""@en ;
    skos:inScheme <https://doi.org/10.6069/uwlswd.ry8c-5814> ;
    skos:notation "z" ;
    skos:prefLabel "other"@en .

<https://doi.org/10.6069/uwlswd.ry8c-5814> a skos:ConceptScheme ;
    dc:contributor "Metadata Management Associates"@en ;
    dc:language "en" ;
    dct:alternative """MARC21 007/09 values for tactile material expressed using
         RDF"""@en ;
    dct:contributor <http://viaf.org/viaf/151962300> ;
    dct:creator <http://viaf.org/viaf/139541794> ;
    dct:description """Special physical characteristics about the
         braille."""@en ;
    dct:format <http://www.w3.org/ns/formats/Turtle> ;
    dct:hasFormat <https://uwlib-cams.github.io/uwlswd_vocabs_marc_007/tactile_material_special_physical_characteristics/tactile_material_special_physical_characteristics.html>,
        <https://uwlib-cams.github.io/uwlswd_vocabs_marc_007/tactile_material_special_physical_characteristics/tactile_material_special_physical_characteristics.jsonld>,
        <https://uwlib-cams.github.io/uwlswd_vocabs_marc_007/tactile_material_special_physical_characteristics/tactile_material_special_physical_characteristics.nt>,
        <https://uwlib-cams.github.io/uwlswd_vocabs_marc_007/tactile_material_special_physical_characteristics/tactile_material_special_physical_characteristics.rdf> ;
    dct:issued "2024" ;
    dct:license <http://creativecommons.org/publicdomain/zero/1.0> ;
    dct:provenance <https://doi.org/10.6069/uwlswd.2e2b-y833#marc00Xvalues> ;
    dct:publisher <http://viaf.org/viaf/139541794> ;
    dct:source <http://marc21rdf.info>,
        <https://www.loc.gov/marc/bibliographic/bd007.html> ;
    dct:title "Tactile material: special physical characteristics"@en ;
    dct:type <http://purl.org/dc/dcmitype/Dataset> ;
    schema:disambiguatingDescription """SKOS Concept Scheme for MARC 00X
         Values"""@en ;
    schema:version "1-0-0" .

