<?xml version="1.0" encoding="utf-8"?>
<rdf:RDF
   xmlns:dc="http://purl.org/dc/elements/1.1/"
   xmlns:dct="http://purl.org/dc/terms/"
   xmlns:rdf="http://www.w3.org/1999/02/22-rdf-syntax-ns#"
   xmlns:schema="https://schema.org/"
   xmlns:skos="http://www.w3.org/2004/02/skos/core#"
>
  <rdf:Description rdf:about="https://doi.org/10.6069/uwlswd.enb6-8r41#s">
    <rdf:type rdf:resource="http://www.w3.org/2004/02/skos/core#Concept"/>
    <skos:inScheme rdf:resource="https://doi.org/10.6069/uwlswd.enb6-8r41"/>
    <skos:prefLabel xml:lang="en">sound cassette</skos:prefLabel>
    <skos:definition xml:lang="en">A container holding a narrow, usually 1/8 inch, sound tape on
         two reels, one to feed (and rewind) and the other to take up the sound
         tape.</skos:definition>
    <skos:notation>s</skos:notation>
  </rdf:Description>
  <rdf:Description rdf:about="https://doi.org/10.6069/uwlswd.enb6-8r41#d">
    <rdf:type rdf:resource="http://www.w3.org/2004/02/skos/core#Concept"/>
    <skos:inScheme rdf:resource="https://doi.org/10.6069/uwlswd.enb6-8r41"/>
    <skos:prefLabel xml:lang="en">sound disc</skos:prefLabel>
    <skos:definition xml:lang="en">Thin circular objects that vary in diameter (e.g., 7 in., 10
         in., 12 in.), on which sound waves, recorded as modulations or pulses, are incised or
         indented. Compact audio discs are typically 4 3/4 in. in diameter.</skos:definition>
    <skos:notation>d</skos:notation>
  </rdf:Description>
  <rdf:Description rdf:about="https://doi.org/10.6069/uwlswd.enb6-8r41">
    <rdf:type rdf:resource="http://www.w3.org/2004/02/skos/core#ConceptScheme"/>
    <dct:type rdf:resource="http://purl.org/dc/dcmitype/Dataset"/>
    <dct:title xml:lang="en">Sound recording: specific material designation</dct:title>
    <dct:alternative xml:lang="en">MARC21 007/01 values for sound recordings expressed using
         RDF</dct:alternative>
    <dct:description xml:lang="en">Special class of sound recording to which the item belongs
         (e.g., a cylinder).</dct:description>
    <schema:disambiguatingDescription xml:lang="en">SKOS Concept Scheme for MARC 00X
         Values</schema:disambiguatingDescription>
    <dct:publisher rdf:resource="http://viaf.org/viaf/139541794"/>
    <dct:source rdf:resource="https://www.loc.gov/marc/bibliographic/bd007.html"/>
    <dct:source rdf:resource="http://marc21rdf.info"/>
    <dct:provenance rdf:resource="https://doi.org/10.6069/uwlswd.2e2b-y833#marc00Xvalues"/>
    <dct:creator rdf:resource="http://viaf.org/viaf/139541794"/>
    <dct:contributor rdf:resource="http://viaf.org/viaf/151962300"/>
    <dct:issued>2024</dct:issued>
    <dc:contributor xml:lang="en">Metadata Management Associates</dc:contributor>
    <dc:language>en</dc:language>
    <dct:license rdf:resource="http://creativecommons.org/publicdomain/zero/1.0"/>
    <schema:version>1-0-0</schema:version>
    <dct:format rdf:resource="http://www.w3.org/ns/formats/RDF_XML"/>
    <dct:hasFormat rdf:resource="https://uwlib-cams.github.io/uwlswd_vocabs_marc_007/sound_recording_specific_material_designation/sound_recording_specific_material_designation.ttl"/>
    <dct:hasFormat rdf:resource="https://uwlib-cams.github.io/uwlswd_vocabs_marc_007/sound_recording_specific_material_designation/sound_recording_specific_material_designation.nt"/>
    <dct:hasFormat rdf:resource="https://uwlib-cams.github.io/uwlswd_vocabs_marc_007/sound_recording_specific_material_designation/sound_recording_specific_material_designation.jsonld"/>
    <dct:hasFormat rdf:resource="https://uwlib-cams.github.io/uwlswd_vocabs_marc_007/sound_recording_specific_material_designation/sound_recording_specific_material_designation.html"/>
  </rdf:Description>
  <rdf:Description rdf:about="https://doi.org/10.6069/uwlswd.enb6-8r41#i">
    <rdf:type rdf:resource="http://www.w3.org/2004/02/skos/core#Concept"/>
    <skos:inScheme rdf:resource="https://doi.org/10.6069/uwlswd.enb6-8r41"/>
    <skos:prefLabel xml:lang="en">sound-track film</skos:prefLabel>
    <skos:definition xml:lang="en">A sound recording on film that is not intended to accompany
         visual images.</skos:definition>
    <skos:scopeNote xml:lang="en">Also when it is not known if a sound recording on film is
         intended to accompany visual images.</skos:scopeNote>
    <skos:notation>i</skos:notation>
  </rdf:Description>
  <rdf:Description rdf:about="https://doi.org/10.6069/uwlswd.enb6-8r41#q">
    <rdf:type rdf:resource="http://www.w3.org/2004/02/skos/core#Concept"/>
    <skos:inScheme rdf:resource="https://doi.org/10.6069/uwlswd.enb6-8r41"/>
    <skos:prefLabel xml:lang="en">roll</skos:prefLabel>
    <skos:definition xml:lang="en">Roll of paper, for example, for player piano or player organ,
         on which the notes of a musical composition are represented by perforations in the paper
         and from which sound can be mechanically produced.</skos:definition>
    <skos:notation>q</skos:notation>
  </rdf:Description>
  <rdf:Description rdf:about="https://doi.org/10.6069/uwlswd.enb6-8r41#z">
    <rdf:type rdf:resource="http://www.w3.org/2004/02/skos/core#Concept"/>
    <skos:inScheme rdf:resource="https://doi.org/10.6069/uwlswd.enb6-8r41"/>
    <skos:prefLabel xml:lang="en">other</skos:prefLabel>
    <skos:definition xml:lang="en">Specific material designation other than belt, sound disc,
         cylinder, sound cartridge, sound-track film, roll, remote, sound cassette, sound-tape reel,
         or wire recording.</skos:definition>
    <skos:notation>z</skos:notation>
  </rdf:Description>
  <rdf:Description rdf:about="https://doi.org/10.6069/uwlswd.enb6-8r41#c">
    <rdf:type rdf:resource="http://www.w3.org/2004/02/skos/core#Concept"/>
    <skos:inScheme rdf:resource="https://doi.org/10.6069/uwlswd.enb6-8r41"/>
    <skos:prefLabel xml:lang="en">cylinder [obsolete]</skos:prefLabel>
    <skos:notation>c</skos:notation>
  </rdf:Description>
  <rdf:Description rdf:about="https://doi.org/10.6069/uwlswd.enb6-8r41#u">
    <rdf:type rdf:resource="http://www.w3.org/2004/02/skos/core#Concept"/>
    <skos:inScheme rdf:resource="https://doi.org/10.6069/uwlswd.enb6-8r41"/>
    <skos:prefLabel xml:lang="en">unspecified</skos:prefLabel>
    <skos:definition xml:lang="en">Special material designation for the sound recording is not
         specified.</skos:definition>
    <skos:notation>u</skos:notation>
  </rdf:Description>
  <rdf:Description rdf:about="https://doi.org/10.6069/uwlswd.enb6-8r41#w">
    <rdf:type rdf:resource="http://www.w3.org/2004/02/skos/core#Concept"/>
    <skos:inScheme rdf:resource="https://doi.org/10.6069/uwlswd.enb6-8r41"/>
    <skos:prefLabel xml:lang="en">wire recording</skos:prefLabel>
    <skos:definition xml:lang="en">A round steel wire on which sound waves are magnetically
         recorded.</skos:definition>
    <skos:notation>w</skos:notation>
  </rdf:Description>
  <rdf:Description rdf:about="https://doi.org/10.6069/uwlswd.enb6-8r41#t">
    <rdf:type rdf:resource="http://www.w3.org/2004/02/skos/core#Concept"/>
    <skos:inScheme rdf:resource="https://doi.org/10.6069/uwlswd.enb6-8r41"/>
    <skos:prefLabel xml:lang="en">sound-tape reel</skos:prefLabel>
    <skos:definition xml:lang="en">An audiotape-transport system with separate supply (feed) and
         take-up reels. Usually designated an Open Reel or Reel-to-Reel.</skos:definition>
    <skos:notation>t</skos:notation>
  </rdf:Description>
  <rdf:Description rdf:about="https://doi.org/10.6069/uwlswd.enb6-8r41#rx">
    <rdf:type rdf:resource="http://www.w3.org/2004/02/skos/core#Concept"/>
    <skos:inScheme rdf:resource="https://doi.org/10.6069/uwlswd.enb6-8r41"/>
    <skos:prefLabel xml:lang="en">roll [obsolete]</skos:prefLabel>
    <skos:notation>r</skos:notation>
  </rdf:Description>
  <rdf:Description rdf:about="https://doi.org/10.6069/uwlswd.enb6-8r41#f">
    <rdf:type rdf:resource="http://www.w3.org/2004/02/skos/core#Concept"/>
    <skos:inScheme rdf:resource="https://doi.org/10.6069/uwlswd.enb6-8r41"/>
    <skos:prefLabel xml:lang="en">sound-track film [obsolete]</skos:prefLabel>
    <skos:notation>f</skos:notation>
  </rdf:Description>
  <rdf:Description rdf:about="https://doi.org/10.6069/uwlswd.enb6-8r41#b">
    <rdf:type rdf:resource="http://www.w3.org/2004/02/skos/core#Concept"/>
    <skos:inScheme rdf:resource="https://doi.org/10.6069/uwlswd.enb6-8r41"/>
    <skos:prefLabel xml:lang="en">belt</skos:prefLabel>
    <skos:definition xml:lang="en">A loop of flexible plastic or magnetic film on which audio
         signals are mechanically recorded.</skos:definition>
    <skos:scopeNote xml:lang="en">Commonly known under the trade name Dictabelt.</skos:scopeNote>
    <skos:notation>b</skos:notation>
  </rdf:Description>
  <rdf:Description rdf:about="https://doi.org/10.6069/uwlswd.enb6-8r41#g">
    <rdf:type rdf:resource="http://www.w3.org/2004/02/skos/core#Concept"/>
    <skos:inScheme rdf:resource="https://doi.org/10.6069/uwlswd.enb6-8r41"/>
    <skos:prefLabel xml:lang="en">sound cartridge</skos:prefLabel>
    <skos:definition xml:lang="en">Containers holding a single sound tape, run as an endless
         loop.</skos:definition>
    <skos:notation>g</skos:notation>
  </rdf:Description>
  <rdf:Description rdf:about="https://doi.org/10.6069/uwlswd.enb6-8r41#r">
    <rdf:type rdf:resource="http://www.w3.org/2004/02/skos/core#Concept"/>
    <skos:inScheme rdf:resource="https://doi.org/10.6069/uwlswd.enb6-8r41"/>
    <skos:prefLabel xml:lang="en">remote</skos:prefLabel>
    <skos:definition xml:lang="en">Digital sound recording that is accessed, processed, executed,
         etc. remotely. In this case, the digital sound recording is used via input/output devices
         connected electronically to a computer. Frequently this involves connection through a
         computer network.</skos:definition>
    <skos:notation>r</skos:notation>
  </rdf:Description>
  <rdf:Description rdf:about="https://doi.org/10.6069/uwlswd.enb6-8r41#e">
    <rdf:type rdf:resource="http://www.w3.org/2004/02/skos/core#Concept"/>
    <skos:inScheme rdf:resource="https://doi.org/10.6069/uwlswd.enb6-8r41"/>
    <skos:prefLabel xml:lang="en">cylinder</skos:prefLabel>
    <skos:definition xml:lang="en">Cylindrical objects on which sound waves are incised or
         indented in a continuous circular groove.</skos:definition>
    <skos:scopeNote xml:lang="en">Mass-produced cylinders are made of plastic. Early cylinders
         were made of tinfoil or wax.</skos:scopeNote>
    <skos:notation>e</skos:notation>
  </rdf:Description>
</rdf:RDF>
