<?xml version="1.0" encoding="UTF-8"?><rdf:RDF xmlns:dc="http://purl.org/dc/elements/1.1/" xmlns:dct="http://purl.org/dc/terms/" xmlns:rdf="http://www.w3.org/1999/02/22-rdf-syntax-ns#" xmlns:rdfs="http://www.w3.org/2000/01/rdf-schema#" xmlns:schema="https://schema.org/" xmlns:skos="http://www.w3.org/2004/02/skos/core#" xmlns:uw="https://www.lib.washington.edu/static/public/cams/data/localResources/properties_local.html" xmlns:uwp="https://doi.org/10.6069/uwlib.55.d.3#">


   <rdf:Description rdf:about="http://fakeIRI.edu/terms/electroant"><rdf:type rdf:resource="http://www.w3.org/2004/02/skos/core#ConceptScheme"/><dct:type rdf:resource="http://purl.org/dc/dcmitype/Dataset"/><dct:title xml:lang="en">Electronic resource: antecedent/source</dct:title><dct:alternative xml:lang="en">MARC21 007/11 values for electronic resources expressed using RDF</dct:alternative><dct:description xml:lang="en">Information about the source of a digital file important to the creation, use and management of digitally reformatted materials.</dct:description><schema:disambiguatingDescription>SKOS Concept Scheme for MARC 00X Values</schema:disambiguatingDescription><dct:publisher rdf:resource="http://viaf.org/viaf/139541794"/><dct:source rdf:resource="https://www.loc.gov/marc/bibliographic/bd007.html"/><dct:source rdf:resource="http://marc21rdf.info"/><dct:provenance rdf:resource="https://doi.org/10.6069/uwlswd.2e2b-y833"/><dct:creator rdf:resource="http://viaf.org/viaf/139541794"/><dct:contributor rdf:resource="http://viaf.org/viaf/151962300"/><dct:issued>2024</dct:issued><dc:contributor xml:lang="en">Metadata Management Associates</dc:contributor><dc:language>en</dc:language><dct:license rdf:resource="http://creativecommons.org/publicdomain/zero/1.0"/><schema:version>1-0-0</schema:version><dct:issued>2024</dct:issued><dct:format rdf:resource="http://www.w3.org/ns/formats/RDF_XML"/></rdf:Description>
   
   <rdf:Description rdf:about="http://fakeIRI.edu/terms/electroant#c"><rdf:type rdf:resource="http://www.w3.org/2004/02/skos/core#Concept"/><skos:inScheme rdf:resource="http://fakeIRI.edu/terms/electroant"/><skos:prefLabel xml:lang="en">file reproduced from an electronic resource</skos:prefLabel><skos:definition xml:lang="en">Electronic resource has been created or copied from an existing electronic resource.</skos:definition><skos:scopeNote xml:lang="en">E.g., to generate new copies or derivative copies with lower resolution or smaller file size; to process an existing file with Optical Character Recognition - OCR - software; etc.</skos:scopeNote><skos:notation xml:lang="en">c</skos:notation></rdf:Description>
   
   <rdf:Description rdf:about="http://fakeIRI.edu/terms/electroant#d"><rdf:type rdf:resource="http://www.w3.org/2004/02/skos/core#Concept"/><skos:inScheme rdf:resource="http://fakeIRI.edu/terms/electroant"/><skos:prefLabel xml:lang="en">file reproduced from an intermediate (not microform</skos:prefLabel><skos:definition xml:lang="en">Content comprising the electronic resource has been created by reformatting/digitizing from an intermediate other than microform.</skos:definition><skos:scopeNote xml:lang="en">Common examples of non-microfom intermediates for visual and textual materials are: photocopies, 35 mm film, transparencies, slides, 2nd generation video tape, etc. A common example of an intermediate for audio materials is 2nd generation analog tapes.</skos:scopeNote><skos:notation xml:lang="en">d</skos:notation></rdf:Description>
   
   <rdf:Description rdf:about="http://fakeIRI.edu/terms/electroant#b"><rdf:type rdf:resource="http://www.w3.org/2004/02/skos/core#Concept"/><skos:inScheme rdf:resource="http://fakeIRI.edu/terms/electroant"/><skos:prefLabel xml:lang="en">file reproduced from microform</skos:prefLabel><skos:definition xml:lang="en">Content comprising the electronic resource has been created by scanning from microform.</skos:definition><skos:scopeNote xml:lang="en">Examples of microform are: 16mm microfilm, 35mm microfilm, 105mm microfiche, microcard, micro-opaque, etc.</skos:scopeNote><skos:notation xml:lang="en">b</skos:notation></rdf:Description>
   
   <rdf:Description rdf:about="http://fakeIRI.edu/terms/electroant#a"><rdf:type rdf:resource="http://www.w3.org/2004/02/skos/core#Concept"/><skos:inScheme rdf:resource="http://fakeIRI.edu/terms/electroant"/><skos:prefLabel xml:lang="en">file reproduced from original</skos:prefLabel><skos:definition xml:lang="en">Content (image, audio, or video) comprising the electronic resource has been created by digitization of the original item.</skos:definition><skos:scopeNote xml:lang="en">Common examples of original objects include: printed or manuscript texts and/or images that are made on paper or on vellum; photographic prints (and in some instances photographic negatives, depending on creator's intent); analog audio formats; and video formats. This value does not pertain to microform even if microform is the original.</skos:scopeNote><skos:notation xml:lang="en">a</skos:notation></rdf:Description>
   
   <rdf:Description rdf:about="http://fakeIRI.edu/terms/electroant#m"><rdf:type rdf:resource="http://www.w3.org/2004/02/skos/core#Concept"/><skos:inScheme rdf:resource="http://fakeIRI.edu/terms/electroant"/><skos:prefLabel xml:lang="en">mixed</skos:prefLabel><skos:definition xml:lang="en">Images comprising the electronic resource have been created from mixed sources.</skos:definition><skos:scopeNote xml:lang="en">Portions scanned from original item, portions scanned from microfilm, etc.</skos:scopeNote><skos:notation xml:lang="en">m</skos:notation></rdf:Description>
   
   <rdf:Description rdf:about="http://fakeIRI.edu/terms/electroant#n"><rdf:type rdf:resource="http://www.w3.org/2004/02/skos/core#Concept"/><skos:inScheme rdf:resource="http://fakeIRI.edu/terms/electroant"/><skos:prefLabel xml:lang="en">not applicable</skos:prefLabel><skos:definition xml:lang="en">Antecedent or source are not applicable to this electronic resource.</skos:definition><skos:scopeNote xml:lang="en">Appropriate for electronic resources other than those created during a reformatting process.</skos:scopeNote><skos:notation xml:lang="en">n</skos:notation></rdf:Description>
   
   <rdf:Description rdf:about="http://fakeIRI.edu/terms/electroant#u"><rdf:type rdf:resource="http://www.w3.org/2004/02/skos/core#Concept"/><skos:inScheme rdf:resource="http://fakeIRI.edu/terms/electroant"/><skos:prefLabel xml:lang="en">unknown</skos:prefLabel><skos:definition xml:lang="en">Antecedent or source of this reformatted electronic resource is not known.</skos:definition><skos:notation xml:lang="en">u</skos:notation></rdf:Description>
</rdf:RDF>