<?xml version="1.0" encoding="utf-8"?>
<rdf:RDF
   xmlns:dc="http://purl.org/dc/elements/1.1/"
   xmlns:dct="http://purl.org/dc/terms/"
   xmlns:rdf="http://www.w3.org/1999/02/22-rdf-syntax-ns#"
   xmlns:schema="https://schema.org/"
   xmlns:skos="http://www.w3.org/2004/02/skos/core#"
>
  <rdf:Description rdf:about="https://doi.org/10.6069/uwlswd.brtx-qb17">
    <rdf:type rdf:resource="http://www.w3.org/2004/02/skos/core#ConceptScheme"/>
    <dct:type rdf:resource="http://purl.org/dc/dcmitype/Dataset"/>
    <dct:title xml:lang="en">Electronic resource: antecedent/source</dct:title>
    <dct:alternative xml:lang="en">MARC21 007/11 values for electronic resources expressed using
         RDF</dct:alternative>
    <dct:description xml:lang="en">Information about the source of a digital file important to the
         creation, use and management of digitally reformatted materials.</dct:description>
    <schema:disambiguatingDescription xml:lang="en">SKOS Concept Scheme for MARC 00X
         Values</schema:disambiguatingDescription>
    <dct:publisher rdf:resource="http://viaf.org/viaf/139541794"/>
    <dct:source rdf:resource="https://www.loc.gov/marc/bibliographic/bd007.html"/>
    <dct:source rdf:resource="http://marc21rdf.info"/>
    <dct:provenance rdf:resource="https://doi.org/10.6069/uwlswd.2e2b-y833#marc00Xvalues"/>
    <dct:creator rdf:resource="http://viaf.org/viaf/139541794"/>
    <dct:contributor rdf:resource="http://viaf.org/viaf/151962300"/>
    <dct:issued>2024</dct:issued>
    <dc:contributor xml:lang="en">Metadata Management Associates</dc:contributor>
    <dc:language>en</dc:language>
    <dct:license rdf:resource="http://creativecommons.org/publicdomain/zero/1.0"/>
    <schema:version>1-0-0</schema:version>
    <dct:format rdf:resource="http://www.w3.org/ns/formats/RDF_XML"/>
    <dct:hasFormat rdf:resource="https://uwlib-cams.github.io/uwlswd_vocabs_marc_007/electronic_resource_antecedent_or_source/electronic_resource_antecedent_or_source.ttl"/>
    <dct:hasFormat rdf:resource="https://uwlib-cams.github.io/uwlswd_vocabs_marc_007/electronic_resource_antecedent_or_source/electronic_resource_antecedent_or_source.nt"/>
    <dct:hasFormat rdf:resource="https://uwlib-cams.github.io/uwlswd_vocabs_marc_007/electronic_resource_antecedent_or_source/electronic_resource_antecedent_or_source.jsonld"/>
    <dct:hasFormat rdf:resource="https://uwlib-cams.github.io/uwlswd_vocabs_marc_007/electronic_resource_antecedent_or_source/electronic_resource_antecedent_or_source.html"/>
  </rdf:Description>
  <rdf:Description rdf:about="https://doi.org/10.6069/uwlswd.brtx-qb17#a">
    <rdf:type rdf:resource="http://www.w3.org/2004/02/skos/core#Concept"/>
    <skos:inScheme rdf:resource="https://doi.org/10.6069/uwlswd.brtx-qb17"/>
    <skos:prefLabel xml:lang="en">file reproduced from original</skos:prefLabel>
    <skos:definition xml:lang="en">Content (image, audio, or video) comprising the electronic
         resource has been created by digitization of the original item.</skos:definition>
    <skos:scopeNote xml:lang="en">Common examples of original objects include: printed or
         manuscript texts and/or images that are made on paper or on vellum; photographic prints
         (and in some instances photographic negatives, depending on creator's intent); analog audio
         formats; and video formats. This value does not pertain to microform even if microform is
         the original.</skos:scopeNote>
    <skos:notation>a</skos:notation>
  </rdf:Description>
  <rdf:Description rdf:about="https://doi.org/10.6069/uwlswd.brtx-qb17#u">
    <rdf:type rdf:resource="http://www.w3.org/2004/02/skos/core#Concept"/>
    <skos:inScheme rdf:resource="https://doi.org/10.6069/uwlswd.brtx-qb17"/>
    <skos:prefLabel xml:lang="en">unknown</skos:prefLabel>
    <skos:definition xml:lang="en">Antecedent or source of this reformatted electronic resource is
         not known.</skos:definition>
    <skos:notation>u</skos:notation>
  </rdf:Description>
  <rdf:Description rdf:about="https://doi.org/10.6069/uwlswd.brtx-qb17#d">
    <rdf:type rdf:resource="http://www.w3.org/2004/02/skos/core#Concept"/>
    <skos:inScheme rdf:resource="https://doi.org/10.6069/uwlswd.brtx-qb17"/>
    <skos:prefLabel xml:lang="en">file reproduced from an intermediate (not
         microform</skos:prefLabel>
    <skos:definition xml:lang="en">Content comprising the electronic resource has been created by
         reformatting/digitizing from an intermediate other than microform.</skos:definition>
    <skos:scopeNote xml:lang="en">Common examples of non-microfom intermediates for visual and
         textual materials are: photocopies, 35 mm film, transparencies, slides, 2nd generation
         video tape, etc. A common example of an intermediate for audio materials is 2nd generation
         analog tapes.</skos:scopeNote>
    <skos:notation>d</skos:notation>
  </rdf:Description>
  <rdf:Description rdf:about="https://doi.org/10.6069/uwlswd.brtx-qb17#c">
    <rdf:type rdf:resource="http://www.w3.org/2004/02/skos/core#Concept"/>
    <skos:inScheme rdf:resource="https://doi.org/10.6069/uwlswd.brtx-qb17"/>
    <skos:prefLabel xml:lang="en">file reproduced from an electronic resource</skos:prefLabel>
    <skos:definition xml:lang="en">Electronic resource has been created or copied from an existing
         electronic resource.</skos:definition>
    <skos:scopeNote xml:lang="en">E.g., to generate new copies or derivative copies with lower
         resolution or smaller file size; to process an existing file with Optical Character
         Recognition - OCR - software; etc.</skos:scopeNote>
    <skos:notation>c</skos:notation>
  </rdf:Description>
  <rdf:Description rdf:about="https://doi.org/10.6069/uwlswd.brtx-qb17#m">
    <rdf:type rdf:resource="http://www.w3.org/2004/02/skos/core#Concept"/>
    <skos:inScheme rdf:resource="https://doi.org/10.6069/uwlswd.brtx-qb17"/>
    <skos:prefLabel xml:lang="en">mixed</skos:prefLabel>
    <skos:definition xml:lang="en">Images comprising the electronic resource have been created
         from mixed sources.</skos:definition>
    <skos:scopeNote xml:lang="en">Portions scanned from original item, portions scanned from
         microfilm, etc.</skos:scopeNote>
    <skos:notation>m</skos:notation>
  </rdf:Description>
  <rdf:Description rdf:about="https://doi.org/10.6069/uwlswd.brtx-qb17#n">
    <rdf:type rdf:resource="http://www.w3.org/2004/02/skos/core#Concept"/>
    <skos:inScheme rdf:resource="https://doi.org/10.6069/uwlswd.brtx-qb17"/>
    <skos:prefLabel xml:lang="en">not applicable</skos:prefLabel>
    <skos:definition xml:lang="en">Antecedent or source are not applicable to this electronic
         resource.</skos:definition>
    <skos:scopeNote xml:lang="en">Appropriate for electronic resources other than those created
         during a reformatting process.</skos:scopeNote>
    <skos:notation>n</skos:notation>
  </rdf:Description>
  <rdf:Description rdf:about="https://doi.org/10.6069/uwlswd.brtx-qb17#b">
    <rdf:type rdf:resource="http://www.w3.org/2004/02/skos/core#Concept"/>
    <skos:inScheme rdf:resource="https://doi.org/10.6069/uwlswd.brtx-qb17"/>
    <skos:prefLabel xml:lang="en">file reproduced from microform</skos:prefLabel>
    <skos:definition xml:lang="en">Content comprising the electronic resource has been created by
         scanning from microform.</skos:definition>
    <skos:scopeNote xml:lang="en">Examples of microform are: 16mm microfilm, 35mm microfilm, 105mm
         microfiche, microcard, micro-opaque, etc.</skos:scopeNote>
    <skos:notation>b</skos:notation>
  </rdf:Description>
</rdf:RDF>
