@prefix dc: <http://purl.org/dc/elements/1.1/> .
@prefix dct: <http://purl.org/dc/terms/> .
@prefix schema: <https://schema.org/> .
@prefix skos: <http://www.w3.org/2004/02/skos/core#> .

<https://doi.org/10.6069/uwlswd.k2b6-k011#a> a skos:Concept ;
    skos:definition """Quality assurance targets were not included at the time of
         reformatting and/or are not present in the electronic resource."""@en ;
    skos:inScheme <https://doi.org/10.6069/uwlswd.k2b6-k011> ;
    skos:notation "a" ;
    skos:prefLabel "absent"@en .

<https://doi.org/10.6069/uwlswd.k2b6-k011#n> a skos:Concept ;
    skos:definition """Inclusion of quality assurance targets is not applicable to
         this electronic resource."""@en ;
    skos:inScheme <https://doi.org/10.6069/uwlswd.k2b6-k011> ;
    skos:notation "n" ;
    skos:prefLabel "not applicable"@en .

<https://doi.org/10.6069/uwlswd.k2b6-k011#p> a skos:Concept ;
    skos:definition """One or more quality assurance targets were appropriately
         included at the time of reformatting and are present in the electronic
         resource."""@en ;
    skos:inScheme <https://doi.org/10.6069/uwlswd.k2b6-k011> ;
    skos:notation "p" ;
    skos:prefLabel "present"@en ;
    skos:scopeNote """Commonly found quality control targets for scanning include the
         Kodak Q13 or Q14 Color Separation Guide and Gray Scale; Kodak Q60 Color Input Target; AIIM
         Scanning Test Chart #2; and the RIT Alphanumeric Resolution Test Object. Commonly found
         quality assurance targets for re-recording/transfer of audio files include reference and
         azimuth tones."""@en .

<https://doi.org/10.6069/uwlswd.k2b6-k011#u> a skos:Concept ;
    skos:definition """Presence of quality assurance targets in the electronic
         resource is not known."""@en ;
    skos:inScheme <https://doi.org/10.6069/uwlswd.k2b6-k011> ;
    skos:notation "u" ;
    skos:prefLabel "unknown"@en .

<https://doi.org/10.6069/uwlswd.k2b6-k011> a skos:ConceptScheme ;
    dc:contributor "Metadata Management Associates"@en ;
    dc:language "en" ;
    dct:alternative """MARC21 007/10 values for electronic resources expressed using
         RDF"""@en ;
    dct:contributor <http://viaf.org/viaf/151962300> ;
    dct:creator <http://viaf.org/viaf/139541794> ;
    dct:description """Whether quality assurance targets have been included
         appropriately at the time of reformatting/creation of the electronic resource. Targets are
         standard reference points which can be interpreted by a human or machine and used to
         measure resolution, color, faithfulness of representation to the original,
         etc."""@en ;
    dct:format <http://www.w3.org/ns/formats/Turtle> ;
    dct:hasFormat <https://uwlib-cams.github.io/uwlswd_vocabs_marc_007/electronic_resource_quality_assurance_targets/electronic_resource_quality_assurance_targets.html>,
        <https://uwlib-cams.github.io/uwlswd_vocabs_marc_007/electronic_resource_quality_assurance_targets/electronic_resource_quality_assurance_targets.jsonld>,
        <https://uwlib-cams.github.io/uwlswd_vocabs_marc_007/electronic_resource_quality_assurance_targets/electronic_resource_quality_assurance_targets.nt>,
        <https://uwlib-cams.github.io/uwlswd_vocabs_marc_007/electronic_resource_quality_assurance_targets/electronic_resource_quality_assurance_targets.rdf> ;
    dct:issued "2024" ;
    dct:license <http://creativecommons.org/publicdomain/zero/1.0> ;
    dct:provenance <https://doi.org/10.6069/uwlswd.2e2b-y833#marc00Xvalues> ;
    dct:publisher <http://viaf.org/viaf/139541794> ;
    dct:source <http://marc21rdf.info>,
        <https://www.loc.gov/marc/bibliographic/bd007.html> ;
    dct:title "Electronic resource: quality assurance targets"@en ;
    dct:type <http://purl.org/dc/dcmitype/Dataset> ;
    schema:disambiguatingDescription """SKOS Concept Scheme for MARC 00X
         Values"""@en ;
    schema:version "1-0-0" .

