@prefix dc: <http://purl.org/dc/elements/1.1/> .
@prefix dct: <http://purl.org/dc/terms/> .
@prefix schema: <https://schema.org/> .
@prefix skos: <http://www.w3.org/2004/02/skos/core#> .

<https://doi.org/10.6069/uwlswd.bfyv-x467#a> a skos:Concept ;
    skos:definition """Colors and/or tonal values are the same as the original subject
         matter."""@en ;
    skos:inScheme <https://doi.org/10.6069/uwlswd.bfyv-x467> ;
    skos:notation "a" ;
    skos:prefLabel "positive"@en .

<https://doi.org/10.6069/uwlswd.bfyv-x467#b> a skos:Concept ;
    skos:definition """For a black-and-white film, tonal values are the opposite of
         those in the original subject matter. For a color film, tonal values are the complements of
         the original subject matter (e.g., red appears as green in a color
         negative)."""@en ;
    skos:inScheme <https://doi.org/10.6069/uwlswd.bfyv-x467> ;
    skos:notation "b" ;
    skos:prefLabel "negative"@en .

<https://doi.org/10.6069/uwlswd.bfyv-x467#n> a skos:Concept ;
    skos:definition """Film does not have a positive/negative
         aspect."""@en ;
    skos:inScheme <https://doi.org/10.6069/uwlswd.bfyv-x467> ;
    skos:notation "n" ;
    skos:prefLabel "not applicable"@en .

<https://doi.org/10.6069/uwlswd.bfyv-x467#u> a skos:Concept ;
    skos:definition """Positive/negative aspect of the film is not
         known."""@en ;
    skos:inScheme <https://doi.org/10.6069/uwlswd.bfyv-x467> ;
    skos:notation "u" ;
    skos:prefLabel "unknown"@en .

<https://doi.org/10.6069/uwlswd.bfyv-x467#z> a skos:Concept ;
    skos:definition """Positive/negative aspect other than positive or
         negative."""@en ;
    skos:inScheme <https://doi.org/10.6069/uwlswd.bfyv-x467> ;
    skos:notation "z" ;
    skos:prefLabel "other"@en .

<https://doi.org/10.6069/uwlswd.bfyv-x467> a skos:ConceptScheme ;
    dc:contributor "Metadata Management Associates"@en ;
    dc:language "en" ;
    dct:alternative """MARC21 007/10 values for motion pictures expressed using
         RDF"""@en ;
    dct:contributor <http://viaf.org/viaf/151962300> ;
    dct:creator <http://viaf.org/viaf/139541794> ;
    dct:description "Whether the film is positive or negative."@en ;
    dct:format <http://www.w3.org/ns/formats/Turtle> ;
    dct:hasFormat <https://uwlib-cams.github.io/uwlswd_vocabs_marc_007/motion_picture_positive_or_negative_aspect/motion_picture_positive_or_negative_aspect.html>,
        <https://uwlib-cams.github.io/uwlswd_vocabs_marc_007/motion_picture_positive_or_negative_aspect/motion_picture_positive_or_negative_aspect.jsonld>,
        <https://uwlib-cams.github.io/uwlswd_vocabs_marc_007/motion_picture_positive_or_negative_aspect/motion_picture_positive_or_negative_aspect.nt>,
        <https://uwlib-cams.github.io/uwlswd_vocabs_marc_007/motion_picture_positive_or_negative_aspect/motion_picture_positive_or_negative_aspect.rdf> ;
    dct:issued "2024" ;
    dct:license <http://creativecommons.org/publicdomain/zero/1.0> ;
    dct:provenance <https://doi.org/10.6069/uwlswd.2e2b-y833#marc00Xvalues> ;
    dct:publisher <http://viaf.org/viaf/139541794> ;
    dct:source <http://marc21rdf.info>,
        <https://www.loc.gov/marc/bibliographic/bd007.html> ;
    dct:title "Motion picture: positive/negative aspect"@en ;
    dct:type <http://purl.org/dc/dcmitype/Dataset> ;
    schema:disambiguatingDescription """SKOS Concept Scheme for MARC 00X
         Values"""@en ;
    schema:version "1-0-0" .

