@prefix dc: <http://purl.org/dc/elements/1.1/> .
@prefix dct: <http://purl.org/dc/terms/> .
@prefix schema: <https://schema.org/> .
@prefix skos: <http://www.w3.org/2004/02/skos/core#> .

<https://doi.org/10.6069/uwlswd.fqx4-1d72#a> a skos:Concept ;
    skos:definition """Safety base film whose type has not been
         identified."""@en ;
    skos:inScheme <https://doi.org/10.6069/uwlswd.fqx4-1d72> ;
    skos:notation "a" ;
    skos:prefLabel "safety base, undetermined"@en .

<https://doi.org/10.6069/uwlswd.fqx4-1d72#c> a skos:Concept ;
    skos:definition """Acetate safety base film whose exact type cannot be determined,
         i.e., where it is unknown if the type is diacetate or triacetate."""@en ;
    skos:inScheme <https://doi.org/10.6069/uwlswd.fqx4-1d72> ;
    skos:notation "c" ;
    skos:prefLabel "safety base, acetate undetermined"@en .

<https://doi.org/10.6069/uwlswd.fqx4-1d72#d> a skos:Concept ;
    skos:definition "Cellulose diacetate film base."@en ;
    skos:inScheme <https://doi.org/10.6069/uwlswd.fqx4-1d72> ;
    skos:notation "d" ;
    skos:prefLabel "safety base, diacetate"@en ;
    skos:scopeNote """Introduced before World War I for home movies, diacetate base
         was more expensive and unpredictable than nitrate base and so failed to gain acceptance in
         professional 35 mm. film production."""@en .

<https://doi.org/10.6069/uwlswd.fqx4-1d72#i> a skos:Concept ;
    skos:definition "Cellulose nitrate film base."@en ;
    skos:inScheme <https://doi.org/10.6069/uwlswd.fqx4-1d72> ;
    skos:notation "i" ;
    skos:prefLabel "nitrate base"@en ;
    skos:scopeNote """Cellulose nitrate support or base was used in the manufacture of
         35 mm. film (and some 17.5 mm. film) until 1951. Nitrate base film is no longer
         manufactured."""@en .

<https://doi.org/10.6069/uwlswd.fqx4-1d72#m> a skos:Concept ;
    skos:definition """Combination of nitrate base and safety base
         film."""@en ;
    skos:inScheme <https://doi.org/10.6069/uwlswd.fqx4-1d72> ;
    skos:notation "m" ;
    skos:prefLabel "mixed base (nitrate and safety)"@en ;
    skos:scopeNote """The use of a mixed base was common in the early 1950s when
         nitrate base stock shots were spliced with safety base film for low-budget motion pictures.
         In such releases, up to 50% of the film consisted of stock shots on nitrate base
         film."""@en .

<https://doi.org/10.6069/uwlswd.fqx4-1d72#n> a skos:Concept ;
    skos:definition "Item does not have a film base."@en ;
    skos:inScheme <https://doi.org/10.6069/uwlswd.fqx4-1d72> ;
    skos:notation "n" ;
    skos:prefLabel "not applicable"@en ;
    skos:scopeNote "E.g., paper film."@en .

<https://doi.org/10.6069/uwlswd.fqx4-1d72#p> a skos:Concept ;
    skos:definition "Film base made of a synthetic resin."@en ;
    skos:inScheme <https://doi.org/10.6069/uwlswd.fqx4-1d72> ;
    skos:notation "p" ;
    skos:prefLabel "safety base, polyester"@en ;
    skos:scopeNote "E.g., estar."@en .

<https://doi.org/10.6069/uwlswd.fqx4-1d72#r> a skos:Concept ;
    skos:definition """Mixed safety base films spliced together; but contains no
         nitrate film."""@en ;
    skos:inScheme <https://doi.org/10.6069/uwlswd.fqx4-1d72> ;
    skos:notation "r" ;
    skos:prefLabel "safety base, mixed"@en .

<https://doi.org/10.6069/uwlswd.fqx4-1d72#t> a skos:Concept ;
    skos:definition "Cellulose triacetate film base."@en ;
    skos:inScheme <https://doi.org/10.6069/uwlswd.fqx4-1d72> ;
    skos:notation "t" ;
    skos:prefLabel "safety base, triacetate"@en ;
    skos:scopeNote """Cellulose triacetate is a high acetal compound with very low
         flammability and slow burning characteristics. From 1951, triacetate has been used for
         professional as well as for amateur produced moving image film."""@en .

<https://doi.org/10.6069/uwlswd.fqx4-1d72#u> a skos:Concept ;
    skos:definition "Base of the film is not known."@en ;
    skos:inScheme <https://doi.org/10.6069/uwlswd.fqx4-1d72> ;
    skos:notation "u" ;
    skos:prefLabel "unknown"@en .

<https://doi.org/10.6069/uwlswd.fqx4-1d72#z> a skos:Concept ;
    skos:definition """Base of film other than safety base, undetermined, safety base,
         acetate undetermined, safety base, diacetate, nitrate base, mixed base (nitrate and
         safety), not applicable, safety base, polyester, safety base, mixed, safety base, or
         triacetate."""@en ;
    skos:inScheme <https://doi.org/10.6069/uwlswd.fqx4-1d72> ;
    skos:notation "z" ;
    skos:prefLabel "other"@en .

<https://doi.org/10.6069/uwlswd.fqx4-1d72> a skos:ConceptScheme ;
    dc:contributor "Metadata Management Associates"@en ;
    dc:language "en" ;
    dct:alternative """MARC21 007/12 values for motion pictures expressed using
         RDF"""@en ;
    dct:contributor <http://viaf.org/viaf/151962300> ;
    dct:creator <http://viaf.org/viaf/139541794> ;
    dct:description "Base of the film."@en ;
    dct:format <http://www.w3.org/ns/formats/Turtle> ;
    dct:hasFormat <https://uwlib-cams.github.io/uwlswd_vocabs_marc_007/motion_picture_base_of_film/motion_picture_base_of_film.html>,
        <https://uwlib-cams.github.io/uwlswd_vocabs_marc_007/motion_picture_base_of_film/motion_picture_base_of_film.jsonld>,
        <https://uwlib-cams.github.io/uwlswd_vocabs_marc_007/motion_picture_base_of_film/motion_picture_base_of_film.nt>,
        <https://uwlib-cams.github.io/uwlswd_vocabs_marc_007/motion_picture_base_of_film/motion_picture_base_of_film.rdf> ;
    dct:issued "2024" ;
    dct:license <http://creativecommons.org/publicdomain/zero/1.0> ;
    dct:provenance <https://doi.org/10.6069/uwlswd.2e2b-y833#marc00Xvalues> ;
    dct:publisher <http://viaf.org/viaf/139541794> ;
    dct:source <http://marc21rdf.info>,
        <https://www.loc.gov/marc/bibliographic/bd007.html> ;
    dct:title "Motion picture: base of film"@en ;
    dct:type <http://purl.org/dc/dcmitype/Dataset> ;
    schema:disambiguatingDescription """SKOS Concept Scheme for MARC 00X
         Values"""@en ;
    schema:version "1-0-0" .

