@prefix dc: <http://purl.org/dc/elements/1.1/> .
@prefix dct: <http://purl.org/dc/terms/> .
@prefix schema: <https://schema.org/> .
@prefix skos: <http://www.w3.org/2004/02/skos/core#> .

<https://doi.org/10.6069/uwlswd.fq7b-6k65#a> a skos:Concept ;
    skos:definition """Remote-sensing image was made from a device located on the
         surface of a body, usually a planet or moon."""@en ;
    skos:inScheme <https://doi.org/10.6069/uwlswd.fq7b-6k65> ;
    skos:notation "a" ;
    skos:prefLabel "surface"@en .

<https://doi.org/10.6069/uwlswd.fq7b-6k65#b> a skos:Concept ;
    skos:definition """Remote-sensing image was made from a device above the surface
         of a body, generally in the atmosphere, an aircraft, balloon, or some other airborne
         device."""@en ;
    skos:inScheme <https://doi.org/10.6069/uwlswd.fq7b-6k65> ;
    skos:notation "b" ;
    skos:prefLabel "airborne"@en .

<https://doi.org/10.6069/uwlswd.fq7b-6k65#c> a skos:Concept ;
    skos:definition """Remote-sensing image was made from a device in space.
         Spaceborne sensors are those located outside the primary layers of an atmosphere (usually
         in orbit) and beyond."""@en ;
    skos:inScheme <https://doi.org/10.6069/uwlswd.fq7b-6k65> ;
    skos:notation "c" ;
    skos:prefLabel "spaceborne"@en .

<https://doi.org/10.6069/uwlswd.fq7b-6k65#n> a skos:Concept ;
    skos:definition """Altitude of the sensor is not applicable to the
         image."""@en ;
    skos:inScheme <https://doi.org/10.6069/uwlswd.fq7b-6k65> ;
    skos:notation "n" ;
    skos:prefLabel "not applicable"@en .

<https://doi.org/10.6069/uwlswd.fq7b-6k65#u> a skos:Concept ;
    skos:definition """Altitude of the sensor from which the image was made is not
         known."""@en ;
    skos:inScheme <https://doi.org/10.6069/uwlswd.fq7b-6k65> ;
    skos:notation "u" ;
    skos:prefLabel "unknown"@en .

<https://doi.org/10.6069/uwlswd.fq7b-6k65#z> a skos:Concept ;
    skos:definition """Altitude of sensor other than surface, airborne, or
         spaceborne."""@en ;
    skos:inScheme <https://doi.org/10.6069/uwlswd.fq7b-6k65> ;
    skos:notation "z" ;
    skos:prefLabel "other"@en .

<https://doi.org/10.6069/uwlswd.fq7b-6k65> a skos:ConceptScheme ;
    dc:contributor "Metadata Management Associates"@en ;
    dc:language "en" ;
    dct:alternative """MARC21 007/03 values for remote-sensing images expressed using
         RDF"""@en ;
    dct:contributor <http://viaf.org/viaf/151962300> ;
    dct:creator <http://viaf.org/viaf/139541794> ;
    dct:description """General position of the sensor relative to to the object under
         study."""@en ;
    dct:format <http://www.w3.org/ns/formats/Turtle> ;
    dct:hasFormat <https://uwlib-cams.github.io/uwlswd_vocabs_marc_007/remote-sensing_image_altitude_of_sensor/remote-sensing_image_altitude_of_sensor.html>,
        <https://uwlib-cams.github.io/uwlswd_vocabs_marc_007/remote-sensing_image_altitude_of_sensor/remote-sensing_image_altitude_of_sensor.jsonld>,
        <https://uwlib-cams.github.io/uwlswd_vocabs_marc_007/remote-sensing_image_altitude_of_sensor/remote-sensing_image_altitude_of_sensor.nt>,
        <https://uwlib-cams.github.io/uwlswd_vocabs_marc_007/remote-sensing_image_altitude_of_sensor/remote-sensing_image_altitude_of_sensor.rdf> ;
    dct:issued "2024" ;
    dct:license <http://creativecommons.org/publicdomain/zero/1.0> ;
    dct:provenance <https://doi.org/10.6069/uwlswd.2e2b-y833#marc00Xvalues> ;
    dct:publisher <http://viaf.org/viaf/139541794> ;
    dct:source <http://marc21rdf.info>,
        <https://www.loc.gov/marc/bibliographic/bd007.html> ;
    dct:title "Remote-sensing image: altitude of sensor"@en ;
    dct:type <http://purl.org/dc/dcmitype/Dataset> ;
    schema:disambiguatingDescription """SKOS Concept Scheme for MARC 00X
         Values"""@en ;
    schema:version "1-0-0" .

