<?xml version='1.0' encoding='UTF-8'?>
<rdf:RDF xmlns:dc="http://purl.org/dc/elements/1.1/" xmlns:dct="http://purl.org/dc/terms/" xmlns:rdf="http://www.w3.org/1999/02/22-rdf-syntax-ns#" xmlns:schema="https://schema.org/" xmlns:skos="http://www.w3.org/2004/02/skos/core#">
  <rdf:Description rdf:about="https://doi.org/10.6069/uwlswd.4sxq-pn90#b">
    <rdf:type rdf:resource="http://www.w3.org/2004/02/skos/core#Concept"/>
    <skos:inScheme rdf:resource="https://doi.org/10.6069/uwlswd.4sxq-pn90"/>
    <skos:prefLabel xml:lang="en">tape duplication master</skos:prefLabel>
    <skos:definition xml:lang="en">Sound tape produced from the master tape.</skos:definition>
    <skos:scopeNote xml:lang="en">Tape duplication master is played on a tape reproducer to
         produce the sound tape for cassette, cartridge, or reel.</skos:scopeNote>
    <skos:notation>b</skos:notation>
  </rdf:Description>
  <rdf:Description rdf:about="https://doi.org/10.6069/uwlswd.4sxq-pn90#s">
    <rdf:type rdf:resource="http://www.w3.org/2004/02/skos/core#Concept"/>
    <skos:inScheme rdf:resource="https://doi.org/10.6069/uwlswd.4sxq-pn90"/>
    <skos:prefLabel xml:lang="en">stamper (negative)</skos:prefLabel>
    <skos:definition xml:lang="en">Negative metal part, produced from the mother in an
         electroplating procedure, from which 500 to 750 discs may be pressed.</skos:definition>
    <skos:notation>s</skos:notation>
  </rdf:Description>
  <rdf:Description rdf:about="https://doi.org/10.6069/uwlswd.4sxq-pn90#t">
    <rdf:type rdf:resource="http://www.w3.org/2004/02/skos/core#Concept"/>
    <skos:inScheme rdf:resource="https://doi.org/10.6069/uwlswd.4sxq-pn90"/>
    <skos:prefLabel xml:lang="en">test pressing</skos:prefLabel>
    <skos:definition xml:lang="en">Either one finished disc or one of a very limited pressing is
         made, designed to be examined aurally before a decision is made to proceed with a
         pressing.</skos:definition>
    <skos:notation>t</skos:notation>
  </rdf:Description>
  <rdf:Description rdf:about="https://doi.org/10.6069/uwlswd.4sxq-pn90#z">
    <rdf:type rdf:resource="http://www.w3.org/2004/02/skos/core#Concept"/>
    <skos:inScheme rdf:resource="https://doi.org/10.6069/uwlswd.4sxq-pn90"/>
    <skos:prefLabel xml:lang="en">other</skos:prefLabel>
    <skos:definition xml:lang="en">Kind of disc, cylinder or tape other than master tape, tape
         duplication master, disc master (negative), instantaneous (recorded on the spot), mass
         produced, mother (positive), stamper (negative), or test pressing.</skos:definition>
    <skos:notation>z</skos:notation>
  </rdf:Description>
  <rdf:Description rdf:about="https://doi.org/10.6069/uwlswd.4sxq-pn90#u">
    <rdf:type rdf:resource="http://www.w3.org/2004/02/skos/core#Concept"/>
    <skos:inScheme rdf:resource="https://doi.org/10.6069/uwlswd.4sxq-pn90"/>
    <skos:prefLabel xml:lang="en">unknown</skos:prefLabel>
    <skos:definition xml:lang="en">Type of disc, cylinder, or tape is not known.</skos:definition>
    <skos:scopeNote xml:lang="en">Also used when it cannot be determined whether the item is
         instantaneous or mass-produced.</skos:scopeNote>
    <skos:notation>u</skos:notation>
  </rdf:Description>
  <rdf:Description rdf:about="https://doi.org/10.6069/uwlswd.4sxq-pn90">
    <rdf:type rdf:resource="http://www.w3.org/2004/02/skos/core#ConceptScheme"/>
    <dct:type rdf:resource="http://purl.org/dc/dcmitype/Dataset"/>
    <dct:title xml:lang="en">Sound recording: kind of disc, cylinder or tape</dct:title>
    <dct:alternative xml:lang="en">MARC21 007/09 values for sound recordings expressed using
         RDF</dct:alternative>
    <dct:description xml:lang="en">Kind of disc, cylinder or tape.</dct:description>
    <schema:disambiguatingDescription xml:lang="en">SKOS Concept Scheme for MARC 00X
         Values</schema:disambiguatingDescription>
    <dct:publisher rdf:resource="http://viaf.org/viaf/139541794"/>
    <dct:source rdf:resource="https://www.loc.gov/marc/bibliographic/bd007.html"/>
    <dct:source rdf:resource="http://marc21rdf.info"/>
    <dct:provenance rdf:resource="https://doi.org/10.6069/uwlswd.2e2b-y833#marc00Xvalues"/>
    <dct:creator rdf:resource="http://viaf.org/viaf/139541794"/>
    <dct:contributor rdf:resource="http://viaf.org/viaf/151962300"/>
    <dct:issued>2024</dct:issued>
    <dc:contributor xml:lang="en">Metadata Management Associates</dc:contributor>
    <dc:language>en</dc:language>
    <dct:license rdf:resource="http://creativecommons.org/publicdomain/zero/1.0"/>
    <schema:version>1-0-0</schema:version>
    <dct:format rdf:resource="http://www.w3.org/ns/formats/RDF_XML"/>
  </rdf:Description>
  <rdf:Description rdf:about="https://doi.org/10.6069/uwlswd.4sxq-pn90#m">
    <rdf:type rdf:resource="http://www.w3.org/2004/02/skos/core#Concept"/>
    <skos:inScheme rdf:resource="https://doi.org/10.6069/uwlswd.4sxq-pn90"/>
    <skos:prefLabel xml:lang="en">mass produced</skos:prefLabel>
    <skos:definition xml:lang="en">Mass produced.</skos:definition>
    <skos:scopeNote xml:lang="en">Includes discs or tapes issued as limited pressing or limited
         issue for private distribution. Most commercial discs are mass-produced. Mass-produced
         discs are mechanically pressed for distribution, either commercially or privately; also,
         tapes reproduced from a tape duplication master for distribution either commercially or
         privately. Mass-produced discs, cylinders, and tapes usually include the name of the
         issuing company, the issue number, and bibliographic information on a printed label or on
         the container in which the disc, tape, or cylinder is packaged.</skos:scopeNote>
    <skos:notation>m</skos:notation>
  </rdf:Description>
  <rdf:Description rdf:about="https://doi.org/10.6069/uwlswd.4sxq-pn90#d">
    <rdf:type rdf:resource="http://www.w3.org/2004/02/skos/core#Concept"/>
    <skos:inScheme rdf:resource="https://doi.org/10.6069/uwlswd.4sxq-pn90"/>
    <skos:prefLabel xml:lang="en">disc master (negative)</skos:prefLabel>
    <skos:definition xml:lang="en">Negative disc master that is used for the preparation of the
         mother from which more serviceable and longer lasting metal stampers can be
         made.</skos:definition>
    <skos:scopeNote xml:lang="en">In the early years of recording, discs were pressed from the
         metal-plated disc master or matrix. As commercial recording developed, the disc master was
         used, and continues to be used, for the preparation of the mother.</skos:scopeNote>
    <skos:notation>d</skos:notation>
  </rdf:Description>
  <rdf:Description rdf:about="https://doi.org/10.6069/uwlswd.4sxq-pn90#r">
    <rdf:type rdf:resource="http://www.w3.org/2004/02/skos/core#Concept"/>
    <skos:inScheme rdf:resource="https://doi.org/10.6069/uwlswd.4sxq-pn90"/>
    <skos:prefLabel xml:lang="en">mother (positive)</skos:prefLabel>
    <skos:definition xml:lang="en">Exact copy of the original disc recording pressed from the disc
         master. From the metal mother a negative metal stamper is made to press discs for
         distribution.</skos:definition>
    <skos:scopeNote xml:lang="en">Many stampers may be made from a single mother.</skos:scopeNote>
    <skos:notation>r</skos:notation>
  </rdf:Description>
  <rdf:Description rdf:about="https://doi.org/10.6069/uwlswd.4sxq-pn90#n">
    <rdf:type rdf:resource="http://www.w3.org/2004/02/skos/core#Concept"/>
    <skos:inScheme rdf:resource="https://doi.org/10.6069/uwlswd.4sxq-pn90"/>
    <skos:prefLabel xml:lang="en">not applicable</skos:prefLabel>
    <skos:definition xml:lang="en">Item is not a disc, cylinder, or tape.</skos:definition>
    <skos:notation>n</skos:notation>
  </rdf:Description>
  <rdf:Description rdf:about="https://doi.org/10.6069/uwlswd.4sxq-pn90#i">
    <rdf:type rdf:resource="http://www.w3.org/2004/02/skos/core#Concept"/>
    <skos:inScheme rdf:resource="https://doi.org/10.6069/uwlswd.4sxq-pn90"/>
    <skos:prefLabel xml:lang="en">instantaneous (recorded on the spot)</skos:prefLabel>
    <skos:definition xml:lang="en">Original recording of a sound event or performance intended for
         direct reproduction without further processing.</skos:definition>
    <skos:scopeNote xml:lang="en">In the early years of recording, a single sound event was
         sometimes recorded simultaneously on several cylinders or discs. All of these recordings
         would be instantaneous.</skos:scopeNote>
    <skos:notation>i</skos:notation>
  </rdf:Description>
  <rdf:Description rdf:about="https://doi.org/10.6069/uwlswd.4sxq-pn90#a">
    <rdf:type rdf:resource="http://www.w3.org/2004/02/skos/core#Concept"/>
    <skos:inScheme rdf:resource="https://doi.org/10.6069/uwlswd.4sxq-pn90"/>
    <skos:prefLabel xml:lang="en">master tape</skos:prefLabel>
    <skos:definition xml:lang="en">Final tape production master that is used to make a disc master
         or a tape duplication master.</skos:definition>
    <skos:scopeNote xml:lang="en">Represents the final mix including special processing such as
         equalization, compression, phasing, and sound synthesis.</skos:scopeNote>
    <skos:notation>a</skos:notation>
  </rdf:Description>
</rdf:RDF>