<?xml version="1.0" encoding="UTF-8"?><rdf:RDF xmlns:dc="http://purl.org/dc/elements/1.1/" xmlns:dct="http://purl.org/dc/terms/" xmlns:rdf="http://www.w3.org/1999/02/22-rdf-syntax-ns#" xmlns:rdfs="http://www.w3.org/2000/01/rdf-schema#" xmlns:schema="https://schema.org/" xmlns:skos="http://www.w3.org/2004/02/skos/core#" xmlns:uw="https://www.lib.washington.edu/static/public/cams/data/localResources/properties_local.html" xmlns:uwp="https://doi.org/10.6069/uwlib.55.d.3#">


   <rdf:Description rdf:about="http://fakeIRI.edu/terms/remotesensingclo"><rdf:type rdf:resource="http://www.w3.org/2004/02/skos/core#ConceptScheme"/><dct:type rdf:resource="http://purl.org/dc/dcmitype/Dataset"/><dct:title xml:lang="en">Remote-sensing image: cloud cover</dct:title><dct:alternative xml:lang="en">MARC21 007/05 values for remote-sensing images expressed using RDF</dct:alternative><dct:description xml:lang="en">Amount of cloud cover that was present when a remote-sensing image was made.</dct:description><schema:disambiguatingDescription>SKOS Concept Scheme for MARC 00X Values</schema:disambiguatingDescription><dct:publisher rdf:resource="http://viaf.org/viaf/139541794"/><dct:source rdf:resource="https://www.loc.gov/marc/bibliographic/bd007.html"/><dct:source rdf:resource="http://marc21rdf.info"/><dct:provenance rdf:resource="https://doi.org/10.6069/uwlswd.2e2b-y833"/><dct:creator rdf:resource="http://viaf.org/viaf/139541794"/><dct:contributor rdf:resource="http://viaf.org/viaf/151962300"/><dct:issued>2024</dct:issued><dc:contributor xml:lang="en">Metadata Management Associates</dc:contributor><dc:language>en</dc:language><dct:license rdf:resource="http://creativecommons.org/publicdomain/zero/1.0"/><schema:version>1-0-0</schema:version><dct:issued>2024</dct:issued><dct:format rdf:resource="http://www.w3.org/ns/formats/RDF_XML"/></rdf:Description>
   
   <rdf:Description rdf:about="http://fakeIRI.edu/terms/remotesensingclo#0"><rdf:type rdf:resource="http://www.w3.org/2004/02/skos/core#Concept"/><skos:inScheme rdf:resource="http://fakeIRI.edu/terms/remotesensingclo"/><skos:prefLabel xml:lang="en">0-9%</skos:prefLabel><skos:definition xml:lang="en">Cloud cover present when an image was taken was between 0 and 9%.</skos:definition><skos:notation xml:lang="en">0</skos:notation></rdf:Description>
   
   <rdf:Description rdf:about="http://fakeIRI.edu/terms/remotesensingclo#1"><rdf:type rdf:resource="http://www.w3.org/2004/02/skos/core#Concept"/><skos:inScheme rdf:resource="http://fakeIRI.edu/terms/remotesensingclo"/><skos:prefLabel xml:lang="en">10-19%</skos:prefLabel><skos:definition xml:lang="en">Cloud cover present when an image was taken was between 10 and 19%.</skos:definition><skos:notation xml:lang="en">1</skos:notation></rdf:Description>
   
   <rdf:Description rdf:about="http://fakeIRI.edu/terms/remotesensingclo#2"><rdf:type rdf:resource="http://www.w3.org/2004/02/skos/core#Concept"/><skos:inScheme rdf:resource="http://fakeIRI.edu/terms/remotesensingclo"/><skos:prefLabel xml:lang="en">20-29%</skos:prefLabel><skos:definition xml:lang="en">Cloud cover present when an image was taken was between 20 and 29%.</skos:definition><skos:notation xml:lang="en">2</skos:notation></rdf:Description>
   
   <rdf:Description rdf:about="http://fakeIRI.edu/terms/remotesensingclo#3"><rdf:type rdf:resource="http://www.w3.org/2004/02/skos/core#Concept"/><skos:inScheme rdf:resource="http://fakeIRI.edu/terms/remotesensingclo"/><skos:prefLabel xml:lang="en">30-39%</skos:prefLabel><skos:definition xml:lang="en">Cloud cover present when an image was taken was between 30 and 39%.</skos:definition><skos:notation xml:lang="en">3</skos:notation></rdf:Description>
   
   <rdf:Description rdf:about="http://fakeIRI.edu/terms/remotesensingclo#4"><rdf:type rdf:resource="http://www.w3.org/2004/02/skos/core#Concept"/><skos:inScheme rdf:resource="http://fakeIRI.edu/terms/remotesensingclo"/><skos:prefLabel xml:lang="en">40-49%</skos:prefLabel><skos:definition xml:lang="en">Cloud cover present when an image was taken was between 40 and 49%.</skos:definition><skos:notation xml:lang="en">4</skos:notation></rdf:Description>
   
   <rdf:Description rdf:about="http://fakeIRI.edu/terms/remotesensingclo#5"><rdf:type rdf:resource="http://www.w3.org/2004/02/skos/core#Concept"/><skos:inScheme rdf:resource="http://fakeIRI.edu/terms/remotesensingclo"/><skos:prefLabel xml:lang="en">50-59%</skos:prefLabel><skos:definition xml:lang="en">Cloud cover present when an image was taken was between 50 and 59%.</skos:definition><skos:notation xml:lang="en">5</skos:notation></rdf:Description>
   
   <rdf:Description rdf:about="http://fakeIRI.edu/terms/remotesensingclo#6"><rdf:type rdf:resource="http://www.w3.org/2004/02/skos/core#Concept"/><skos:inScheme rdf:resource="http://fakeIRI.edu/terms/remotesensingclo"/><skos:prefLabel xml:lang="en">60-69%</skos:prefLabel><skos:definition xml:lang="en">Cloud cover present when an image was taken was between 60 and 69%.</skos:definition><skos:notation xml:lang="en">6</skos:notation></rdf:Description>
   
   <rdf:Description rdf:about="http://fakeIRI.edu/terms/remotesensingclo#7"><rdf:type rdf:resource="http://www.w3.org/2004/02/skos/core#Concept"/><skos:inScheme rdf:resource="http://fakeIRI.edu/terms/remotesensingclo"/><skos:prefLabel xml:lang="en">70-79%</skos:prefLabel><skos:definition xml:lang="en">Cloud cover present when an image was taken was between 70 and 79%.</skos:definition><skos:notation xml:lang="en">7</skos:notation></rdf:Description>
   
   <rdf:Description rdf:about="http://fakeIRI.edu/terms/remotesensingclo#8"><rdf:type rdf:resource="http://www.w3.org/2004/02/skos/core#Concept"/><skos:inScheme rdf:resource="http://fakeIRI.edu/terms/remotesensingclo"/><skos:prefLabel xml:lang="en">80-89%</skos:prefLabel><skos:definition xml:lang="en">Cloud cover present when an image was taken was between 80 and 89%.</skos:definition><skos:notation xml:lang="en">8</skos:notation></rdf:Description>
   
   <rdf:Description rdf:about="http://fakeIRI.edu/terms/remotesensingclo#9"><rdf:type rdf:resource="http://www.w3.org/2004/02/skos/core#Concept"/><skos:inScheme rdf:resource="http://fakeIRI.edu/terms/remotesensingclo"/><skos:prefLabel xml:lang="en">90-100%</skos:prefLabel><skos:definition xml:lang="en">Cloud cover present when an image was taken was between 90 and 100%.</skos:definition><skos:notation xml:lang="en">9</skos:notation></rdf:Description>
   
   <rdf:Description rdf:about="http://fakeIRI.edu/terms/remotesensingclo#n"><rdf:type rdf:resource="http://www.w3.org/2004/02/skos/core#Concept"/><skos:inScheme rdf:resource="http://fakeIRI.edu/terms/remotesensingclo"/><skos:prefLabel xml:lang="en">not applicable</skos:prefLabel><skos:definition xml:lang="en">Cloud cover is not applicable to the image.</skos:definition><skos:notation xml:lang="en">n</skos:notation></rdf:Description>
   
   <rdf:Description rdf:about="http://fakeIRI.edu/terms/remotesensingclo#u"><rdf:type rdf:resource="http://www.w3.org/2004/02/skos/core#Concept"/><skos:inScheme rdf:resource="http://fakeIRI.edu/terms/remotesensingclo"/><skos:prefLabel xml:lang="en">unknown</skos:prefLabel><skos:definition xml:lang="en">Amount of cloud cover is not known.</skos:definition><skos:notation xml:lang="en">u</skos:notation></rdf:Description>
</rdf:RDF>