@prefix dc: <http://purl.org/dc/elements/1.1/> .
@prefix dct: <http://purl.org/dc/terms/> .
@prefix schema: <https://schema.org/> .
@prefix skos: <http://www.w3.org/2004/02/skos/core#> .

<https://doi.org/10.6069/uwlswd.xmqe-4733#0> a skos:Concept ;
    skos:definition """Cloud cover present when an image was taken was between 0 and
         9%."""@en ;
    skos:inScheme <https://doi.org/10.6069/uwlswd.xmqe-4733> ;
    skos:notation "0" ;
    skos:prefLabel "0-9%"@en .

<https://doi.org/10.6069/uwlswd.xmqe-4733#1> a skos:Concept ;
    skos:definition """Cloud cover present when an image was taken was between 10 and
         19%."""@en ;
    skos:inScheme <https://doi.org/10.6069/uwlswd.xmqe-4733> ;
    skos:notation "1" ;
    skos:prefLabel "10-19%"@en .

<https://doi.org/10.6069/uwlswd.xmqe-4733#2> a skos:Concept ;
    skos:definition """Cloud cover present when an image was taken was between 20 and
         29%."""@en ;
    skos:inScheme <https://doi.org/10.6069/uwlswd.xmqe-4733> ;
    skos:notation "2" ;
    skos:prefLabel "20-29%"@en .

<https://doi.org/10.6069/uwlswd.xmqe-4733#3> a skos:Concept ;
    skos:definition """Cloud cover present when an image was taken was between 30 and
         39%."""@en ;
    skos:inScheme <https://doi.org/10.6069/uwlswd.xmqe-4733> ;
    skos:notation "3" ;
    skos:prefLabel "30-39%"@en .

<https://doi.org/10.6069/uwlswd.xmqe-4733#4> a skos:Concept ;
    skos:definition """Cloud cover present when an image was taken was between 40 and
         49%."""@en ;
    skos:inScheme <https://doi.org/10.6069/uwlswd.xmqe-4733> ;
    skos:notation "4" ;
    skos:prefLabel "40-49%"@en .

<https://doi.org/10.6069/uwlswd.xmqe-4733#5> a skos:Concept ;
    skos:definition """Cloud cover present when an image was taken was between 50 and
         59%."""@en ;
    skos:inScheme <https://doi.org/10.6069/uwlswd.xmqe-4733> ;
    skos:notation "5" ;
    skos:prefLabel "50-59%"@en .

<https://doi.org/10.6069/uwlswd.xmqe-4733#6> a skos:Concept ;
    skos:definition """Cloud cover present when an image was taken was between 60 and
         69%."""@en ;
    skos:inScheme <https://doi.org/10.6069/uwlswd.xmqe-4733> ;
    skos:notation "6" ;
    skos:prefLabel "60-69%"@en .

<https://doi.org/10.6069/uwlswd.xmqe-4733#7> a skos:Concept ;
    skos:definition """Cloud cover present when an image was taken was between 70 and
         79%."""@en ;
    skos:inScheme <https://doi.org/10.6069/uwlswd.xmqe-4733> ;
    skos:notation "7" ;
    skos:prefLabel "70-79%"@en .

<https://doi.org/10.6069/uwlswd.xmqe-4733#8> a skos:Concept ;
    skos:definition """Cloud cover present when an image was taken was between 80 and
         89%."""@en ;
    skos:inScheme <https://doi.org/10.6069/uwlswd.xmqe-4733> ;
    skos:notation "8" ;
    skos:prefLabel "80-89%"@en .

<https://doi.org/10.6069/uwlswd.xmqe-4733#9> a skos:Concept ;
    skos:definition """Cloud cover present when an image was taken was between 90 and
         100%."""@en ;
    skos:inScheme <https://doi.org/10.6069/uwlswd.xmqe-4733> ;
    skos:notation "9" ;
    skos:prefLabel "90-100%"@en .

<https://doi.org/10.6069/uwlswd.xmqe-4733#n> a skos:Concept ;
    skos:definition "Cloud cover is not applicable to the image."@en ;
    skos:inScheme <https://doi.org/10.6069/uwlswd.xmqe-4733> ;
    skos:notation "n" ;
    skos:prefLabel "not applicable"@en .

<https://doi.org/10.6069/uwlswd.xmqe-4733#u> a skos:Concept ;
    skos:definition "Amount of cloud cover is not known."@en ;
    skos:inScheme <https://doi.org/10.6069/uwlswd.xmqe-4733> ;
    skos:notation "u" ;
    skos:prefLabel "unknown"@en .

<https://doi.org/10.6069/uwlswd.xmqe-4733> a skos:ConceptScheme ;
    dc:contributor "Metadata Management Associates"@en ;
    dc:language "en" ;
    dct:alternative """MARC21 007/05 values for remote-sensing images expressed using
         RDF"""@en ;
    dct:contributor <http://viaf.org/viaf/151962300> ;
    dct:creator <http://viaf.org/viaf/139541794> ;
    dct:description """Amount of cloud cover that was present when a remote-sensing
         image was made."""@en ;
    dct:format <http://www.w3.org/ns/formats/Turtle> ;
    dct:hasFormat <https://uwlib-cams.github.io/uwlswd_vocabs_marc_007/remote-sensing_image_cloud_cover/remote-sensing_image_cloud_cover.html>,
        <https://uwlib-cams.github.io/uwlswd_vocabs_marc_007/remote-sensing_image_cloud_cover/remote-sensing_image_cloud_cover.jsonld>,
        <https://uwlib-cams.github.io/uwlswd_vocabs_marc_007/remote-sensing_image_cloud_cover/remote-sensing_image_cloud_cover.nt>,
        <https://uwlib-cams.github.io/uwlswd_vocabs_marc_007/remote-sensing_image_cloud_cover/remote-sensing_image_cloud_cover.rdf> ;
    dct:issued "2024" ;
    dct:license <http://creativecommons.org/publicdomain/zero/1.0> ;
    dct:provenance <https://doi.org/10.6069/uwlswd.2e2b-y833#marc00Xvalues> ;
    dct:publisher <http://viaf.org/viaf/139541794> ;
    dct:source <http://marc21rdf.info>,
        <https://www.loc.gov/marc/bibliographic/bd007.html> ;
    dct:title "Remote-sensing image: cloud cover"@en ;
    dct:type <http://purl.org/dc/dcmitype/Dataset> ;
    schema:disambiguatingDescription """SKOS Concept Scheme for MARC 00X
         Values"""@en ;
    schema:version "1-0-0" .

