<?xml version='1.0' encoding='UTF-8'?>
<rdf:RDF xmlns:dc="http://purl.org/dc/elements/1.1/" xmlns:dct="http://purl.org/dc/terms/" xmlns:rdf="http://www.w3.org/1999/02/22-rdf-syntax-ns#" xmlns:schema="https://schema.org/" xmlns:skos="http://www.w3.org/2004/02/skos/core#">
  <rdf:Description rdf:about="https://doi.org/10.6069/uwlswd.v463-4g79#v">
    <rdf:type rdf:resource="http://www.w3.org/2004/02/skos/core#Concept"/>
    <skos:inScheme rdf:resource="https://doi.org/10.6069/uwlswd.v463-4g79"/>
    <skos:prefLabel xml:lang="en">8 in.</skos:prefLabel>
    <skos:definition xml:lang="en">Diameter of the medium is 8 inches.</skos:definition>
    <skos:scopeNote xml:lang="en">Usually refers to the diameter of a magnetic disk or optical
         disc.</skos:scopeNote>
    <skos:notation>v</skos:notation>
  </rdf:Description>
  <rdf:Description rdf:about="https://doi.org/10.6069/uwlswd.v463-4g79">
    <rdf:type rdf:resource="http://www.w3.org/2004/02/skos/core#ConceptScheme"/>
    <dct:type rdf:resource="http://purl.org/dc/dcmitype/Dataset"/>
    <dct:title xml:lang="en">Electronic resource: dimensions</dct:title>
    <dct:alternative xml:lang="en">MARC21 007/04 values for electronic resources expressed using
         RDF</dct:alternative>
    <dct:description xml:lang="en">Dimensions of the medium used to encode the electronic
         resource.</dct:description>
    <schema:disambiguatingDescription xml:lang="en">SKOS Concept Scheme for MARC 00X
         Values</schema:disambiguatingDescription>
    <dct:publisher rdf:resource="http://viaf.org/viaf/139541794"/>
    <dct:source rdf:resource="https://www.loc.gov/marc/bibliographic/bd007.html"/>
    <dct:source rdf:resource="http://marc21rdf.info"/>
    <dct:provenance rdf:resource="https://doi.org/10.6069/uwlswd.2e2b-y833#marc00Xvalues"/>
    <dct:creator rdf:resource="http://viaf.org/viaf/139541794"/>
    <dct:contributor rdf:resource="http://viaf.org/viaf/151962300"/>
    <dct:issued>2024</dct:issued>
    <dc:contributor xml:lang="en">Metadata Management Associates</dc:contributor>
    <dc:language>en</dc:language>
    <dct:license rdf:resource="http://creativecommons.org/publicdomain/zero/1.0"/>
    <schema:version>1-0-0</schema:version>
    <dct:format rdf:resource="http://www.w3.org/ns/formats/RDF_XML"/>
  </rdf:Description>
  <rdf:Description rdf:about="https://doi.org/10.6069/uwlswd.v463-4g79#a">
    <rdf:type rdf:resource="http://www.w3.org/2004/02/skos/core#Concept"/>
    <skos:inScheme rdf:resource="https://doi.org/10.6069/uwlswd.v463-4g79"/>
    <skos:prefLabel xml:lang="en">3 1/2 in.</skos:prefLabel>
    <skos:definition xml:lang="en">Diameter of the medium is 3 1/2 inches.</skos:definition>
    <skos:scopeNote xml:lang="en">Usually refers to the diameter of a magnetic
         disk.</skos:scopeNote>
    <skos:notation>a</skos:notation>
  </rdf:Description>
  <rdf:Description rdf:about="https://doi.org/10.6069/uwlswd.v463-4g79#n">
    <rdf:type rdf:resource="http://www.w3.org/2004/02/skos/core#Concept"/>
    <skos:inScheme rdf:resource="https://doi.org/10.6069/uwlswd.v463-4g79"/>
    <skos:prefLabel xml:lang="en">not applicable</skos:prefLabel>
    <skos:definition xml:lang="en">Physical dimensions are not applicable to the electronic
         resource.</skos:definition>
    <skos:scopeNote xml:lang="en">Appropriate for remote electronic resources and electronic
         resources whose specific medium varies.</skos:scopeNote>
    <skos:notation>n</skos:notation>
  </rdf:Description>
  <rdf:Description rdf:about="https://doi.org/10.6069/uwlswd.v463-4g79#z">
    <rdf:type rdf:resource="http://www.w3.org/2004/02/skos/core#Concept"/>
    <skos:inScheme rdf:resource="https://doi.org/10.6069/uwlswd.v463-4g79"/>
    <skos:prefLabel xml:lang="en">other</skos:prefLabel>
    <skos:definition xml:lang="en">Dimensions other than 3 1/2 in., 12 in., 4 3/4 in. or 12 cm., 1
         1/8 x 2 3/8 in., 3 7/8 x 2 1/2 in., 5 1/4 in., or 8 in.</skos:definition>
    <skos:notation>z</skos:notation>
  </rdf:Description>
  <rdf:Description rdf:about="https://doi.org/10.6069/uwlswd.v463-4g79#j">
    <rdf:type rdf:resource="http://www.w3.org/2004/02/skos/core#Concept"/>
    <skos:inScheme rdf:resource="https://doi.org/10.6069/uwlswd.v463-4g79"/>
    <skos:prefLabel xml:lang="en">3 7/8 x 2 1/2 in.</skos:prefLabel>
    <skos:definition xml:lang="en">Dimensions of the container used for the medium are 3 7/8 x 2
         1/2 inches.</skos:definition>
    <skos:scopeNote xml:lang="en">Usually refers to cartridges.</skos:scopeNote>
    <skos:notation>j</skos:notation>
  </rdf:Description>
  <rdf:Description rdf:about="https://doi.org/10.6069/uwlswd.v463-4g79#u">
    <rdf:type rdf:resource="http://www.w3.org/2004/02/skos/core#Concept"/>
    <skos:inScheme rdf:resource="https://doi.org/10.6069/uwlswd.v463-4g79"/>
    <skos:prefLabel xml:lang="en">unknown</skos:prefLabel>
    <skos:definition xml:lang="en">Dimensions of the medium used for the electronic resource are
         not known.</skos:definition>
    <skos:notation>u</skos:notation>
  </rdf:Description>
  <rdf:Description rdf:about="https://doi.org/10.6069/uwlswd.v463-4g79#e">
    <rdf:type rdf:resource="http://www.w3.org/2004/02/skos/core#Concept"/>
    <skos:inScheme rdf:resource="https://doi.org/10.6069/uwlswd.v463-4g79"/>
    <skos:prefLabel xml:lang="en">12 in.</skos:prefLabel>
    <skos:definition xml:lang="en">Diameter of the medium is 12 inches.</skos:definition>
    <skos:scopeNote xml:lang="en">Usually refers to optical or magneto-optical
         disc.</skos:scopeNote>
    <skos:notation>e</skos:notation>
  </rdf:Description>
  <rdf:Description rdf:about="https://doi.org/10.6069/uwlswd.v463-4g79#g">
    <rdf:type rdf:resource="http://www.w3.org/2004/02/skos/core#Concept"/>
    <skos:inScheme rdf:resource="https://doi.org/10.6069/uwlswd.v463-4g79"/>
    <skos:prefLabel xml:lang="en">4 3/4 in. or 12 cm.</skos:prefLabel>
    <skos:definition xml:lang="en">Diameter of the medium is 4 3/4 inches (or 12
         cm.).</skos:definition>
    <skos:scopeNote xml:lang="en">Usually refers to optical or magneto-optical
         disc.</skos:scopeNote>
    <skos:notation>g</skos:notation>
  </rdf:Description>
  <rdf:Description rdf:about="https://doi.org/10.6069/uwlswd.v463-4g79#o">
    <rdf:type rdf:resource="http://www.w3.org/2004/02/skos/core#Concept"/>
    <skos:inScheme rdf:resource="https://doi.org/10.6069/uwlswd.v463-4g79"/>
    <skos:prefLabel xml:lang="en">5 1/4 in.</skos:prefLabel>
    <skos:definition xml:lang="en">Diameter of the medium is 5 1/4 inches.</skos:definition>
    <skos:scopeNote xml:lang="en">Usually refers to the dimensions of a magnetic
         disk.</skos:scopeNote>
    <skos:notation>o</skos:notation>
  </rdf:Description>
  <rdf:Description rdf:about="https://doi.org/10.6069/uwlswd.v463-4g79#i">
    <rdf:type rdf:resource="http://www.w3.org/2004/02/skos/core#Concept"/>
    <skos:inScheme rdf:resource="https://doi.org/10.6069/uwlswd.v463-4g79"/>
    <skos:prefLabel xml:lang="en">1 1/8 x 2 3/8 in.</skos:prefLabel>
    <skos:definition xml:lang="en">Dimensions of the container used for the medium are 1 1/8 x 2
         3/8 inches.</skos:definition>
    <skos:scopeNote xml:lang="en">Usually refers to cartridges.</skos:scopeNote>
    <skos:notation>i</skos:notation>
  </rdf:Description>
</rdf:RDF>