@prefix dc: <http://purl.org/dc/elements/1.1/> .
@prefix dct: <http://purl.org/dc/terms/> .
@prefix schema: <https://schema.org/> .
@prefix skos: <http://www.w3.org/2004/02/skos/core#> .

<https://doi.org/10.6069/uwlswd.v463-4g79#a> a skos:Concept ;
    skos:definition "Diameter of the medium is 3 1/2 inches."@en ;
    skos:inScheme <https://doi.org/10.6069/uwlswd.v463-4g79> ;
    skos:notation "a" ;
    skos:prefLabel "3 1/2 in."@en ;
    skos:scopeNote """Usually refers to the diameter of a magnetic
         disk."""@en .

<https://doi.org/10.6069/uwlswd.v463-4g79#e> a skos:Concept ;
    skos:definition "Diameter of the medium is 12 inches."@en ;
    skos:inScheme <https://doi.org/10.6069/uwlswd.v463-4g79> ;
    skos:notation "e" ;
    skos:prefLabel "12 in."@en ;
    skos:scopeNote """Usually refers to optical or magneto-optical
         disc."""@en .

<https://doi.org/10.6069/uwlswd.v463-4g79#g> a skos:Concept ;
    skos:definition """Diameter of the medium is 4 3/4 inches (or 12
         cm.)."""@en ;
    skos:inScheme <https://doi.org/10.6069/uwlswd.v463-4g79> ;
    skos:notation "g" ;
    skos:prefLabel "4 3/4 in. or 12 cm."@en ;
    skos:scopeNote """Usually refers to optical or magneto-optical
         disc."""@en .

<https://doi.org/10.6069/uwlswd.v463-4g79#i> a skos:Concept ;
    skos:definition """Dimensions of the container used for the medium are 1 1/8 x 2
         3/8 inches."""@en ;
    skos:inScheme <https://doi.org/10.6069/uwlswd.v463-4g79> ;
    skos:notation "i" ;
    skos:prefLabel "1 1/8 x 2 3/8 in."@en ;
    skos:scopeNote "Usually refers to cartridges."@en .

<https://doi.org/10.6069/uwlswd.v463-4g79#j> a skos:Concept ;
    skos:definition """Dimensions of the container used for the medium are 3 7/8 x 2
         1/2 inches."""@en ;
    skos:inScheme <https://doi.org/10.6069/uwlswd.v463-4g79> ;
    skos:notation "j" ;
    skos:prefLabel "3 7/8 x 2 1/2 in."@en ;
    skos:scopeNote "Usually refers to cartridges."@en .

<https://doi.org/10.6069/uwlswd.v463-4g79#n> a skos:Concept ;
    skos:definition """Physical dimensions are not applicable to the electronic
         resource."""@en ;
    skos:inScheme <https://doi.org/10.6069/uwlswd.v463-4g79> ;
    skos:notation "n" ;
    skos:prefLabel "not applicable"@en ;
    skos:scopeNote """Appropriate for remote electronic resources and electronic
         resources whose specific medium varies."""@en .

<https://doi.org/10.6069/uwlswd.v463-4g79#o> a skos:Concept ;
    skos:definition "Diameter of the medium is 5 1/4 inches."@en ;
    skos:inScheme <https://doi.org/10.6069/uwlswd.v463-4g79> ;
    skos:notation "o" ;
    skos:prefLabel "5 1/4 in."@en ;
    skos:scopeNote """Usually refers to the dimensions of a magnetic
         disk."""@en .

<https://doi.org/10.6069/uwlswd.v463-4g79#u> a skos:Concept ;
    skos:definition """Dimensions of the medium used for the electronic resource are
         not known."""@en ;
    skos:inScheme <https://doi.org/10.6069/uwlswd.v463-4g79> ;
    skos:notation "u" ;
    skos:prefLabel "unknown"@en .

<https://doi.org/10.6069/uwlswd.v463-4g79#v> a skos:Concept ;
    skos:definition "Diameter of the medium is 8 inches."@en ;
    skos:inScheme <https://doi.org/10.6069/uwlswd.v463-4g79> ;
    skos:notation "v" ;
    skos:prefLabel "8 in."@en ;
    skos:scopeNote """Usually refers to the diameter of a magnetic disk or optical
         disc."""@en .

<https://doi.org/10.6069/uwlswd.v463-4g79#z> a skos:Concept ;
    skos:definition """Dimensions other than 3 1/2 in., 12 in., 4 3/4 in. or 12 cm., 1
         1/8 x 2 3/8 in., 3 7/8 x 2 1/2 in., 5 1/4 in., or 8 in."""@en ;
    skos:inScheme <https://doi.org/10.6069/uwlswd.v463-4g79> ;
    skos:notation "z" ;
    skos:prefLabel "other"@en .

<https://doi.org/10.6069/uwlswd.v463-4g79> a skos:ConceptScheme ;
    dc:contributor "Metadata Management Associates"@en ;
    dc:language "en" ;
    dct:alternative """MARC21 007/04 values for electronic resources expressed using
         RDF"""@en ;
    dct:contributor <http://viaf.org/viaf/151962300> ;
    dct:creator <http://viaf.org/viaf/139541794> ;
    dct:description """Dimensions of the medium used to encode the electronic
         resource."""@en ;
    dct:format <http://www.w3.org/ns/formats/Turtle> ;
    dct:hasFormat <https://uwlib-cams.github.io/uwlswd_vocabs_marc_007/electronic_resource_dimensions/electronic_resource_dimensions.html>,
        <https://uwlib-cams.github.io/uwlswd_vocabs_marc_007/electronic_resource_dimensions/electronic_resource_dimensions.jsonld>,
        <https://uwlib-cams.github.io/uwlswd_vocabs_marc_007/electronic_resource_dimensions/electronic_resource_dimensions.nt>,
        <https://uwlib-cams.github.io/uwlswd_vocabs_marc_007/electronic_resource_dimensions/electronic_resource_dimensions.rdf> ;
    dct:issued "2024" ;
    dct:license <http://creativecommons.org/publicdomain/zero/1.0> ;
    dct:provenance <https://doi.org/10.6069/uwlswd.2e2b-y833#marc00Xvalues> ;
    dct:publisher <http://viaf.org/viaf/139541794> ;
    dct:source <http://marc21rdf.info>,
        <https://www.loc.gov/marc/bibliographic/bd007.html> ;
    dct:title "Electronic resource: dimensions"@en ;
    dct:type <http://purl.org/dc/dcmitype/Dataset> ;
    schema:disambiguatingDescription """SKOS Concept Scheme for MARC 00X
         Values"""@en ;
    schema:version "1-0-0" .

