<?xml version="1.0" encoding="utf-8"?>
<rdf:RDF
   xmlns:dc="http://purl.org/dc/elements/1.1/"
   xmlns:dct="http://purl.org/dc/terms/"
   xmlns:rdf="http://www.w3.org/1999/02/22-rdf-syntax-ns#"
   xmlns:schema="https://schema.org/"
   xmlns:skos="http://www.w3.org/2004/02/skos/core#"
>
  <rdf:Description rdf:about="https://doi.org/10.6069/uwlswd.dfav-1729">
    <rdf:type rdf:resource="http://www.w3.org/2004/02/skos/core#ConceptScheme"/>
    <dct:type rdf:resource="http://purl.org/dc/dcmitype/Dataset"/>
    <dct:title xml:lang="en">Motion picture: deterioration stage</dct:title>
    <dct:alternative xml:lang="en">MARC21 007/15 values for motion pictures expressed using
         RDF</dct:alternative>
    <dct:description xml:lang="en">Level of deterioration of the motion picture
         film.</dct:description>
    <schema:disambiguatingDescription xml:lang="en">SKOS Concept Scheme for MARC 00X
         Values</schema:disambiguatingDescription>
    <dct:publisher rdf:resource="http://viaf.org/viaf/139541794"/>
    <dct:source rdf:resource="https://www.loc.gov/marc/bibliographic/bd007.html"/>
    <dct:source rdf:resource="http://marc21rdf.info"/>
    <dct:provenance rdf:resource="https://doi.org/10.6069/uwlswd.2e2b-y833#marc00Xvalues"/>
    <dct:creator rdf:resource="http://viaf.org/viaf/139541794"/>
    <dct:contributor rdf:resource="http://viaf.org/viaf/151962300"/>
    <dct:issued>2024</dct:issued>
    <dc:contributor xml:lang="en">Metadata Management Associates</dc:contributor>
    <dc:language>en</dc:language>
    <dct:license rdf:resource="http://creativecommons.org/publicdomain/zero/1.0"/>
    <schema:version>1-0-0</schema:version>
    <dct:format rdf:resource="http://www.w3.org/ns/formats/RDF_XML"/>
    <dct:hasFormat rdf:resource="https://uwlib-cams.github.io/uwlswd_vocabs_marc_007/motion_picture_deterioration_stage/motion_picture_deterioration_stage.ttl"/>
    <dct:hasFormat rdf:resource="https://uwlib-cams.github.io/uwlswd_vocabs_marc_007/motion_picture_deterioration_stage/motion_picture_deterioration_stage.nt"/>
    <dct:hasFormat rdf:resource="https://uwlib-cams.github.io/uwlswd_vocabs_marc_007/motion_picture_deterioration_stage/motion_picture_deterioration_stage.jsonld"/>
    <dct:hasFormat rdf:resource="https://uwlib-cams.github.io/uwlswd_vocabs_marc_007/motion_picture_deterioration_stage/motion_picture_deterioration_stage.html"/>
  </rdf:Description>
  <rdf:Description rdf:about="https://doi.org/10.6069/uwlswd.dfav-1729#g">
    <rdf:type rdf:resource="http://www.w3.org/2004/02/skos/core#Concept"/>
    <skos:inScheme rdf:resource="https://doi.org/10.6069/uwlswd.dfav-1729"/>
    <skos:prefLabel xml:lang="en">nitrate: congealed</skos:prefLabel>
    <skos:definition xml:lang="en">Deterioration of nitrate materials characterized as
         congealed.</skos:definition>
    <skos:notation>g</skos:notation>
  </rdf:Description>
  <rdf:Description rdf:about="https://doi.org/10.6069/uwlswd.dfav-1729#f">
    <rdf:type rdf:resource="http://www.w3.org/2004/02/skos/core#Concept"/>
    <skos:inScheme rdf:resource="https://doi.org/10.6069/uwlswd.dfav-1729"/>
    <skos:prefLabel xml:lang="en">nitrate: frothy, bubbles, blisters</skos:prefLabel>
    <skos:definition xml:lang="en">Deterioration of nitrate materials characterized as frothy,
         bubbles, or blisters.</skos:definition>
    <skos:notation>f</skos:notation>
  </rdf:Description>
  <rdf:Description rdf:about="https://doi.org/10.6069/uwlswd.dfav-1729#d">
    <rdf:type rdf:resource="http://www.w3.org/2004/02/skos/core#Concept"/>
    <skos:inScheme rdf:resource="https://doi.org/10.6069/uwlswd.dfav-1729"/>
    <skos:prefLabel xml:lang="en">nitrate: brownish, discoloration, fading, dusty</skos:prefLabel>
    <skos:definition xml:lang="en">Deterioration of nitrate materials characterized as brownish,
         discoloration, fading, or dusty.</skos:definition>
    <skos:notation>d</skos:notation>
  </rdf:Description>
  <rdf:Description rdf:about="https://doi.org/10.6069/uwlswd.dfav-1729#a">
    <rdf:type rdf:resource="http://www.w3.org/2004/02/skos/core#Concept"/>
    <skos:inScheme rdf:resource="https://doi.org/10.6069/uwlswd.dfav-1729"/>
    <skos:prefLabel xml:lang="en">none apparent</skos:prefLabel>
    <skos:definition xml:lang="en">No deterioration is apparent on either nitrate or non-nitrate
         motion picture film.</skos:definition>
    <skos:notation>a</skos:notation>
  </rdf:Description>
  <rdf:Description rdf:about="https://doi.org/10.6069/uwlswd.dfav-1729#b">
    <rdf:type rdf:resource="http://www.w3.org/2004/02/skos/core#Concept"/>
    <skos:inScheme rdf:resource="https://doi.org/10.6069/uwlswd.dfav-1729"/>
    <skos:prefLabel xml:lang="en">nitrate: suspicious odor</skos:prefLabel>
    <skos:definition xml:lang="en">Deterioration of nitrate materials characterized as suspicious
         odor.</skos:definition>
    <skos:notation>b</skos:notation>
  </rdf:Description>
  <rdf:Description rdf:about="https://doi.org/10.6069/uwlswd.dfav-1729#m">
    <rdf:type rdf:resource="http://www.w3.org/2004/02/skos/core#Concept"/>
    <skos:inScheme rdf:resource="https://doi.org/10.6069/uwlswd.dfav-1729"/>
    <skos:prefLabel xml:lang="en">non-nitrate: disaster</skos:prefLabel>
    <skos:definition xml:lang="en">Deterioration of non-nitrate materials (safety film, etc.)
         characterized as disaster.</skos:definition>
    <skos:notation>m</skos:notation>
  </rdf:Description>
  <rdf:Description rdf:about="https://doi.org/10.6069/uwlswd.dfav-1729#k">
    <rdf:type rdf:resource="http://www.w3.org/2004/02/skos/core#Concept"/>
    <skos:inScheme rdf:resource="https://doi.org/10.6069/uwlswd.dfav-1729"/>
    <skos:prefLabel xml:lang="en">non-nitrate: detectable deterioration</skos:prefLabel>
    <skos:definition xml:lang="en">Deterioration of non-nitrate materials (safety film, etc.)
         characterized as detectable deterioration.</skos:definition>
    <skos:notation>k</skos:notation>
  </rdf:Description>
  <rdf:Description rdf:about="https://doi.org/10.6069/uwlswd.dfav-1729#e">
    <rdf:type rdf:resource="http://www.w3.org/2004/02/skos/core#Concept"/>
    <skos:inScheme rdf:resource="https://doi.org/10.6069/uwlswd.dfav-1729"/>
    <skos:prefLabel xml:lang="en">nitrate: sticky</skos:prefLabel>
    <skos:definition xml:lang="en">Deterioration of nitrate materials characterized as
         sticky.</skos:definition>
    <skos:notation>e</skos:notation>
  </rdf:Description>
  <rdf:Description rdf:about="https://doi.org/10.6069/uwlswd.dfav-1729#l">
    <rdf:type rdf:resource="http://www.w3.org/2004/02/skos/core#Concept"/>
    <skos:inScheme rdf:resource="https://doi.org/10.6069/uwlswd.dfav-1729"/>
    <skos:prefLabel xml:lang="en">non-nitrate: advanced deterioration</skos:prefLabel>
    <skos:definition xml:lang="en">Deterioration of non-nitrate materials (safety film, etc.)
         characterized as advanced deterioration.</skos:definition>
    <skos:notation>l</skos:notation>
  </rdf:Description>
  <rdf:Description rdf:about="https://doi.org/10.6069/uwlswd.dfav-1729#c">
    <rdf:type rdf:resource="http://www.w3.org/2004/02/skos/core#Concept"/>
    <skos:inScheme rdf:resource="https://doi.org/10.6069/uwlswd.dfav-1729"/>
    <skos:prefLabel xml:lang="en">nitrate: pungent odor</skos:prefLabel>
    <skos:definition xml:lang="en">Deterioration of nitrate materials characterized as pungent
         odor.</skos:definition>
    <skos:notation>c</skos:notation>
  </rdf:Description>
  <rdf:Description rdf:about="https://doi.org/10.6069/uwlswd.dfav-1729#h">
    <rdf:type rdf:resource="http://www.w3.org/2004/02/skos/core#Concept"/>
    <skos:inScheme rdf:resource="https://doi.org/10.6069/uwlswd.dfav-1729"/>
    <skos:prefLabel xml:lang="en">nitrate: powder</skos:prefLabel>
    <skos:definition xml:lang="en">Deterioration of nitrate materials characterized as
         powder.</skos:definition>
    <skos:notation>h</skos:notation>
  </rdf:Description>
</rdf:RDF>
