@prefix dc: <http://purl.org/dc/elements/1.1/> .
@prefix dct: <http://purl.org/dc/terms/> .
@prefix schema: <https://schema.org/> .
@prefix skos: <http://www.w3.org/2004/02/skos/core#> .

<https://doi.org/10.6069/uwlswd.gdvf-z086#a> a skos:Concept ;
    skos:definition """Three layers of emulsion: cyan, magenta, and yellow. Each layer
         is sensitive to its own primary color."""@en ;
    skos:inScheme <https://doi.org/10.6069/uwlswd.gdvf-z086> ;
    skos:notation "a" ;
    skos:prefLabel "3 layer color"@en ;
    skos:scopeNote """Beginning in the early 1950s, color film work has been done
         primarily on 3 layer, also called multilayer, film. This process is also known as integral
         tri-pack."""@en .

<https://doi.org/10.6069/uwlswd.gdvf-z086#b> a skos:Concept ;
    skos:definition """Single strip of film was exposed with pairs of images by means
         of a beam-splitter prism. One of the pairs of images was exposed through a red filter and
         one through a green filter. The resulting negative was used to produce both prints
         consisting of two strips cemented together, and, later in the history of the process, two
         color dye transfer prints."""@en ;
    skos:inScheme <https://doi.org/10.6069/uwlswd.gdvf-z086> ;
    skos:notation "b" ;
    skos:prefLabel "2 color, single strip"@en ;
    skos:scopeNote """Also known as red and green Technicolor, the process was used
         exclusively by Technicolor and had its heyday between 1922 and 1933, although it was used
         until 1936 for animated cartoons."""@en .

<https://doi.org/10.6069/uwlswd.gdvf-z086#c> a skos:Concept ;
    skos:definition """System of color reproduction, which cannot be specifically
         identified, in which the visible spectrum is divided either into blue and red regions or
         into green and red regions for recording and presentation."""@en ;
    skos:inScheme <https://doi.org/10.6069/uwlswd.gdvf-z086> ;
    skos:notation "c" ;
    skos:prefLabel "undetermined 2 color"@en ;
    skos:scopeNote """Although extensively used in early color film processes, the
         inherent inability of two components to reproduce a satisfactory range of hues rendered all
         such systems obsolete when three-color processes became readily available and relatively
         inexpensive."""@en .

<https://doi.org/10.6069/uwlswd.gdvf-z086#d> a skos:Concept ;
    skos:definition """System of color reproduction, which cannot be specifically
         identified, in which the visible spectrum is divided into three sections, normally red,
         green, and blue, for the purposes of recording and presentation."""@en ;
    skos:inScheme <https://doi.org/10.6069/uwlswd.gdvf-z086> ;
    skos:notation "d" ;
    skos:prefLabel "undetermined 3 color"@en .

<https://doi.org/10.6069/uwlswd.gdvf-z086#e> a skos:Concept ;
    skos:definition """Color system in which three color-separation negatives were
         produced on black-and-white film."""@en ;
    skos:inScheme <https://doi.org/10.6069/uwlswd.gdvf-z086> ;
    skos:notation "e" ;
    skos:prefLabel "3 strip color"@en ;
    skos:scopeNote """3 strip color is often used synonymously with the trademark
         Technicolor. In the Technicolor three-component system, light reflected from the subject
         matter is transmitted through the single lens of a special camera where it strikes a prism.
         One part of the light is passed through the prism and a green filter to produce a green
         record. The remainder of the light is reflected from the prism and absorbed by negatives to
         produce red and blue records. Each of the negatives is developed to produce new negatives
         which resemble black-and-white negatives."""@en .

<https://doi.org/10.6069/uwlswd.gdvf-z086#f> a skos:Concept ;
    skos:definition """Color system in which two strips of film, one to record red
         light and one to record blue, were run through the camera simultaneously and exposed
         through the base of the front piece of film. These two strips of negatives were then used
         to produce prints of duplitized film stock (film stock with emulsion on both sides of the
         base), with a red-dyed image on one side, and a blue-dyed or -toned image on the
         other."""@en ;
    skos:inScheme <https://doi.org/10.6069/uwlswd.gdvf-z086> ;
    skos:notation "f" ;
    skos:prefLabel "2 strip color"@en ;
    skos:scopeNote """Although extensively used in early color film processes, the
         inherent inability of two components to reproduce the visible color spectrum rendered all
         such systems obsolete when three-color processes became readily available. The process used
         from about 1929 to about 1950 by, among others, the following companies: Cinecolor,
         Magnacolor, and Multicolor."""@en .

<https://doi.org/10.6069/uwlswd.gdvf-z086#g> a skos:Concept ;
    skos:definition """Cinecolor process, in which the color separation record of
         blue-green light prints as red. In the Super Cinecolor process, the color separation record
         of green light which prints as magenta (called "red" by Cinecolor). In the two-color
         Technicolor process, the color separation record of green light which prints as
         red."""@en ;
    skos:inScheme <https://doi.org/10.6069/uwlswd.gdvf-z086> ;
    skos:notation "g" ;
    skos:prefLabel "red strip"@en .

<https://doi.org/10.6069/uwlswd.gdvf-z086#h> a skos:Concept ;
    skos:definition """Cinecolor process and the Super Cinecolor process, in which the
         blue strip is the color separation record of red light which prints as blue-green (called
         "blue" by Cinecolor). In the two-color Technicolor process, the green strip is the color
         separation record of magenta-red light which prints as green."""@en ;
    skos:inScheme <https://doi.org/10.6069/uwlswd.gdvf-z086> ;
    skos:notation "h" ;
    skos:prefLabel "blue or green strip"@en .

<https://doi.org/10.6069/uwlswd.gdvf-z086#i> a skos:Concept ;
    skos:definition """Color separation record of red light which prints as
         cyan."""@en ;
    skos:inScheme <https://doi.org/10.6069/uwlswd.gdvf-z086> ;
    skos:notation "i" ;
    skos:prefLabel "cyan strip"@en .

<https://doi.org/10.6069/uwlswd.gdvf-z086#j> a skos:Concept ;
    skos:definition """Color separation record of green light which prints as
         magenta."""@en ;
    skos:inScheme <https://doi.org/10.6069/uwlswd.gdvf-z086> ;
    skos:notation "j" ;
    skos:prefLabel "magenta strip"@en .

<https://doi.org/10.6069/uwlswd.gdvf-z086#k> a skos:Concept ;
    skos:definition """Color separation record of blue light which prints as
         yellow."""@en ;
    skos:inScheme <https://doi.org/10.6069/uwlswd.gdvf-z086> ;
    skos:notation "k" ;
    skos:prefLabel "yellow strip"@en .

<https://doi.org/10.6069/uwlswd.gdvf-z086#l> a skos:Concept ;
    skos:definition """Successive exposure negative 2. S E N 2 is a method of motion
         picture color photography in which two color separation negative images were recorded on
         one strip of film by photographing each frame two times successively through red and blue
         filters. The resultant negative was subsequently optically printed by the use of a
         skip-frame mechanism."""@en ;
    skos:inScheme <https://doi.org/10.6069/uwlswd.gdvf-z086> ;
    skos:notation "l" ;
    skos:prefLabel "S E N 2"@en ;
    skos:scopeNote """The process was restricted to the photography of animated
         cartoon and puppet subjects in which the movement from frame to frame could be controlled.
         The successive exposure process was rendered obsolete by the introduction of 3 layer
         (multilayer) color negative film."""@en .

<https://doi.org/10.6069/uwlswd.gdvf-z086#m> a skos:Concept ;
    skos:definition """Successive exposure negative 3. S E N 3 is a method of motion
         picture color photography in which three color separation negative images were recorded on
         one strip of film by photographing each frame three times successively through red, blue,
         and green filters. The resultant negative was subsequently optically printed by the use of
         a skip-frame mechanism."""@en ;
    skos:inScheme <https://doi.org/10.6069/uwlswd.gdvf-z086> ;
    skos:notation "m" ;
    skos:prefLabel "S E N 3"@en ;
    skos:scopeNote """The process was usually restricted to the photography of
         animated cartoon and puppet subjects in which the movement from frame to frame could be
         controlled. The successive exposure process was rarely used after the introduction of 3
         layer (multilayer) color negative film."""@en .

<https://doi.org/10.6069/uwlswd.gdvf-z086#n> a skos:Concept ;
    skos:definition "Item is not a color film."@en ;
    skos:inScheme <https://doi.org/10.6069/uwlswd.gdvf-z086> ;
    skos:notation "n" ;
    skos:prefLabel "not applicable"@en .

<https://doi.org/10.6069/uwlswd.gdvf-z086#p> a skos:Concept ;
    skos:definition """A conversion of a black-and-white image in silver to sepia (a
         brownish grey to dark olive brown) by metallic compounds."""@en ;
    skos:inScheme <https://doi.org/10.6069/uwlswd.gdvf-z086> ;
    skos:notation "p" ;
    skos:prefLabel "sepia tone"@en ;
    skos:scopeNote """Sepia was the most common tone used, and was used in
         black-and-white prints of films for special sequences to enhance the dramatic or pictorial
         effect."""@en .

<https://doi.org/10.6069/uwlswd.gdvf-z086#q> a skos:Concept ;
    skos:definition """Color created by chemically altering the color, for example,
         uranium produces red, or increasing the brilliance of a print. Toning differs from tinting
         in that the clear portions of the film remain unaffected. Only the silver image of the
         positive film becomes colored."""@en ;
    skos:inScheme <https://doi.org/10.6069/uwlswd.gdvf-z086> ;
    skos:notation "q" ;
    skos:prefLabel "other tone"@en .

<https://doi.org/10.6069/uwlswd.gdvf-z086#r> a skos:Concept ;
    skos:definition """Early in the history of tinting, a tint was created by dipping
         film in a bath of chemical dyes to get a dominant hue. Later raw stock became available
         already tinted in eleven stock shades: peach blow, blue for moonlight, amber for firelight,
         etc."""@en ;
    skos:inScheme <https://doi.org/10.6069/uwlswd.gdvf-z086> ;
    skos:notation "r" ;
    skos:prefLabel "tint"@en ;
    skos:scopeNote """The tinting of a film may be in whole or in part. Tinting was
         common until the advent of sound."""@en .

<https://doi.org/10.6069/uwlswd.gdvf-z086#s> a skos:Concept ;
    skos:definition """Color has been added to a film by using a tinted base and a
         toned emulsion."""@en ;
    skos:inScheme <https://doi.org/10.6069/uwlswd.gdvf-z086> ;
    skos:notation "s" ;
    skos:prefLabel "tinted and toned"@en .

<https://doi.org/10.6069/uwlswd.gdvf-z086#t> a skos:Concept ;
    skos:definition """Color is added using stencils, one cut for each
         color."""@en ;
    skos:inScheme <https://doi.org/10.6069/uwlswd.gdvf-z086> ;
    skos:notation "t" ;
    skos:prefLabel "stencil color"@en ;
    skos:scopeNote """Stencil color replaced the hand-coloring used in earlier
         years."""@en .

<https://doi.org/10.6069/uwlswd.gdvf-z086#u> a skos:Concept ;
    skos:definition "Refined category of color is not known."@en ;
    skos:inScheme <https://doi.org/10.6069/uwlswd.gdvf-z086> ;
    skos:notation "u" ;
    skos:prefLabel "unknown"@en .

<https://doi.org/10.6069/uwlswd.gdvf-z086#v> a skos:Concept ;
    skos:definition """Image, produced by a photographic process, is hand
         colored."""@en ;
    skos:inScheme <https://doi.org/10.6069/uwlswd.gdvf-z086> ;
    skos:notation "v" ;
    skos:prefLabel "hand colored"@en .

<https://doi.org/10.6069/uwlswd.gdvf-z086#z> a skos:Concept ;
    skos:definition """Refined categories of color other than 3 layer color, 2 color
         single strip, undetermined 2 color, undetermined 3 color, 3 strip color 2 strip color, red
         strip, blue or green strip, cyan strip, magenta strip, yellow strip, S E N 2, S E N 3,
         sepia tone, other tone, tint, tinted and toned, stencil color, or hand
         colored."""@en ;
    skos:inScheme <https://doi.org/10.6069/uwlswd.gdvf-z086> ;
    skos:notation "z" ;
    skos:prefLabel "other"@en .

<https://doi.org/10.6069/uwlswd.gdvf-z086> a skos:ConceptScheme ;
    dc:contributor "Metadata Management Associates"@en ;
    dc:language "en" ;
    dct:alternative """MARC21 007/13 values for motion pictures expressed using
         RDF"""@en ;
    dct:contributor <http://viaf.org/viaf/151962300> ;
    dct:creator <http://viaf.org/viaf/139541794> ;
    dct:description """Specific color characteristics of the moving
         image."""@en ;
    dct:format <http://www.w3.org/ns/formats/Turtle> ;
    dct:hasFormat <https://uwlib-cams.github.io/uwlswd_vocabs_marc_007/motion_picture_refined_categories_of_color/motion_picture_refined_categories_of_color.html>,
        <https://uwlib-cams.github.io/uwlswd_vocabs_marc_007/motion_picture_refined_categories_of_color/motion_picture_refined_categories_of_color.jsonld>,
        <https://uwlib-cams.github.io/uwlswd_vocabs_marc_007/motion_picture_refined_categories_of_color/motion_picture_refined_categories_of_color.nt>,
        <https://uwlib-cams.github.io/uwlswd_vocabs_marc_007/motion_picture_refined_categories_of_color/motion_picture_refined_categories_of_color.rdf> ;
    dct:issued "2024" ;
    dct:license <http://creativecommons.org/publicdomain/zero/1.0> ;
    dct:provenance <https://doi.org/10.6069/uwlswd.2e2b-y833#marc00Xvalues> ;
    dct:publisher <http://viaf.org/viaf/139541794> ;
    dct:source <http://marc21rdf.info>,
        <https://www.loc.gov/marc/bibliographic/bd007.html> ;
    dct:title "Motion picture: refined categories of color"@en ;
    dct:type <http://purl.org/dc/dcmitype/Dataset> ;
    schema:disambiguatingDescription """SKOS Concept Scheme for MARC 00X
         Values"""@en ;
    schema:version "1-0-0" .

