<?xml version="1.0" encoding="utf-8"?>
<rdf:RDF
   xmlns:dc="http://purl.org/dc/elements/1.1/"
   xmlns:dct="http://purl.org/dc/terms/"
   xmlns:rdf="http://www.w3.org/1999/02/22-rdf-syntax-ns#"
   xmlns:schema="https://schema.org/"
   xmlns:skos="http://www.w3.org/2004/02/skos/core#"
>
  <rdf:Description rdf:about="https://doi.org/10.6069/uwlswd.9r2z-x073">
    <rdf:type rdf:resource="http://www.w3.org/2004/02/skos/core#ConceptScheme"/>
    <dct:type rdf:resource="http://purl.org/dc/dcmitype/Dataset"/>
    <dct:title xml:lang="en">Videorecording: medium for sound</dct:title>
    <dct:alternative xml:lang="en">MARC21 007/06 values for videorecordings expressed using
         RDF</dct:alternative>
    <dct:description xml:lang="en">Specific medium used to carry the sound of an item, whether
         that sound is carried on the videorecording or is separate, and the type of sound playback
         required for the item.</dct:description>
    <schema:disambiguatingDescription xml:lang="en">SKOS Concept Scheme for MARC 00X
         Values</schema:disambiguatingDescription>
    <dct:publisher rdf:resource="http://viaf.org/viaf/139541794"/>
    <dct:source rdf:resource="https://www.loc.gov/marc/bibliographic/bd007.html"/>
    <dct:source rdf:resource="http://marc21rdf.info"/>
    <dct:provenance rdf:resource="https://doi.org/10.6069/uwlswd.2e2b-y833#marc00Xvalues"/>
    <dct:creator rdf:resource="http://viaf.org/viaf/139541794"/>
    <dct:contributor rdf:resource="http://viaf.org/viaf/151962300"/>
    <dct:issued>2024</dct:issued>
    <dc:contributor xml:lang="en">Metadata Management Associates</dc:contributor>
    <dc:language>en</dc:language>
    <dct:license rdf:resource="http://creativecommons.org/publicdomain/zero/1.0"/>
    <schema:version>1-0-0</schema:version>
    <dct:format rdf:resource="http://www.w3.org/ns/formats/RDF_XML"/>
    <dct:hasFormat rdf:resource="https://uwlib-cams.github.io/uwlswd_vocabs_marc_007/videorecording_medium_for_sound/videorecording_medium_for_sound.ttl"/>
    <dct:hasFormat rdf:resource="https://uwlib-cams.github.io/uwlswd_vocabs_marc_007/videorecording_medium_for_sound/videorecording_medium_for_sound.nt"/>
    <dct:hasFormat rdf:resource="https://uwlib-cams.github.io/uwlswd_vocabs_marc_007/videorecording_medium_for_sound/videorecording_medium_for_sound.jsonld"/>
    <dct:hasFormat rdf:resource="https://uwlib-cams.github.io/uwlswd_vocabs_marc_007/videorecording_medium_for_sound/videorecording_medium_for_sound.html"/>
  </rdf:Description>
  <rdf:Description rdf:about="https://doi.org/10.6069/uwlswd.9r2z-x073#u">
    <rdf:type rdf:resource="http://www.w3.org/2004/02/skos/core#Concept"/>
    <skos:inScheme rdf:resource="https://doi.org/10.6069/uwlswd.9r2z-x073"/>
    <skos:prefLabel xml:lang="en">unknown</skos:prefLabel>
    <skos:definition xml:lang="en">Medium for sound is not known.</skos:definition>
    <skos:notation>u</skos:notation>
  </rdf:Description>
  <rdf:Description rdf:about="https://doi.org/10.6069/uwlswd.9r2z-x073#b">
    <rdf:type rdf:resource="http://www.w3.org/2004/02/skos/core#Concept"/>
    <skos:inScheme rdf:resource="https://doi.org/10.6069/uwlswd.9r2z-x073"/>
    <skos:prefLabel xml:lang="en">magnetic sound track on motion picture film</skos:prefLabel>
    <skos:definition xml:lang="en">Sound to accompany a videorecording is carried on a magnetic
         track that is part of a motion picture film.</skos:definition>
    <skos:scopeNote xml:lang="en">It would be rare for this to occur.</skos:scopeNote>
    <skos:notation>b</skos:notation>
  </rdf:Description>
  <rdf:Description rdf:about="https://doi.org/10.6069/uwlswd.9r2z-x073#c">
    <rdf:type rdf:resource="http://www.w3.org/2004/02/skos/core#Concept"/>
    <skos:inScheme rdf:resource="https://doi.org/10.6069/uwlswd.9r2z-x073"/>
    <skos:prefLabel xml:lang="en">magnetic audio tape in cartridge</skos:prefLabel>
    <skos:definition xml:lang="en">Sound to accompany a videorecording is carried on a magnetic
         audio tape cartridge.</skos:definition>
    <skos:notation>c</skos:notation>
  </rdf:Description>
  <rdf:Description rdf:about="https://doi.org/10.6069/uwlswd.9r2z-x073#a">
    <rdf:type rdf:resource="http://www.w3.org/2004/02/skos/core#Concept"/>
    <skos:inScheme rdf:resource="https://doi.org/10.6069/uwlswd.9r2z-x073"/>
    <skos:prefLabel xml:lang="en">optical sound track on motion picture film</skos:prefLabel>
    <skos:definition xml:lang="en">Sound to accompany a videorecording is carried on an optical
         track that is part of a motion picture film.</skos:definition>
    <skos:scopeNote xml:lang="en">It would be rare for this to occur.</skos:scopeNote>
    <skos:notation>a</skos:notation>
  </rdf:Description>
  <rdf:Description rdf:about="https://doi.org/10.6069/uwlswd.9r2z-x073#h">
    <rdf:type rdf:resource="http://www.w3.org/2004/02/skos/core#Concept"/>
    <skos:inScheme rdf:resource="https://doi.org/10.6069/uwlswd.9r2z-x073"/>
    <skos:prefLabel xml:lang="en">videotape</skos:prefLabel>
    <skos:definition xml:lang="en">Sound to accompany a videorecording is included as part of the
         videotape.</skos:definition>
    <skos:scopeNote xml:lang="en">Videotape is not ordinarily used to record only
         sound.</skos:scopeNote>
    <skos:notation>h</skos:notation>
  </rdf:Description>
  <rdf:Description rdf:about="https://doi.org/10.6069/uwlswd.9r2z-x073#pound">
    <rdf:type rdf:resource="http://www.w3.org/2004/02/skos/core#Concept"/>
    <skos:inScheme rdf:resource="https://doi.org/10.6069/uwlswd.9r2z-x073"/>
    <skos:prefLabel xml:lang="en">no sound (silent)</skos:prefLabel>
    <skos:definition xml:lang="en">Sound is not present (i.e., the item is intended to be
         silent).</skos:definition>
    <skos:notation>#</skos:notation>
  </rdf:Description>
  <rdf:Description rdf:about="https://doi.org/10.6069/uwlswd.9r2z-x073#d">
    <rdf:type rdf:resource="http://www.w3.org/2004/02/skos/core#Concept"/>
    <skos:inScheme rdf:resource="https://doi.org/10.6069/uwlswd.9r2z-x073"/>
    <skos:prefLabel xml:lang="en">sound disc</skos:prefLabel>
    <skos:definition xml:lang="en">Sound to accompany a videorecording is carried on a sound
         disc.</skos:definition>
    <skos:scopeNote xml:lang="en">Sound discs include 7, 10, and 12 inch vinyl phonograph records
         and 4 3/4 inch compact discs.</skos:scopeNote>
    <skos:notation>d</skos:notation>
  </rdf:Description>
  <rdf:Description rdf:about="https://doi.org/10.6069/uwlswd.9r2z-x073#z">
    <rdf:type rdf:resource="http://www.w3.org/2004/02/skos/core#Concept"/>
    <skos:inScheme rdf:resource="https://doi.org/10.6069/uwlswd.9r2z-x073"/>
    <skos:prefLabel xml:lang="en">other</skos:prefLabel>
    <skos:definition xml:lang="en">Medium for sound other than no sound (silent), optical sound
         track on motion picture film, magnetic sound track on motion picture film, magnetic audio
         tape in cartridge, sound disc, magnetic audio tape on reel, magnetic audio tape in
         cassette, optical and magnetic sound track on motion picture film, videotape, or
         videodisc.</skos:definition>
    <skos:notation>z</skos:notation>
  </rdf:Description>
  <rdf:Description rdf:about="https://doi.org/10.6069/uwlswd.9r2z-x073#gx">
    <rdf:type rdf:resource="http://www.w3.org/2004/02/skos/core#Concept"/>
    <skos:inScheme rdf:resource="https://doi.org/10.6069/uwlswd.9r2z-x073"/>
    <skos:prefLabel xml:lang="en">other [obsolete]</skos:prefLabel>
    <skos:notation>g</skos:notation>
  </rdf:Description>
  <rdf:Description rdf:about="https://doi.org/10.6069/uwlswd.9r2z-x073#f">
    <rdf:type rdf:resource="http://www.w3.org/2004/02/skos/core#Concept"/>
    <skos:inScheme rdf:resource="https://doi.org/10.6069/uwlswd.9r2z-x073"/>
    <skos:prefLabel xml:lang="en">magnetic audio tape in cassette</skos:prefLabel>
    <skos:definition xml:lang="en">Sound to accompany a videorecording is carried on a cassette of
         magnetic audio tape.</skos:definition>
    <skos:notation>f</skos:notation>
  </rdf:Description>
  <rdf:Description rdf:about="https://doi.org/10.6069/uwlswd.9r2z-x073#g">
    <rdf:type rdf:resource="http://www.w3.org/2004/02/skos/core#Concept"/>
    <skos:inScheme rdf:resource="https://doi.org/10.6069/uwlswd.9r2z-x073"/>
    <skos:prefLabel xml:lang="en">optical and magnetic sound track on motion picture
         film</skos:prefLabel>
    <skos:definition xml:lang="en">Sound to accompany a videorecording is carried on both an
         optical and magnetic track on a motion picture film.</skos:definition>
    <skos:scopeNote xml:lang="en">It would be rare for this to occur.</skos:scopeNote>
    <skos:notation>g</skos:notation>
  </rdf:Description>
  <rdf:Description rdf:about="https://doi.org/10.6069/uwlswd.9r2z-x073#e">
    <rdf:type rdf:resource="http://www.w3.org/2004/02/skos/core#Concept"/>
    <skos:inScheme rdf:resource="https://doi.org/10.6069/uwlswd.9r2z-x073"/>
    <skos:prefLabel xml:lang="en">magnetic audio tape on reel</skos:prefLabel>
    <skos:definition xml:lang="en">Sound to accompany a videorecording is carried on a reel of
         magnetic audio tape.</skos:definition>
    <skos:notation>e</skos:notation>
  </rdf:Description>
  <rdf:Description rdf:about="https://doi.org/10.6069/uwlswd.9r2z-x073#i">
    <rdf:type rdf:resource="http://www.w3.org/2004/02/skos/core#Concept"/>
    <skos:inScheme rdf:resource="https://doi.org/10.6069/uwlswd.9r2z-x073"/>
    <skos:prefLabel xml:lang="en">videodisc</skos:prefLabel>
    <skos:definition xml:lang="en">Sound to accompany a videorecording is included as part of the
         videodisc.</skos:definition>
    <skos:scopeNote xml:lang="en">Videodiscs are not ordinarily used to record only sound. A
         distinction must be made between videodiscs (e.g., 12 inch laser optical videodiscs that
         include video information) and compact discs that are used to record sound only (e.g., 4
         3/4 inch audio compact discs). The technology to physically record video or audio
         information on digital disc systems is the same.</skos:scopeNote>
    <skos:notation>i</skos:notation>
  </rdf:Description>
</rdf:RDF>
