@prefix dc: <http://purl.org/dc/elements/1.1/> .
@prefix dct: <http://purl.org/dc/terms/> .
@prefix schema: <https://schema.org/> .
@prefix skos: <http://www.w3.org/2004/02/skos/core#> .

<https://doi.org/10.6069/uwlswd.9r2z-x073#a> a skos:Concept ;
    skos:definition """Sound to accompany a videorecording is carried on an optical
         track that is part of a motion picture film."""@en ;
    skos:inScheme <https://doi.org/10.6069/uwlswd.9r2z-x073> ;
    skos:notation "a" ;
    skos:prefLabel "optical sound track on motion picture film"@en ;
    skos:scopeNote "It would be rare for this to occur."@en .

<https://doi.org/10.6069/uwlswd.9r2z-x073#b> a skos:Concept ;
    skos:definition """Sound to accompany a videorecording is carried on a magnetic
         track that is part of a motion picture film."""@en ;
    skos:inScheme <https://doi.org/10.6069/uwlswd.9r2z-x073> ;
    skos:notation "b" ;
    skos:prefLabel "magnetic sound track on motion picture film"@en ;
    skos:scopeNote "It would be rare for this to occur."@en .

<https://doi.org/10.6069/uwlswd.9r2z-x073#c> a skos:Concept ;
    skos:definition """Sound to accompany a videorecording is carried on a magnetic
         audio tape cartridge."""@en ;
    skos:inScheme <https://doi.org/10.6069/uwlswd.9r2z-x073> ;
    skos:notation "c" ;
    skos:prefLabel "magnetic audio tape in cartridge"@en .

<https://doi.org/10.6069/uwlswd.9r2z-x073#d> a skos:Concept ;
    skos:definition """Sound to accompany a videorecording is carried on a sound
         disc."""@en ;
    skos:inScheme <https://doi.org/10.6069/uwlswd.9r2z-x073> ;
    skos:notation "d" ;
    skos:prefLabel "sound disc"@en ;
    skos:scopeNote """Sound discs include 7, 10, and 12 inch vinyl phonograph records
         and 4 3/4 inch compact discs."""@en .

<https://doi.org/10.6069/uwlswd.9r2z-x073#e> a skos:Concept ;
    skos:definition """Sound to accompany a videorecording is carried on a reel of
         magnetic audio tape."""@en ;
    skos:inScheme <https://doi.org/10.6069/uwlswd.9r2z-x073> ;
    skos:notation "e" ;
    skos:prefLabel "magnetic audio tape on reel"@en .

<https://doi.org/10.6069/uwlswd.9r2z-x073#f> a skos:Concept ;
    skos:definition """Sound to accompany a videorecording is carried on a cassette of
         magnetic audio tape."""@en ;
    skos:inScheme <https://doi.org/10.6069/uwlswd.9r2z-x073> ;
    skos:notation "f" ;
    skos:prefLabel "magnetic audio tape in cassette"@en .

<https://doi.org/10.6069/uwlswd.9r2z-x073#g> a skos:Concept ;
    skos:definition """Sound to accompany a videorecording is carried on both an
         optical and magnetic track on a motion picture film."""@en ;
    skos:inScheme <https://doi.org/10.6069/uwlswd.9r2z-x073> ;
    skos:notation "g" ;
    skos:prefLabel """optical and magnetic sound track on motion picture
         film"""@en ;
    skos:scopeNote "It would be rare for this to occur."@en .

<https://doi.org/10.6069/uwlswd.9r2z-x073#gx> a skos:Concept ;
    skos:inScheme <https://doi.org/10.6069/uwlswd.9r2z-x073> ;
    skos:notation "g" ;
    skos:prefLabel "other [obsolete]"@en .

<https://doi.org/10.6069/uwlswd.9r2z-x073#h> a skos:Concept ;
    skos:definition """Sound to accompany a videorecording is included as part of the
         videotape."""@en ;
    skos:inScheme <https://doi.org/10.6069/uwlswd.9r2z-x073> ;
    skos:notation "h" ;
    skos:prefLabel "videotape"@en ;
    skos:scopeNote """Videotape is not ordinarily used to record only
         sound."""@en .

<https://doi.org/10.6069/uwlswd.9r2z-x073#i> a skos:Concept ;
    skos:definition """Sound to accompany a videorecording is included as part of the
         videodisc."""@en ;
    skos:inScheme <https://doi.org/10.6069/uwlswd.9r2z-x073> ;
    skos:notation "i" ;
    skos:prefLabel "videodisc"@en ;
    skos:scopeNote """Videodiscs are not ordinarily used to record only sound. A
         distinction must be made between videodiscs (e.g., 12 inch laser optical videodiscs that
         include video information) and compact discs that are used to record sound only (e.g., 4
         3/4 inch audio compact discs). The technology to physically record video or audio
         information on digital disc systems is the same."""@en .

<https://doi.org/10.6069/uwlswd.9r2z-x073#pound> a skos:Concept ;
    skos:definition """Sound is not present (i.e., the item is intended to be
         silent)."""@en ;
    skos:inScheme <https://doi.org/10.6069/uwlswd.9r2z-x073> ;
    skos:notation "#" ;
    skos:prefLabel "no sound (silent)"@en .

<https://doi.org/10.6069/uwlswd.9r2z-x073#u> a skos:Concept ;
    skos:definition "Medium for sound is not known."@en ;
    skos:inScheme <https://doi.org/10.6069/uwlswd.9r2z-x073> ;
    skos:notation "u" ;
    skos:prefLabel "unknown"@en .

<https://doi.org/10.6069/uwlswd.9r2z-x073#z> a skos:Concept ;
    skos:definition """Medium for sound other than no sound (silent), optical sound
         track on motion picture film, magnetic sound track on motion picture film, magnetic audio
         tape in cartridge, sound disc, magnetic audio tape on reel, magnetic audio tape in
         cassette, optical and magnetic sound track on motion picture film, videotape, or
         videodisc."""@en ;
    skos:inScheme <https://doi.org/10.6069/uwlswd.9r2z-x073> ;
    skos:notation "z" ;
    skos:prefLabel "other"@en .

<https://doi.org/10.6069/uwlswd.9r2z-x073> a skos:ConceptScheme ;
    dc:contributor "Metadata Management Associates"@en ;
    dc:language "en" ;
    dct:alternative """MARC21 007/06 values for videorecordings expressed using
         RDF"""@en ;
    dct:contributor <http://viaf.org/viaf/151962300> ;
    dct:creator <http://viaf.org/viaf/139541794> ;
    dct:description """Specific medium used to carry the sound of an item, whether
         that sound is carried on the videorecording or is separate, and the type of sound playback
         required for the item."""@en ;
    dct:format <http://www.w3.org/ns/formats/Turtle> ;
    dct:hasFormat <https://uwlib-cams.github.io/uwlswd_vocabs_marc_007/videorecording_medium_for_sound/videorecording_medium_for_sound.html>,
        <https://uwlib-cams.github.io/uwlswd_vocabs_marc_007/videorecording_medium_for_sound/videorecording_medium_for_sound.jsonld>,
        <https://uwlib-cams.github.io/uwlswd_vocabs_marc_007/videorecording_medium_for_sound/videorecording_medium_for_sound.nt>,
        <https://uwlib-cams.github.io/uwlswd_vocabs_marc_007/videorecording_medium_for_sound/videorecording_medium_for_sound.rdf> ;
    dct:issued "2024" ;
    dct:license <http://creativecommons.org/publicdomain/zero/1.0> ;
    dct:provenance <https://doi.org/10.6069/uwlswd.2e2b-y833#marc00Xvalues> ;
    dct:publisher <http://viaf.org/viaf/139541794> ;
    dct:source <http://marc21rdf.info>,
        <https://www.loc.gov/marc/bibliographic/bd007.html> ;
    dct:title "Videorecording: medium for sound"@en ;
    dct:type <http://purl.org/dc/dcmitype/Dataset> ;
    schema:disambiguatingDescription """SKOS Concept Scheme for MARC 00X
         Values"""@en ;
    schema:version "1-0-0" .

