<?xml version="1.0" encoding="utf-8"?>
<rdf:RDF
   xmlns:dc="http://purl.org/dc/elements/1.1/"
   xmlns:dct="http://purl.org/dc/terms/"
   xmlns:rdf="http://www.w3.org/1999/02/22-rdf-syntax-ns#"
   xmlns:schema="https://schema.org/"
   xmlns:skos="http://www.w3.org/2004/02/skos/core#"
>
  <rdf:Description rdf:about="https://doi.org/10.6069/uwlswd.3z3f-7k53#a">
    <rdf:type rdf:resource="http://www.w3.org/2004/02/skos/core#Concept"/>
    <skos:inScheme rdf:resource="https://doi.org/10.6069/uwlswd.3z3f-7k53"/>
    <skos:prefLabel xml:lang="en">one color</skos:prefLabel>
    <skos:definition xml:lang="en">Printed or executed in a single color.</skos:definition>
    <skos:scopeNote xml:lang="en">Used for monochrome art works. It is not used with photographic
         materials. Does not include black.</skos:scopeNote>
    <skos:notation xml:lang="en">a</skos:notation>
  </rdf:Description>
  <rdf:Description rdf:about="https://doi.org/10.6069/uwlswd.3z3f-7k53#z">
    <rdf:type rdf:resource="http://www.w3.org/2004/02/skos/core#Concept"/>
    <skos:inScheme rdf:resource="https://doi.org/10.6069/uwlswd.3z3f-7k53"/>
    <skos:prefLabel xml:lang="en">other</skos:prefLabel>
    <skos:definition xml:lang="en">Color other than one color, black-and-white, multicolored, hand
         colored, or mixed.</skos:definition>
    <skos:scopeNote xml:lang="en">Includes stained, tinted, or toned items(e.g., sepia toned
         photographic items).</skos:scopeNote>
    <skos:notation xml:lang="en">z</skos:notation>
  </rdf:Description>
  <rdf:Description rdf:about="https://doi.org/10.6069/uwlswd.3z3f-7k53#b">
    <rdf:type rdf:resource="http://www.w3.org/2004/02/skos/core#Concept"/>
    <skos:inScheme rdf:resource="https://doi.org/10.6069/uwlswd.3z3f-7k53"/>
    <skos:prefLabel xml:lang="en">black-and-white</skos:prefLabel>
    <skos:definition xml:lang="en">Printed or executed in black-and-white.</skos:definition>
    <skos:scopeNote xml:lang="en">Refers to monochrome photographic materials executed in
         black-and-white.</skos:scopeNote>
    <skos:notation xml:lang="en">b</skos:notation>
  </rdf:Description>
  <rdf:Description rdf:about="https://doi.org/10.6069/uwlswd.3z3f-7k53#c">
    <rdf:type rdf:resource="http://www.w3.org/2004/02/skos/core#Concept"/>
    <skos:inScheme rdf:resource="https://doi.org/10.6069/uwlswd.3z3f-7k53"/>
    <skos:prefLabel xml:lang="en">multicolored</skos:prefLabel>
    <skos:definition xml:lang="en">Printed or executed in more than one color.</skos:definition>
    <skos:scopeNote xml:lang="en">Used for color photographic processes.</skos:scopeNote>
    <skos:notation xml:lang="en">c</skos:notation>
  </rdf:Description>
  <rdf:Description rdf:about="https://doi.org/10.6069/uwlswd.3z3f-7k53#n">
    <rdf:type rdf:resource="http://www.w3.org/2004/02/skos/core#Concept"/>
    <skos:inScheme rdf:resource="https://doi.org/10.6069/uwlswd.3z3f-7k53"/>
    <skos:prefLabel xml:lang="en">mixed</skos:prefLabel>
    <skos:definition xml:lang="en">Work or collection is a combination of one color,
         black-and-white, multicolored, hand colored, and/or other images.</skos:definition>
    <skos:notation xml:lang="en">n</skos:notation>
  </rdf:Description>
  <rdf:Description rdf:about="https://doi.org/10.6069/uwlswd.3z3f-7k53#h">
    <rdf:type rdf:resource="http://www.w3.org/2004/02/skos/core#Concept"/>
    <skos:inScheme rdf:resource="https://doi.org/10.6069/uwlswd.3z3f-7k53"/>
    <skos:prefLabel xml:lang="en">hand colored</skos:prefLabel>
    <skos:definition xml:lang="en">Image, produced by a printing or photographic process, is hand
         colored.</skos:definition>
    <skos:scopeNote xml:lang="en">Rarely used with commercial visual materials since these are not
         typically issued with hand coloring.</skos:scopeNote>
    <skos:notation xml:lang="en">h</skos:notation>
  </rdf:Description>
  <rdf:Description rdf:about="https://doi.org/10.6069/uwlswd.3z3f-7k53">
    <rdf:type rdf:resource="http://www.w3.org/2004/02/skos/core#ConceptScheme"/>
    <dct:type rdf:resource="http://purl.org/dc/dcmitype/Dataset"/>
    <dct:title xml:lang="en">Nonprojected graphic: color</dct:title>
    <dct:alternative xml:lang="en">MARC21 007/03 values for nonprojected graphics expressed using
         RDF</dct:alternative>
    <dct:description xml:lang="en">Color characteristics of the nonprojected
         graphic.</dct:description>
    <schema:disambiguatingDescription>SKOS Concept Scheme for MARC 00X
         Values</schema:disambiguatingDescription>
    <dct:publisher rdf:resource="http://viaf.org/viaf/139541794"/>
    <dct:source rdf:resource="https://www.loc.gov/marc/bibliographic/bd007.html"/>
    <dct:source rdf:resource="http://marc21rdf.info"/>
    <dct:provenance rdf:resource="https://doi.org/10.6069/uwlswd.2e2b-y833"/>
    <dct:creator rdf:resource="http://viaf.org/viaf/139541794"/>
    <dct:contributor rdf:resource="http://viaf.org/viaf/151962300"/>
    <dct:issued>2024</dct:issued>
    <dc:contributor xml:lang="en">Metadata Management Associates</dc:contributor>
    <dc:language>en</dc:language>
    <dct:license rdf:resource="http://creativecommons.org/publicdomain/zero/1.0"/>
    <schema:version>1-0-0</schema:version>
    <dct:format rdf:resource="http://www.w3.org/ns/formats/RDF_XML"/>
  </rdf:Description>
  <rdf:Description rdf:about="https://doi.org/10.6069/uwlswd.3z3f-7k53#u">
    <rdf:type rdf:resource="http://www.w3.org/2004/02/skos/core#Concept"/>
    <skos:inScheme rdf:resource="https://doi.org/10.6069/uwlswd.3z3f-7k53"/>
    <skos:prefLabel xml:lang="en">unknown</skos:prefLabel>
    <skos:definition xml:lang="en">Color characteristics of the item are not
         known.</skos:definition>
    <skos:notation xml:lang="en">u</skos:notation>
  </rdf:Description>
</rdf:RDF>
