@prefix dc: <http://purl.org/dc/elements/1.1/> .
@prefix dct: <http://purl.org/dc/terms/> .
@prefix schema: <https://schema.org/> .
@prefix skos: <http://www.w3.org/2004/02/skos/core#> .

<https://doi.org/10.6069/uwlswd.404b-ss58#a> a skos:Concept ;
    skos:definition "Type has not been identified."@en ;
    skos:inScheme <https://doi.org/10.6069/uwlswd.404b-ss58> ;
    skos:notation "a" ;
    skos:prefLabel "safety base, undetermined"@en .

<https://doi.org/10.6069/uwlswd.404b-ss58#b> a skos:Concept ;
    skos:inScheme <https://doi.org/10.6069/uwlswd.404b-ss58> ;
    skos:notation "b" ;
    skos:prefLabel "not safety base [obsolete]"@en .

<https://doi.org/10.6069/uwlswd.404b-ss58#c> a skos:Concept ;
    skos:definition """Acetate safety base film whose exact type cannot be
         determined."""@en ;
    skos:inScheme <https://doi.org/10.6069/uwlswd.404b-ss58> ;
    skos:notation "c" ;
    skos:prefLabel "safety base, acetate undetermined"@en ;
    skos:scopeNote """I.e., where it is unknown if the type is diacetate or
         triacetate."""@en .

<https://doi.org/10.6069/uwlswd.404b-ss58#d> a skos:Concept ;
    skos:definition "Cellulose diacetate film base."@en ;
    skos:inScheme <https://doi.org/10.6069/uwlswd.404b-ss58> ;
    skos:notation "d" ;
    skos:prefLabel "safety base, diacetate"@en .

<https://doi.org/10.6069/uwlswd.404b-ss58#i> a skos:Concept ;
    skos:definition "Cellulose nitrate film."@en ;
    skos:inScheme <https://doi.org/10.6069/uwlswd.404b-ss58> ;
    skos:notation "i" ;
    skos:prefLabel "nitrate base"@en .

<https://doi.org/10.6069/uwlswd.404b-ss58#m> a skos:Concept ;
    skos:definition """Combination of nitrate base and safety base
         film."""@en ;
    skos:inScheme <https://doi.org/10.6069/uwlswd.404b-ss58> ;
    skos:notation "m" ;
    skos:prefLabel "mixed base (nitrate and safety)"@en .

<https://doi.org/10.6069/uwlswd.404b-ss58#n> a skos:Concept ;
    skos:definition """On a reflective rather than a transparent
         base."""@en ;
    skos:inScheme <https://doi.org/10.6069/uwlswd.404b-ss58> ;
    skos:notation "n" ;
    skos:prefLabel "not applicable"@en ;
    skos:scopeNote """Used for microopaques (which can be termed microcard or
         microprint)."""@en .

<https://doi.org/10.6069/uwlswd.404b-ss58#p> a skos:Concept ;
    skos:definition """Film base is made of a synthetic resin (e.g.,
         estar)."""@en ;
    skos:inScheme <https://doi.org/10.6069/uwlswd.404b-ss58> ;
    skos:notation "p" ;
    skos:prefLabel "safety base, polyester"@en .

<https://doi.org/10.6069/uwlswd.404b-ss58#r> a skos:Concept ;
    skos:definition """Mixed safety base films are spliced together; no nitrate
         film."""@en ;
    skos:inScheme <https://doi.org/10.6069/uwlswd.404b-ss58> ;
    skos:notation "r" ;
    skos:prefLabel "safety base, mixed"@en .

<https://doi.org/10.6069/uwlswd.404b-ss58#t> a skos:Concept ;
    skos:definition "Cellulose triacetate film base."@en ;
    skos:inScheme <https://doi.org/10.6069/uwlswd.404b-ss58> ;
    skos:notation "t" ;
    skos:prefLabel "safety base, triacetate"@en .

<https://doi.org/10.6069/uwlswd.404b-ss58#u> a skos:Concept ;
    skos:inScheme <https://doi.org/10.6069/uwlswd.404b-ss58> ;
    skos:notation "u" ;
    skos:prefLabel "unknown"@en .

<https://doi.org/10.6069/uwlswd.404b-ss58#z> a skos:Concept ;
    skos:definition """Base of film other than safety base, undetermined, safety base,
         acetate undetermined, safety base, diacetate, nitrate base, mixed base (nitrate and
         safety), not applicable, safety base, polyester, safety base, mixed, safety base, or
         triacetate."""@en ;
    skos:inScheme <https://doi.org/10.6069/uwlswd.404b-ss58> ;
    skos:notation "z" ;
    skos:prefLabel "other"@en .

<https://doi.org/10.6069/uwlswd.404b-ss58> a skos:ConceptScheme ;
    dc:contributor "Metadata Management Associates"@en ;
    dc:language "en" ;
    dct:alternative """MARC21 007/12 values for microform expressed using
         RDF"""@en ;
    dct:contributor <http://viaf.org/viaf/151962300> ;
    dct:creator <http://viaf.org/viaf/139541794> ;
    dct:description "Base of the film."@en ;
    dct:format <http://www.w3.org/ns/formats/Turtle> ;
    dct:hasFormat <https://uwlib-cams.github.io/uwlswd_vocabs_marc_007/microform_base_of_film/microform_base_of_film.html>,
        <https://uwlib-cams.github.io/uwlswd_vocabs_marc_007/microform_base_of_film/microform_base_of_film.jsonld>,
        <https://uwlib-cams.github.io/uwlswd_vocabs_marc_007/microform_base_of_film/microform_base_of_film.nt>,
        <https://uwlib-cams.github.io/uwlswd_vocabs_marc_007/microform_base_of_film/microform_base_of_film.rdf> ;
    dct:issued "2024" ;
    dct:license <http://creativecommons.org/publicdomain/zero/1.0> ;
    dct:provenance <https://doi.org/10.6069/uwlswd.2e2b-y833#marc00Xvalues> ;
    dct:publisher <http://viaf.org/viaf/139541794> ;
    dct:source <http://marc21rdf.info>,
        <https://www.loc.gov/marc/bibliographic/bd007.html> ;
    dct:title "Microform: base of film"@en ;
    dct:type <http://purl.org/dc/dcmitype/Dataset> ;
    schema:disambiguatingDescription """SKOS Concept Scheme for MARC 00X
         Values"""@en ;
    schema:version "1-0-0" .

