@prefix dc: <http://purl.org/dc/elements/1.1/> .
@prefix dct: <http://purl.org/dc/terms/> .
@prefix schema: <https://schema.org/> .
@prefix skos: <http://www.w3.org/2004/02/skos/core#> .

<https://doi.org/10.6069/uwlswd.v4qn-rb56#a> a skos:Concept ;
    skos:definition """Usually a disc or cylinder recording, captured using an
         acoustical horn and diaphragm and stored directly on a master surface."""@en ;
    skos:inScheme <https://doi.org/10.6069/uwlswd.v4qn-rb56> ;
    skos:notation "a" ;
    skos:prefLabel "acoustical capture, direct storage"@en ;
    skos:scopeNote """Most acoustical recordings date from before 1927/29 when
         electrical recording equipment became available."""@en .

<https://doi.org/10.6069/uwlswd.v4qn-rb56#b> a skos:Concept ;
    skos:definition """Disc recordings captured using electrical equipment and stored
         directly on a master surface."""@en ;
    skos:inScheme <https://doi.org/10.6069/uwlswd.v4qn-rb56> ;
    skos:notation "b" ;
    skos:prefLabel "direct storage, not acoustical"@en ;
    skos:scopeNote """All recordings made with microphones and other electrical
         equipment prior to the availability of magnetic recording techniques in the late 1940s used
         direct storage. Commercial recordings marked "direct to disc" or some equivalent phrase
         also use this technique. Also known as electromechanical recording."""@en .

<https://doi.org/10.6069/uwlswd.v4qn-rb56#d> a skos:Concept ;
    skos:definition """Sound recordings which were captured electrically and stored
         using digital techniques."""@en ;
    skos:inScheme <https://doi.org/10.6069/uwlswd.v4qn-rb56> ;
    skos:notation "d" ;
    skos:prefLabel "digital storage"@en ;
    skos:scopeNote """Such recordings, which became available in the 1980s, are
         normally identified as "digitally recorded" or some similar phrase on the label or package.
         "Digital remaster" or "digital mixing" does not imply original digital storage. Note that
         Digital storage and digital playback should not be confused."""@en .

<https://doi.org/10.6069/uwlswd.v4qn-rb56#e> a skos:Concept ;
    skos:definition """Sound recordings which were captured using electrical
         techniques and stored as modulations and pulses on a magnetic surface."""@en ;
    skos:inScheme <https://doi.org/10.6069/uwlswd.v4qn-rb56> ;
    skos:notation "e" ;
    skos:prefLabel "analog electrical storage"@en ;
    skos:scopeNote """Most recordings made from the late 1940s until early 1980s are
         analog electrical recordings."""@en .

<https://doi.org/10.6069/uwlswd.v4qn-rb56#u> a skos:Concept ;
    skos:definition "Capture and storage technique are not known."@en ;
    skos:inScheme <https://doi.org/10.6069/uwlswd.v4qn-rb56> ;
    skos:notation "u" ;
    skos:prefLabel "unknown"@en .

<https://doi.org/10.6069/uwlswd.v4qn-rb56#z> a skos:Concept ;
    skos:definition """Capture and storage technique other than acoustical capture,
         direct storage; direct storage, not acoustical; digital storage; or analog electrical
         storage."""@en ;
    skos:inScheme <https://doi.org/10.6069/uwlswd.v4qn-rb56> ;
    skos:notation "z" ;
    skos:prefLabel "other"@en .

<https://doi.org/10.6069/uwlswd.v4qn-rb56> a skos:ConceptScheme ;
    dc:contributor "Metadata Management Associates"@en ;
    dc:language "en" ;
    dct:alternative """MARC21 007/13 values for sound recordings expressed using RDF
         Formerly: Capture and storage technique"""@en ;
    dct:contributor <http://viaf.org/viaf/151962300> ;
    dct:creator <http://viaf.org/viaf/139541794> ;
    dct:description """How the sound was originally captured and
         stored."""@en ;
    dct:format <http://www.w3.org/ns/formats/Turtle> ;
    dct:hasFormat <https://uwlib-cams.github.io/uwlswd_vocabs_marc_007/sound_recording_original_capture_and_storage_technique/sound_recording_original_capture_and_storage_technique.html>,
        <https://uwlib-cams.github.io/uwlswd_vocabs_marc_007/sound_recording_original_capture_and_storage_technique/sound_recording_original_capture_and_storage_technique.jsonld>,
        <https://uwlib-cams.github.io/uwlswd_vocabs_marc_007/sound_recording_original_capture_and_storage_technique/sound_recording_original_capture_and_storage_technique.nt>,
        <https://uwlib-cams.github.io/uwlswd_vocabs_marc_007/sound_recording_original_capture_and_storage_technique/sound_recording_original_capture_and_storage_technique.rdf> ;
    dct:issued "2024" ;
    dct:license <http://creativecommons.org/publicdomain/zero/1.0> ;
    dct:provenance <https://doi.org/10.6069/uwlswd.2e2b-y833#marc00Xvalues> ;
    dct:publisher <http://viaf.org/viaf/139541794> ;
    dct:source <http://marc21rdf.info>,
        <https://www.loc.gov/marc/bibliographic/bd007.html> ;
    dct:title "Sound recording: original capture and storage technique"@en ;
    dct:type <http://purl.org/dc/dcmitype/Dataset> ;
    schema:disambiguatingDescription """SKOS Concept Scheme for MARC 00X
         Values"""@en ;
    schema:version "1-0-0" .

