<?xml version="1.0" encoding="utf-8"?>
<rdf:RDF
   xmlns:dc="http://purl.org/dc/elements/1.1/"
   xmlns:dct="http://purl.org/dc/terms/"
   xmlns:rdf="http://www.w3.org/1999/02/22-rdf-syntax-ns#"
   xmlns:schema="https://schema.org/"
   xmlns:skos="http://www.w3.org/2004/02/skos/core#"
>
  <rdf:Description rdf:about="https://doi.org/10.6069/uwlswd.v4qn-rb56#a">
    <rdf:type rdf:resource="http://www.w3.org/2004/02/skos/core#Concept"/>
    <skos:inScheme rdf:resource="https://doi.org/10.6069/uwlswd.v4qn-rb56"/>
    <skos:prefLabel xml:lang="en">acoustical capture, direct storage</skos:prefLabel>
    <skos:definition xml:lang="en">Usually a disc or cylinder recording, captured using an
         acoustical horn and diaphragm and stored directly on a master surface.</skos:definition>
    <skos:scopeNote xml:lang="en">Most acoustical recordings date from before 1927/29 when
         electrical recording equipment became available.</skos:scopeNote>
    <skos:notation>a</skos:notation>
  </rdf:Description>
  <rdf:Description rdf:about="https://doi.org/10.6069/uwlswd.v4qn-rb56#b">
    <rdf:type rdf:resource="http://www.w3.org/2004/02/skos/core#Concept"/>
    <skos:inScheme rdf:resource="https://doi.org/10.6069/uwlswd.v4qn-rb56"/>
    <skos:prefLabel xml:lang="en">direct storage, not acoustical</skos:prefLabel>
    <skos:definition xml:lang="en">Disc recordings captured using electrical equipment and stored
         directly on a master surface.</skos:definition>
    <skos:scopeNote xml:lang="en">All recordings made with microphones and other electrical
         equipment prior to the availability of magnetic recording techniques in the late 1940s used
         direct storage. Commercial recordings marked "direct to disc" or some equivalent phrase
         also use this technique. Also known as electromechanical recording.</skos:scopeNote>
    <skos:notation>b</skos:notation>
  </rdf:Description>
  <rdf:Description rdf:about="https://doi.org/10.6069/uwlswd.v4qn-rb56">
    <rdf:type rdf:resource="http://www.w3.org/2004/02/skos/core#ConceptScheme"/>
    <dct:type rdf:resource="http://purl.org/dc/dcmitype/Dataset"/>
    <dct:title xml:lang="en">Sound recording: original capture and storage technique</dct:title>
    <dct:alternative xml:lang="en">MARC21 007/13 values for sound recordings expressed using RDF
         Formerly: Capture and storage technique</dct:alternative>
    <dct:description xml:lang="en">How the sound was originally captured and
         stored.</dct:description>
    <schema:disambiguatingDescription xml:lang="en">SKOS Concept Scheme for MARC 00X
         Values</schema:disambiguatingDescription>
    <dct:publisher rdf:resource="http://viaf.org/viaf/139541794"/>
    <dct:source rdf:resource="https://www.loc.gov/marc/bibliographic/bd007.html"/>
    <dct:source rdf:resource="http://marc21rdf.info"/>
    <dct:provenance rdf:resource="https://doi.org/10.6069/uwlswd.2e2b-y833#marc00Xvalues"/>
    <dct:creator rdf:resource="http://viaf.org/viaf/139541794"/>
    <dct:contributor rdf:resource="http://viaf.org/viaf/151962300"/>
    <dct:issued>2024</dct:issued>
    <dc:contributor xml:lang="en">Metadata Management Associates</dc:contributor>
    <dc:language>en</dc:language>
    <dct:license rdf:resource="http://creativecommons.org/publicdomain/zero/1.0"/>
    <schema:version>1-0-0</schema:version>
    <dct:format rdf:resource="http://www.w3.org/ns/formats/RDF_XML"/>
    <dct:hasFormat rdf:resource="https://uwlib-cams.github.io/uwlswd_vocabs_marc_007/sound_recording_original_capture_and_storage_technique/sound_recording_original_capture_and_storage_technique.ttl"/>
    <dct:hasFormat rdf:resource="https://uwlib-cams.github.io/uwlswd_vocabs_marc_007/sound_recording_original_capture_and_storage_technique/sound_recording_original_capture_and_storage_technique.nt"/>
    <dct:hasFormat rdf:resource="https://uwlib-cams.github.io/uwlswd_vocabs_marc_007/sound_recording_original_capture_and_storage_technique/sound_recording_original_capture_and_storage_technique.jsonld"/>
    <dct:hasFormat rdf:resource="https://uwlib-cams.github.io/uwlswd_vocabs_marc_007/sound_recording_original_capture_and_storage_technique/sound_recording_original_capture_and_storage_technique.html"/>
  </rdf:Description>
  <rdf:Description rdf:about="https://doi.org/10.6069/uwlswd.v4qn-rb56#z">
    <rdf:type rdf:resource="http://www.w3.org/2004/02/skos/core#Concept"/>
    <skos:inScheme rdf:resource="https://doi.org/10.6069/uwlswd.v4qn-rb56"/>
    <skos:prefLabel xml:lang="en">other</skos:prefLabel>
    <skos:definition xml:lang="en">Capture and storage technique other than acoustical capture,
         direct storage; direct storage, not acoustical; digital storage; or analog electrical
         storage.</skos:definition>
    <skos:notation>z</skos:notation>
  </rdf:Description>
  <rdf:Description rdf:about="https://doi.org/10.6069/uwlswd.v4qn-rb56#u">
    <rdf:type rdf:resource="http://www.w3.org/2004/02/skos/core#Concept"/>
    <skos:inScheme rdf:resource="https://doi.org/10.6069/uwlswd.v4qn-rb56"/>
    <skos:prefLabel xml:lang="en">unknown</skos:prefLabel>
    <skos:definition xml:lang="en">Capture and storage technique are not known.</skos:definition>
    <skos:notation>u</skos:notation>
  </rdf:Description>
  <rdf:Description rdf:about="https://doi.org/10.6069/uwlswd.v4qn-rb56#d">
    <rdf:type rdf:resource="http://www.w3.org/2004/02/skos/core#Concept"/>
    <skos:inScheme rdf:resource="https://doi.org/10.6069/uwlswd.v4qn-rb56"/>
    <skos:prefLabel xml:lang="en">digital storage</skos:prefLabel>
    <skos:definition xml:lang="en">Sound recordings which were captured electrically and stored
         using digital techniques.</skos:definition>
    <skos:scopeNote xml:lang="en">Such recordings, which became available in the 1980s, are
         normally identified as "digitally recorded" or some similar phrase on the label or package.
         "Digital remaster" or "digital mixing" does not imply original digital storage. Note that
         Digital storage and digital playback should not be confused.</skos:scopeNote>
    <skos:notation>d</skos:notation>
  </rdf:Description>
  <rdf:Description rdf:about="https://doi.org/10.6069/uwlswd.v4qn-rb56#e">
    <rdf:type rdf:resource="http://www.w3.org/2004/02/skos/core#Concept"/>
    <skos:inScheme rdf:resource="https://doi.org/10.6069/uwlswd.v4qn-rb56"/>
    <skos:prefLabel xml:lang="en">analog electrical storage</skos:prefLabel>
    <skos:definition xml:lang="en">Sound recordings which were captured using electrical
         techniques and stored as modulations and pulses on a magnetic surface.</skos:definition>
    <skos:scopeNote xml:lang="en">Most recordings made from the late 1940s until early 1980s are
         analog electrical recordings.</skos:scopeNote>
    <skos:notation>e</skos:notation>
  </rdf:Description>
</rdf:RDF>
