<?xml version="1.0" encoding="utf-8"?>
<rdf:RDF
   xmlns:dc="http://purl.org/dc/elements/1.1/"
   xmlns:dct="http://purl.org/dc/terms/"
   xmlns:rdf="http://www.w3.org/1999/02/22-rdf-syntax-ns#"
   xmlns:schema="https://schema.org/"
   xmlns:skos="http://www.w3.org/2004/02/skos/core#"
>
  <rdf:Description rdf:about="https://doi.org/10.6069/uwlswd.n7sa-ny50#d">
    <rdf:type rdf:resource="http://www.w3.org/2004/02/skos/core#Concept"/>
    <skos:inScheme rdf:resource="https://doi.org/10.6069/uwlswd.n7sa-ny50"/>
    <skos:prefLabel xml:lang="en">videodisc</skos:prefLabel>
    <skos:definition xml:lang="en">Flat disc of plastic or other material on which video signals,
         with or without sound, are recorded.</skos:definition>
    <skos:scopeNote xml:lang="en">Various videodisc systems have been developed (e.g.,
         laser-optical, capacitance, magnetic, etc.).</skos:scopeNote>
    <skos:notation>d</skos:notation>
  </rdf:Description>
  <rdf:Description rdf:about="https://doi.org/10.6069/uwlswd.n7sa-ny50">
    <rdf:type rdf:resource="http://www.w3.org/2004/02/skos/core#ConceptScheme"/>
    <dct:type rdf:resource="http://purl.org/dc/dcmitype/Dataset"/>
    <dct:title xml:lang="en">Videorecording: specific material designation</dct:title>
    <dct:alternative xml:lang="en">MARC21 007/01 values for videorecordings expressed using
         RDF</dct:alternative>
    <dct:description xml:lang="en">Special class of videorecording to which an item
         belongs.</dct:description>
    <schema:disambiguatingDescription xml:lang="en">SKOS Concept Scheme for MARC 00X
         Values</schema:disambiguatingDescription>
    <dct:publisher rdf:resource="http://viaf.org/viaf/139541794"/>
    <dct:source rdf:resource="https://www.loc.gov/marc/bibliographic/bd007.html"/>
    <dct:source rdf:resource="http://marc21rdf.info"/>
    <dct:provenance rdf:resource="https://doi.org/10.6069/uwlswd.2e2b-y833#marc00Xvalues"/>
    <dct:creator rdf:resource="http://viaf.org/viaf/139541794"/>
    <dct:contributor rdf:resource="http://viaf.org/viaf/151962300"/>
    <dct:issued>2024</dct:issued>
    <dc:contributor xml:lang="en">Metadata Management Associates</dc:contributor>
    <dc:language>en</dc:language>
    <dct:license rdf:resource="http://creativecommons.org/publicdomain/zero/1.0"/>
    <schema:version>1-0-0</schema:version>
    <dct:format rdf:resource="http://www.w3.org/ns/formats/RDF_XML"/>
    <dct:hasFormat rdf:resource="https://uwlib-cams.github.io/uwlswd_vocabs_marc_007/videorecording_specific_material_designation/videorecording_specific_material_designation.ttl"/>
    <dct:hasFormat rdf:resource="https://uwlib-cams.github.io/uwlswd_vocabs_marc_007/videorecording_specific_material_designation/videorecording_specific_material_designation.nt"/>
    <dct:hasFormat rdf:resource="https://uwlib-cams.github.io/uwlswd_vocabs_marc_007/videorecording_specific_material_designation/videorecording_specific_material_designation.jsonld"/>
    <dct:hasFormat rdf:resource="https://uwlib-cams.github.io/uwlswd_vocabs_marc_007/videorecording_specific_material_designation/videorecording_specific_material_designation.html"/>
  </rdf:Description>
  <rdf:Description rdf:about="https://doi.org/10.6069/uwlswd.n7sa-ny50#f">
    <rdf:type rdf:resource="http://www.w3.org/2004/02/skos/core#Concept"/>
    <skos:inScheme rdf:resource="https://doi.org/10.6069/uwlswd.n7sa-ny50"/>
    <skos:prefLabel xml:lang="en">videocassette</skos:prefLabel>
    <skos:definition xml:lang="en">Videorecording on tape encased in a cassette which runs
         reel-to-reel.</skos:definition>
    <skos:notation>f</skos:notation>
  </rdf:Description>
  <rdf:Description rdf:about="https://doi.org/10.6069/uwlswd.n7sa-ny50#r">
    <rdf:type rdf:resource="http://www.w3.org/2004/02/skos/core#Concept"/>
    <skos:inScheme rdf:resource="https://doi.org/10.6069/uwlswd.n7sa-ny50"/>
    <skos:prefLabel xml:lang="en">videoreel</skos:prefLabel>
    <skos:definition xml:lang="en">Videorecording on a spool of tape mounted on a reel and
         designed to play from reel-to-reel across a playback pick-up device.</skos:definition>
    <skos:notation>r</skos:notation>
  </rdf:Description>
  <rdf:Description rdf:about="https://doi.org/10.6069/uwlswd.n7sa-ny50#n">
    <rdf:type rdf:resource="http://www.w3.org/2004/02/skos/core#Concept"/>
    <skos:inScheme rdf:resource="https://doi.org/10.6069/uwlswd.n7sa-ny50"/>
    <skos:prefLabel xml:lang="en">not applicable [obsolete]</skos:prefLabel>
    <skos:notation>n</skos:notation>
  </rdf:Description>
  <rdf:Description rdf:about="https://doi.org/10.6069/uwlswd.n7sa-ny50#z">
    <rdf:type rdf:resource="http://www.w3.org/2004/02/skos/core#Concept"/>
    <skos:inScheme rdf:resource="https://doi.org/10.6069/uwlswd.n7sa-ny50"/>
    <skos:prefLabel xml:lang="en">other</skos:prefLabel>
    <skos:definition xml:lang="en">Specific material designation other than videocartridge,
         videodisc, videocassette, or videoreel.</skos:definition>
    <skos:notation>z</skos:notation>
  </rdf:Description>
  <rdf:Description rdf:about="https://doi.org/10.6069/uwlswd.n7sa-ny50#u">
    <rdf:type rdf:resource="http://www.w3.org/2004/02/skos/core#Concept"/>
    <skos:inScheme rdf:resource="https://doi.org/10.6069/uwlswd.n7sa-ny50"/>
    <skos:prefLabel xml:lang="en">unspecified</skos:prefLabel>
    <skos:definition xml:lang="en">Special material designation for the videorecording is not
         specified.</skos:definition>
    <skos:notation>u</skos:notation>
  </rdf:Description>
  <rdf:Description rdf:about="https://doi.org/10.6069/uwlswd.n7sa-ny50#c">
    <rdf:type rdf:resource="http://www.w3.org/2004/02/skos/core#Concept"/>
    <skos:inScheme rdf:resource="https://doi.org/10.6069/uwlswd.n7sa-ny50"/>
    <skos:prefLabel xml:lang="en">videocartridge</skos:prefLabel>
    <skos:definition xml:lang="en">Videorecording on tape encased in a cartridge and which has the
         ends joined together to form a continuous loop.</skos:definition>
    <skos:notation>c</skos:notation>
  </rdf:Description>
  <rdf:Description rdf:about="https://doi.org/10.6069/uwlswd.n7sa-ny50#pound">
    <rdf:type rdf:resource="http://www.w3.org/2004/02/skos/core#Concept"/>
    <skos:inScheme rdf:resource="https://doi.org/10.6069/uwlswd.n7sa-ny50"/>
    <skos:prefLabel xml:lang="en">not applicable or no attempt to code [obsolete]</skos:prefLabel>
    <skos:notation>#</skos:notation>
  </rdf:Description>
</rdf:RDF>
