@prefix dc: <http://purl.org/dc/elements/1.1/> .
@prefix dct: <http://purl.org/dc/terms/> .
@prefix schema: <https://schema.org/> .
@prefix skos: <http://www.w3.org/2004/02/skos/core#> .

<https://doi.org/10.6069/uwlswd.n7sa-ny50#c> a skos:Concept ;
    skos:definition """Videorecording on tape encased in a cartridge and which has the
         ends joined together to form a continuous loop."""@en ;
    skos:inScheme <https://doi.org/10.6069/uwlswd.n7sa-ny50> ;
    skos:notation "c" ;
    skos:prefLabel "videocartridge"@en .

<https://doi.org/10.6069/uwlswd.n7sa-ny50#d> a skos:Concept ;
    skos:definition """Flat disc of plastic or other material on which video signals,
         with or without sound, are recorded."""@en ;
    skos:inScheme <https://doi.org/10.6069/uwlswd.n7sa-ny50> ;
    skos:notation "d" ;
    skos:prefLabel "videodisc"@en ;
    skos:scopeNote """Various videodisc systems have been developed (e.g.,
         laser-optical, capacitance, magnetic, etc.)."""@en .

<https://doi.org/10.6069/uwlswd.n7sa-ny50#f> a skos:Concept ;
    skos:definition """Videorecording on tape encased in a cassette which runs
         reel-to-reel."""@en ;
    skos:inScheme <https://doi.org/10.6069/uwlswd.n7sa-ny50> ;
    skos:notation "f" ;
    skos:prefLabel "videocassette"@en .

<https://doi.org/10.6069/uwlswd.n7sa-ny50#n> a skos:Concept ;
    skos:inScheme <https://doi.org/10.6069/uwlswd.n7sa-ny50> ;
    skos:notation "n" ;
    skos:prefLabel "not applicable [obsolete]"@en .

<https://doi.org/10.6069/uwlswd.n7sa-ny50#pound> a skos:Concept ;
    skos:inScheme <https://doi.org/10.6069/uwlswd.n7sa-ny50> ;
    skos:notation "#" ;
    skos:prefLabel "not applicable or no attempt to code [obsolete]"@en .

<https://doi.org/10.6069/uwlswd.n7sa-ny50#r> a skos:Concept ;
    skos:definition """Videorecording on a spool of tape mounted on a reel and
         designed to play from reel-to-reel across a playback pick-up device."""@en ;
    skos:inScheme <https://doi.org/10.6069/uwlswd.n7sa-ny50> ;
    skos:notation "r" ;
    skos:prefLabel "videoreel"@en .

<https://doi.org/10.6069/uwlswd.n7sa-ny50#u> a skos:Concept ;
    skos:definition """Special material designation for the videorecording is not
         specified."""@en ;
    skos:inScheme <https://doi.org/10.6069/uwlswd.n7sa-ny50> ;
    skos:notation "u" ;
    skos:prefLabel "unspecified"@en .

<https://doi.org/10.6069/uwlswd.n7sa-ny50#z> a skos:Concept ;
    skos:definition """Specific material designation other than videocartridge,
         videodisc, videocassette, or videoreel."""@en ;
    skos:inScheme <https://doi.org/10.6069/uwlswd.n7sa-ny50> ;
    skos:notation "z" ;
    skos:prefLabel "other"@en .

<https://doi.org/10.6069/uwlswd.n7sa-ny50> a skos:ConceptScheme ;
    dc:contributor "Metadata Management Associates"@en ;
    dc:language "en" ;
    dct:alternative """MARC21 007/01 values for videorecordings expressed using
         RDF"""@en ;
    dct:contributor <http://viaf.org/viaf/151962300> ;
    dct:creator <http://viaf.org/viaf/139541794> ;
    dct:description """Special class of videorecording to which an item
         belongs."""@en ;
    dct:format <http://www.w3.org/ns/formats/Turtle> ;
    dct:hasFormat <https://uwlib-cams.github.io/uwlswd_vocabs_marc_007/videorecording_specific_material_designation/videorecording_specific_material_designation.html>,
        <https://uwlib-cams.github.io/uwlswd_vocabs_marc_007/videorecording_specific_material_designation/videorecording_specific_material_designation.jsonld>,
        <https://uwlib-cams.github.io/uwlswd_vocabs_marc_007/videorecording_specific_material_designation/videorecording_specific_material_designation.nt>,
        <https://uwlib-cams.github.io/uwlswd_vocabs_marc_007/videorecording_specific_material_designation/videorecording_specific_material_designation.rdf> ;
    dct:issued "2024" ;
    dct:license <http://creativecommons.org/publicdomain/zero/1.0> ;
    dct:provenance <https://doi.org/10.6069/uwlswd.2e2b-y833#marc00Xvalues> ;
    dct:publisher <http://viaf.org/viaf/139541794> ;
    dct:source <http://marc21rdf.info>,
        <https://www.loc.gov/marc/bibliographic/bd007.html> ;
    dct:title "Videorecording: specific material designation"@en ;
    dct:type <http://purl.org/dc/dcmitype/Dataset> ;
    schema:disambiguatingDescription """SKOS Concept Scheme for MARC 00X
         Values"""@en ;
    schema:version "1-0-0" .

