@prefix dc: <http://purl.org/dc/elements/1.1/> .
@prefix dct: <http://purl.org/dc/terms/> .
@prefix schema: <https://schema.org/> .
@prefix skos: <http://www.w3.org/2004/02/skos/core#> .

<https://doi.org/10.6069/uwlswd.yayd-4y11#a> a skos:Concept ;
    skos:definition """Sound to accompany a projected graphic is carried on an optical
         track that is part of a film."""@en ;
    skos:inScheme <https://doi.org/10.6069/uwlswd.yayd-4y11> ;
    skos:notation "a" ;
    skos:prefLabel "optical sound track on motion picture film"@en ;
    skos:scopeNote """For 16 and 35 mm. films, it is usually assumed that sound is
         carried on an optical track."""@en .

<https://doi.org/10.6069/uwlswd.yayd-4y11#b> a skos:Concept ;
    skos:definition """Sound to accompany a projected graphic is carried on a magnetic
         track that is part of the film."""@en ;
    skos:inScheme <https://doi.org/10.6069/uwlswd.yayd-4y11> ;
    skos:notation "b" ;
    skos:prefLabel "magnetic sound track on motion picture film"@en ;
    skos:scopeNote """70 mm. motion picture films often include magnetic sound
         tracks."""@en .

<https://doi.org/10.6069/uwlswd.yayd-4y11#c> a skos:Concept ;
    skos:definition """Sound to accompany an item is carried on a magnetic audio tape
         cartridge."""@en ;
    skos:inScheme <https://doi.org/10.6069/uwlswd.yayd-4y11> ;
    skos:notation "c" ;
    skos:prefLabel "magnetic audio tape in cartridge"@en .

<https://doi.org/10.6069/uwlswd.yayd-4y11#d> a skos:Concept ;
    skos:definition """Sound to accompany an item is carried on a sound
         disc."""@en ;
    skos:inScheme <https://doi.org/10.6069/uwlswd.yayd-4y11> ;
    skos:notation "d" ;
    skos:prefLabel "sound disc"@en ;
    skos:scopeNote """This method of providing for sound is typically used with
         filmstrips. Sound discs include 7, 10, and 12 in. vinyl phonograph records and 4 3/4 in.
         compact discs."""@en .

<https://doi.org/10.6069/uwlswd.yayd-4y11#e> a skos:Concept ;
    skos:definition """Sound to accompany an item is carried on a reel of magnetic
         audio tape."""@en ;
    skos:inScheme <https://doi.org/10.6069/uwlswd.yayd-4y11> ;
    skos:notation "e" ;
    skos:prefLabel "magnetic audio tape on reel"@en .

<https://doi.org/10.6069/uwlswd.yayd-4y11#f> a skos:Concept ;
    skos:definition """Sound to accompany an item is carried on a cassette of magnetic
         audio tape."""@en ;
    skos:inScheme <https://doi.org/10.6069/uwlswd.yayd-4y11> ;
    skos:notation "f" ;
    skos:prefLabel "magnetic audio tape in cassette"@en .

<https://doi.org/10.6069/uwlswd.yayd-4y11#g> a skos:Concept ;
    skos:definition """Sound to accompany a projected graphic is carried on both an
         optical and magnetic track."""@en ;
    skos:inScheme <https://doi.org/10.6069/uwlswd.yayd-4y11> ;
    skos:notation "g" ;
    skos:prefLabel """optical and magnetic sound track on motion picture
         film"""@en .

<https://doi.org/10.6069/uwlswd.yayd-4y11#gx> a skos:Concept ;
    skos:inScheme <https://doi.org/10.6069/uwlswd.yayd-4y11> ;
    skos:notation "g" ;
    skos:prefLabel "other [obsolete]"@en .

<https://doi.org/10.6069/uwlswd.yayd-4y11#h> a skos:Concept ;
    skos:definition """Sound to accompany an item is included as part of a
         videotape."""@en ;
    skos:inScheme <https://doi.org/10.6069/uwlswd.yayd-4y11> ;
    skos:notation "h" ;
    skos:prefLabel "videotape"@en ;
    skos:scopeNote """Videotape is not ordinarily used to record only
         sound."""@en .

<https://doi.org/10.6069/uwlswd.yayd-4y11#i> a skos:Concept ;
    skos:definition """Sound to accompany an item is included as part of a
         videodisc."""@en ;
    skos:inScheme <https://doi.org/10.6069/uwlswd.yayd-4y11> ;
    skos:notation "i" ;
    skos:prefLabel "videodisc"@en ;
    skos:scopeNote """Videodiscs are not ordinarily used to record only sound. A
         distinction must be made between videodiscs (e.g., 12 in. laser-scan videodiscs that
         include video information) and compact discs that are used to record sound only (e.g., 4
         3/4 in. audio compact discs). The technology to physically record video or audio
         information on digital disc systems is the same."""@en .

<https://doi.org/10.6069/uwlswd.yayd-4y11#pound> a skos:Concept ;
    skos:definition "Sound is not present."@en ;
    skos:inScheme <https://doi.org/10.6069/uwlswd.yayd-4y11> ;
    skos:notation "#" ;
    skos:prefLabel "no sound (silent)"@en .

<https://doi.org/10.6069/uwlswd.yayd-4y11#u> a skos:Concept ;
    skos:definition "Medium for sound is not known."@en ;
    skos:inScheme <https://doi.org/10.6069/uwlswd.yayd-4y11> ;
    skos:notation "u" ;
    skos:prefLabel "unknown"@en .

<https://doi.org/10.6069/uwlswd.yayd-4y11#z> a skos:Concept ;
    skos:definition """Medium for sound other than no sound (silent), optical sound
         track on motion picture film, magnetic sound track on motion picture film, magnetic audio
         tape in cartridge, sound disc, magnetic audio tape on reel, magnetic audio tape in
         cassette, optical and magnetic sound track on videotape, or videodisc."""@en ;
    skos:inScheme <https://doi.org/10.6069/uwlswd.yayd-4y11> ;
    skos:notation "z" ;
    skos:prefLabel "other"@en .

<https://doi.org/10.6069/uwlswd.yayd-4y11> a skos:ConceptScheme ;
    dc:contributor "Metadata Management Associates"@en ;
    dc:language "en" ;
    dct:alternative """MARC21 007/06 values for projected graphics expressed using
         RDF"""@en ;
    dct:contributor <http://viaf.org/viaf/151962300> ;
    dct:creator <http://viaf.org/viaf/139541794> ;
    dct:description """Specific medium used to carry the sound of an item (whether the
         sound is on the projected graphic or separate) and the type of sound playback required for
         the item."""@en ;
    dct:format <http://www.w3.org/ns/formats/Turtle> ;
    dct:hasFormat <https://uwlib-cams.github.io/uwlswd_vocabs_marc_007/projected_graphic_medium_for_sound/projected_graphic_medium_for_sound.html>,
        <https://uwlib-cams.github.io/uwlswd_vocabs_marc_007/projected_graphic_medium_for_sound/projected_graphic_medium_for_sound.jsonld>,
        <https://uwlib-cams.github.io/uwlswd_vocabs_marc_007/projected_graphic_medium_for_sound/projected_graphic_medium_for_sound.nt>,
        <https://uwlib-cams.github.io/uwlswd_vocabs_marc_007/projected_graphic_medium_for_sound/projected_graphic_medium_for_sound.rdf> ;
    dct:issued "2024" ;
    dct:license <http://creativecommons.org/publicdomain/zero/1.0> ;
    dct:provenance <https://doi.org/10.6069/uwlswd.2e2b-y833#marc00Xvalues> ;
    dct:publisher <http://viaf.org/viaf/139541794> ;
    dct:source <http://marc21rdf.info>,
        <https://www.loc.gov/marc/bibliographic/bd007.html> ;
    dct:title "Projected graphic: medium for sound"@en ;
    dct:type <http://purl.org/dc/dcmitype/Dataset> ;
    schema:disambiguatingDescription """SKOS Concept Scheme for MARC 00X
         Values"""@en ;
    schema:version "1-0-0" .

