<?xml version='1.0' encoding='UTF-8'?>
<rdf:RDF xmlns:dc="http://purl.org/dc/elements/1.1/" xmlns:dct="http://purl.org/dc/terms/" xmlns:rdf="http://www.w3.org/1999/02/22-rdf-syntax-ns#" xmlns:schema="https://schema.org/" xmlns:skos="http://www.w3.org/2004/02/skos/core#">
  <rdf:Description rdf:about="https://doi.org/10.6069/uwlswd.b441-n943#v">
    <rdf:type rdf:resource="http://www.w3.org/2004/02/skos/core#Concept"/>
    <skos:inScheme rdf:resource="https://doi.org/10.6069/uwlswd.b441-n943"/>
    <skos:prefLabel xml:lang="en">DVD</skos:prefLabel>
    <skos:definition xml:lang="en">Laser optical (reflective) videorecording system that uses a
         digital technique called PCM (Pulse Code Modulation) to represent video information on a
         grooveless, smooth, round plastic disc. The disc is read (played back) by a weak laser beam
         that registers data appearing on the disc as tiny pits or depressions of uniform
         length.</skos:definition>
    <skos:scopeNote xml:lang="en">DVDs are usually 4 3/4 inch in diameter (but a smaller 3 inch
         diameter disc may be produced commercially in some cases) and the disc or its packaging
         usually bear the term or trademark: DVD, DVD VIDEO, or VIDEO CD (in this case, the
         trademark is the standard one for COMPACT DISC, but with the added phrase DIGITAL VIDEO
         below it). This system has been in use commercially since late 1996.</skos:scopeNote>
    <skos:notation>v</skos:notation>
  </rdf:Description>
  <rdf:Description rdf:about="https://doi.org/10.6069/uwlswd.b441-n943#u">
    <rdf:type rdf:resource="http://www.w3.org/2004/02/skos/core#Concept"/>
    <skos:inScheme rdf:resource="https://doi.org/10.6069/uwlswd.b441-n943"/>
    <skos:prefLabel xml:lang="en">unknown</skos:prefLabel>
    <skos:definition xml:lang="en">Videorecording format is not known.</skos:definition>
    <skos:notation>u</skos:notation>
  </rdf:Description>
  <rdf:Description rdf:about="https://doi.org/10.6069/uwlswd.b441-n943#e">
    <rdf:type rdf:resource="http://www.w3.org/2004/02/skos/core#Concept"/>
    <skos:inScheme rdf:resource="https://doi.org/10.6069/uwlswd.b441-n943"/>
    <skos:prefLabel xml:lang="en">Type C (1 in., reel)</skos:prefLabel>
    <skos:definition xml:lang="en">Used for the 1 inch videotape recording system utilizing one
         video head and tape runs at 9.61 inches per second. Type B system uses 2 heads and runs at
         9.65 inches per second; Type A is an obsolete early system. Type B is still used in the
         U.S. and overseas (as of 1982), but Type C is the 1 inch format most widely employed as the
         broadcasting standard in the U.S. and overseas. Type C equipment and technology are made by
         Sony, RCA, and others.</skos:definition>
    <skos:notation>e</skos:notation>
  </rdf:Description>
  <rdf:Description rdf:about="https://doi.org/10.6069/uwlswd.b441-n943#q">
    <rdf:type rdf:resource="http://www.w3.org/2004/02/skos/core#Concept"/>
    <skos:inScheme rdf:resource="https://doi.org/10.6069/uwlswd.b441-n943"/>
    <skos:prefLabel xml:lang="en">Hi-8 mm.</skos:prefLabel>
    <skos:definition xml:lang="en">8 mm. format designed for higher resolution than standard 8mm.
         tape. It is a consumer-market format that uses 8 mm. metal particle or evaportated metal
         tape, housed in a mini-cassette.</skos:definition>
    <skos:notation>q</skos:notation>
  </rdf:Description>
  <rdf:Description rdf:about="https://doi.org/10.6069/uwlswd.b441-n943">
    <rdf:type rdf:resource="http://www.w3.org/2004/02/skos/core#ConceptScheme"/>
    <dct:type rdf:resource="http://purl.org/dc/dcmitype/Dataset"/>
    <dct:title xml:lang="en">Videorecording: format</dct:title>
    <dct:alternative xml:lang="en">MARC21 007/04 values for videorecordings expressed using
         RDF</dct:alternative>
    <dct:description xml:lang="en">Videotape or videodisc recording format.</dct:description>
    <schema:disambiguatingDescription xml:lang="en">SKOS Concept Scheme for MARC 00X
         Values</schema:disambiguatingDescription>
    <dct:publisher rdf:resource="http://viaf.org/viaf/139541794"/>
    <dct:source rdf:resource="https://www.loc.gov/marc/bibliographic/bd007.html"/>
    <dct:source rdf:resource="http://marc21rdf.info"/>
    <dct:provenance rdf:resource="https://doi.org/10.6069/uwlswd.2e2b-y833#marc00Xvalues"/>
    <dct:creator rdf:resource="http://viaf.org/viaf/139541794"/>
    <dct:contributor rdf:resource="http://viaf.org/viaf/151962300"/>
    <dct:issued>2024</dct:issued>
    <dc:contributor xml:lang="en">Metadata Management Associates</dc:contributor>
    <dc:language>en</dc:language>
    <dct:license rdf:resource="http://creativecommons.org/publicdomain/zero/1.0"/>
    <schema:version>1-0-0</schema:version>
    <dct:format rdf:resource="http://www.w3.org/ns/formats/RDF_XML"/>
  </rdf:Description>
  <rdf:Description rdf:about="https://doi.org/10.6069/uwlswd.b441-n943#g">
    <rdf:type rdf:resource="http://www.w3.org/2004/02/skos/core#Concept"/>
    <skos:inScheme rdf:resource="https://doi.org/10.6069/uwlswd.b441-n943"/>
    <skos:prefLabel xml:lang="en">laserdisc</skos:prefLabel>
    <skos:definition xml:lang="en">Laser optical (reflective) videorecording system that uses an
         analog technique called PWM (Pulse Width Modulation) to represent video information on a
         grooveless, smooth, round plastic disc. The disc is read (played back) by a weak laser beam
         that registers data appearing on the disc as tiny pits or depressions of varying
         lengths.</skos:definition>
    <skos:scopeNote xml:lang="en">Laserdiscs exist in three standard commercially produced sizes:
         12, 8, and 4 3/4 inch. The 12 inch disc is the most common size and is typically used for
         movies; the disc or its packaging usually bears an LD trademark (the phrase "LASER DISC" or
         "Laser Vision" usually appears as the lower part of that LD trademark); alternatively,
         LASER VIDEODISC, DiscoVision, LaserDisc, LaserVision, or a similar phrase may appear
         instead of the LD trademark. The 8 and 4 3/4 inch discs are uncommon and typically used for
         music videos or other short video programs; the disc or its packaging usually bears one of
         these terms or trademarks: CDV (CD VIDEO), VSD (VIDEO SINGLE DISC), or LD (LASER DISC).
         This system started commercial use in 1978, but production declined rapidly after 1998 due
         to the success of the DVD format.</skos:scopeNote>
    <skos:notation>g</skos:notation>
  </rdf:Description>
  <rdf:Description rdf:about="https://doi.org/10.6069/uwlswd.b441-n943#a">
    <rdf:type rdf:resource="http://www.w3.org/2004/02/skos/core#Concept"/>
    <skos:inScheme rdf:resource="https://doi.org/10.6069/uwlswd.b441-n943"/>
    <skos:prefLabel xml:lang="en">Beta (1/2 in., videocassette)</skos:prefLabel>
    <skos:definition xml:lang="en">Used for the home video system introduced in 1975 by Sony for
         home videorecording and playback on 1/2 inch videotape. It is distinguished by the size of
         the cassette, its U-load tape threading, and technical capabilities. This format is also
         known as Betamax.</skos:definition>
    <skos:notation>a</skos:notation>
  </rdf:Description>
  <rdf:Description rdf:about="https://doi.org/10.6069/uwlswd.b441-n943#p">
    <rdf:type rdf:resource="http://www.w3.org/2004/02/skos/core#Concept"/>
    <skos:inScheme rdf:resource="https://doi.org/10.6069/uwlswd.b441-n943"/>
    <skos:prefLabel xml:lang="en">8 mm.</skos:prefLabel>
    <skos:definition xml:lang="en">8 mm. format designed for small consumer-market
         camera/recorders (camcorders) using 8 mm. metal particle tape, housed in a mini-cassette.
         The video quality is comparable to standard VHS. The audio quality is superior to similar
         mini formats.</skos:definition>
    <skos:notation>p</skos:notation>
  </rdf:Description>
  <rdf:Description rdf:about="https://doi.org/10.6069/uwlswd.b441-n943#o">
    <rdf:type rdf:resource="http://www.w3.org/2004/02/skos/core#Concept"/>
    <skos:inScheme rdf:resource="https://doi.org/10.6069/uwlswd.b441-n943"/>
    <skos:prefLabel xml:lang="en">D-2 (3/4 in., videocassette)</skos:prefLabel>
    <skos:definition xml:lang="en">D-2 videorecording format, a professional digital
         videorecording format using composite coding on 3/4 inch metal particle tape, housed in a
         cassette. The digital encoding allows for multi-generation signal transfer (copying or
         dubbing) without signal degradation. Duplicate recordings are effectively identical to the
         original master. There are four independently editable PCM audio channels, offering a
         dynamic range of more than 90 db (decibels). Additionally, it has separate tracks for an
         analog audio cue and time code.</skos:definition>
    <skos:notation>o</skos:notation>
  </rdf:Description>
  <rdf:Description rdf:about="https://doi.org/10.6069/uwlswd.b441-n943#pound">
    <rdf:type rdf:resource="http://www.w3.org/2004/02/skos/core#Concept"/>
    <skos:inScheme rdf:resource="https://doi.org/10.6069/uwlswd.b441-n943"/>
    <skos:prefLabel xml:lang="en">not applicable or no attempt to code [obsolete]</skos:prefLabel>
    <skos:notation>#</skos:notation>
  </rdf:Description>
  <rdf:Description rdf:about="https://doi.org/10.6069/uwlswd.b441-n943#j">
    <rdf:type rdf:resource="http://www.w3.org/2004/02/skos/core#Concept"/>
    <skos:inScheme rdf:resource="https://doi.org/10.6069/uwlswd.b441-n943"/>
    <skos:prefLabel xml:lang="en">Betacam SP (1/2 in., videocassette)</skos:prefLabel>
    <skos:definition xml:lang="en">Betacam SP videorecording format, a professional analog format
         using component coding recorded on 1/2 inch metal tape, housed in a cassette. It is
         designed to yield a higher grade recording than the regular Betacam format, providing
         improved video quality and a better audio signal-to-noise ratio. There are two analog video
         tracks plus two FM (CD quality) audio tracks.</skos:definition>
    <skos:notation>j</skos:notation>
  </rdf:Description>
  <rdf:Description rdf:about="https://doi.org/10.6069/uwlswd.b441-n943#h">
    <rdf:type rdf:resource="http://www.w3.org/2004/02/skos/core#Concept"/>
    <skos:inScheme rdf:resource="https://doi.org/10.6069/uwlswd.b441-n943"/>
    <skos:prefLabel xml:lang="en">ced (capacitance electronic disc) videodisc</skos:prefLabel>
    <skos:definition xml:lang="en">CED videorecording system is based on a plastic disc, usually
         12 in. in diameter, on which visual information is recorded as deep pits in the bottom of
         the grooves. This visual information is read by a needle-in-the-groove type of electronic
         stylus that translates variance in capacitance into a video and audio signal. The CED disc
         is characteristically housed in a protective jacket.</skos:definition>
    <skos:scopeNote xml:lang="en">In 1984, the manufacturer of CED players, RCA, announced its
         decision to cease production of the "RCA Selectavision" players.</skos:scopeNote>
    <skos:notation>h</skos:notation>
  </rdf:Description>
  <rdf:Description rdf:about="https://doi.org/10.6069/uwlswd.b441-n943#k">
    <rdf:type rdf:resource="http://www.w3.org/2004/02/skos/core#Concept"/>
    <skos:inScheme rdf:resource="https://doi.org/10.6069/uwlswd.b441-n943"/>
    <skos:prefLabel xml:lang="en">Super-VHS (1/2 in., videocassette)</skos:prefLabel>
    <skos:definition xml:lang="en">Super-VHS format, which was originally designed for the
         consumer market to encode analog signals using a helical scan on 1/2 inch ferric-oxide
         tape, is housed in a standard cassette. It has gained acceptance professionally in the
         broadcast industry and is now considered a professional format. Super-VHS format machines
         encode 400 lines of horizontal resolution and can play back videotapes recorded on regular
         VHS machines. Super-VHS requires high-grade tape and a high-resolution monitor equipped
         with separate Y/C (Luminance/Chrominance) video inputs. Super-VHS-C is the same video
         format but uses a special compact mini-cassette (often used with hand-held video cameras).
         These mini-cassettes can be used with standard VHS recorders by means of a special adapter
         cassette into which the mini-cassette is inserted.</skos:definition>
    <skos:notation>k</skos:notation>
  </rdf:Description>
  <rdf:Description rdf:about="https://doi.org/10.6069/uwlswd.b441-n943#s">
    <rdf:type rdf:resource="http://www.w3.org/2004/02/skos/core#Concept"/>
    <skos:inScheme rdf:resource="https://doi.org/10.6069/uwlswd.b441-n943"/>
    <skos:prefLabel xml:lang="en">Blu-ray disc</skos:prefLabel>
    <skos:definition xml:lang="en">Optical disc format designed for high-definition video and data
         storage developed by Sony/Phillips. Blu-ray uses a blue-violet laser with a shorter wave
         length to allow for greater data storage in a smaller space. Requires a special player to
         view the disc.</skos:definition>
    <skos:notation>s</skos:notation>
  </rdf:Description>
  <rdf:Description rdf:about="https://doi.org/10.6069/uwlswd.b441-n943#b">
    <rdf:type rdf:resource="http://www.w3.org/2004/02/skos/core#Concept"/>
    <skos:inScheme rdf:resource="https://doi.org/10.6069/uwlswd.b441-n943"/>
    <skos:prefLabel xml:lang="en">VHS (1/2 in., videocassette)</skos:prefLabel>
    <skos:definition xml:lang="en">Used for the home video system introduced in 1977 by Japan
         Victor Corporation (JVC) for home videorecording and playback on 1/2 inch videotape. It is
         distinguished by the size of the cassette, its M-load tape threading, and technical
         capabilities. VHS stands for "Video Home System."</skos:definition>
    <skos:notation>b</skos:notation>
  </rdf:Description>
  <rdf:Description rdf:about="https://doi.org/10.6069/uwlswd.b441-n943#z">
    <rdf:type rdf:resource="http://www.w3.org/2004/02/skos/core#Concept"/>
    <skos:inScheme rdf:resource="https://doi.org/10.6069/uwlswd.b441-n943"/>
    <skos:prefLabel xml:lang="en">other</skos:prefLabel>
    <skos:definition xml:lang="en">Videorecording format other than Beta (1/2 in., videocassette),
         VHS (1/2 in., videocassette), U-matic (3/4 in., videocassette), EIAJ (1/2 in. reel), Type C
         (1 in., reel), Quadruplex (1 in. or 2 in., reel), Laserdisc, CED (Capacitance Electronic
         Disc) videodisc, Betacam (1/2 in., videocassette), Betacam SP (1/2 in., videocassette),
         Super-VHS (1/2 in., videocassette), M-II (1/2 in., videocassette), D-2 (3/4 in.,
         videocassette), 8 mm., Hi-8 mm., DVD, or Blu-ray disc.</skos:definition>
    <skos:notation>z</skos:notation>
  </rdf:Description>
  <rdf:Description rdf:about="https://doi.org/10.6069/uwlswd.b441-n943#d">
    <rdf:type rdf:resource="http://www.w3.org/2004/02/skos/core#Concept"/>
    <skos:inScheme rdf:resource="https://doi.org/10.6069/uwlswd.b441-n943"/>
    <skos:prefLabel xml:lang="en">EIAJ (1/2 in. reel)</skos:prefLabel>
    <skos:definition xml:lang="en">Used for the standard 1/2 inch reel-to-reel helical scan
         videotape system named for the Electronics Industries Association of Japan which set the
         standards for 1/2 in. video tape recorders manufactured since 1969. Referred to as "the old
         trailblazer."</skos:definition>
    <skos:notation>d</skos:notation>
  </rdf:Description>
  <rdf:Description rdf:about="https://doi.org/10.6069/uwlswd.b441-n943#c">
    <rdf:type rdf:resource="http://www.w3.org/2004/02/skos/core#Concept"/>
    <skos:inScheme rdf:resource="https://doi.org/10.6069/uwlswd.b441-n943"/>
    <skos:prefLabel xml:lang="en">U-matic (3/4 in., videocassette)</skos:prefLabel>
    <skos:definition xml:lang="en">Used for a video format using Sony's trademark name which
         refers to its tape threading path in a U-shape. It is the worldwide standard for 3/4 inch
         videotape and is used extensively in industrial and broadcast production. Like the two 1/2
         in. home video formats, it uses a helical scan recording system. It is also known as U type
         standard.</skos:definition>
    <skos:notation>c</skos:notation>
  </rdf:Description>
  <rdf:Description rdf:about="https://doi.org/10.6069/uwlswd.b441-n943#i">
    <rdf:type rdf:resource="http://www.w3.org/2004/02/skos/core#Concept"/>
    <skos:inScheme rdf:resource="https://doi.org/10.6069/uwlswd.b441-n943"/>
    <skos:prefLabel xml:lang="en">Betacam (1/2 in., videocassette)</skos:prefLabel>
    <skos:definition xml:lang="en">Betacam videorecording format, a professional analog format
         using component coding recorded on 1/2 inch oxide tape, housed in a
         cassette.</skos:definition>
    <skos:notation>i</skos:notation>
  </rdf:Description>
  <rdf:Description rdf:about="https://doi.org/10.6069/uwlswd.b441-n943#m">
    <rdf:type rdf:resource="http://www.w3.org/2004/02/skos/core#Concept"/>
    <skos:inScheme rdf:resource="https://doi.org/10.6069/uwlswd.b441-n943"/>
    <skos:prefLabel xml:lang="en">M-II (1/2 in., videocassette)</skos:prefLabel>
    <skos:definition xml:lang="en">M-II videorecording format, a professional analog format using
         1/2 inch metallic tape, housed in a cassette.</skos:definition>
    <skos:scopeNote xml:lang="en">It was developed by Panasonic as an alternative to the Betacam
         format developed by Sony.</skos:scopeNote>
    <skos:notation>m</skos:notation>
  </rdf:Description>
  <rdf:Description rdf:about="https://doi.org/10.6069/uwlswd.b441-n943#n">
    <rdf:type rdf:resource="http://www.w3.org/2004/02/skos/core#Concept"/>
    <skos:inScheme rdf:resource="https://doi.org/10.6069/uwlswd.b441-n943"/>
    <skos:prefLabel xml:lang="en">not applicable [obsolete]</skos:prefLabel>
    <skos:notation>n</skos:notation>
  </rdf:Description>
  <rdf:Description rdf:about="https://doi.org/10.6069/uwlswd.b441-n943#f">
    <rdf:type rdf:resource="http://www.w3.org/2004/02/skos/core#Concept"/>
    <skos:inScheme rdf:resource="https://doi.org/10.6069/uwlswd.b441-n943"/>
    <skos:prefLabel xml:lang="en">Quadruplex (1 in. or 2 in., reel)</skos:prefLabel>
    <skos:definition xml:lang="en">As opposed to the helical scan system, which uses one head, the
         Quadruplex videorecording system uses four videorecording heads. Often referred to as Quad,
         it was developed by Ampex in the mid-1950s. It provided higher quality resolution and color
         than did helical scanning.</skos:definition>
    <skos:scopeNote xml:lang="en">Quadruplex was the broadcast standard until recently, when less
         expensive helical scan systems have begun to overtake it.</skos:scopeNote>
    <skos:notation>f</skos:notation>
  </rdf:Description>
</rdf:RDF>