<?xml version="1.0" encoding="utf-8"?>
<rdf:RDF
   xmlns:dc="http://purl.org/dc/elements/1.1/"
   xmlns:dct="http://purl.org/dc/terms/"
   xmlns:rdf="http://www.w3.org/1999/02/22-rdf-syntax-ns#"
   xmlns:schema="https://schema.org/"
   xmlns:skos="http://www.w3.org/2004/02/skos/core#"
>
  <rdf:Description rdf:about="https://doi.org/10.6069/uwlswd.8svz-r036#n">
    <rdf:type rdf:resource="http://www.w3.org/2004/02/skos/core#Concept"/>
    <skos:inScheme rdf:resource="https://doi.org/10.6069/uwlswd.8svz-r036"/>
    <skos:prefLabel xml:lang="en">not applicable</skos:prefLabel>
    <skos:definition xml:lang="en">Reformatting quality is not applicable to the electronic
         resource.</skos:definition>
    <skos:notation xml:lang="en">n</skos:notation>
  </rdf:Description>
  <rdf:Description rdf:about="https://doi.org/10.6069/uwlswd.8svz-r036">
    <rdf:type rdf:resource="http://www.w3.org/2004/02/skos/core#ConceptScheme"/>
    <dct:type rdf:resource="http://purl.org/dc/dcmitype/Dataset"/>
    <dct:title xml:lang="en">Electronic resource: reformatting quality</dct:title>
    <dct:alternative xml:lang="en">MARC21 007/13 values for electronic resources expressed using
         RDF</dct:alternative>
    <dct:description xml:lang="en">An overall assessment of the physical quality of the electronic
         resource in relation to its intended use.</dct:description>
    <schema:disambiguatingDescription>SKOS Concept Scheme for MARC 00X
         Values</schema:disambiguatingDescription>
    <dct:publisher rdf:resource="http://viaf.org/viaf/139541794"/>
    <dct:source rdf:resource="https://www.loc.gov/marc/bibliographic/bd007.html"/>
    <dct:source rdf:resource="http://marc21rdf.info"/>
    <dct:provenance rdf:resource="https://doi.org/10.6069/uwlswd.2e2b-y833"/>
    <dct:creator rdf:resource="http://viaf.org/viaf/139541794"/>
    <dct:contributor rdf:resource="http://viaf.org/viaf/151962300"/>
    <dct:issued>2024</dct:issued>
    <dc:contributor xml:lang="en">Metadata Management Associates</dc:contributor>
    <dc:language>en</dc:language>
    <dct:license rdf:resource="http://creativecommons.org/publicdomain/zero/1.0"/>
    <schema:version>1-0-0</schema:version>
    <dct:format rdf:resource="http://www.w3.org/ns/formats/RDF_XML"/>
  </rdf:Description>
  <rdf:Description rdf:about="https://doi.org/10.6069/uwlswd.8svz-r036#p">
    <rdf:type rdf:resource="http://www.w3.org/2004/02/skos/core#Concept"/>
    <skos:inScheme rdf:resource="https://doi.org/10.6069/uwlswd.8svz-r036"/>
    <skos:prefLabel xml:lang="en">preservation</skos:prefLabel>
    <skos:definition xml:lang="en">Electronic resource was created via reformatting to help
         preserve the original item.</skos:definition>
    <skos:scopeNote xml:lang="en">Capture and storage techniques associated with preservation
         files ensure high-quality, long-term electronic resources that warrant long-term
         protection.</skos:scopeNote>
    <skos:notation xml:lang="en">p</skos:notation>
  </rdf:Description>
  <rdf:Description rdf:about="https://doi.org/10.6069/uwlswd.8svz-r036#a">
    <rdf:type rdf:resource="http://www.w3.org/2004/02/skos/core#Concept"/>
    <skos:inScheme rdf:resource="https://doi.org/10.6069/uwlswd.8svz-r036"/>
    <skos:prefLabel xml:lang="en">access</skos:prefLabel>
    <skos:definition xml:lang="en">Electronic resource is of a quality that will support current
         electronic access to the original item (reference use), but is not sufficient to serve as a
         preservation copy.</skos:definition>
    <skos:scopeNote xml:lang="en">Examples of electronic resources created for access purposes may
         include images created for a temporary, online exhibition (possibly to mirror an in-house
         installation); compressed, lower resolution versions of higher-quality master files that
         allow for easier transmission and access over the Internet; video converted to MPEG-2 for
         Internet access; photos which have been scanned at lower resolutions to create an online
         browsing tool for a collection; or articles scanned as a part of an E-Reserve collection
         which will be discarded in accordance with previous copyright agreements which specify a
         time limit on the retention of the electronic resource.</skos:scopeNote>
    <skos:notation xml:lang="en">a</skos:notation>
  </rdf:Description>
  <rdf:Description rdf:about="https://doi.org/10.6069/uwlswd.8svz-r036#r">
    <rdf:type rdf:resource="http://www.w3.org/2004/02/skos/core#Concept"/>
    <skos:inScheme rdf:resource="https://doi.org/10.6069/uwlswd.8svz-r036"/>
    <skos:prefLabel xml:lang="en">replacement</skos:prefLabel>
    <skos:definition xml:lang="en">Electronic resource is of very high quality and, when printed
         out, viewed on screen or played via a listening device, could serve as a replacement should
         the original be lost, damaged, or destroyed.</skos:definition>
    <skos:notation xml:lang="en">r</skos:notation>
  </rdf:Description>
  <rdf:Description rdf:about="https://doi.org/10.6069/uwlswd.8svz-r036#u">
    <rdf:type rdf:resource="http://www.w3.org/2004/02/skos/core#Concept"/>
    <skos:inScheme rdf:resource="https://doi.org/10.6069/uwlswd.8svz-r036"/>
    <skos:prefLabel xml:lang="en">unknown</skos:prefLabel>
    <skos:definition xml:lang="en">Reformatting quality of the electronic resource is not
         known.</skos:definition>
    <skos:notation xml:lang="en">u</skos:notation>
  </rdf:Description>
</rdf:RDF>
