@prefix dc: <http://purl.org/dc/elements/1.1/> .
@prefix dct: <http://purl.org/dc/terms/> .
@prefix schema: <https://schema.org/> .
@prefix skos: <http://www.w3.org/2004/02/skos/core#> .

<https://doi.org/10.6069/uwlswd.8svz-r036#a> a skos:Concept ;
    skos:definition """Electronic resource is of a quality that will support current
         electronic access to the original item (reference use), but is not sufficient to serve as a
         preservation copy."""@en ;
    skos:inScheme <https://doi.org/10.6069/uwlswd.8svz-r036> ;
    skos:notation "a" ;
    skos:prefLabel "access"@en ;
    skos:scopeNote """Examples of electronic resources created for access purposes may
         include images created for a temporary, online exhibition (possibly to mirror an in-house
         installation); compressed, lower resolution versions of higher-quality master files that
         allow for easier transmission and access over the Internet; video converted to MPEG-2 for
         Internet access; photos which have been scanned at lower resolutions to create an online
         browsing tool for a collection; or articles scanned as a part of an E-Reserve collection
         which will be discarded in accordance with previous copyright agreements which specify a
         time limit on the retention of the electronic resource."""@en .

<https://doi.org/10.6069/uwlswd.8svz-r036#n> a skos:Concept ;
    skos:definition """Reformatting quality is not applicable to the electronic
         resource."""@en ;
    skos:inScheme <https://doi.org/10.6069/uwlswd.8svz-r036> ;
    skos:notation "n" ;
    skos:prefLabel "not applicable"@en .

<https://doi.org/10.6069/uwlswd.8svz-r036#p> a skos:Concept ;
    skos:definition """Electronic resource was created via reformatting to help
         preserve the original item."""@en ;
    skos:inScheme <https://doi.org/10.6069/uwlswd.8svz-r036> ;
    skos:notation "p" ;
    skos:prefLabel "preservation"@en ;
    skos:scopeNote """Capture and storage techniques associated with preservation
         files ensure high-quality, long-term electronic resources that warrant long-term
         protection."""@en .

<https://doi.org/10.6069/uwlswd.8svz-r036#r> a skos:Concept ;
    skos:definition """Electronic resource is of very high quality and, when printed
         out, viewed on screen or played via a listening device, could serve as a replacement should
         the original be lost, damaged, or destroyed."""@en ;
    skos:inScheme <https://doi.org/10.6069/uwlswd.8svz-r036> ;
    skos:notation "r" ;
    skos:prefLabel "replacement"@en .

<https://doi.org/10.6069/uwlswd.8svz-r036#u> a skos:Concept ;
    skos:definition """Reformatting quality of the electronic resource is not
         known."""@en ;
    skos:inScheme <https://doi.org/10.6069/uwlswd.8svz-r036> ;
    skos:notation "u" ;
    skos:prefLabel "unknown"@en .

<https://doi.org/10.6069/uwlswd.8svz-r036> a skos:ConceptScheme ;
    dc:contributor "Metadata Management Associates"@en ;
    dc:language "en" ;
    dct:alternative """MARC21 007/13 values for electronic resources expressed using
         RDF"""@en ;
    dct:contributor <http://viaf.org/viaf/151962300> ;
    dct:creator <http://viaf.org/viaf/139541794> ;
    dct:description """An overall assessment of the physical quality of the electronic
         resource in relation to its intended use."""@en ;
    dct:format <http://www.w3.org/ns/formats/Turtle> ;
    dct:hasFormat <https://uwlib-cams.github.io/uwlswd_vocabs_marc_007/electronic_resource_reformatting_quality/electronic_resource_reformatting_quality.html>,
        <https://uwlib-cams.github.io/uwlswd_vocabs_marc_007/electronic_resource_reformatting_quality/electronic_resource_reformatting_quality.jsonld>,
        <https://uwlib-cams.github.io/uwlswd_vocabs_marc_007/electronic_resource_reformatting_quality/electronic_resource_reformatting_quality.nt>,
        <https://uwlib-cams.github.io/uwlswd_vocabs_marc_007/electronic_resource_reformatting_quality/electronic_resource_reformatting_quality.rdf> ;
    dct:issued "2024" ;
    dct:license <http://creativecommons.org/publicdomain/zero/1.0> ;
    dct:provenance <https://doi.org/10.6069/uwlswd.2e2b-y833#marc00Xvalues> ;
    dct:publisher <http://viaf.org/viaf/139541794> ;
    dct:source <http://marc21rdf.info>,
        <https://www.loc.gov/marc/bibliographic/bd007.html> ;
    dct:title "Electronic resource: reformatting quality"@en ;
    dct:type <http://purl.org/dc/dcmitype/Dataset> ;
    schema:disambiguatingDescription """SKOS Concept Scheme for MARC 00X
         Values"""@en ;
    schema:version "1-0-0" .

