@prefix dc: <http://purl.org/dc/elements/1.1/> .
@prefix dct: <http://purl.org/dc/terms/> .
@prefix schema: <https://schema.org/> .
@prefix skos: <http://www.w3.org/2004/02/skos/core#> .

<https://doi.org/10.6069/uwlswd.qpp2-sz54#a> a skos:Concept ;
    skos:definition "Sound."@en ;
    skos:inScheme <https://doi.org/10.6069/uwlswd.qpp2-sz54> ;
    skos:notation "a" ;
    skos:prefLabel "sound"@en ;
    skos:scopeNote """Includes digitally encoded sound or is intended to produce
         sound."""@en .

<https://doi.org/10.6069/uwlswd.qpp2-sz54#pound> a skos:Concept ;
    skos:definition "Not intended to produce sound."@en ;
    skos:inScheme <https://doi.org/10.6069/uwlswd.qpp2-sz54> ;
    skos:notation "#" ;
    skos:prefLabel "no sound (silent)"@en .

<https://doi.org/10.6069/uwlswd.qpp2-sz54#u> a skos:Concept ;
    skos:definition """Presence or absence of sound or the ability of an electronic
         resource to produce sound is not known."""@en ;
    skos:inScheme <https://doi.org/10.6069/uwlswd.qpp2-sz54> ;
    skos:notation "u" ;
    skos:prefLabel "unknown"@en .

<https://doi.org/10.6069/uwlswd.qpp2-sz54> a skos:ConceptScheme ;
    dc:contributor "Metadata Management Associates"@en ;
    dc:language "en" ;
    dct:alternative """MARC21 007/05 values for electronic resources expressed using
         RDF"""@en ;
    dct:contributor <http://viaf.org/viaf/151962300> ;
    dct:creator <http://viaf.org/viaf/139541794> ;
    dct:description """Whether the production of sound is an integral part of an
         electronic resource."""@en ;
    dct:format <http://www.w3.org/ns/formats/Turtle> ;
    dct:hasFormat <https://uwlib-cams.github.io/uwlswd_vocabs_marc_007/electronic_resource_sound/electronic_resource_sound.html>,
        <https://uwlib-cams.github.io/uwlswd_vocabs_marc_007/electronic_resource_sound/electronic_resource_sound.jsonld>,
        <https://uwlib-cams.github.io/uwlswd_vocabs_marc_007/electronic_resource_sound/electronic_resource_sound.nt>,
        <https://uwlib-cams.github.io/uwlswd_vocabs_marc_007/electronic_resource_sound/electronic_resource_sound.rdf> ;
    dct:issued "2024" ;
    dct:license <http://creativecommons.org/publicdomain/zero/1.0> ;
    dct:provenance <https://doi.org/10.6069/uwlswd.2e2b-y833#marc00Xvalues> ;
    dct:publisher <http://viaf.org/viaf/139541794> ;
    dct:source <http://marc21rdf.info>,
        <https://www.loc.gov/marc/bibliographic/bd007.html> ;
    dct:title "Electronic resource: sound"@en ;
    dct:type <http://purl.org/dc/dcmitype/Dataset> ;
    schema:disambiguatingDescription """SKOS Concept Scheme for MARC 00X
         Values"""@en ;
    schema:version "1-0-0" .

