@prefix dc: <http://purl.org/dc/elements/1.1/> .
@prefix dct: <http://purl.org/dc/terms/> .
@prefix schema: <https://schema.org/> .
@prefix skos: <http://www.w3.org/2004/02/skos/core#> .

<https://doi.org/10.6069/uwlswd.99xj-7684#m> a skos:Concept ;
    skos:definition "Microgroove disc or a fine cylinder."@en ;
    skos:inScheme <https://doi.org/10.6069/uwlswd.99xj-7684> ;
    skos:notation "m" ;
    skos:prefLabel "microgroove/fine"@en ;
    skos:scopeNote """Discs issued at 16, 33 1/3, and 45 rpm are usually issued as
         microgroove. Cylinders issued at 160 rpm (which have 200 grooves per inch) are usually
         issued as fine."""@en .

<https://doi.org/10.6069/uwlswd.99xj-7684#n> a skos:Concept ;
    skos:definition "Item does not contain grooves."@en ;
    skos:inScheme <https://doi.org/10.6069/uwlswd.99xj-7684> ;
    skos:notation "n" ;
    skos:prefLabel "not applicable"@en ;
    skos:scopeNote "Used for tapes and compact audio discs."@en .

<https://doi.org/10.6069/uwlswd.99xj-7684#s> a skos:Concept ;
    skos:definition "Coarse or standard groove."@en ;
    skos:inScheme <https://doi.org/10.6069/uwlswd.99xj-7684> ;
    skos:notation "s" ;
    skos:prefLabel "coarse/standard"@en ;
    skos:scopeNote """Discs issued at 78 rpm are usually coarse. Cylinders issued at
         120 rpm (which have 100 grooves per inch) are usually standard."""@en .

<https://doi.org/10.6069/uwlswd.99xj-7684#u> a skos:Concept ;
    skos:definition "Groove width/groove pitch is not known."@en ;
    skos:inScheme <https://doi.org/10.6069/uwlswd.99xj-7684> ;
    skos:notation "u" ;
    skos:prefLabel "unknown"@en .

<https://doi.org/10.6069/uwlswd.99xj-7684#z> a skos:Concept ;
    skos:definition """Groove width/groove pitch other than microgroove/fine or
         coarse/standard."""@en ;
    skos:inScheme <https://doi.org/10.6069/uwlswd.99xj-7684> ;
    skos:notation "z" ;
    skos:prefLabel "other"@en .

<https://doi.org/10.6069/uwlswd.99xj-7684> a skos:ConceptScheme ;
    dc:contributor "Metadata Management Associates"@en ;
    dc:language "en" ;
    dct:alternative """MARC21 007/05 values for sound recordings expressed using
         RDF"""@en ;
    dct:contributor <http://viaf.org/viaf/151962300> ;
    dct:creator <http://viaf.org/viaf/139541794> ;
    dct:description """Width of the groove of the recording for discs or the pitch of
         the groove for cylinders."""@en ;
    dct:format <http://www.w3.org/ns/formats/Turtle> ;
    dct:hasFormat <https://uwlib-cams.github.io/uwlswd_vocabs_marc_007/sound_recording_groove_width_or_groove_pitch/sound_recording_groove_width_or_groove_pitch.html>,
        <https://uwlib-cams.github.io/uwlswd_vocabs_marc_007/sound_recording_groove_width_or_groove_pitch/sound_recording_groove_width_or_groove_pitch.jsonld>,
        <https://uwlib-cams.github.io/uwlswd_vocabs_marc_007/sound_recording_groove_width_or_groove_pitch/sound_recording_groove_width_or_groove_pitch.nt>,
        <https://uwlib-cams.github.io/uwlswd_vocabs_marc_007/sound_recording_groove_width_or_groove_pitch/sound_recording_groove_width_or_groove_pitch.rdf> ;
    dct:issued "2024" ;
    dct:license <http://creativecommons.org/publicdomain/zero/1.0> ;
    dct:provenance <https://doi.org/10.6069/uwlswd.2e2b-y833#marc00Xvalues> ;
    dct:publisher <http://viaf.org/viaf/139541794> ;
    dct:source <http://marc21rdf.info>,
        <https://www.loc.gov/marc/bibliographic/bd007.html> ;
    dct:title "Sound recording: groove width/groove pitch"@en ;
    dct:type <http://purl.org/dc/dcmitype/Dataset> ;
    schema:disambiguatingDescription """SKOS Concept Scheme for MARC 00X
         Values"""@en ;
    schema:version "1-0-0" .

