@prefix dc: <http://purl.org/dc/elements/1.1/> .
@prefix dct: <http://purl.org/dc/terms/> .
@prefix schema: <https://schema.org/> .
@prefix skos: <http://www.w3.org/2004/02/skos/core#> .

<https://doi.org/10.6069/uwlswd.v2wq-nz72#a> a skos:Concept ;
    skos:definition """Lines and characters appear dark against a light
         background."""@en ;
    skos:inScheme <https://doi.org/10.6069/uwlswd.v2wq-nz72> ;
    skos:notation "a" ;
    skos:prefLabel "positive"@en ;
    skos:scopeNote "Used for microopaques."@en .

<https://doi.org/10.6069/uwlswd.v2wq-nz72#b> a skos:Concept ;
    skos:definition """Lines and characters appear light against a dark
         background."""@en ;
    skos:inScheme <https://doi.org/10.6069/uwlswd.v2wq-nz72> ;
    skos:notation "b" ;
    skos:prefLabel "negative"@en .

<https://doi.org/10.6069/uwlswd.v2wq-nz72#m> a skos:Concept ;
    skos:definition "Mixture of positive and negative images."@en ;
    skos:inScheme <https://doi.org/10.6069/uwlswd.v2wq-nz72> ;
    skos:notation "m" ;
    skos:prefLabel "mixed polarity"@en .

<https://doi.org/10.6069/uwlswd.v2wq-nz72#u> a skos:Concept ;
    skos:definition "Polarity of the microform is not known."@en ;
    skos:inScheme <https://doi.org/10.6069/uwlswd.v2wq-nz72> ;
    skos:notation "u" ;
    skos:prefLabel "unknown"@en .

<https://doi.org/10.6069/uwlswd.v2wq-nz72> a skos:ConceptScheme ;
    dc:contributor "Metadata Management Associates"@en ;
    dc:language "en" ;
    dct:alternative """MARC21 007/03 values for microform expressed using
         RDF"""@en ;
    dct:contributor <http://viaf.org/viaf/151962300> ;
    dct:creator <http://viaf.org/viaf/139541794> ;
    dct:description """Positive/negative polarity of the microform. This
         characteristic is also referred to as the polarity."""@en ;
    dct:format <http://www.w3.org/ns/formats/Turtle> ;
    dct:hasFormat <https://uwlib-cams.github.io/uwlswd_vocabs_marc_007/microform_positive_or_negative_aspect/microform_positive_or_negative_aspect.html>,
        <https://uwlib-cams.github.io/uwlswd_vocabs_marc_007/microform_positive_or_negative_aspect/microform_positive_or_negative_aspect.jsonld>,
        <https://uwlib-cams.github.io/uwlswd_vocabs_marc_007/microform_positive_or_negative_aspect/microform_positive_or_negative_aspect.nt>,
        <https://uwlib-cams.github.io/uwlswd_vocabs_marc_007/microform_positive_or_negative_aspect/microform_positive_or_negative_aspect.rdf> ;
    dct:issued "2024" ;
    dct:license <http://creativecommons.org/publicdomain/zero/1.0> ;
    dct:provenance <https://doi.org/10.6069/uwlswd.2e2b-y833#marc00Xvalues> ;
    dct:publisher <http://viaf.org/viaf/139541794> ;
    dct:source <http://marc21rdf.info>,
        <https://www.loc.gov/marc/bibliographic/bd007.html> ;
    dct:title "Microform: positive/negative aspect"@en ;
    dct:type <http://purl.org/dc/dcmitype/Dataset> ;
    schema:disambiguatingDescription """SKOS Concept Scheme for MARC 00X
         Values"""@en ;
    schema:version "1-0-0" .

