<?xml version="1.0" encoding="UTF-8"?>
<rdf:RDF xmlns:dc="http://purl.org/dc/elements/1.1/" xmlns:dct="http://purl.org/dc/terms/"
   xmlns:rdf="http://www.w3.org/1999/02/22-rdf-syntax-ns#"
   xmlns:rdfs="http://www.w3.org/2000/01/rdf-schema#" xmlns:schema="https://schema.org/"
   xmlns:skos="http://www.w3.org/2004/02/skos/core#"
   xmlns:uw="https://www.lib.washington.edu/static/public/cams/data/localResources/properties_local.html"
   xmlns:uwp="https://doi.org/10.6069/uwlib.55.d.3#">


   <rdf:Description rdf:about="http://fakeIRI.edu/terms/globemed">
      <rdf:type rdf:resource="http://www.w3.org/2004/02/skos/core#ConceptScheme"/>
      <dct:type rdf:resource="http://purl.org/dc/dcmitype/Dataset"/>
      <dct:title xml:lang="en">Globe: physical medium</dct:title>
      <dct:alternative xml:lang="en">MARC21 007/04 values for globes expressed using
         RDF</dct:alternative>
      <dct:description xml:lang="en">Material out of which the globe is made.</dct:description>
      <schema:disambiguatingDescription>SKOS Concept Scheme for MARC 00X
         Values</schema:disambiguatingDescription>
      <dct:publisher rdf:resource="http://viaf.org/viaf/139541794"/>
      <dct:source rdf:resource="https://www.loc.gov/marc/bibliographic/bd007.html"/>
      <dct:source rdf:resource="http://marc21rdf.info"/>
      <dct:provenance rdf:resource="https://doi.org/10.6069/uwlswd.2e2b-y833"/>
      <dct:creator rdf:resource="http://viaf.org/viaf/139541794"/>
      <dct:contributor rdf:resource="http://viaf.org/viaf/151962300"/>
      <dct:issued>2024</dct:issued>
      <dc:contributor xml:lang="en">Metadata Management Associates</dc:contributor>
      <dc:language>en</dc:language>
      <dct:license rdf:resource="http://creativecommons.org/publicdomain/zero/1.0"/>
      <schema:version>1-0-0</schema:version>
      <dct:issued>2024</dct:issued>
      <dct:format rdf:resource="http://www.w3.org/ns/formats/RDF_XML"/>
   </rdf:Description>

   <rdf:Description rdf:about="http://fakeIRI.edu/terms/globemed#v">
      <rdf:type rdf:resource="http://www.w3.org/2004/02/skos/core#Concept"/>
      <skos:inScheme rdf:resource="http://fakeIRI.edu/terms/globemed"/>
      <skos:prefLabel xml:lang="en">leather</skos:prefLabel>
      <skos:definition xml:lang="en">Animal skin dressed for use.</skos:definition>
      <skos:notation xml:lang="en">v</skos:notation>
   </rdf:Description>

   <rdf:Description rdf:about="http://fakeIRI.edu/terms/globemed#d">
      <rdf:type rdf:resource="http://www.w3.org/2004/02/skos/core#Concept"/>
      <skos:inScheme rdf:resource="http://fakeIRI.edu/terms/globemed"/>
      <skos:prefLabel xml:lang="en">metal</skos:prefLabel>
      <skos:definition xml:lang="en">Metal.</skos:definition>
      <skos:notation xml:lang="en">d</skos:notation>
   </rdf:Description>

   <rdf:Description rdf:about="http://fakeIRI.edu/terms/globemed#z">
      <rdf:type rdf:resource="http://www.w3.org/2004/02/skos/core#Concept"/>
      <skos:inScheme rdf:resource="http://fakeIRI.edu/terms/globemed"/>
      <skos:prefLabel xml:lang="en">other</skos:prefLabel>
      <skos:definition xml:lang="en">Physical medium other than paper, wood, stone, metal,
         synthetic, skin, textile, vinyl, vellum, plaster, leather, or parchment.</skos:definition>
      <skos:notation xml:lang="en">z</skos:notation>
   </rdf:Description>

   <rdf:Description rdf:about="http://fakeIRI.edu/terms/globemed#a">
      <rdf:type rdf:resource="http://www.w3.org/2004/02/skos/core#Concept"/>
      <skos:inScheme rdf:resource="http://fakeIRI.edu/terms/globemed"/>
      <skos:prefLabel xml:lang="en">paper</skos:prefLabel>
      <skos:definition xml:lang="en">Any kind of cellulose-based paper.</skos:definition>
      <skos:notation xml:lang="en">a</skos:notation>
   </rdf:Description>

   <rdf:Description rdf:about="http://fakeIRI.edu/terms/globemed#w">
      <rdf:type rdf:resource="http://www.w3.org/2004/02/skos/core#Concept"/>
      <skos:inScheme rdf:resource="http://fakeIRI.edu/terms/globemed"/>
      <skos:prefLabel xml:lang="en">parchment</skos:prefLabel>
      <skos:definition xml:lang="en">Skin of a sheep or goat prepared for writing
         on.</skos:definition>
      <skos:notation xml:lang="en">w</skos:notation>
   </rdf:Description>

   <rdf:Description rdf:about="http://fakeIRI.edu/terms/globemed#p">
      <rdf:type rdf:resource="http://www.w3.org/2004/02/skos/core#Concept"/>
      <skos:inScheme rdf:resource="http://fakeIRI.edu/terms/globemed"/>
      <skos:prefLabel xml:lang="en">plaster</skos:prefLabel>
      <skos:definition xml:lang="en">Plaster.</skos:definition>
      <skos:scopeNote xml:lang="en">Used also for mixtures of ground solids and
         plaster.</skos:scopeNote>
      <skos:notation xml:lang="en">p</skos:notation>
   </rdf:Description>

   <rdf:Description rdf:about="http://fakeIRI.edu/terms/globemed#f">
      <rdf:type rdf:resource="http://www.w3.org/2004/02/skos/core#Concept"/>
      <skos:inScheme rdf:resource="http://fakeIRI.edu/terms/globemed"/>
      <skos:prefLabel xml:lang="en">skin</skos:prefLabel>
      <skos:definition xml:lang="en">Skin.</skos:definition>
      <skos:scopeNote xml:lang="en">Excludes leather, parchment, and vellum.</skos:scopeNote>
      <skos:scopeNote xml:lang="en">Synthetic materials that are made to resemble animal skin are
         coded as synthetic.</skos:scopeNote>
      <skos:notation xml:lang="en">f</skos:notation>
   </rdf:Description>

   <rdf:Description rdf:about="http://fakeIRI.edu/terms/globemed#c">
      <rdf:type rdf:resource="http://www.w3.org/2004/02/skos/core#Concept"/>
      <skos:inScheme rdf:resource="http://fakeIRI.edu/terms/globemed"/>
      <skos:prefLabel xml:lang="en">stone</skos:prefLabel>
      <skos:definition xml:lang="en">Stone.</skos:definition>
      <skos:notation xml:lang="en">c</skos:notation>
   </rdf:Description>

   <rdf:Description rdf:about="http://fakeIRI.edu/terms/globemed#e">
      <rdf:type rdf:resource="http://www.w3.org/2004/02/skos/core#Concept"/>
      <skos:inScheme rdf:resource="http://fakeIRI.edu/terms/globemed"/>
      <skos:prefLabel xml:lang="en">synthetic</skos:prefLabel>
      <skos:definition xml:lang="en">Man-made substances other than textiles, plastic, and
         vinyl.</skos:definition>
      <skos:notation xml:lang="en">e</skos:notation>
   </rdf:Description>

   <rdf:Description rdf:about="http://fakeIRI.edu/terms/globemed#g">
      <rdf:type rdf:resource="http://www.w3.org/2004/02/skos/core#Concept"/>
      <skos:inScheme rdf:resource="http://fakeIRI.edu/terms/globemed"/>
      <skos:prefLabel xml:lang="en">textile</skos:prefLabel>
      <skos:definition xml:lang="en">Textile.</skos:definition>
      <skos:scopeNote xml:lang="en">Used for all fabrics, whether made from natural or synthetic
         fibers.</skos:scopeNote>
      <skos:notation xml:lang="en">g</skos:notation>
   </rdf:Description>

   <rdf:Description rdf:about="http://fakeIRI.edu/terms/globemed#u">
      <rdf:type rdf:resource="http://www.w3.org/2004/02/skos/core#Concept"/>
      <skos:inScheme rdf:resource="http://fakeIRI.edu/terms/globemed"/>
      <skos:prefLabel xml:lang="en">unknown</skos:prefLabel>
      <skos:definition xml:lang="en">Physical medium of which the globe is made is not
         known.</skos:definition>
      <skos:notation xml:lang="en">u</skos:notation>
   </rdf:Description>

   <rdf:Description rdf:about="http://fakeIRI.edu/terms/globemed#n">
      <rdf:type rdf:resource="http://www.w3.org/2004/02/skos/core#Concept"/>
      <skos:inScheme rdf:resource="http://fakeIRI.edu/terms/globemed"/>
      <skos:prefLabel xml:lang="en">vellum</skos:prefLabel>
      <skos:definition xml:lang="en">Fine-grained unsplit lambskin, kidskin, or calfskin prepared
         especially for writing or drawing on.</skos:definition>
      <skos:notation xml:lang="en">n</skos:notation>
   </rdf:Description>

   <rdf:Description rdf:about="http://fakeIRI.edu/terms/globemed#l">
      <rdf:type rdf:resource="http://www.w3.org/2004/02/skos/core#Concept"/>
      <skos:inScheme rdf:resource="http://fakeIRI.edu/terms/globemed"/>
      <skos:prefLabel xml:lang="en">vinyl</skos:prefLabel>
      <skos:definition xml:lang="en">Vinyl.</skos:definition>
      <skos:notation xml:lang="en">l</skos:notation>
   </rdf:Description>

   <rdf:Description rdf:about="http://fakeIRI.edu/terms/globemed#b">
      <rdf:type rdf:resource="http://www.w3.org/2004/02/skos/core#Concept"/>
      <skos:inScheme rdf:resource="http://fakeIRI.edu/terms/globemed"/>
      <skos:prefLabel xml:lang="en">wood</skos:prefLabel>
      <skos:definition xml:lang="en">Wood.</skos:definition>
      <skos:scopeNote xml:lang="en">A material that is based on wood particles or fibers may or may
         not be considered wood. Consider particle board to be wood.</skos:scopeNote>
      <skos:notation xml:lang="en">b</skos:notation>
   </rdf:Description>
</rdf:RDF>
