<?xml version="1.0" encoding="utf-8"?>
<rdf:RDF
   xmlns:dc="http://purl.org/dc/elements/1.1/"
   xmlns:dct="http://purl.org/dc/terms/"
   xmlns:rdf="http://www.w3.org/1999/02/22-rdf-syntax-ns#"
   xmlns:schema="https://schema.org/"
   xmlns:skos="http://www.w3.org/2004/02/skos/core#"
>
  <rdf:Description rdf:about="https://doi.org/10.6069/uwlswd.db6k-dw63#g">
    <rdf:type rdf:resource="http://www.w3.org/2004/02/skos/core#Concept"/>
    <skos:inScheme rdf:resource="https://doi.org/10.6069/uwlswd.db6k-dw63"/>
    <skos:prefLabel xml:lang="en">textile</skos:prefLabel>
    <skos:definition xml:lang="en">Textile.</skos:definition>
    <skos:scopeNote xml:lang="en">Used for all fabrics, whether made from natural or synthetic
         fibers.</skos:scopeNote>
    <skos:notation>g</skos:notation>
  </rdf:Description>
  <rdf:Description rdf:about="https://doi.org/10.6069/uwlswd.db6k-dw63#u">
    <rdf:type rdf:resource="http://www.w3.org/2004/02/skos/core#Concept"/>
    <skos:inScheme rdf:resource="https://doi.org/10.6069/uwlswd.db6k-dw63"/>
    <skos:prefLabel xml:lang="en">unknown</skos:prefLabel>
    <skos:definition xml:lang="en">Physical medium of which the globe is made is not
         known.</skos:definition>
    <skos:notation>u</skos:notation>
  </rdf:Description>
  <rdf:Description rdf:about="https://doi.org/10.6069/uwlswd.db6k-dw63#v">
    <rdf:type rdf:resource="http://www.w3.org/2004/02/skos/core#Concept"/>
    <skos:inScheme rdf:resource="https://doi.org/10.6069/uwlswd.db6k-dw63"/>
    <skos:prefLabel xml:lang="en">leather</skos:prefLabel>
    <skos:definition xml:lang="en">Animal skin dressed for use.</skos:definition>
    <skos:notation>v</skos:notation>
  </rdf:Description>
  <rdf:Description rdf:about="https://doi.org/10.6069/uwlswd.db6k-dw63">
    <rdf:type rdf:resource="http://www.w3.org/2004/02/skos/core#ConceptScheme"/>
    <dct:type rdf:resource="http://purl.org/dc/dcmitype/Dataset"/>
    <dct:title xml:lang="en">Globe: physical medium</dct:title>
    <dct:alternative xml:lang="en">MARC21 007/04 values for globes expressed using
         RDF</dct:alternative>
    <dct:description xml:lang="en">Material out of which the globe is made.</dct:description>
    <schema:disambiguatingDescription xml:lang="en">SKOS Concept Scheme for MARC 00X
         Values</schema:disambiguatingDescription>
    <dct:publisher rdf:resource="http://viaf.org/viaf/139541794"/>
    <dct:source rdf:resource="https://www.loc.gov/marc/bibliographic/bd007.html"/>
    <dct:source rdf:resource="http://marc21rdf.info"/>
    <dct:provenance rdf:resource="https://doi.org/10.6069/uwlswd.2e2b-y833#marc00Xvalues"/>
    <dct:creator rdf:resource="http://viaf.org/viaf/139541794"/>
    <dct:contributor rdf:resource="http://viaf.org/viaf/151962300"/>
    <dct:issued>2024</dct:issued>
    <dc:contributor xml:lang="en">Metadata Management Associates</dc:contributor>
    <dc:language>en</dc:language>
    <dct:license rdf:resource="http://creativecommons.org/publicdomain/zero/1.0"/>
    <schema:version>1-0-0</schema:version>
    <dct:format rdf:resource="http://www.w3.org/ns/formats/RDF_XML"/>
    <dct:hasFormat rdf:resource="https://uwlib-cams.github.io/uwlswd_vocabs_marc_007/globe_physical_medium/globe_physical_medium.ttl"/>
    <dct:hasFormat rdf:resource="https://uwlib-cams.github.io/uwlswd_vocabs_marc_007/globe_physical_medium/globe_physical_medium.nt"/>
    <dct:hasFormat rdf:resource="https://uwlib-cams.github.io/uwlswd_vocabs_marc_007/globe_physical_medium/globe_physical_medium.jsonld"/>
    <dct:hasFormat rdf:resource="https://uwlib-cams.github.io/uwlswd_vocabs_marc_007/globe_physical_medium/globe_physical_medium.html"/>
  </rdf:Description>
  <rdf:Description rdf:about="https://doi.org/10.6069/uwlswd.db6k-dw63#z">
    <rdf:type rdf:resource="http://www.w3.org/2004/02/skos/core#Concept"/>
    <skos:inScheme rdf:resource="https://doi.org/10.6069/uwlswd.db6k-dw63"/>
    <skos:prefLabel xml:lang="en">other</skos:prefLabel>
    <skos:definition xml:lang="en">Physical medium other than paper, wood, stone, metal,
         synthetic, skin, textile, vinyl, vellum, plaster, leather, or parchment.</skos:definition>
    <skos:notation>z</skos:notation>
  </rdf:Description>
  <rdf:Description rdf:about="https://doi.org/10.6069/uwlswd.db6k-dw63#f">
    <rdf:type rdf:resource="http://www.w3.org/2004/02/skos/core#Concept"/>
    <skos:inScheme rdf:resource="https://doi.org/10.6069/uwlswd.db6k-dw63"/>
    <skos:prefLabel xml:lang="en">skin</skos:prefLabel>
    <skos:definition xml:lang="en">Skin.</skos:definition>
    <skos:scopeNote xml:lang="en">Excludes leather, parchment, and vellum.</skos:scopeNote>
    <skos:scopeNote xml:lang="en">Synthetic materials that are made to resemble animal skin are
         coded as synthetic.</skos:scopeNote>
    <skos:notation>f</skos:notation>
  </rdf:Description>
  <rdf:Description rdf:about="https://doi.org/10.6069/uwlswd.db6k-dw63#n">
    <rdf:type rdf:resource="http://www.w3.org/2004/02/skos/core#Concept"/>
    <skos:inScheme rdf:resource="https://doi.org/10.6069/uwlswd.db6k-dw63"/>
    <skos:prefLabel xml:lang="en">vellum</skos:prefLabel>
    <skos:definition xml:lang="en">Fine-grained unsplit lambskin, kidskin, or calfskin prepared
         especially for writing or drawing on.</skos:definition>
    <skos:notation>n</skos:notation>
  </rdf:Description>
  <rdf:Description rdf:about="https://doi.org/10.6069/uwlswd.db6k-dw63#p">
    <rdf:type rdf:resource="http://www.w3.org/2004/02/skos/core#Concept"/>
    <skos:inScheme rdf:resource="https://doi.org/10.6069/uwlswd.db6k-dw63"/>
    <skos:prefLabel xml:lang="en">plaster</skos:prefLabel>
    <skos:definition xml:lang="en">Plaster.</skos:definition>
    <skos:scopeNote xml:lang="en">Used also for mixtures of ground solids and
         plaster.</skos:scopeNote>
    <skos:notation>p</skos:notation>
  </rdf:Description>
  <rdf:Description rdf:about="https://doi.org/10.6069/uwlswd.db6k-dw63#d">
    <rdf:type rdf:resource="http://www.w3.org/2004/02/skos/core#Concept"/>
    <skos:inScheme rdf:resource="https://doi.org/10.6069/uwlswd.db6k-dw63"/>
    <skos:prefLabel xml:lang="en">metal</skos:prefLabel>
    <skos:definition xml:lang="en">Metal.</skos:definition>
    <skos:notation>d</skos:notation>
  </rdf:Description>
  <rdf:Description rdf:about="https://doi.org/10.6069/uwlswd.db6k-dw63#w">
    <rdf:type rdf:resource="http://www.w3.org/2004/02/skos/core#Concept"/>
    <skos:inScheme rdf:resource="https://doi.org/10.6069/uwlswd.db6k-dw63"/>
    <skos:prefLabel xml:lang="en">parchment</skos:prefLabel>
    <skos:definition xml:lang="en">Skin of a sheep or goat prepared for writing
         on.</skos:definition>
    <skos:notation>w</skos:notation>
  </rdf:Description>
  <rdf:Description rdf:about="https://doi.org/10.6069/uwlswd.db6k-dw63#l">
    <rdf:type rdf:resource="http://www.w3.org/2004/02/skos/core#Concept"/>
    <skos:inScheme rdf:resource="https://doi.org/10.6069/uwlswd.db6k-dw63"/>
    <skos:prefLabel xml:lang="en">vinyl</skos:prefLabel>
    <skos:definition xml:lang="en">Vinyl.</skos:definition>
    <skos:notation>l</skos:notation>
  </rdf:Description>
  <rdf:Description rdf:about="https://doi.org/10.6069/uwlswd.db6k-dw63#c">
    <rdf:type rdf:resource="http://www.w3.org/2004/02/skos/core#Concept"/>
    <skos:inScheme rdf:resource="https://doi.org/10.6069/uwlswd.db6k-dw63"/>
    <skos:prefLabel xml:lang="en">stone</skos:prefLabel>
    <skos:definition xml:lang="en">Stone.</skos:definition>
    <skos:notation>c</skos:notation>
  </rdf:Description>
  <rdf:Description rdf:about="https://doi.org/10.6069/uwlswd.db6k-dw63#e">
    <rdf:type rdf:resource="http://www.w3.org/2004/02/skos/core#Concept"/>
    <skos:inScheme rdf:resource="https://doi.org/10.6069/uwlswd.db6k-dw63"/>
    <skos:prefLabel xml:lang="en">synthetic</skos:prefLabel>
    <skos:definition xml:lang="en">Man-made substances other than textiles, plastic, and
         vinyl.</skos:definition>
    <skos:notation>e</skos:notation>
  </rdf:Description>
  <rdf:Description rdf:about="https://doi.org/10.6069/uwlswd.db6k-dw63#a">
    <rdf:type rdf:resource="http://www.w3.org/2004/02/skos/core#Concept"/>
    <skos:inScheme rdf:resource="https://doi.org/10.6069/uwlswd.db6k-dw63"/>
    <skos:prefLabel xml:lang="en">paper</skos:prefLabel>
    <skos:definition xml:lang="en">Any kind of cellulose-based paper.</skos:definition>
    <skos:notation>a</skos:notation>
  </rdf:Description>
  <rdf:Description rdf:about="https://doi.org/10.6069/uwlswd.db6k-dw63#b">
    <rdf:type rdf:resource="http://www.w3.org/2004/02/skos/core#Concept"/>
    <skos:inScheme rdf:resource="https://doi.org/10.6069/uwlswd.db6k-dw63"/>
    <skos:prefLabel xml:lang="en">wood</skos:prefLabel>
    <skos:definition xml:lang="en">Wood.</skos:definition>
    <skos:scopeNote xml:lang="en">A material that is based on wood particles or fibers may or may
         not be considered wood. Consider particle board to be wood.</skos:scopeNote>
    <skos:notation>b</skos:notation>
  </rdf:Description>
</rdf:RDF>
