<?xml version="1.0" encoding="UTF-8"?>
<rdf:RDF xmlns:dc="http://purl.org/dc/elements/1.1/" xmlns:dct="http://purl.org/dc/terms/"
   xmlns:rdf="http://www.w3.org/1999/02/22-rdf-syntax-ns#"
   xmlns:rdfs="http://www.w3.org/2000/01/rdf-schema#" xmlns:schema="https://schema.org/"
   xmlns:skos="http://www.w3.org/2004/02/skos/core#"
   xmlns:uw="https://www.lib.washington.edu/static/public/cams/data/localResources/properties_local.html"
   xmlns:uwp="https://doi.org/10.6069/uwlib.55.d.3#">


   <rdf:Description rdf:about="http://fakeIRI.edu/terms/mappor">
      <rdf:type rdf:resource="http://www.w3.org/2004/02/skos/core#ConceptScheme"/>
      <dct:type rdf:resource="http://purl.org/dc/dcmitype/Dataset"/>
      <dct:title xml:lang="en">Map: production/reproduction details</dct:title>
      <dct:alternative xml:lang="en">MARC21 007/06 values for maps expressed using
         RDF</dct:alternative>
      <dct:description xml:lang="en">Technique used to produce the cartographic
         resource.</dct:description>
      <schema:disambiguatingDescription>SKOS Concept Scheme for MARC 00X
         Values</schema:disambiguatingDescription>
      <dct:publisher rdf:resource="http://viaf.org/viaf/139541794"/>
      <dct:source rdf:resource="https://www.loc.gov/marc/bibliographic/bd007.html"/>
      <dct:source rdf:resource="http://marc21rdf.info"/>
      <dct:provenance rdf:resource="https://doi.org/10.6069/uwlswd.2e2b-y833"/>
      <dct:creator rdf:resource="http://viaf.org/viaf/139541794"/>
      <dct:contributor rdf:resource="http://viaf.org/viaf/151962300"/>
      <dct:issued>2024</dct:issued>
      <dc:contributor xml:lang="en">Metadata Management Associates</dc:contributor>
      <dc:language>en</dc:language>
      <dct:license rdf:resource="http://creativecommons.org/publicdomain/zero/1.0"/>
      <schema:version>1-0-0</schema:version>
      <dct:issued>2024</dct:issued>
      <dct:format rdf:resource="http://www.w3.org/ns/formats/RDF_XML"/>
   </rdf:Description>

   <rdf:Description rdf:about="http://fakeIRI.edu/terms/mappor#d">
      <rdf:type rdf:resource="http://www.w3.org/2004/02/skos/core#Concept"/>
      <skos:inScheme rdf:resource="http://fakeIRI.edu/terms/mappor"/>
      <skos:prefLabel xml:lang="en">film</skos:prefLabel>
      <skos:definition xml:lang="en">Film copy of the original.</skos:definition>
      <skos:notation xml:lang="en">d</skos:notation>
   </rdf:Description>

   <rdf:Description rdf:about="http://fakeIRI.edu/terms/mappor#z">
      <rdf:type rdf:resource="http://www.w3.org/2004/02/skos/core#Concept"/>
      <skos:inScheme rdf:resource="http://fakeIRI.edu/terms/mappor"/>
      <skos:prefLabel xml:lang="en">other</skos:prefLabel>
      <skos:definition xml:lang="en">Production or reproduction details other than photocopy,
         blueline print, photocopy, photographic pre-production, or film.</skos:definition>
      <skos:notation xml:lang="en">z</skos:notation>
   </rdf:Description>

   <rdf:Description rdf:about="http://fakeIRI.edu/terms/mappor#b">
      <rdf:type rdf:resource="http://www.w3.org/2004/02/skos/core#Concept"/>
      <skos:inScheme rdf:resource="http://fakeIRI.edu/terms/mappor"/>
      <skos:prefLabel xml:lang="en">photocopy</skos:prefLabel>
      <skos:definition xml:lang="en">Photocopy.</skos:definition>
      <skos:notation xml:lang="en">b</skos:notation>
   </rdf:Description>

   <rdf:Description rdf:about="http://fakeIRI.edu/terms/mappor#a ">
      <rdf:type rdf:resource="http://www.w3.org/2004/02/skos/core#Concept"/>
      <skos:inScheme rdf:resource="http://fakeIRI.edu/terms/mappor"/>
      <skos:prefLabel xml:lang="en">photocopy, blueline print</skos:prefLabel>
      <skos:definition xml:lang="en">A blueline image on a white background and reproduced by the
         whiteprint process.</skos:definition>
      <skos:scopeNote xml:lang="en">Bluelines are made from vellum, film positives, or any
         translucent or transparent original on which an image has been made.</skos:scopeNote>
      <skos:notation xml:lang="en">a</skos:notation>
   </rdf:Description>

   <rdf:Description rdf:about="http://fakeIRI.edu/terms/mappor#c">
      <rdf:type rdf:resource="http://www.w3.org/2004/02/skos/core#Concept"/>
      <skos:inScheme rdf:resource="http://fakeIRI.edu/terms/mappor"/>
      <skos:prefLabel xml:lang="en">photographic pre-production</skos:prefLabel>
      <skos:definition xml:lang="en">Photographic pre-production (proof) copy intended for
         review.</skos:definition>
      <skos:notation xml:lang="en">c</skos:notation>
   </rdf:Description>

   <rdf:Description rdf:about="http://fakeIRI.edu/terms/mappor#u">
      <rdf:type rdf:resource="http://www.w3.org/2004/02/skos/core#Concept"/>
      <skos:inScheme rdf:resource="http://fakeIRI.edu/terms/mappor"/>
      <skos:prefLabel xml:lang="en">unknown</skos:prefLabel>
      <skos:definition xml:lang="en">Production/reproduction details are not
         known.</skos:definition>
      <skos:notation xml:lang="en">u</skos:notation>
   </rdf:Description>
</rdf:RDF>
