<?xml version="1.0" encoding="UTF-8"?>
<rdf:RDF xmlns:dc="http://purl.org/dc/elements/1.1/" xmlns:dct="http://purl.org/dc/terms/"
   xmlns:rdf="http://www.w3.org/1999/02/22-rdf-syntax-ns#"
   xmlns:rdfs="http://www.w3.org/2000/01/rdf-schema#" xmlns:schema="https://schema.org/"
   xmlns:skos="http://www.w3.org/2004/02/skos/core#"
   xmlns:uw="https://www.lib.washington.edu/static/public/cams/data/localResources/properties_local.html"
   xmlns:uwp="https://doi.org/10.6069/uwlib.55.d.3#">


   <rdf:Description rdf:about="http://fakeIRI.edu/terms/remotesensingpct">
      <rdf:type rdf:resource="http://www.w3.org/2004/02/skos/core#ConceptScheme"/>
      <dct:type rdf:resource="http://purl.org/dc/dcmitype/Dataset"/>
      <dct:title xml:lang="en">Remote-sensing image: platform construction type</dct:title>
      <dct:alternative xml:lang="en">MARC21 007/06 values for remote-sensing images expressed using
         RDF</dct:alternative>
      <dct:description xml:lang="en">Type of construction of the platform serving as the base for
         the remote-sensing device. For the purposes of this data element, "platform" refers to any
         structure that serves as a base, not only flat surfaces.</dct:description>
      <schema:disambiguatingDescription>SKOS Concept Scheme for MARC 00X
         Values</schema:disambiguatingDescription>
      <dct:publisher rdf:resource="http://viaf.org/viaf/139541794"/>
      <dct:source rdf:resource="https://www.loc.gov/marc/bibliographic/bd007.html"/>
      <dct:source rdf:resource="http://marc21rdf.info"/>
      <dct:provenance rdf:resource="https://doi.org/10.6069/uwlswd.2e2b-y833"/>
      <dct:creator rdf:resource="http://viaf.org/viaf/139541794"/>
      <dct:contributor rdf:resource="http://viaf.org/viaf/151962300"/>
      <dct:issued>2024</dct:issued>
      <dc:contributor xml:lang="en">Metadata Management Associates</dc:contributor>
      <dc:language>en</dc:language>
      <dct:license rdf:resource="http://creativecommons.org/publicdomain/zero/1.0"/>
      <schema:version>1-0-0</schema:version>
      <dct:issued>2024</dct:issued>
      <dct:format rdf:resource="http://www.w3.org/ns/formats/RDF_XML"/>
   </rdf:Description>

   <rdf:Description rdf:about="http://fakeIRI.edu/terms/remotesensingpct#d">
      <rdf:type rdf:resource="http://www.w3.org/2004/02/skos/core#Concept"/>
      <skos:inScheme rdf:resource="http://fakeIRI.edu/terms/remotesensingpct"/>
      <skos:prefLabel xml:lang="en">aircraft - high altitude</skos:prefLabel>
      <skos:definition xml:lang="en">Base for the remote-sensing device was an dynamic lift aircraft
         designed for high altitude flight (above 49,000 ft. (14,810 m.)).</skos:definition>
      <skos:notation xml:lang="en">d</skos:notation>
   </rdf:Description>

   <rdf:Description rdf:about="http://fakeIRI.edu/terms/remotesensingpct#b">
      <rdf:type rdf:resource="http://www.w3.org/2004/02/skos/core#Concept"/>
      <skos:inScheme rdf:resource="http://fakeIRI.edu/terms/remotesensingpct"/>
      <skos:prefLabel xml:lang="en">aircraft - low altitude</skos:prefLabel>
      <skos:definition xml:lang="en">Base for the remote-sensing device was an dynamic lift aircraft
         designed for low altitude flight (below 29,500 ft. (8,962 m.)).</skos:definition>
      <skos:notation xml:lang="en">b</skos:notation>
   </rdf:Description>

   <rdf:Description rdf:about="http://fakeIRI.edu/terms/remotesensingpct#c">
      <rdf:type rdf:resource="http://www.w3.org/2004/02/skos/core#Concept"/>
      <skos:inScheme rdf:resource="http://fakeIRI.edu/terms/remotesensingpct"/>
      <skos:prefLabel xml:lang="en">aircraft - medium altitude</skos:prefLabel>
      <skos:definition xml:lang="en">Base for the remote-sensing device was an dynamic lift aircraft
         designed for medium altitude flight (between 29,500 ft. (8,962 m.) and 49,000 ft. (14,810
         m.)).</skos:definition>
      <skos:notation xml:lang="en">c</skos:notation>
   </rdf:Description>

   <rdf:Description rdf:about="http://fakeIRI.edu/terms/remotesensingpct#a">
      <rdf:type rdf:resource="http://www.w3.org/2004/02/skos/core#Concept"/>
      <skos:inScheme rdf:resource="http://fakeIRI.edu/terms/remotesensingpct"/>
      <skos:prefLabel xml:lang="en">balloon</skos:prefLabel>
      <skos:definition xml:lang="en">Base for the remote-sensing device was a balloon or similar
         lighter-than-air platform.</skos:definition>
      <skos:notation xml:lang="en">a</skos:notation>
   </rdf:Description>

   <rdf:Description rdf:about="http://fakeIRI.edu/terms/remotesensingpct#g">
      <rdf:type rdf:resource="http://www.w3.org/2004/02/skos/core#Concept"/>
      <skos:inScheme rdf:resource="http://fakeIRI.edu/terms/remotesensingpct"/>
      <skos:prefLabel xml:lang="en">land-based remote-sensing device</skos:prefLabel>
      <skos:definition xml:lang="en">Base for the remote-sensing device was a
         land-based.</skos:definition>
      <skos:notation xml:lang="en">g</skos:notation>
   </rdf:Description>

   <rdf:Description rdf:about="http://fakeIRI.edu/terms/remotesensingpct#e">
      <rdf:type rdf:resource="http://www.w3.org/2004/02/skos/core#Concept"/>
      <skos:inScheme rdf:resource="http://fakeIRI.edu/terms/remotesensingpct"/>
      <skos:prefLabel xml:lang="en">manned spacecraft</skos:prefLabel>
      <skos:definition xml:lang="en">Base for the remote-sensing device was a manned
         spacecraft.</skos:definition>
      <skos:notation xml:lang="en">e</skos:notation>
   </rdf:Description>

   <rdf:Description rdf:about="http://fakeIRI.edu/terms/remotesensingpct#n">
      <rdf:type rdf:resource="http://www.w3.org/2004/02/skos/core#Concept"/>
      <skos:inScheme rdf:resource="http://fakeIRI.edu/terms/remotesensingpct"/>
      <skos:prefLabel xml:lang="en">not applicable</skos:prefLabel>
      <skos:definition xml:lang="en">Not applicable.</skos:definition>
      <skos:notation xml:lang="en">n</skos:notation>
   </rdf:Description>

   <rdf:Description rdf:about="http://fakeIRI.edu/terms/remotesensingpct#z">
      <rdf:type rdf:resource="http://www.w3.org/2004/02/skos/core#Concept"/>
      <skos:inScheme rdf:resource="http://fakeIRI.edu/terms/remotesensingpct"/>
      <skos:prefLabel xml:lang="en">other</skos:prefLabel>
      <skos:definition xml:lang="en">Platform construction type other than balloon, aircraft - low
         altitude, aircraft - medium altitude, aircraft - high altitude, manned spacecraft, unmanned
         spacecraft, land-based remote-sensing device, water surface-based remote-sensing device, or
         submersible remote-sensing device.</skos:definition>
      <skos:notation xml:lang="en">z</skos:notation>
   </rdf:Description>

   <rdf:Description rdf:about="http://fakeIRI.edu/terms/remotesensingpct#i">
      <rdf:type rdf:resource="http://www.w3.org/2004/02/skos/core#Concept"/>
      <skos:inScheme rdf:resource="http://fakeIRI.edu/terms/remotesensingpct"/>
      <skos:prefLabel xml:lang="en">submersible remote-sensing device</skos:prefLabel>
      <skos:definition xml:lang="en">Base for the remote-sensing device was designed to be submerged
         beneath the surface of a body of water</skos:definition>
      <skos:scopeNote xml:lang="en">E.g., a submersible vessel or platform</skos:scopeNote>
      <skos:notation xml:lang="en">i</skos:notation>
   </rdf:Description>

   <rdf:Description rdf:about="http://fakeIRI.edu/terms/remotesensingpct#u">
      <rdf:type rdf:resource="http://www.w3.org/2004/02/skos/core#Concept"/>
      <skos:inScheme rdf:resource="http://fakeIRI.edu/terms/remotesensingpct"/>
      <skos:prefLabel xml:lang="en">unknown</skos:prefLabel>
      <skos:definition xml:lang="en">Construction type of the platform from which the remote-sensing
         image was made is not known.</skos:definition>
      <skos:notation xml:lang="en">u</skos:notation>
   </rdf:Description>

   <rdf:Description rdf:about="http://fakeIRI.edu/terms/remotesensingpct#f">
      <rdf:type rdf:resource="http://www.w3.org/2004/02/skos/core#Concept"/>
      <skos:inScheme rdf:resource="http://fakeIRI.edu/terms/remotesensingpct"/>
      <skos:prefLabel xml:lang="en">unmanned spacecraft</skos:prefLabel>
      <skos:definition xml:lang="en">Base for the remote-sensing device was an unmanned
         spacecraft.</skos:definition>
      <skos:notation xml:lang="en">f</skos:notation>
   </rdf:Description>

   <rdf:Description rdf:about="http://fakeIRI.edu/terms/remotesensingpct#h">
      <rdf:type rdf:resource="http://www.w3.org/2004/02/skos/core#Concept"/>
      <skos:inScheme rdf:resource="http://fakeIRI.edu/terms/remotesensingpct"/>
      <skos:prefLabel xml:lang="en">water surface-based remote-sensing device</skos:prefLabel>
      <skos:definition xml:lang="en">Base for the remote-sensing device was designed to remain on
         the surface of a body of water.</skos:definition>
      <skos:scopeNote xml:lang="en">E.g., a ship or floating platform</skos:scopeNote>
      <skos:notation xml:lang="en">h</skos:notation>
   </rdf:Description>
</rdf:RDF>
