<?xml version="1.0" encoding="utf-8"?>
<rdf:RDF
   xmlns:dc="http://purl.org/dc/elements/1.1/"
   xmlns:dct="http://purl.org/dc/terms/"
   xmlns:rdf="http://www.w3.org/1999/02/22-rdf-syntax-ns#"
   xmlns:schema="https://schema.org/"
   xmlns:skos="http://www.w3.org/2004/02/skos/core#"
>
  <rdf:Description rdf:about="https://doi.org/10.6069/uwlswd.dmgc-fs34">
    <rdf:type rdf:resource="http://www.w3.org/2004/02/skos/core#ConceptScheme"/>
    <dct:type rdf:resource="http://purl.org/dc/dcmitype/Dataset"/>
    <dct:title xml:lang="en">Remote-sensing image: platform construction type</dct:title>
    <dct:alternative xml:lang="en">MARC21 007/06 values for remote-sensing images expressed using
         RDF</dct:alternative>
    <dct:description xml:lang="en">Type of construction of the platform serving as the base for
         the remote-sensing device. For the purposes of this data element, "platform" refers to any
         structure that serves as a base, not only flat surfaces.</dct:description>
    <schema:disambiguatingDescription xml:lang="en">SKOS Concept Scheme for MARC 00X
         Values</schema:disambiguatingDescription>
    <dct:publisher rdf:resource="http://viaf.org/viaf/139541794"/>
    <dct:source rdf:resource="https://www.loc.gov/marc/bibliographic/bd007.html"/>
    <dct:source rdf:resource="http://marc21rdf.info"/>
    <dct:provenance rdf:resource="https://doi.org/10.6069/uwlswd.2e2b-y833#marc00Xvalues"/>
    <dct:creator rdf:resource="http://viaf.org/viaf/139541794"/>
    <dct:contributor rdf:resource="http://viaf.org/viaf/151962300"/>
    <dct:issued>2024</dct:issued>
    <dc:contributor xml:lang="en">Metadata Management Associates</dc:contributor>
    <dc:language>en</dc:language>
    <dct:license rdf:resource="http://creativecommons.org/publicdomain/zero/1.0"/>
    <schema:version>1-0-0</schema:version>
    <dct:format rdf:resource="http://www.w3.org/ns/formats/RDF_XML"/>
    <dct:hasFormat rdf:resource="https://uwlib-cams.github.io/uwlswd_vocabs_marc_007/remote-sensing_image_platform_construction_type/remote-sensing_image_platform_construction_type.ttl"/>
    <dct:hasFormat rdf:resource="https://uwlib-cams.github.io/uwlswd_vocabs_marc_007/remote-sensing_image_platform_construction_type/remote-sensing_image_platform_construction_type.nt"/>
    <dct:hasFormat rdf:resource="https://uwlib-cams.github.io/uwlswd_vocabs_marc_007/remote-sensing_image_platform_construction_type/remote-sensing_image_platform_construction_type.jsonld"/>
    <dct:hasFormat rdf:resource="https://uwlib-cams.github.io/uwlswd_vocabs_marc_007/remote-sensing_image_platform_construction_type/remote-sensing_image_platform_construction_type.html"/>
  </rdf:Description>
  <rdf:Description rdf:about="https://doi.org/10.6069/uwlswd.dmgc-fs34#a">
    <rdf:type rdf:resource="http://www.w3.org/2004/02/skos/core#Concept"/>
    <skos:inScheme rdf:resource="https://doi.org/10.6069/uwlswd.dmgc-fs34"/>
    <skos:prefLabel xml:lang="en">balloon</skos:prefLabel>
    <skos:definition xml:lang="en">Base for the remote-sensing device was a balloon or similar
         lighter-than-air platform.</skos:definition>
    <skos:notation>a</skos:notation>
  </rdf:Description>
  <rdf:Description rdf:about="https://doi.org/10.6069/uwlswd.dmgc-fs34#b">
    <rdf:type rdf:resource="http://www.w3.org/2004/02/skos/core#Concept"/>
    <skos:inScheme rdf:resource="https://doi.org/10.6069/uwlswd.dmgc-fs34"/>
    <skos:prefLabel xml:lang="en">aircraft - low altitude</skos:prefLabel>
    <skos:definition xml:lang="en">Base for the remote-sensing device was an dynamic lift aircraft
         designed for low altitude flight (below 29,500 ft. (8,962 m.)).</skos:definition>
    <skos:notation>b</skos:notation>
  </rdf:Description>
  <rdf:Description rdf:about="https://doi.org/10.6069/uwlswd.dmgc-fs34#f">
    <rdf:type rdf:resource="http://www.w3.org/2004/02/skos/core#Concept"/>
    <skos:inScheme rdf:resource="https://doi.org/10.6069/uwlswd.dmgc-fs34"/>
    <skos:prefLabel xml:lang="en">unmanned spacecraft</skos:prefLabel>
    <skos:definition xml:lang="en">Base for the remote-sensing device was an unmanned
         spacecraft.</skos:definition>
    <skos:notation>f</skos:notation>
  </rdf:Description>
  <rdf:Description rdf:about="https://doi.org/10.6069/uwlswd.dmgc-fs34#c">
    <rdf:type rdf:resource="http://www.w3.org/2004/02/skos/core#Concept"/>
    <skos:inScheme rdf:resource="https://doi.org/10.6069/uwlswd.dmgc-fs34"/>
    <skos:prefLabel xml:lang="en">aircraft - medium altitude</skos:prefLabel>
    <skos:definition xml:lang="en">Base for the remote-sensing device was an dynamic lift aircraft
         designed for medium altitude flight (between 29,500 ft. (8,962 m.) and 49,000 ft. (14,810
         m.)).</skos:definition>
    <skos:notation>c</skos:notation>
  </rdf:Description>
  <rdf:Description rdf:about="https://doi.org/10.6069/uwlswd.dmgc-fs34#g">
    <rdf:type rdf:resource="http://www.w3.org/2004/02/skos/core#Concept"/>
    <skos:inScheme rdf:resource="https://doi.org/10.6069/uwlswd.dmgc-fs34"/>
    <skos:prefLabel xml:lang="en">land-based remote-sensing device</skos:prefLabel>
    <skos:definition xml:lang="en">Base for the remote-sensing device was a
         land-based.</skos:definition>
    <skos:notation>g</skos:notation>
  </rdf:Description>
  <rdf:Description rdf:about="https://doi.org/10.6069/uwlswd.dmgc-fs34#z">
    <rdf:type rdf:resource="http://www.w3.org/2004/02/skos/core#Concept"/>
    <skos:inScheme rdf:resource="https://doi.org/10.6069/uwlswd.dmgc-fs34"/>
    <skos:prefLabel xml:lang="en">other</skos:prefLabel>
    <skos:definition xml:lang="en">Platform construction type other than balloon, aircraft - low
         altitude, aircraft - medium altitude, aircraft - high altitude, manned spacecraft, unmanned
         spacecraft, land-based remote-sensing device, water surface-based remote-sensing device, or
         submersible remote-sensing device.</skos:definition>
    <skos:notation>z</skos:notation>
  </rdf:Description>
  <rdf:Description rdf:about="https://doi.org/10.6069/uwlswd.dmgc-fs34#h">
    <rdf:type rdf:resource="http://www.w3.org/2004/02/skos/core#Concept"/>
    <skos:inScheme rdf:resource="https://doi.org/10.6069/uwlswd.dmgc-fs34"/>
    <skos:prefLabel xml:lang="en">water surface-based remote-sensing device</skos:prefLabel>
    <skos:definition xml:lang="en">Base for the remote-sensing device was designed to remain on
         the surface of a body of water.</skos:definition>
    <skos:scopeNote xml:lang="en">E.g., a ship or floating platform</skos:scopeNote>
    <skos:notation>h</skos:notation>
  </rdf:Description>
  <rdf:Description rdf:about="https://doi.org/10.6069/uwlswd.dmgc-fs34#n">
    <rdf:type rdf:resource="http://www.w3.org/2004/02/skos/core#Concept"/>
    <skos:inScheme rdf:resource="https://doi.org/10.6069/uwlswd.dmgc-fs34"/>
    <skos:prefLabel xml:lang="en">not applicable</skos:prefLabel>
    <skos:definition xml:lang="en">Not applicable.</skos:definition>
    <skos:notation>n</skos:notation>
  </rdf:Description>
  <rdf:Description rdf:about="https://doi.org/10.6069/uwlswd.dmgc-fs34#i">
    <rdf:type rdf:resource="http://www.w3.org/2004/02/skos/core#Concept"/>
    <skos:inScheme rdf:resource="https://doi.org/10.6069/uwlswd.dmgc-fs34"/>
    <skos:prefLabel xml:lang="en">submersible remote-sensing device</skos:prefLabel>
    <skos:definition xml:lang="en">Base for the remote-sensing device was designed to be submerged
         beneath the surface of a body of water</skos:definition>
    <skos:scopeNote xml:lang="en">E.g., a submersible vessel or platform</skos:scopeNote>
    <skos:notation>i</skos:notation>
  </rdf:Description>
  <rdf:Description rdf:about="https://doi.org/10.6069/uwlswd.dmgc-fs34#d">
    <rdf:type rdf:resource="http://www.w3.org/2004/02/skos/core#Concept"/>
    <skos:inScheme rdf:resource="https://doi.org/10.6069/uwlswd.dmgc-fs34"/>
    <skos:prefLabel xml:lang="en">aircraft - high altitude</skos:prefLabel>
    <skos:definition xml:lang="en">Base for the remote-sensing device was an dynamic lift aircraft
         designed for high altitude flight (above 49,000 ft. (14,810 m.)).</skos:definition>
    <skos:notation>d</skos:notation>
  </rdf:Description>
  <rdf:Description rdf:about="https://doi.org/10.6069/uwlswd.dmgc-fs34#u">
    <rdf:type rdf:resource="http://www.w3.org/2004/02/skos/core#Concept"/>
    <skos:inScheme rdf:resource="https://doi.org/10.6069/uwlswd.dmgc-fs34"/>
    <skos:prefLabel xml:lang="en">unknown</skos:prefLabel>
    <skos:definition xml:lang="en">Construction type of the platform from which the remote-sensing
         image was made is not known.</skos:definition>
    <skos:notation>u</skos:notation>
  </rdf:Description>
  <rdf:Description rdf:about="https://doi.org/10.6069/uwlswd.dmgc-fs34#e">
    <rdf:type rdf:resource="http://www.w3.org/2004/02/skos/core#Concept"/>
    <skos:inScheme rdf:resource="https://doi.org/10.6069/uwlswd.dmgc-fs34"/>
    <skos:prefLabel xml:lang="en">manned spacecraft</skos:prefLabel>
    <skos:definition xml:lang="en">Base for the remote-sensing device was a manned
         spacecraft.</skos:definition>
    <skos:notation>e</skos:notation>
  </rdf:Description>
</rdf:RDF>
