@prefix dc: <http://purl.org/dc/elements/1.1/> .
@prefix dct: <http://purl.org/dc/terms/> .
@prefix schema: <https://schema.org/> .
@prefix skos: <http://www.w3.org/2004/02/skos/core#> .

<https://doi.org/10.6069/uwlswd.3jgj-j280#a> a skos:Concept ;
    skos:definition "Not contracted."@en ;
    skos:inScheme <https://doi.org/10.6069/uwlswd.3jgj-j280> ;
    skos:notation "a" ;
    skos:prefLabel "uncontracted"@en ;
    skos:scopeNote "Includes grade 1 braille."@en .

<https://doi.org/10.6069/uwlswd.3jgj-j280#b> a skos:Concept ;
    skos:definition "Contracted."@en ;
    skos:inScheme <https://doi.org/10.6069/uwlswd.3jgj-j280> ;
    skos:notation "b" ;
    skos:prefLabel "contracted"@en ;
    skos:scopeNote """Includes Standard English braille, the code for contracted
         braille of the Braille Authority of the United Kingdom and English Braille, American ed.,
         the code for contracted braille of the Braille Authority of North America."""@en .

<https://doi.org/10.6069/uwlswd.3jgj-j280#m> a skos:Concept ;
    skos:definition "A combination of contracted and uncontracted."@en ;
    skos:inScheme <https://doi.org/10.6069/uwlswd.3jgj-j280> ;
    skos:notation "m" ;
    skos:prefLabel "combination"@en .

<https://doi.org/10.6069/uwlswd.3jgj-j280#n> a skos:Concept ;
    skos:definition "Item is not braille or Moon."@en ;
    skos:inScheme <https://doi.org/10.6069/uwlswd.3jgj-j280> ;
    skos:notation "n" ;
    skos:prefLabel "not applicable"@en .

<https://doi.org/10.6069/uwlswd.3jgj-j280#u> a skos:Concept ;
    skos:definition "Level of contraction is not known."@en ;
    skos:inScheme <https://doi.org/10.6069/uwlswd.3jgj-j280> ;
    skos:notation "u" ;
    skos:prefLabel "unknown"@en .

<https://doi.org/10.6069/uwlswd.3jgj-j280#z> a skos:Concept ;
    skos:definition """Level of contraction other than uncontracted, contracted, or
         combination."""@en ;
    skos:inScheme <https://doi.org/10.6069/uwlswd.3jgj-j280> ;
    skos:notation "z" ;
    skos:prefLabel "other"@en .

<https://doi.org/10.6069/uwlswd.3jgj-j280> a skos:ConceptScheme ;
    dc:contributor "Metadata Management Associates"@en ;
    dc:language "en" ;
    dct:alternative """MARC21 007/05 values for tactile material expressed using
         RDF"""@en ;
    dct:contributor <http://viaf.org/viaf/151962300> ;
    dct:creator <http://viaf.org/viaf/139541794> ;
    dct:description """Whether contractions are used. Contractions are abbreviations
         consisting of one or more braille or Moon characters to represent common letter
         combinations."""@en ;
    dct:format <http://www.w3.org/ns/formats/Turtle> ;
    dct:hasFormat <https://uwlib-cams.github.io/uwlswd_vocabs_marc_007/tactile_material_level_of_contraction/tactile_material_level_of_contraction.html>,
        <https://uwlib-cams.github.io/uwlswd_vocabs_marc_007/tactile_material_level_of_contraction/tactile_material_level_of_contraction.jsonld>,
        <https://uwlib-cams.github.io/uwlswd_vocabs_marc_007/tactile_material_level_of_contraction/tactile_material_level_of_contraction.nt>,
        <https://uwlib-cams.github.io/uwlswd_vocabs_marc_007/tactile_material_level_of_contraction/tactile_material_level_of_contraction.rdf> ;
    dct:issued "2024" ;
    dct:license <http://creativecommons.org/publicdomain/zero/1.0> ;
    dct:provenance <https://doi.org/10.6069/uwlswd.2e2b-y833#marc00Xvalues> ;
    dct:publisher <http://viaf.org/viaf/139541794> ;
    dct:source <http://marc21rdf.info>,
        <https://www.loc.gov/marc/bibliographic/bd007.html> ;
    dct:title "Tactile material: level of contraction"@en ;
    dct:type <http://purl.org/dc/dcmitype/Dataset> ;
    schema:disambiguatingDescription """SKOS Concept Scheme for MARC 00X
         Values"""@en ;
    schema:version "1-0-0" .

