@prefix dc: <http://purl.org/dc/elements/1.1/> .
@prefix dct: <http://purl.org/dc/terms/> .
@prefix schema: <https://schema.org/> .
@prefix skos: <http://www.w3.org/2004/02/skos/core#> .

<https://doi.org/10.6069/uwlswd.06cw-h775#a> a skos:Concept ;
    skos:definition """Remote-sensing device is closer to parallel with the surface
         being imaged than perpendicular."""@en ;
    skos:inScheme <https://doi.org/10.6069/uwlswd.06cw-h775> ;
    skos:notation "a" ;
    skos:prefLabel "low oblique"@en .

<https://doi.org/10.6069/uwlswd.06cw-h775#b> a skos:Concept ;
    skos:definition """Remote-sensing device is closer to perpendicular to the surface
         than parallel."""@en ;
    skos:inScheme <https://doi.org/10.6069/uwlswd.06cw-h775> ;
    skos:notation "b" ;
    skos:prefLabel "high oblique"@en .

<https://doi.org/10.6069/uwlswd.06cw-h775#c> a skos:Concept ;
    skos:definition """Angle of the remote-sensing device is vertical to the surface
         being imaged."""@en ;
    skos:inScheme <https://doi.org/10.6069/uwlswd.06cw-h775> ;
    skos:notation "c" ;
    skos:prefLabel "vertical"@en .

<https://doi.org/10.6069/uwlswd.06cw-h775#n> a skos:Concept ;
    skos:definition """Angle of the remote-sensing device is not applicable,
         generally, because the attitude does not affect the image."""@en ;
    skos:inScheme <https://doi.org/10.6069/uwlswd.06cw-h775> ;
    skos:notation "n" ;
    skos:prefLabel "not applicable"@en .

<https://doi.org/10.6069/uwlswd.06cw-h775#u> a skos:Concept ;
    skos:definition """Angle of the remote-sensing device is not
         known."""@en ;
    skos:inScheme <https://doi.org/10.6069/uwlswd.06cw-h775> ;
    skos:notation "u" ;
    skos:prefLabel "unknown"@en .

<https://doi.org/10.6069/uwlswd.06cw-h775> a skos:ConceptScheme ;
    dc:contributor "Metadata Management Associates"@en ;
    dc:language "en" ;
    dct:alternative """MARC21 007/04 values for remote-sensing images expressed using
         RDF"""@en ;
    dct:contributor <http://viaf.org/viaf/151962300> ;
    dct:creator <http://viaf.org/viaf/139541794> ;
    dct:description """General angle of the device from which the remote-sensing image
         is made."""@en ;
    dct:format <http://www.w3.org/ns/formats/Turtle> ;
    dct:hasFormat <https://uwlib-cams.github.io/uwlswd_vocabs_marc_007/remote-sensing_image_attitude_of_sensor/remote-sensing_image_attitude_of_sensor.html>,
        <https://uwlib-cams.github.io/uwlswd_vocabs_marc_007/remote-sensing_image_attitude_of_sensor/remote-sensing_image_attitude_of_sensor.jsonld>,
        <https://uwlib-cams.github.io/uwlswd_vocabs_marc_007/remote-sensing_image_attitude_of_sensor/remote-sensing_image_attitude_of_sensor.nt>,
        <https://uwlib-cams.github.io/uwlswd_vocabs_marc_007/remote-sensing_image_attitude_of_sensor/remote-sensing_image_attitude_of_sensor.rdf> ;
    dct:issued "2024" ;
    dct:license <http://creativecommons.org/publicdomain/zero/1.0> ;
    dct:provenance <https://doi.org/10.6069/uwlswd.2e2b-y833#marc00Xvalues> ;
    dct:publisher <http://viaf.org/viaf/139541794> ;
    dct:source <http://marc21rdf.info>,
        <https://www.loc.gov/marc/bibliographic/bd007.html> ;
    dct:title "Remote-sensing image: attitude of sensor"@en ;
    dct:type <http://purl.org/dc/dcmitype/Dataset> ;
    schema:disambiguatingDescription """SKOS Concept Scheme for MARC 00X
         Values"""@en ;
    schema:version "1-0-0" .

