@prefix dc: <http://purl.org/dc/elements/1.1/> .
@prefix dct: <http://purl.org/dc/terms/> .
@prefix schema: <https://schema.org/> .
@prefix skos: <http://www.w3.org/2004/02/skos/core#> .

<https://doi.org/10.6069/uwlswd.hteb-5554#a> a skos:Concept ;
    skos:definition """Lacquer coated, but the base material on which the lacquer is
         applied is not identified."""@en ;
    skos:inScheme <https://doi.org/10.6069/uwlswd.hteb-5554> ;
    skos:notation "a" ;
    skos:prefLabel "lacquer coating"@en .

<https://doi.org/10.6069/uwlswd.hteb-5554#b> a skos:Concept ;
    skos:definition "Cellulose nitrate base."@en ;
    skos:inScheme <https://doi.org/10.6069/uwlswd.hteb-5554> ;
    skos:notation "b" ;
    skos:prefLabel "cellulose nitrate"@en ;
    skos:scopeNote "used for items such as memovox discs."@en .

<https://doi.org/10.6069/uwlswd.hteb-5554#c> a skos:Concept ;
    skos:definition "Acetate base with a ferrous oxide coating."@en ;
    skos:inScheme <https://doi.org/10.6069/uwlswd.hteb-5554> ;
    skos:notation "c" ;
    skos:prefLabel "acetate tape with ferrous oxide"@en ;
    skos:scopeNote """May include acetate tape and belts, such as
         magnabelts."""@en .

<https://doi.org/10.6069/uwlswd.hteb-5554#g> a skos:Concept ;
    skos:definition "Glass disc base with a lacquer coating."@en ;
    skos:inScheme <https://doi.org/10.6069/uwlswd.hteb-5554> ;
    skos:notation "g" ;
    skos:prefLabel "glass with lacquer"@en .

<https://doi.org/10.6069/uwlswd.hteb-5554#i> a skos:Concept ;
    skos:definition "Aluminum disc base with a lacquer coating."@en ;
    skos:inScheme <https://doi.org/10.6069/uwlswd.hteb-5554> ;
    skos:notation "i" ;
    skos:prefLabel "aluminum with lacquer"@en .

<https://doi.org/10.6069/uwlswd.hteb-5554#l> a skos:Concept ;
    skos:definition "Made entirely of metal."@en ;
    skos:inScheme <https://doi.org/10.6069/uwlswd.hteb-5554> ;
    skos:notation "l" ;
    skos:prefLabel "metal"@en ;
    skos:scopeNote """Includes the earliest cylinders, which were made of tinfoil, and
         aluminum transcription discs with no coating, as well as wire and metal
         tape."""@en .

<https://doi.org/10.6069/uwlswd.hteb-5554#m> a skos:Concept ;
    skos:definition "Made of plastic base with a metal coating."@en ;
    skos:inScheme <https://doi.org/10.6069/uwlswd.hteb-5554> ;
    skos:notation "m" ;
    skos:prefLabel "plastic with metal"@en ;
    skos:scopeNote """The metal part of such an item is often a thin layer applied to
         the plastic base. Includes compact audio discs (CDs)."""@en .

<https://doi.org/10.6069/uwlswd.hteb-5554#mx> a skos:Concept ;
    skos:inScheme <https://doi.org/10.6069/uwlswd.hteb-5554> ;
    skos:notation "m" ;
    skos:prefLabel "molded cylinder-mass produced [obsolete]"@en .

<https://doi.org/10.6069/uwlswd.hteb-5554#nx> a skos:Concept ;
    skos:definition """Item does not have a kind of material that contains sound
         recording information."""@en ;
    skos:inScheme <https://doi.org/10.6069/uwlswd.hteb-5554> ;
    skos:notation "n" ;
    skos:prefLabel "not applicable"@en ;
    skos:scopeNote """Kind of material is not applicable to remote digital sound
         recordings because it pertains to characteristics specific to physical aspects of
         carriers."""@en .

<https://doi.org/10.6069/uwlswd.hteb-5554#p> a skos:Concept ;
    skos:definition "Made entirely of plastic."@en ;
    skos:inScheme <https://doi.org/10.6069/uwlswd.hteb-5554> ;
    skos:notation "p" ;
    skos:prefLabel "plastic"@en ;
    skos:scopeNote """Also includes mylar, polyester and vinyl materials. Since the
         1950s, commercial or mass-produced sound recordings on 16, 33 1/3, and 45 rpm discs,
         cassettes, and cartridges are made of plastic."""@en .

<https://doi.org/10.6069/uwlswd.hteb-5554#r> a skos:Concept ;
    skos:definition """Paper or cardboard disc, tape, or cylinder base with a lacquer
         or ferrous oxide coating."""@en ;
    skos:inScheme <https://doi.org/10.6069/uwlswd.hteb-5554> ;
    skos:notation "r" ;
    skos:prefLabel "paper with lacquer or ferrous oxide"@en .

<https://doi.org/10.6069/uwlswd.hteb-5554#s> a skos:Concept ;
    skos:definition "Made entirely of shellac."@en ;
    skos:inScheme <https://doi.org/10.6069/uwlswd.hteb-5554> ;
    skos:notation "s" ;
    skos:prefLabel "shellac"@en ;
    skos:scopeNote """Most commercial or mass-produced 78 rpm discs are made of
         shellac."""@en .

<https://doi.org/10.6069/uwlswd.hteb-5554#u> a skos:Concept ;
    skos:definition """Kind of material used in the manufacture of the item is not
         known."""@en ;
    skos:inScheme <https://doi.org/10.6069/uwlswd.hteb-5554> ;
    skos:notation "u" ;
    skos:prefLabel "unknown"@en .

<https://doi.org/10.6069/uwlswd.hteb-5554#w> a skos:Concept ;
    skos:definition "Made entirely of wax."@en ;
    skos:inScheme <https://doi.org/10.6069/uwlswd.hteb-5554> ;
    skos:notation "w" ;
    skos:prefLabel "wax"@en ;
    skos:scopeNote "Most instantaneous cylinders were made of wax."@en .

<https://doi.org/10.6069/uwlswd.hteb-5554#z> a skos:Concept ;
    skos:definition """Kind of material other than lacquer coating, cellulose nitrate,
         acetate tape with ferrous oxide. glass with lacquer, aluminum with lacquer, metal, plastic
         with metal, plastic, paper with lacquer or ferrous oxide, shellac, or
         wax."""@en ;
    skos:inScheme <https://doi.org/10.6069/uwlswd.hteb-5554> ;
    skos:notation "z" ;
    skos:prefLabel "other"@en .

<https://doi.org/10.6069/uwlswd.hteb-5554> a skos:ConceptScheme ;
    dc:contributor "Metadata Management Associates"@en ;
    dc:language "en" ;
    dct:alternative """MARC21 007/10 values for sound recordings expressed using
         RDF"""@en ;
    dct:contributor <http://viaf.org/viaf/151962300> ;
    dct:creator <http://viaf.org/viaf/139541794> ;
    dct:description """Kind of material used in the manufacture of sound recordings
         (both instantaneous and mass-produced)."""@en ;
    dct:format <http://www.w3.org/ns/formats/Turtle> ;
    dct:hasFormat <https://uwlib-cams.github.io/uwlswd_vocabs_marc_007/sound_recording_kind_of_material/sound_recording_kind_of_material.html>,
        <https://uwlib-cams.github.io/uwlswd_vocabs_marc_007/sound_recording_kind_of_material/sound_recording_kind_of_material.jsonld>,
        <https://uwlib-cams.github.io/uwlswd_vocabs_marc_007/sound_recording_kind_of_material/sound_recording_kind_of_material.nt>,
        <https://uwlib-cams.github.io/uwlswd_vocabs_marc_007/sound_recording_kind_of_material/sound_recording_kind_of_material.rdf> ;
    dct:issued "2024" ;
    dct:license <http://creativecommons.org/publicdomain/zero/1.0> ;
    dct:provenance <https://doi.org/10.6069/uwlswd.2e2b-y833#marc00Xvalues> ;
    dct:publisher <http://viaf.org/viaf/139541794> ;
    dct:source <http://marc21rdf.info>,
        <https://www.loc.gov/marc/bibliographic/bd007.html> ;
    dct:title "Sound recording: kind of material"@en ;
    dct:type <http://purl.org/dc/dcmitype/Dataset> ;
    schema:disambiguatingDescription """SKOS Concept Scheme for MARC 00X
         Values"""@en ;
    schema:version "1-0-0" .

