<?xml version="1.0" encoding="utf-8"?>
<rdf:RDF
   xmlns:dc="http://purl.org/dc/elements/1.1/"
   xmlns:dct="http://purl.org/dc/terms/"
   xmlns:rdf="http://www.w3.org/1999/02/22-rdf-syntax-ns#"
   xmlns:schema="https://schema.org/"
   xmlns:skos="http://www.w3.org/2004/02/skos/core#"
>
  <rdf:Description rdf:about="http://fakeIRI.edu/terms/soundrecordingmat">
    <rdf:type rdf:resource="http://www.w3.org/2004/02/skos/core#ConceptScheme"/>
    <dct:type rdf:resource="http://purl.org/dc/dcmitype/Dataset"/>
    <dct:title xml:lang="en">Sound recording: kind of material</dct:title>
    <dct:alternative xml:lang="en">MARC21 007/10 values for sound recordings expressed using
         RDF</dct:alternative>
    <dct:description xml:lang="en">Kind of material used in the manufacture of sound recordings
         (both instantaneous and mass-produced).</dct:description>
    <schema:disambiguatingDescription>SKOS Concept Scheme for MARC 00X
         Values</schema:disambiguatingDescription>
    <dct:publisher rdf:resource="http://viaf.org/viaf/139541794"/>
    <dct:source rdf:resource="https://www.loc.gov/marc/bibliographic/bd007.html"/>
    <dct:source rdf:resource="http://marc21rdf.info"/>
    <dct:provenance rdf:resource="https://doi.org/10.6069/uwlswd.2e2b-y833"/>
    <dct:creator rdf:resource="http://viaf.org/viaf/139541794"/>
    <dct:contributor rdf:resource="http://viaf.org/viaf/151962300"/>
    <dct:issued>2024</dct:issued>
    <dc:contributor xml:lang="en">Metadata Management Associates</dc:contributor>
    <dc:language>en</dc:language>
    <dct:license rdf:resource="http://creativecommons.org/publicdomain/zero/1.0"/>
    <schema:version>1-0-0</schema:version>
    <dct:format rdf:resource="http://www.w3.org/ns/formats/RDF_XML"/>
  </rdf:Description>
  <rdf:Description rdf:about="http://fakeIRI.edu/terms/soundrecordingmat#z">
    <rdf:type rdf:resource="http://www.w3.org/2004/02/skos/core#Concept"/>
    <skos:inScheme rdf:resource="http://fakeIRI.edu/terms/soundrecordingmat"/>
    <skos:prefLabel xml:lang="en">other</skos:prefLabel>
    <skos:definition xml:lang="en">Kind of material other than lacquer coating, cellulose nitrate,
         acetate tape with ferrous oxide. glass with lacquer, aluminum with lacquer, metal, plastic
         with metal, plastic, paper with lacquer or ferrous oxide, shellac, or
         wax.</skos:definition>
    <skos:notation xml:lang="en">z</skos:notation>
  </rdf:Description>
  <rdf:Description rdf:about="http://fakeIRI.edu/terms/soundrecordingmat#mx">
    <rdf:type rdf:resource="http://www.w3.org/2004/02/skos/core#Concept"/>
    <skos:inScheme rdf:resource="http://fakeIRI.edu/terms/soundrecordingmat"/>
    <skos:prefLabel xml:lang="en">molded cylinder-mass produced [obsolete]</skos:prefLabel>
    <skos:notation xml:lang="en">m</skos:notation>
  </rdf:Description>
  <rdf:Description rdf:about="http://fakeIRI.edu/terms/soundrecordingmat#w">
    <rdf:type rdf:resource="http://www.w3.org/2004/02/skos/core#Concept"/>
    <skos:inScheme rdf:resource="http://fakeIRI.edu/terms/soundrecordingmat"/>
    <skos:prefLabel xml:lang="en">wax</skos:prefLabel>
    <skos:definition xml:lang="en">Made entirely of wax.</skos:definition>
    <skos:scopeNote xml:lang="en">Most instantaneous cylinders were made of wax.</skos:scopeNote>
    <skos:notation xml:lang="en">w</skos:notation>
  </rdf:Description>
  <rdf:Description rdf:about="http://fakeIRI.edu/terms/soundrecordingmat#a">
    <rdf:type rdf:resource="http://www.w3.org/2004/02/skos/core#Concept"/>
    <skos:inScheme rdf:resource="http://fakeIRI.edu/terms/soundrecordingmat"/>
    <skos:prefLabel xml:lang="en">lacquer coating</skos:prefLabel>
    <skos:definition xml:lang="en">Lacquer coated, but the base material on which the lacquer is
         applied is not identified.</skos:definition>
    <skos:notation xml:lang="en">a</skos:notation>
  </rdf:Description>
  <rdf:Description rdf:about="http://fakeIRI.edu/terms/soundrecordingmat#r">
    <rdf:type rdf:resource="http://www.w3.org/2004/02/skos/core#Concept"/>
    <skos:inScheme rdf:resource="http://fakeIRI.edu/terms/soundrecordingmat"/>
    <skos:prefLabel xml:lang="en">paper with lacquer or ferrous oxide</skos:prefLabel>
    <skos:definition xml:lang="en">Paper or cardboard disc, tape, or cylinder base with a lacquer
         or ferrous oxide coating.</skos:definition>
    <skos:notation xml:lang="en">r</skos:notation>
  </rdf:Description>
  <rdf:Description rdf:about="http://fakeIRI.edu/terms/soundrecordingmat#nx">
    <rdf:type rdf:resource="http://www.w3.org/2004/02/skos/core#Concept"/>
    <skos:inScheme rdf:resource="http://fakeIRI.edu/terms/soundrecordingmat"/>
    <skos:prefLabel xml:lang="en">not applicable</skos:prefLabel>
    <skos:definition xml:lang="en">Item does not have a kind of material that contains sound
         recording information.</skos:definition>
    <skos:scopeNote xml:lang="en">Kind of material is not applicable to remote digital sound
         recordings because it pertains to characteristics specific to physical aspects of
         carriers.</skos:scopeNote>
    <skos:notation xml:lang="en">n</skos:notation>
  </rdf:Description>
  <rdf:Description rdf:about="http://fakeIRI.edu/terms/soundrecordingmat#i">
    <rdf:type rdf:resource="http://www.w3.org/2004/02/skos/core#Concept"/>
    <skos:inScheme rdf:resource="http://fakeIRI.edu/terms/soundrecordingmat"/>
    <skos:prefLabel xml:lang="en">aluminum with lacquer</skos:prefLabel>
    <skos:definition xml:lang="en">Aluminum disc base with a lacquer coating.</skos:definition>
    <skos:notation xml:lang="en">i</skos:notation>
  </rdf:Description>
  <rdf:Description rdf:about="http://fakeIRI.edu/terms/soundrecordingmat#p">
    <rdf:type rdf:resource="http://www.w3.org/2004/02/skos/core#Concept"/>
    <skos:inScheme rdf:resource="http://fakeIRI.edu/terms/soundrecordingmat"/>
    <skos:prefLabel xml:lang="en">plastic</skos:prefLabel>
    <skos:definition xml:lang="en">Made entirely of plastic.</skos:definition>
    <skos:scopeNote xml:lang="en">Also includes mylar, polyester and vinyl materials. Since the
         1950s, commercial or mass-produced sound recordings on 16, 33 1/3, and 45 rpm discs,
         cassettes, and cartridges are made of plastic.</skos:scopeNote>
    <skos:notation xml:lang="en">p</skos:notation>
  </rdf:Description>
  <rdf:Description rdf:about="http://fakeIRI.edu/terms/soundrecordingmat#m">
    <rdf:type rdf:resource="http://www.w3.org/2004/02/skos/core#Concept"/>
    <skos:inScheme rdf:resource="http://fakeIRI.edu/terms/soundrecordingmat"/>
    <skos:prefLabel xml:lang="en">plastic with metal</skos:prefLabel>
    <skos:definition xml:lang="en">Made of plastic base with a metal coating.</skos:definition>
    <skos:scopeNote xml:lang="en">The metal part of such an item is often a thin layer applied to
         the plastic base. Includes compact audio discs (CDs).</skos:scopeNote>
    <skos:notation xml:lang="en">m</skos:notation>
  </rdf:Description>
  <rdf:Description rdf:about="http://fakeIRI.edu/terms/soundrecordingmat#l">
    <rdf:type rdf:resource="http://www.w3.org/2004/02/skos/core#Concept"/>
    <skos:inScheme rdf:resource="http://fakeIRI.edu/terms/soundrecordingmat"/>
    <skos:prefLabel xml:lang="en">metal</skos:prefLabel>
    <skos:definition xml:lang="en">Made entirely of metal.</skos:definition>
    <skos:scopeNote xml:lang="en">Includes the earliest cylinders, which were made of tinfoil, and
         aluminum transcription discs with no coating, as well as wire and metal
         tape.</skos:scopeNote>
    <skos:notation xml:lang="en">l</skos:notation>
  </rdf:Description>
  <rdf:Description rdf:about="http://fakeIRI.edu/terms/soundrecordingmat#g">
    <rdf:type rdf:resource="http://www.w3.org/2004/02/skos/core#Concept"/>
    <skos:inScheme rdf:resource="http://fakeIRI.edu/terms/soundrecordingmat"/>
    <skos:prefLabel xml:lang="en">glass with lacquer</skos:prefLabel>
    <skos:definition xml:lang="en">Glass disc base with a lacquer coating.</skos:definition>
    <skos:notation xml:lang="en">g</skos:notation>
  </rdf:Description>
  <rdf:Description rdf:about="http://fakeIRI.edu/terms/soundrecordingmat#b">
    <rdf:type rdf:resource="http://www.w3.org/2004/02/skos/core#Concept"/>
    <skos:inScheme rdf:resource="http://fakeIRI.edu/terms/soundrecordingmat"/>
    <skos:prefLabel xml:lang="en">cellulose nitrate</skos:prefLabel>
    <skos:definition xml:lang="en">Cellulose nitrate base.</skos:definition>
    <skos:scopeNote xml:lang="en">used for items such as memovox discs.</skos:scopeNote>
    <skos:notation xml:lang="en">b</skos:notation>
  </rdf:Description>
  <rdf:Description rdf:about="http://fakeIRI.edu/terms/soundrecordingmat#s">
    <rdf:type rdf:resource="http://www.w3.org/2004/02/skos/core#Concept"/>
    <skos:inScheme rdf:resource="http://fakeIRI.edu/terms/soundrecordingmat"/>
    <skos:prefLabel xml:lang="en">shellac</skos:prefLabel>
    <skos:definition xml:lang="en">Made entirely of shellac.</skos:definition>
    <skos:scopeNote xml:lang="en">Most commercial or mass-produced 78 rpm discs are made of
         shellac.</skos:scopeNote>
    <skos:notation xml:lang="en">s</skos:notation>
  </rdf:Description>
  <rdf:Description rdf:about="http://fakeIRI.edu/terms/soundrecordingmat#u">
    <rdf:type rdf:resource="http://www.w3.org/2004/02/skos/core#Concept"/>
    <skos:inScheme rdf:resource="http://fakeIRI.edu/terms/soundrecordingmat"/>
    <skos:prefLabel xml:lang="en">unknown</skos:prefLabel>
    <skos:definition xml:lang="en">Kind of material used in the manufacture of the item is not
         known.</skos:definition>
    <skos:notation xml:lang="en">u</skos:notation>
  </rdf:Description>
  <rdf:Description rdf:about="http://fakeIRI.edu/terms/soundrecordingmat#c">
    <rdf:type rdf:resource="http://www.w3.org/2004/02/skos/core#Concept"/>
    <skos:inScheme rdf:resource="http://fakeIRI.edu/terms/soundrecordingmat"/>
    <skos:prefLabel xml:lang="en">acetate tape with ferrous oxide</skos:prefLabel>
    <skos:definition xml:lang="en">Acetate base with a ferrous oxide coating.</skos:definition>
    <skos:scopeNote xml:lang="en">May include acetate tape and belts, such as
         magnabelts.</skos:scopeNote>
    <skos:notation xml:lang="en">c</skos:notation>
  </rdf:Description>
</rdf:RDF>
