@prefix dc: <http://purl.org/dc/elements/1.1/> .
@prefix dct: <http://purl.org/dc/terms/> .
@prefix schema: <https://schema.org/> .
@prefix skos: <http://www.w3.org/2004/02/skos/core#> .

<https://doi.org/10.6069/uwlswd.9het-z010#c> a skos:Concept ;
    skos:definition "Judged to be complete."@en ;
    skos:inScheme <https://doi.org/10.6069/uwlswd.9het-z010> ;
    skos:notation "c" ;
    skos:prefLabel "complete"@en .

<https://doi.org/10.6069/uwlswd.9het-z010#i> a skos:Concept ;
    skos:definition "Judged to be incomplete."@en ;
    skos:inScheme <https://doi.org/10.6069/uwlswd.9het-z010> ;
    skos:notation "i" ;
    skos:prefLabel "incomplete"@en .

<https://doi.org/10.6069/uwlswd.9het-z010#n> a skos:Concept ;
    skos:definition """Completeness is not applicable to the type of motion
         picture."""@en ;
    skos:inScheme <https://doi.org/10.6069/uwlswd.9het-z010> ;
    skos:notation "n" ;
    skos:prefLabel "not applicable"@en ;
    skos:scopeNote """E.g., home movies, unedited footage, outtakes, and in some
         cases, unidentified material, etc."""@en .

<https://doi.org/10.6069/uwlswd.9het-z010#u> a skos:Concept ;
    skos:definition "Completeness of the item is not known."@en ;
    skos:inScheme <https://doi.org/10.6069/uwlswd.9het-z010> ;
    skos:notation "u" ;
    skos:prefLabel "unknown"@en .

<https://doi.org/10.6069/uwlswd.9het-z010> a skos:ConceptScheme ;
    dc:contributor "Metadata Management Associates"@en ;
    dc:language "en" ;
    dct:alternative """MARC21 007/16 values for motion pictures expressed using
         RDF"""@en ;
    dct:contributor <http://viaf.org/viaf/151962300> ;
    dct:creator <http://viaf.org/viaf/139541794> ;
    dct:description """Whether or not the item being cataloged is judged to be
         complete."""@en ;
    dct:format <http://www.w3.org/ns/formats/Turtle> ;
    dct:hasFormat <https://uwlib-cams.github.io/uwlswd_vocabs_marc_007/motion_picture_completeness/motion_picture_completeness.html>,
        <https://uwlib-cams.github.io/uwlswd_vocabs_marc_007/motion_picture_completeness/motion_picture_completeness.jsonld>,
        <https://uwlib-cams.github.io/uwlswd_vocabs_marc_007/motion_picture_completeness/motion_picture_completeness.nt>,
        <https://uwlib-cams.github.io/uwlswd_vocabs_marc_007/motion_picture_completeness/motion_picture_completeness.rdf> ;
    dct:issued "2024" ;
    dct:license <http://creativecommons.org/publicdomain/zero/1.0> ;
    dct:provenance <https://doi.org/10.6069/uwlswd.2e2b-y833#marc00Xvalues> ;
    dct:publisher <http://viaf.org/viaf/139541794> ;
    dct:source <http://marc21rdf.info>,
        <https://www.loc.gov/marc/bibliographic/bd007.html> ;
    dct:title "Motion picture: completeness"@en ;
    dct:type <http://purl.org/dc/dcmitype/Dataset> ;
    schema:disambiguatingDescription """SKOS Concept Scheme for MARC 00X
         Values"""@en ;
    schema:version "1-0-0" .

