@prefix dc: <http://purl.org/dc/elements/1.1/> .
@prefix dct: <http://purl.org/dc/terms/> .
@prefix schema: <https://schema.org/> .
@prefix skos: <http://www.w3.org/2004/02/skos/core#> .

<https://doi.org/10.6069/uwlswd.m9z2-3g03#a> a skos:Concept ;
    skos:definition "A compound of silver and halogens."@en ;
    skos:inScheme <https://doi.org/10.6069/uwlswd.m9z2-3g03> ;
    skos:notation "a" ;
    skos:prefLabel "silver halide"@en ;
    skos:scopeNote """Silver halide microforms always appear black-and-white
         (black-and-transparent)."""@en .

<https://doi.org/10.6069/uwlswd.m9z2-3g03#b> a skos:Concept ;
    skos:definition """Sensitized layers composed of diazonium salts that react with
         couplers to form dye images. The color of the image is determined by the composition of the
         diazonium compound as well as the couplers used in the process."""@en ;
    skos:inScheme <https://doi.org/10.6069/uwlswd.m9z2-3g03> ;
    skos:notation "b" ;
    skos:prefLabel "diazo"@en ;
    skos:scopeNote "May be black, violet, or another color."@en .

<https://doi.org/10.6069/uwlswd.m9z2-3g03#c> a skos:Concept ;
    skos:definition """Light-sensitive component is suspended in a plastic layer. On
         exposure, the component creates optical vesicules (bubbles) in the layers. These bubbles
         form the latent image. The latent image becomes visible and fixed by heating the plastic
         layer and then allowing it to cool."""@en ;
    skos:inScheme <https://doi.org/10.6069/uwlswd.m9z2-3g03> ;
    skos:notation "c" ;
    skos:prefLabel "vesicular"@en ;
    skos:scopeNote """Vesicular films are commonly blue or beige in color. They do not
         appear to have much contrast (very high density) until projected in a microform
         reader."""@en .

<https://doi.org/10.6069/uwlswd.m9z2-3g03#m> a skos:Concept ;
    skos:definition "Mixed emulsion."@en ;
    skos:inScheme <https://doi.org/10.6069/uwlswd.m9z2-3g03> ;
    skos:notation "m" ;
    skos:prefLabel "mixed emulsion"@en ;
    skos:scopeNote """For example, a microfilm may have slices of film with one type
         of emulsion and other slices with another type of emulsion."""@en .

<https://doi.org/10.6069/uwlswd.m9z2-3g03#n> a skos:Concept ;
    skos:definition "Item does not have emulsion on film."@en ;
    skos:inScheme <https://doi.org/10.6069/uwlswd.m9z2-3g03> ;
    skos:notation "n" ;
    skos:prefLabel "not applicable"@en ;
    skos:scopeNote "Used for microopaques."@en .

<https://doi.org/10.6069/uwlswd.m9z2-3g03#u> a skos:Concept ;
    skos:definition "Emulsion on the film is not known."@en ;
    skos:inScheme <https://doi.org/10.6069/uwlswd.m9z2-3g03> ;
    skos:notation "u" ;
    skos:prefLabel "unknown"@en .

<https://doi.org/10.6069/uwlswd.m9z2-3g03#z> a skos:Concept ;
    skos:definition """Emulsion on film other than silver halide, diazo, vesicular,
         mixed emulsion."""@en ;
    skos:inScheme <https://doi.org/10.6069/uwlswd.m9z2-3g03> ;
    skos:notation "z" ;
    skos:prefLabel "other"@en .

<https://doi.org/10.6069/uwlswd.m9z2-3g03> a skos:ConceptScheme ;
    dc:contributor "Metadata Management Associates"@en ;
    dc:language "en" ;
    dct:alternative """MARC21 007/10 values for microform expressed using
         RDF"""@en ;
    dct:contributor <http://viaf.org/viaf/151962300> ;
    dct:creator <http://viaf.org/viaf/139541794> ;
    dct:description "Type of light-sensitive material on the film."@en ;
    dct:format <http://www.w3.org/ns/formats/Turtle> ;
    dct:hasFormat <https://uwlib-cams.github.io/uwlswd_vocabs_marc_007/microform_emulsion_on_film/microform_emulsion_on_film.html>,
        <https://uwlib-cams.github.io/uwlswd_vocabs_marc_007/microform_emulsion_on_film/microform_emulsion_on_film.jsonld>,
        <https://uwlib-cams.github.io/uwlswd_vocabs_marc_007/microform_emulsion_on_film/microform_emulsion_on_film.nt>,
        <https://uwlib-cams.github.io/uwlswd_vocabs_marc_007/microform_emulsion_on_film/microform_emulsion_on_film.rdf> ;
    dct:issued "2024" ;
    dct:license <http://creativecommons.org/publicdomain/zero/1.0> ;
    dct:provenance <https://doi.org/10.6069/uwlswd.2e2b-y833#marc00Xvalues> ;
    dct:publisher <http://viaf.org/viaf/139541794> ;
    dct:source <http://marc21rdf.info>,
        <https://www.loc.gov/marc/bibliographic/bd007.html> ;
    dct:title "Microform: emulsion on film"@en ;
    dct:type <http://purl.org/dc/dcmitype/Dataset> ;
    schema:disambiguatingDescription """SKOS Concept Scheme for MARC 00X
         Values"""@en ;
    schema:version "1-0-0" .

