@prefix dc: <http://purl.org/dc/elements/1.1/> .
@prefix dct: <http://purl.org/dc/terms/> .
@prefix schema: <https://schema.org/> .
@prefix skos: <http://www.w3.org/2004/02/skos/core#> .

<https://doi.org/10.6069/uwlswd.4ee2-4t34#a> a skos:Concept ;
    skos:definition """Images are intended to be produced in a single color other than
         black (e.g. pink and white, brown and white)."""@en ;
    skos:inScheme <https://doi.org/10.6069/uwlswd.4ee2-4t34> ;
    skos:notation "a" ;
    skos:prefLabel "one color"@en .

<https://doi.org/10.6069/uwlswd.4ee2-4t34#b> a skos:Concept ;
    skos:definition """Images are intended to be produced in black and
         white."""@en ;
    skos:inScheme <https://doi.org/10.6069/uwlswd.4ee2-4t34> ;
    skos:notation "b" ;
    skos:prefLabel "black-and-white"@en ;
    skos:scopeNote """Includes ASCII files, which do not include
         color."""@en .

<https://doi.org/10.6069/uwlswd.4ee2-4t34#c> a skos:Concept ;
    skos:definition """Image is printed or executed in more than one
         color."""@en ;
    skos:inScheme <https://doi.org/10.6069/uwlswd.4ee2-4t34> ;
    skos:notation "c" ;
    skos:prefLabel "multicolored"@en ;
    skos:scopeNote "Used for color photographic processes."@en .

<https://doi.org/10.6069/uwlswd.4ee2-4t34#g> a skos:Concept ;
    skos:definition """Image is produced with degrees of dark to light from black to
         gray to white."""@en ;
    skos:inScheme <https://doi.org/10.6069/uwlswd.4ee2-4t34> ;
    skos:notation "g" ;
    skos:prefLabel "gray scale"@en .

<https://doi.org/10.6069/uwlswd.4ee2-4t34#h> a skos:Concept ;
    skos:inScheme <https://doi.org/10.6069/uwlswd.4ee2-4t34> ;
    skos:notation "h" ;
    skos:prefLabel "hand coloured [obsolete]"@en .

<https://doi.org/10.6069/uwlswd.4ee2-4t34#m> a skos:Concept ;
    skos:definition """A combination of one color, black-and-white, multicolored, hand
         colored, and/or other images."""@en ;
    skos:inScheme <https://doi.org/10.6069/uwlswd.4ee2-4t34> ;
    skos:notation "m" ;
    skos:prefLabel "mixed"@en .

<https://doi.org/10.6069/uwlswd.4ee2-4t34#n> a skos:Concept ;
    skos:definition """Color is not applicable to the electronic resource, usually
         because it does not involve anything visual"""@en ;
    skos:inScheme <https://doi.org/10.6069/uwlswd.4ee2-4t34> ;
    skos:notation "n" ;
    skos:prefLabel "not applicable"@en ;
    skos:scopeNote "E.g., digitally encoded audio data."@en .

<https://doi.org/10.6069/uwlswd.4ee2-4t34#u> a skos:Concept ;
    skos:definition """Color characteristics of an item are not
         known."""@en ;
    skos:inScheme <https://doi.org/10.6069/uwlswd.4ee2-4t34> ;
    skos:notation "u" ;
    skos:prefLabel "unknown"@en .

<https://doi.org/10.6069/uwlswd.4ee2-4t34#z> a skos:Concept ;
    skos:definition """Color other than one color, black-and-white, multicolored, gray
         scale, or mixed."""@en ;
    skos:inScheme <https://doi.org/10.6069/uwlswd.4ee2-4t34> ;
    skos:notation "z" ;
    skos:prefLabel "other"@en .

<https://doi.org/10.6069/uwlswd.4ee2-4t34> a skos:ConceptScheme ;
    dc:contributor "Metadata Management Associates"@en ;
    dc:language "en" ;
    dct:alternative """MARC21 007/03 values for electronic resources expressed using
         RDF"""@en ;
    dct:contributor <http://viaf.org/viaf/151962300> ;
    dct:creator <http://viaf.org/viaf/139541794> ;
    dct:description """Whether the item is one color or
         multicolored."""@en ;
    dct:format <http://www.w3.org/ns/formats/Turtle> ;
    dct:hasFormat <https://uwlib-cams.github.io/uwlswd_vocabs_marc_007/electronic_resource_color/electronic_resource_color.html>,
        <https://uwlib-cams.github.io/uwlswd_vocabs_marc_007/electronic_resource_color/electronic_resource_color.jsonld>,
        <https://uwlib-cams.github.io/uwlswd_vocabs_marc_007/electronic_resource_color/electronic_resource_color.nt>,
        <https://uwlib-cams.github.io/uwlswd_vocabs_marc_007/electronic_resource_color/electronic_resource_color.rdf> ;
    dct:issued "2024" ;
    dct:license <http://creativecommons.org/publicdomain/zero/1.0> ;
    dct:provenance <https://doi.org/10.6069/uwlswd.2e2b-y833#marc00Xvalues> ;
    dct:publisher <http://viaf.org/viaf/139541794> ;
    dct:source <http://marc21rdf.info>,
        <https://www.loc.gov/marc/bibliographic/bd007.html> ;
    dct:title "Electronic resource: color"@en ;
    dct:type <http://purl.org/dc/dcmitype/Dataset> ;
    schema:disambiguatingDescription """SKOS Concept Scheme for MARC 00X
         Values"""@en ;
    schema:version "1-0-0" .

