<?xml version='1.0' encoding='UTF-8'?>
<rdf:RDF xmlns:dc="http://purl.org/dc/elements/1.1/" xmlns:dct="http://purl.org/dc/terms/" xmlns:rdf="http://www.w3.org/1999/02/22-rdf-syntax-ns#" xmlns:schema="https://schema.org/" xmlns:skos="http://www.w3.org/2004/02/skos/core#">
  <rdf:Description rdf:about="https://doi.org/10.6069/uwlswd.gs2r-s451#u">
    <rdf:type rdf:resource="http://www.w3.org/2004/02/skos/core#Concept"/>
    <skos:inScheme rdf:resource="https://doi.org/10.6069/uwlswd.gs2r-s451"/>
    <skos:prefLabel xml:lang="en">unspecified</skos:prefLabel>
    <skos:definition xml:lang="en">Special material designation for the nonprojected graphic is
         not specified.</skos:definition>
    <skos:notation>u</skos:notation>
  </rdf:Description>
  <rdf:Description rdf:about="https://doi.org/10.6069/uwlswd.gs2r-s451">
    <rdf:type rdf:resource="http://www.w3.org/2004/02/skos/core#ConceptScheme"/>
    <dct:type rdf:resource="http://purl.org/dc/dcmitype/Dataset"/>
    <dct:title xml:lang="en">Nonprojected graphic: specific material designation</dct:title>
    <dct:alternative xml:lang="en">MARC21 007/01 values for nonprojected graphics expressed using
         RDF</dct:alternative>
    <dct:description xml:lang="en">Special class of nonprojected graphic to which the item
         belongs, (e.g., a picture).</dct:description>
    <schema:disambiguatingDescription xml:lang="en">SKOS Concept Scheme for MARC 00X
         Values</schema:disambiguatingDescription>
    <dct:publisher rdf:resource="http://viaf.org/viaf/139541794"/>
    <dct:source rdf:resource="https://www.loc.gov/marc/bibliographic/bd007.html"/>
    <dct:source rdf:resource="http://marc21rdf.info"/>
    <dct:provenance rdf:resource="https://doi.org/10.6069/uwlswd.2e2b-y833#marc00Xvalues"/>
    <dct:creator rdf:resource="http://viaf.org/viaf/139541794"/>
    <dct:contributor rdf:resource="http://viaf.org/viaf/151962300"/>
    <dct:issued>2024</dct:issued>
    <dc:contributor xml:lang="en">Metadata Management Associates</dc:contributor>
    <dc:language>en</dc:language>
    <dct:license rdf:resource="http://creativecommons.org/publicdomain/zero/1.0"/>
    <schema:version>1-0-0</schema:version>
    <dct:format rdf:resource="http://www.w3.org/ns/formats/RDF_XML"/>
  </rdf:Description>
  <rdf:Description rdf:about="https://doi.org/10.6069/uwlswd.gs2r-s451#c">
    <rdf:type rdf:resource="http://www.w3.org/2004/02/skos/core#Concept"/>
    <skos:inScheme rdf:resource="https://doi.org/10.6069/uwlswd.gs2r-s451"/>
    <skos:prefLabel xml:lang="en">collage</skos:prefLabel>
    <skos:definition xml:lang="en">Original work created by affixing various materials (paper,
         wood, newspaper, cloth, etc.) to a surface.</skos:definition>
    <skos:notation>c</skos:notation>
  </rdf:Description>
  <rdf:Description rdf:about="https://doi.org/10.6069/uwlswd.gs2r-s451#i">
    <rdf:type rdf:resource="http://www.w3.org/2004/02/skos/core#Concept"/>
    <skos:inScheme rdf:resource="https://doi.org/10.6069/uwlswd.gs2r-s451"/>
    <skos:prefLabel xml:lang="en">picture</skos:prefLabel>
    <skos:definition xml:lang="en">Two-dimensional visual representation accessible to the naked
         eye and generally on an opaque backing.</skos:definition>
    <skos:scopeNote xml:lang="en">Used when a more specific designation is unknown or not
         desired.</skos:scopeNote>
    <skos:notation>i</skos:notation>
  </rdf:Description>
  <rdf:Description rdf:about="https://doi.org/10.6069/uwlswd.gs2r-s451#s">
    <rdf:type rdf:resource="http://www.w3.org/2004/02/skos/core#Concept"/>
    <skos:inScheme rdf:resource="https://doi.org/10.6069/uwlswd.gs2r-s451"/>
    <skos:prefLabel xml:lang="en">study print</skos:prefLabel>
    <skos:definition xml:lang="en">Study print.</skos:definition>
    <skos:notation>s</skos:notation>
  </rdf:Description>
  <rdf:Description rdf:about="https://doi.org/10.6069/uwlswd.gs2r-s451#v">
    <rdf:type rdf:resource="http://www.w3.org/2004/02/skos/core#Concept"/>
    <skos:inScheme rdf:resource="https://doi.org/10.6069/uwlswd.gs2r-s451"/>
    <skos:prefLabel xml:lang="en">photograph, type unspecified</skos:prefLabel>
    <skos:definition xml:lang="en">Photograph, type unspecified.</skos:definition>
    <skos:notation>v</skos:notation>
  </rdf:Description>
  <rdf:Description rdf:about="https://doi.org/10.6069/uwlswd.gs2r-s451#g">
    <rdf:type rdf:resource="http://www.w3.org/2004/02/skos/core#Concept"/>
    <skos:inScheme rdf:resource="https://doi.org/10.6069/uwlswd.gs2r-s451"/>
    <skos:prefLabel xml:lang="en">photonegative</skos:prefLabel>
    <skos:definition xml:lang="en">Piece of film, a glass plate, or pattern on which a negative
         image appears, i.e., directly opposite to a positive image (photoprint), slide, or
         transparency, used to produce a positive print.</skos:definition>
    <skos:scopeNote xml:lang="en">Photonegatives do not include negative photoprints, photoprints
         that are a combination of negative and positive images, or photograms or solarized prints,
         all of which are considered to be techniques used when making photoprints.</skos:scopeNote>
    <skos:notation>g</skos:notation>
  </rdf:Description>
  <rdf:Description rdf:about="https://doi.org/10.6069/uwlswd.gs2r-s451#r">
    <rdf:type rdf:resource="http://www.w3.org/2004/02/skos/core#Concept"/>
    <skos:inScheme rdf:resource="https://doi.org/10.6069/uwlswd.gs2r-s451"/>
    <skos:prefLabel xml:lang="en">radiograph</skos:prefLabel>
    <skos:definition xml:lang="en">A photograph produced by the passage of radiation, such as X
         rays, gamma rays, or neutrons, through an opaque object.</skos:definition>
    <skos:notation>r</skos:notation>
  </rdf:Description>
  <rdf:Description rdf:about="https://doi.org/10.6069/uwlswd.gs2r-s451#f">
    <rdf:type rdf:resource="http://www.w3.org/2004/02/skos/core#Concept"/>
    <skos:inScheme rdf:resource="https://doi.org/10.6069/uwlswd.gs2r-s451"/>
    <skos:prefLabel xml:lang="en">photomechanical print</skos:prefLabel>
    <skos:definition xml:lang="en">Any picture produced in imitation of another picture through
         the use of photographic process to transfer the image to a printing
         surface.</skos:definition>
    <skos:scopeNote xml:lang="en">A snapshot made to document a painting or a Xerox copy of a
         print are considered photomechanical reproductions. Art reproductions are included
         here.</skos:scopeNote>
    <skos:notation>f</skos:notation>
  </rdf:Description>
  <rdf:Description rdf:about="https://doi.org/10.6069/uwlswd.gs2r-s451#p">
    <rdf:type rdf:resource="http://www.w3.org/2004/02/skos/core#Concept"/>
    <skos:inScheme rdf:resource="https://doi.org/10.6069/uwlswd.gs2r-s451"/>
    <skos:prefLabel xml:lang="en">postcard</skos:prefLabel>
    <skos:definition xml:lang="en">Postcard.</skos:definition>
    <skos:notation>p</skos:notation>
  </rdf:Description>
  <rdf:Description rdf:about="https://doi.org/10.6069/uwlswd.gs2r-s451#e">
    <rdf:type rdf:resource="http://www.w3.org/2004/02/skos/core#Concept"/>
    <skos:inScheme rdf:resource="https://doi.org/10.6069/uwlswd.gs2r-s451"/>
    <skos:prefLabel xml:lang="en">painting</skos:prefLabel>
    <skos:definition xml:lang="en">Original visual representation produced by applying paint to a
         surface.</skos:definition>
    <skos:notation>e</skos:notation>
  </rdf:Description>
  <rdf:Description rdf:about="https://doi.org/10.6069/uwlswd.gs2r-s451#o">
    <rdf:type rdf:resource="http://www.w3.org/2004/02/skos/core#Concept"/>
    <skos:inScheme rdf:resource="https://doi.org/10.6069/uwlswd.gs2r-s451"/>
    <skos:prefLabel xml:lang="en">flash card</skos:prefLabel>
    <skos:definition xml:lang="en">Card or other opaque material printed with words, numerals, or
         pictures and designed for rapid display.</skos:definition>
    <skos:notation>o</skos:notation>
  </rdf:Description>
  <rdf:Description rdf:about="https://doi.org/10.6069/uwlswd.gs2r-s451#d">
    <rdf:type rdf:resource="http://www.w3.org/2004/02/skos/core#Concept"/>
    <skos:inScheme rdf:resource="https://doi.org/10.6069/uwlswd.gs2r-s451"/>
    <skos:prefLabel xml:lang="en">drawing</skos:prefLabel>
    <skos:definition xml:lang="en">Original visual representation (other than a print or painting)
         made with pencil, pen, chalk, or other writing instrument usually on paper or similar
         nonrigid support.</skos:definition>
    <skos:notation>d</skos:notation>
  </rdf:Description>
  <rdf:Description rdf:about="https://doi.org/10.6069/uwlswd.gs2r-s451#k">
    <rdf:type rdf:resource="http://www.w3.org/2004/02/skos/core#Concept"/>
    <skos:inScheme rdf:resource="https://doi.org/10.6069/uwlswd.gs2r-s451"/>
    <skos:prefLabel xml:lang="en">poster</skos:prefLabel>
    <skos:definition xml:lang="en">Poster.</skos:definition>
    <skos:notation>k</skos:notation>
  </rdf:Description>
  <rdf:Description rdf:about="https://doi.org/10.6069/uwlswd.gs2r-s451#a">
    <rdf:type rdf:resource="http://www.w3.org/2004/02/skos/core#Concept"/>
    <skos:inScheme rdf:resource="https://doi.org/10.6069/uwlswd.gs2r-s451"/>
    <skos:prefLabel xml:lang="en">activity card</skos:prefLabel>
    <skos:definition xml:lang="en">A card printed with words, numerals, and/or pictures to be used
         by an individual or a group as a basis for performing a specific
         activity.</skos:definition>
    <skos:notation>a</skos:notation>
  </rdf:Description>
  <rdf:Description rdf:about="https://doi.org/10.6069/uwlswd.gs2r-s451#q">
    <rdf:type rdf:resource="http://www.w3.org/2004/02/skos/core#Concept"/>
    <skos:inScheme rdf:resource="https://doi.org/10.6069/uwlswd.gs2r-s451"/>
    <skos:prefLabel xml:lang="en">icon</skos:prefLabel>
    <skos:definition xml:lang="en">Icon.</skos:definition>
    <skos:notation>q</skos:notation>
  </rdf:Description>
  <rdf:Description rdf:about="https://doi.org/10.6069/uwlswd.gs2r-s451#h">
    <rdf:type rdf:resource="http://www.w3.org/2004/02/skos/core#Concept"/>
    <skos:inScheme rdf:resource="https://doi.org/10.6069/uwlswd.gs2r-s451"/>
    <skos:prefLabel xml:lang="en">photoprint</skos:prefLabel>
    <skos:definition xml:lang="en">Photoprints have a positive image made either directly or
         indirectly on a sensitized surface by the action of light or other radiant energy. The term
         photoprint rather than photograph is used here as a more precise term than photograph,
         which technically can cover both the print and the negative.</skos:definition>
    <skos:scopeNote xml:lang="en">Opaque stereographs are included here.</skos:scopeNote>
    <skos:notation>h</skos:notation>
  </rdf:Description>
  <rdf:Description rdf:about="https://doi.org/10.6069/uwlswd.gs2r-s451#l">
    <rdf:type rdf:resource="http://www.w3.org/2004/02/skos/core#Concept"/>
    <skos:inScheme rdf:resource="https://doi.org/10.6069/uwlswd.gs2r-s451"/>
    <skos:prefLabel xml:lang="en">technical drawing</skos:prefLabel>
    <skos:definition xml:lang="en">Cross section, detail, diagram, elevation, perspective, plan,
         working plan, etc., made for use in an engineering or other technical
         context.</skos:definition>
    <skos:notation>l</skos:notation>
  </rdf:Description>
  <rdf:Description rdf:about="https://doi.org/10.6069/uwlswd.gs2r-s451#z">
    <rdf:type rdf:resource="http://www.w3.org/2004/02/skos/core#Concept"/>
    <skos:inScheme rdf:resource="https://doi.org/10.6069/uwlswd.gs2r-s451"/>
    <skos:prefLabel xml:lang="en">other</skos:prefLabel>
    <skos:definition xml:lang="en">Specific material designation other than activity card,
         collage, drawing, painting, photomechanical print, photonegative, photoprint, picture,
         print, poster, technical drawing, chart, flash card, postcard, icon, radiograph, study
         print, or photograph type unspecified.</skos:definition>
    <skos:notation>z</skos:notation>
  </rdf:Description>
  <rdf:Description rdf:about="https://doi.org/10.6069/uwlswd.gs2r-s451#n">
    <rdf:type rdf:resource="http://www.w3.org/2004/02/skos/core#Concept"/>
    <skos:inScheme rdf:resource="https://doi.org/10.6069/uwlswd.gs2r-s451"/>
    <skos:prefLabel xml:lang="en">chart</skos:prefLabel>
    <skos:definition xml:lang="en">Opaque sheet that exhibits data in graphic or tabular
         form.</skos:definition>
    <skos:scopeNote xml:lang="en">E.g., a wall chart.</skos:scopeNote>
    <skos:notation>n</skos:notation>
  </rdf:Description>
  <rdf:Description rdf:about="https://doi.org/10.6069/uwlswd.gs2r-s451#j">
    <rdf:type rdf:resource="http://www.w3.org/2004/02/skos/core#Concept"/>
    <skos:inScheme rdf:resource="https://doi.org/10.6069/uwlswd.gs2r-s451"/>
    <skos:prefLabel xml:lang="en">print</skos:prefLabel>
    <skos:definition xml:lang="en">Design or picture transferred from an engraved plate, wood
         block, lithographic stone, or other medium. Generally there are four types: planographic
         print, relief print, intaglio print, and stencil print.</skos:definition>
    <skos:notation>j</skos:notation>
  </rdf:Description>
</rdf:RDF>