@prefix dc: <http://purl.org/dc/elements/1.1/> .
@prefix dct: <http://purl.org/dc/terms/> .
@prefix schema: <https://schema.org/> .
@prefix skos: <http://www.w3.org/2004/02/skos/core#> .

<https://doi.org/10.6069/uwlswd.gs2r-s451#a> a skos:Concept ;
    skos:definition """A card printed with words, numerals, and/or pictures to be used
         by an individual or a group as a basis for performing a specific
         activity."""@en ;
    skos:inScheme <https://doi.org/10.6069/uwlswd.gs2r-s451> ;
    skos:notation "a" ;
    skos:prefLabel "activity card"@en .

<https://doi.org/10.6069/uwlswd.gs2r-s451#c> a skos:Concept ;
    skos:definition """Original work created by affixing various materials (paper,
         wood, newspaper, cloth, etc.) to a surface."""@en ;
    skos:inScheme <https://doi.org/10.6069/uwlswd.gs2r-s451> ;
    skos:notation "c" ;
    skos:prefLabel "collage"@en .

<https://doi.org/10.6069/uwlswd.gs2r-s451#d> a skos:Concept ;
    skos:definition """Original visual representation (other than a print or painting)
         made with pencil, pen, chalk, or other writing instrument usually on paper or similar
         nonrigid support."""@en ;
    skos:inScheme <https://doi.org/10.6069/uwlswd.gs2r-s451> ;
    skos:notation "d" ;
    skos:prefLabel "drawing"@en .

<https://doi.org/10.6069/uwlswd.gs2r-s451#e> a skos:Concept ;
    skos:definition """Original visual representation produced by applying paint to a
         surface."""@en ;
    skos:inScheme <https://doi.org/10.6069/uwlswd.gs2r-s451> ;
    skos:notation "e" ;
    skos:prefLabel "painting"@en .

<https://doi.org/10.6069/uwlswd.gs2r-s451#f> a skos:Concept ;
    skos:definition """Any picture produced in imitation of another picture through
         the use of photographic process to transfer the image to a printing
         surface."""@en ;
    skos:inScheme <https://doi.org/10.6069/uwlswd.gs2r-s451> ;
    skos:notation "f" ;
    skos:prefLabel "photomechanical print"@en ;
    skos:scopeNote """A snapshot made to document a painting or a Xerox copy of a
         print are considered photomechanical reproductions. Art reproductions are included
         here."""@en .

<https://doi.org/10.6069/uwlswd.gs2r-s451#g> a skos:Concept ;
    skos:definition """Piece of film, a glass plate, or pattern on which a negative
         image appears, i.e., directly opposite to a positive image (photoprint), slide, or
         transparency, used to produce a positive print."""@en ;
    skos:inScheme <https://doi.org/10.6069/uwlswd.gs2r-s451> ;
    skos:notation "g" ;
    skos:prefLabel "photonegative"@en ;
    skos:scopeNote """Photonegatives do not include negative photoprints, photoprints
         that are a combination of negative and positive images, or photograms or solarized prints,
         all of which are considered to be techniques used when making photoprints."""@en .

<https://doi.org/10.6069/uwlswd.gs2r-s451#h> a skos:Concept ;
    skos:definition """Photoprints have a positive image made either directly or
         indirectly on a sensitized surface by the action of light or other radiant energy. The term
         photoprint rather than photograph is used here as a more precise term than photograph,
         which technically can cover both the print and the negative."""@en ;
    skos:inScheme <https://doi.org/10.6069/uwlswd.gs2r-s451> ;
    skos:notation "h" ;
    skos:prefLabel "photoprint"@en ;
    skos:scopeNote "Opaque stereographs are included here."@en .

<https://doi.org/10.6069/uwlswd.gs2r-s451#i> a skos:Concept ;
    skos:definition """Two-dimensional visual representation accessible to the naked
         eye and generally on an opaque backing."""@en ;
    skos:inScheme <https://doi.org/10.6069/uwlswd.gs2r-s451> ;
    skos:notation "i" ;
    skos:prefLabel "picture"@en ;
    skos:scopeNote """Used when a more specific designation is unknown or not
         desired."""@en .

<https://doi.org/10.6069/uwlswd.gs2r-s451#j> a skos:Concept ;
    skos:definition """Design or picture transferred from an engraved plate, wood
         block, lithographic stone, or other medium. Generally there are four types: planographic
         print, relief print, intaglio print, and stencil print."""@en ;
    skos:inScheme <https://doi.org/10.6069/uwlswd.gs2r-s451> ;
    skos:notation "j" ;
    skos:prefLabel "print"@en .

<https://doi.org/10.6069/uwlswd.gs2r-s451#k> a skos:Concept ;
    skos:definition "Poster."@en ;
    skos:inScheme <https://doi.org/10.6069/uwlswd.gs2r-s451> ;
    skos:notation "k" ;
    skos:prefLabel "poster"@en .

<https://doi.org/10.6069/uwlswd.gs2r-s451#l> a skos:Concept ;
    skos:definition """Cross section, detail, diagram, elevation, perspective, plan,
         working plan, etc., made for use in an engineering or other technical
         context."""@en ;
    skos:inScheme <https://doi.org/10.6069/uwlswd.gs2r-s451> ;
    skos:notation "l" ;
    skos:prefLabel "technical drawing"@en .

<https://doi.org/10.6069/uwlswd.gs2r-s451#n> a skos:Concept ;
    skos:definition """Opaque sheet that exhibits data in graphic or tabular
         form."""@en ;
    skos:inScheme <https://doi.org/10.6069/uwlswd.gs2r-s451> ;
    skos:notation "n" ;
    skos:prefLabel "chart"@en ;
    skos:scopeNote "E.g., a wall chart."@en .

<https://doi.org/10.6069/uwlswd.gs2r-s451#o> a skos:Concept ;
    skos:definition """Card or other opaque material printed with words, numerals, or
         pictures and designed for rapid display."""@en ;
    skos:inScheme <https://doi.org/10.6069/uwlswd.gs2r-s451> ;
    skos:notation "o" ;
    skos:prefLabel "flash card"@en .

<https://doi.org/10.6069/uwlswd.gs2r-s451#p> a skos:Concept ;
    skos:definition "Postcard."@en ;
    skos:inScheme <https://doi.org/10.6069/uwlswd.gs2r-s451> ;
    skos:notation "p" ;
    skos:prefLabel "postcard"@en .

<https://doi.org/10.6069/uwlswd.gs2r-s451#q> a skos:Concept ;
    skos:definition "Icon."@en ;
    skos:inScheme <https://doi.org/10.6069/uwlswd.gs2r-s451> ;
    skos:notation "q" ;
    skos:prefLabel "icon"@en .

<https://doi.org/10.6069/uwlswd.gs2r-s451#r> a skos:Concept ;
    skos:definition """A photograph produced by the passage of radiation, such as X
         rays, gamma rays, or neutrons, through an opaque object."""@en ;
    skos:inScheme <https://doi.org/10.6069/uwlswd.gs2r-s451> ;
    skos:notation "r" ;
    skos:prefLabel "radiograph"@en .

<https://doi.org/10.6069/uwlswd.gs2r-s451#s> a skos:Concept ;
    skos:definition "Study print."@en ;
    skos:inScheme <https://doi.org/10.6069/uwlswd.gs2r-s451> ;
    skos:notation "s" ;
    skos:prefLabel "study print"@en .

<https://doi.org/10.6069/uwlswd.gs2r-s451#u> a skos:Concept ;
    skos:definition """Special material designation for the nonprojected graphic is
         not specified."""@en ;
    skos:inScheme <https://doi.org/10.6069/uwlswd.gs2r-s451> ;
    skos:notation "u" ;
    skos:prefLabel "unspecified"@en .

<https://doi.org/10.6069/uwlswd.gs2r-s451#v> a skos:Concept ;
    skos:definition "Photograph, type unspecified."@en ;
    skos:inScheme <https://doi.org/10.6069/uwlswd.gs2r-s451> ;
    skos:notation "v" ;
    skos:prefLabel "photograph, type unspecified"@en .

<https://doi.org/10.6069/uwlswd.gs2r-s451#z> a skos:Concept ;
    skos:definition """Specific material designation other than activity card,
         collage, drawing, painting, photomechanical print, photonegative, photoprint, picture,
         print, poster, technical drawing, chart, flash card, postcard, icon, radiograph, study
         print, or photograph type unspecified."""@en ;
    skos:inScheme <https://doi.org/10.6069/uwlswd.gs2r-s451> ;
    skos:notation "z" ;
    skos:prefLabel "other"@en .

<https://doi.org/10.6069/uwlswd.gs2r-s451> a skos:ConceptScheme ;
    dc:contributor "Metadata Management Associates"@en ;
    dc:language "en" ;
    dct:alternative """MARC21 007/01 values for nonprojected graphics expressed using
         RDF"""@en ;
    dct:contributor <http://viaf.org/viaf/151962300> ;
    dct:creator <http://viaf.org/viaf/139541794> ;
    dct:description """Special class of nonprojected graphic to which the item
         belongs, (e.g., a picture)."""@en ;
    dct:format <http://www.w3.org/ns/formats/Turtle> ;
    dct:hasFormat <https://uwlib-cams.github.io/uwlswd_vocabs_marc_007/nonprojected_graphic_specific_material_designation/nonprojected_graphic_specific_material_designation.html>,
        <https://uwlib-cams.github.io/uwlswd_vocabs_marc_007/nonprojected_graphic_specific_material_designation/nonprojected_graphic_specific_material_designation.jsonld>,
        <https://uwlib-cams.github.io/uwlswd_vocabs_marc_007/nonprojected_graphic_specific_material_designation/nonprojected_graphic_specific_material_designation.nt>,
        <https://uwlib-cams.github.io/uwlswd_vocabs_marc_007/nonprojected_graphic_specific_material_designation/nonprojected_graphic_specific_material_designation.rdf> ;
    dct:issued "2024" ;
    dct:license <http://creativecommons.org/publicdomain/zero/1.0> ;
    dct:provenance <https://doi.org/10.6069/uwlswd.2e2b-y833#marc00Xvalues> ;
    dct:publisher <http://viaf.org/viaf/139541794> ;
    dct:source <http://marc21rdf.info>,
        <https://www.loc.gov/marc/bibliographic/bd007.html> ;
    dct:title "Nonprojected graphic: specific material designation"@en ;
    dct:type <http://purl.org/dc/dcmitype/Dataset> ;
    schema:disambiguatingDescription """SKOS Concept Scheme for MARC 00X
         Values"""@en ;
    schema:version "1-0-0" .

