@prefix dc: <http://purl.org/dc/elements/1.1/> .
@prefix dct: <http://purl.org/dc/terms/> .
@prefix schema: <https://schema.org/> .
@prefix skos: <http://www.w3.org/2004/02/skos/core#> .

<https://doi.org/10.6069/uwlswd.c9fa-t776#a> a skos:Concept ;
    skos:definition """Image is printed or executed in a single color (i.e.,
         monochromatic)."""@en ;
    skos:inScheme <https://doi.org/10.6069/uwlswd.c9fa-t776> ;
    skos:notation "a" ;
    skos:prefLabel "one color"@en ;
    skos:scopeNote """Used only for transparency sets. Does not include
         black."""@en .

<https://doi.org/10.6069/uwlswd.c9fa-t776#b> a skos:Concept ;
    skos:definition """Image is printed or executed in black-and-white. Refers to
         monochrome photographic materials (including film) and videorecordings, or to overhead
         transparencies executed in black-and-white."""@en ;
    skos:inScheme <https://doi.org/10.6069/uwlswd.c9fa-t776> ;
    skos:notation "b" ;
    skos:prefLabel "black-and-white"@en ;
    skos:scopeNote """Does not include tinted, toned, or stained
         items."""@en .

<https://doi.org/10.6069/uwlswd.c9fa-t776#c> a skos:Concept ;
    skos:definition """Image is printed or executed in more than one color. The color
         is a result of a number of processes, either photographic or electronic, capable of
         reproducing a reasonable range of hues, or of original application of color materials, for
         example, paint."""@en ;
    skos:inScheme <https://doi.org/10.6069/uwlswd.c9fa-t776> ;
    skos:notation "c" ;
    skos:prefLabel "multicolored"@en ;
    skos:scopeNote """Used for color photographic processes (motion pictures,
         filmstrips, transparencies, and slides), color videorecordings, or multicolored overhead
         transparencies."""@en .

<https://doi.org/10.6069/uwlswd.c9fa-t776#h> a skos:Concept ;
    skos:definition """Image, produced by a printing or photographic process, is hand
         colored."""@en ;
    skos:inScheme <https://doi.org/10.6069/uwlswd.c9fa-t776> ;
    skos:notation "h" ;
    skos:prefLabel "hand colored"@en ;
    skos:scopeNote """Rarely used with commercial audiovisual materials since these
         are not typically issued with hand coloring."""@en .

<https://doi.org/10.6069/uwlswd.c9fa-t776#m> a skos:Concept ;
    skos:definition """A combination of one color, black and white, colored, hand
         colored, and/or other images."""@en ;
    skos:inScheme <https://doi.org/10.6069/uwlswd.c9fa-t776> ;
    skos:notation "m" ;
    skos:prefLabel "mixed"@en .

<https://doi.org/10.6069/uwlswd.c9fa-t776#n> a skos:Concept ;
    skos:definition "Item has no images."@en ;
    skos:inScheme <https://doi.org/10.6069/uwlswd.c9fa-t776> ;
    skos:notation "n" ;
    skos:prefLabel "not applicable"@en ;
    skos:scopeNote """For example, when the item in hand is sound track film intended
         to accompany visual images not actually present."""@en .

<https://doi.org/10.6069/uwlswd.c9fa-t776#u> a skos:Concept ;
    skos:definition """Color characteristics of the projected graphic are not
         known."""@en ;
    skos:inScheme <https://doi.org/10.6069/uwlswd.c9fa-t776> ;
    skos:notation "u" ;
    skos:prefLabel "unknown"@en .

<https://doi.org/10.6069/uwlswd.c9fa-t776#z> a skos:Concept ;
    skos:definition """Color other than one color, black-and-white, multicolored, hand
         colored, or, mixed."""@en ;
    skos:inScheme <https://doi.org/10.6069/uwlswd.c9fa-t776> ;
    skos:notation "z" ;
    skos:prefLabel "other"@en .

<https://doi.org/10.6069/uwlswd.c9fa-t776> a skos:ConceptScheme ;
    dc:contributor "Metadata Management Associates"@en ;
    dc:language "en" ;
    dct:alternative """MARC21 007/03 values for projected graphics expressed using
         RDF"""@en ;
    dct:contributor <http://viaf.org/viaf/151962300> ;
    dct:creator <http://viaf.org/viaf/139541794> ;
    dct:description "Color characteristics of a projected graphic."@en ;
    dct:format <http://www.w3.org/ns/formats/Turtle> ;
    dct:hasFormat <https://uwlib-cams.github.io/uwlswd_vocabs_marc_007/projected_graphic_color/projected_graphic_color.html>,
        <https://uwlib-cams.github.io/uwlswd_vocabs_marc_007/projected_graphic_color/projected_graphic_color.jsonld>,
        <https://uwlib-cams.github.io/uwlswd_vocabs_marc_007/projected_graphic_color/projected_graphic_color.nt>,
        <https://uwlib-cams.github.io/uwlswd_vocabs_marc_007/projected_graphic_color/projected_graphic_color.rdf> ;
    dct:issued "2024" ;
    dct:license <http://creativecommons.org/publicdomain/zero/1.0> ;
    dct:provenance <https://doi.org/10.6069/uwlswd.2e2b-y833#marc00Xvalues> ;
    dct:publisher <http://viaf.org/viaf/139541794> ;
    dct:source <http://marc21rdf.info>,
        <https://www.loc.gov/marc/bibliographic/bd007.html> ;
    dct:title "Projected graphic: color"@en ;
    dct:type <http://purl.org/dc/dcmitype/Dataset> ;
    schema:disambiguatingDescription """SKOS Concept Scheme for MARC 00X
         Values"""@en ;
    schema:version "1-0-0" .

