<?xml version="1.0" encoding="utf-8"?>
<rdf:RDF
   xmlns:dc="http://purl.org/dc/elements/1.1/"
   xmlns:dct="http://purl.org/dc/terms/"
   xmlns:rdf="http://www.w3.org/1999/02/22-rdf-syntax-ns#"
   xmlns:schema="https://schema.org/"
   xmlns:skos="http://www.w3.org/2004/02/skos/core#"
>
  <rdf:Description rdf:about="http://fakeIRI.edu/terms/projectedcol#c">
    <rdf:type rdf:resource="http://www.w3.org/2004/02/skos/core#Concept"/>
    <skos:inScheme rdf:resource="http://fakeIRI.edu/terms/projectedcol"/>
    <skos:prefLabel xml:lang="en">multicolored</skos:prefLabel>
    <skos:definition xml:lang="en">Image is printed or executed in more than one color. The color
         is a result of a number of processes, either photographic or electronic, capable of
         reproducing a reasonable range of hues, or of original application of color materials, for
         example, paint.</skos:definition>
    <skos:scopeNote xml:lang="en">Used for color photographic processes (motion pictures,
         filmstrips, transparencies, and slides), color videorecordings, or multicolored overhead
         transparencies.</skos:scopeNote>
    <skos:notation xml:lang="en">c</skos:notation>
  </rdf:Description>
  <rdf:Description rdf:about="http://fakeIRI.edu/terms/projectedcol#n">
    <rdf:type rdf:resource="http://www.w3.org/2004/02/skos/core#Concept"/>
    <skos:inScheme rdf:resource="http://fakeIRI.edu/terms/projectedcol"/>
    <skos:prefLabel xml:lang="en">not applicable</skos:prefLabel>
    <skos:definition xml:lang="en">Item has no images.</skos:definition>
    <skos:scopeNote xml:lang="en">For example, when the item in hand is sound track film intended
         to accompany visual images not actually present.</skos:scopeNote>
    <skos:notation xml:lang="en">n</skos:notation>
  </rdf:Description>
  <rdf:Description rdf:about="http://fakeIRI.edu/terms/projectedcol">
    <rdf:type rdf:resource="http://www.w3.org/2004/02/skos/core#ConceptScheme"/>
    <dct:type rdf:resource="http://purl.org/dc/dcmitype/Dataset"/>
    <dct:title xml:lang="en">Projected graphic: color</dct:title>
    <dct:alternative xml:lang="en">MARC21 007/03 values for projected graphics expressed using
         RDF</dct:alternative>
    <dct:description xml:lang="en">Color characteristics of a projected graphic.</dct:description>
    <schema:disambiguatingDescription>SKOS Concept Scheme for MARC 00X
         Values</schema:disambiguatingDescription>
    <dct:publisher rdf:resource="http://viaf.org/viaf/139541794"/>
    <dct:source rdf:resource="https://www.loc.gov/marc/bibliographic/bd007.html"/>
    <dct:source rdf:resource="http://marc21rdf.info"/>
    <dct:provenance rdf:resource="https://doi.org/10.6069/uwlswd.2e2b-y833"/>
    <dct:creator rdf:resource="http://viaf.org/viaf/139541794"/>
    <dct:contributor rdf:resource="http://viaf.org/viaf/151962300"/>
    <dct:issued>2024</dct:issued>
    <dc:contributor xml:lang="en">Metadata Management Associates</dc:contributor>
    <dc:language>en</dc:language>
    <dct:license rdf:resource="http://creativecommons.org/publicdomain/zero/1.0"/>
    <schema:version>1-0-0</schema:version>
    <dct:format rdf:resource="http://www.w3.org/ns/formats/RDF_XML"/>
  </rdf:Description>
  <rdf:Description rdf:about="http://fakeIRI.edu/terms/projectedcol#a">
    <rdf:type rdf:resource="http://www.w3.org/2004/02/skos/core#Concept"/>
    <skos:inScheme rdf:resource="http://fakeIRI.edu/terms/projectedcol"/>
    <skos:prefLabel xml:lang="en">one color</skos:prefLabel>
    <skos:definition xml:lang="en">Image is printed or executed in a single color (i.e.,
         monochromatic).</skos:definition>
    <skos:scopeNote xml:lang="en">Used only for transparency sets. Does not include
         black.</skos:scopeNote>
    <skos:notation xml:lang="en">a</skos:notation>
  </rdf:Description>
  <rdf:Description rdf:about="http://fakeIRI.edu/terms/projectedcol#b">
    <rdf:type rdf:resource="http://www.w3.org/2004/02/skos/core#Concept"/>
    <skos:inScheme rdf:resource="http://fakeIRI.edu/terms/projectedcol"/>
    <skos:prefLabel xml:lang="en">black-and-white</skos:prefLabel>
    <skos:definition xml:lang="en">Image is printed or executed in black-and-white. Refers to
         monochrome photographic materials (including film) and videorecordings, or to overhead
         transparencies executed in black-and-white.</skos:definition>
    <skos:scopeNote xml:lang="en">Does not include tinted, toned, or stained
         items.</skos:scopeNote>
    <skos:notation xml:lang="en">b</skos:notation>
  </rdf:Description>
  <rdf:Description rdf:about="http://fakeIRI.edu/terms/projectedcol#u">
    <rdf:type rdf:resource="http://www.w3.org/2004/02/skos/core#Concept"/>
    <skos:inScheme rdf:resource="http://fakeIRI.edu/terms/projectedcol"/>
    <skos:prefLabel xml:lang="en">unknown</skos:prefLabel>
    <skos:definition xml:lang="en">Color characteristics of the projected graphic are not
         known.</skos:definition>
    <skos:notation xml:lang="en">u</skos:notation>
  </rdf:Description>
  <rdf:Description rdf:about="http://fakeIRI.edu/terms/projectedcol#h">
    <rdf:type rdf:resource="http://www.w3.org/2004/02/skos/core#Concept"/>
    <skos:inScheme rdf:resource="http://fakeIRI.edu/terms/projectedcol"/>
    <skos:prefLabel xml:lang="en">hand colored</skos:prefLabel>
    <skos:definition xml:lang="en">Image, produced by a printing or photographic process, is hand
         colored.</skos:definition>
    <skos:scopeNote xml:lang="en">Rarely used with commercial audiovisual materials since these
         are not typically issued with hand coloring.</skos:scopeNote>
    <skos:notation xml:lang="en">h</skos:notation>
  </rdf:Description>
  <rdf:Description rdf:about="http://fakeIRI.edu/terms/projectedcol#m">
    <rdf:type rdf:resource="http://www.w3.org/2004/02/skos/core#Concept"/>
    <skos:inScheme rdf:resource="http://fakeIRI.edu/terms/projectedcol"/>
    <skos:prefLabel xml:lang="en">mixed</skos:prefLabel>
    <skos:definition xml:lang="en">A combination of one color, black and white, colored, hand
         colored, and/or other images.</skos:definition>
    <skos:notation xml:lang="en">m</skos:notation>
  </rdf:Description>
  <rdf:Description rdf:about="http://fakeIRI.edu/terms/projectedcol#z">
    <rdf:type rdf:resource="http://www.w3.org/2004/02/skos/core#Concept"/>
    <skos:inScheme rdf:resource="http://fakeIRI.edu/terms/projectedcol"/>
    <skos:prefLabel xml:lang="en">other</skos:prefLabel>
    <skos:definition xml:lang="en">Color other than one color, black-and-white, multicolored, hand
         colored, or, mixed.</skos:definition>
    <skos:notation xml:lang="en">z</skos:notation>
  </rdf:Description>
</rdf:RDF>
