<?xml version="1.0" encoding="utf-8"?>
<rdf:RDF
   xmlns:dc="http://purl.org/dc/elements/1.1/"
   xmlns:dct="http://purl.org/dc/terms/"
   xmlns:rdf="http://www.w3.org/1999/02/22-rdf-syntax-ns#"
   xmlns:schema="https://schema.org/"
   xmlns:skos="http://www.w3.org/2004/02/skos/core#"
>
  <rdf:Description rdf:about="http://fakeIRI.edu/terms/videosom">
    <rdf:type rdf:resource="http://www.w3.org/2004/02/skos/core#ConceptScheme"/>
    <dct:type rdf:resource="http://purl.org/dc/dcmitype/Dataset"/>
    <dct:title xml:lang="en">Videorecording: sound on medium or separate</dct:title>
    <dct:alternative xml:lang="en">MARC21 007/05 values for videorecordings expressed using
         RDF</dct:alternative>
    <dct:description xml:lang="en">Whether the sound is on the item or separate from the item
         (i.e., on the accompanying material).</dct:description>
    <schema:disambiguatingDescription>SKOS Concept Scheme for MARC 00X
         Values</schema:disambiguatingDescription>
    <dct:publisher rdf:resource="http://viaf.org/viaf/139541794"/>
    <dct:source rdf:resource="https://www.loc.gov/marc/bibliographic/bd007.html"/>
    <dct:source rdf:resource="http://marc21rdf.info"/>
    <dct:provenance rdf:resource="https://doi.org/10.6069/uwlswd.2e2b-y833"/>
    <dct:creator rdf:resource="http://viaf.org/viaf/139541794"/>
    <dct:contributor rdf:resource="http://viaf.org/viaf/151962300"/>
    <dct:issued>2024</dct:issued>
    <dc:contributor xml:lang="en">Metadata Management Associates</dc:contributor>
    <dc:language>en</dc:language>
    <dct:license rdf:resource="http://creativecommons.org/publicdomain/zero/1.0"/>
    <schema:version>1-0-0</schema:version>
    <dct:format rdf:resource="http://www.w3.org/ns/formats/RDF_XML"/>
  </rdf:Description>
  <rdf:Description rdf:about="http://fakeIRI.edu/terms/videosom#b">
    <rdf:type rdf:resource="http://www.w3.org/2004/02/skos/core#Concept"/>
    <skos:inScheme rdf:resource="http://fakeIRI.edu/terms/videosom"/>
    <skos:prefLabel xml:lang="en">sound separate from medium</skos:prefLabel>
    <skos:definition xml:lang="en">Sound is on a separate medium, designed to accompany the
         images.</skos:definition>
    <skos:notation xml:lang="en">b</skos:notation>
  </rdf:Description>
  <rdf:Description rdf:about="http://fakeIRI.edu/terms/videosom#pound">
    <rdf:type rdf:resource="http://www.w3.org/2004/02/skos/core#Concept"/>
    <skos:inScheme rdf:resource="http://fakeIRI.edu/terms/videosom"/>
    <skos:prefLabel xml:lang="en">no sound (silent)</skos:prefLabel>
    <skos:definition xml:lang="en">Sound is not present (i.e., the item is intended to be
         silent).</skos:definition>
    <skos:notation xml:lang="en">#</skos:notation>
  </rdf:Description>
  <rdf:Description rdf:about="http://fakeIRI.edu/terms/videosom#a">
    <rdf:type rdf:resource="http://www.w3.org/2004/02/skos/core#Concept"/>
    <skos:inScheme rdf:resource="http://fakeIRI.edu/terms/videosom"/>
    <skos:prefLabel xml:lang="en">sound on medium</skos:prefLabel>
    <skos:definition xml:lang="en">Sound is on the item, whether or not visual images are
         included.</skos:definition>
    <skos:notation xml:lang="en">a</skos:notation>
  </rdf:Description>
  <rdf:Description rdf:about="http://fakeIRI.edu/terms/videosom#u">
    <rdf:type rdf:resource="http://www.w3.org/2004/02/skos/core#Concept"/>
    <skos:inScheme rdf:resource="http://fakeIRI.edu/terms/videosom"/>
    <skos:prefLabel xml:lang="en">unknown</skos:prefLabel>
    <skos:definition xml:lang="en">Presence or absence of sound on the item is not
         known.</skos:definition>
    <skos:notation xml:lang="en">u</skos:notation>
  </rdf:Description>
</rdf:RDF>
