<?xml version="1.0" encoding="utf-8"?>
<rdf:RDF
   xmlns:dc="http://purl.org/dc/elements/1.1/"
   xmlns:dct="http://purl.org/dc/terms/"
   xmlns:rdf="http://www.w3.org/1999/02/22-rdf-syntax-ns#"
   xmlns:schema="https://schema.org/"
   xmlns:skos="http://www.w3.org/2004/02/skos/core#"
>
  <rdf:Description rdf:about="https://doi.org/10.6069/uwlswd.kdz3-qx35#u">
    <rdf:type rdf:resource="http://www.w3.org/2004/02/skos/core#Concept"/>
    <skos:inScheme rdf:resource="https://doi.org/10.6069/uwlswd.kdz3-qx35"/>
    <skos:prefLabel xml:lang="en">unspecified</skos:prefLabel>
    <skos:definition xml:lang="en">The specific material designation for the projected graphic is
         unspecified.</skos:definition>
    <skos:notation xml:lang="en">u</skos:notation>
  </rdf:Description>
  <rdf:Description rdf:about="https://doi.org/10.6069/uwlswd.kdz3-qx35">
    <rdf:type rdf:resource="http://www.w3.org/2004/02/skos/core#ConceptScheme"/>
    <dct:type rdf:resource="http://purl.org/dc/dcmitype/Dataset"/>
    <dct:title xml:lang="en">Projected graphic: specific material designation</dct:title>
    <dct:alternative xml:lang="en">MARC21 007/01 values for projected graphics expressed using
         RDF</dct:alternative>
    <dct:description xml:lang="en">Special class of projected graphic to which the item belongs,
         e.g., a slide.</dct:description>
    <schema:disambiguatingDescription>SKOS Concept Scheme for MARC 00X
         Values</schema:disambiguatingDescription>
    <dct:publisher rdf:resource="http://viaf.org/viaf/139541794"/>
    <dct:source rdf:resource="https://www.loc.gov/marc/bibliographic/bd007.html"/>
    <dct:source rdf:resource="http://marc21rdf.info"/>
    <dct:provenance rdf:resource="https://doi.org/10.6069/uwlswd.2e2b-y833"/>
    <dct:creator rdf:resource="http://viaf.org/viaf/139541794"/>
    <dct:contributor rdf:resource="http://viaf.org/viaf/151962300"/>
    <dct:issued>2024</dct:issued>
    <dc:contributor xml:lang="en">Metadata Management Associates</dc:contributor>
    <dc:language>en</dc:language>
    <dct:license rdf:resource="http://creativecommons.org/publicdomain/zero/1.0"/>
    <schema:version>1-0-0</schema:version>
    <dct:format rdf:resource="http://www.w3.org/ns/formats/RDF_XML"/>
  </rdf:Description>
  <rdf:Description rdf:about="https://doi.org/10.6069/uwlswd.kdz3-qx35#o">
    <rdf:type rdf:resource="http://www.w3.org/2004/02/skos/core#Concept"/>
    <skos:inScheme rdf:resource="https://doi.org/10.6069/uwlswd.kdz3-qx35"/>
    <skos:prefLabel xml:lang="en">filmstrip roll</skos:prefLabel>
    <skos:definition xml:lang="en">A roll of film on which still images are recorded, presenting
         an integrated communication. It is intended for projection frame by
         frame.</skos:definition>
    <skos:notation xml:lang="en">o</skos:notation>
  </rdf:Description>
  <rdf:Description rdf:about="https://doi.org/10.6069/uwlswd.kdz3-qx35#s">
    <rdf:type rdf:resource="http://www.w3.org/2004/02/skos/core#Concept"/>
    <skos:inScheme rdf:resource="https://doi.org/10.6069/uwlswd.kdz3-qx35"/>
    <skos:prefLabel xml:lang="en">slide</skos:prefLabel>
    <skos:definition xml:lang="en">Transparent material on which there is a two-dimensional image,
         usually held in a mount, and designed for use in a projector or viewer.</skos:definition>
    <skos:scopeNote xml:lang="en">Includes modern stereographs, e.g., Viewmaster
         reels.</skos:scopeNote>
    <skos:notation xml:lang="en">s</skos:notation>
  </rdf:Description>
  <rdf:Description rdf:about="https://doi.org/10.6069/uwlswd.kdz3-qx35#z">
    <rdf:type rdf:resource="http://www.w3.org/2004/02/skos/core#Concept"/>
    <skos:inScheme rdf:resource="https://doi.org/10.6069/uwlswd.kdz3-qx35"/>
    <skos:prefLabel xml:lang="en">other</skos:prefLabel>
    <skos:definition xml:lang="en">Specific material designation other than filmstrip cartridge,
         filmslip, other filmstrip type, filmstrip roll, slide, or transparency.</skos:definition>
    <skos:notation xml:lang="en">z</skos:notation>
  </rdf:Description>
  <rdf:Description rdf:about="https://doi.org/10.6069/uwlswd.kdz3-qx35#t">
    <rdf:type rdf:resource="http://www.w3.org/2004/02/skos/core#Concept"/>
    <skos:inScheme rdf:resource="https://doi.org/10.6069/uwlswd.kdz3-qx35"/>
    <skos:prefLabel xml:lang="en">transparency</skos:prefLabel>
    <skos:definition xml:lang="en">Transparent material on which an image is recorded. They are
         designed for use with a projector or a light box.</skos:definition>
    <skos:scopeNote xml:lang="en">Includes X-rays.</skos:scopeNote>
    <skos:notation xml:lang="en">t</skos:notation>
  </rdf:Description>
  <rdf:Description rdf:about="https://doi.org/10.6069/uwlswd.kdz3-qx35#pound">
    <rdf:type rdf:resource="http://www.w3.org/2004/02/skos/core#Concept"/>
    <skos:inScheme rdf:resource="https://doi.org/10.6069/uwlswd.kdz3-qx35"/>
    <skos:prefLabel xml:lang="en">not applicable or no attempt to code [obsolete]</skos:prefLabel>
    <skos:notation xml:lang="en">#</skos:notation>
  </rdf:Description>
  <rdf:Description rdf:about="https://doi.org/10.6069/uwlswd.kdz3-qx35#d">
    <rdf:type rdf:resource="http://www.w3.org/2004/02/skos/core#Concept"/>
    <skos:inScheme rdf:resource="https://doi.org/10.6069/uwlswd.kdz3-qx35"/>
    <skos:prefLabel xml:lang="en">filmslip</skos:prefLabel>
    <skos:definition xml:lang="en">A short filmstrip not in a roll.</skos:definition>
    <skos:notation xml:lang="en">d</skos:notation>
  </rdf:Description>
  <rdf:Description rdf:about="https://doi.org/10.6069/uwlswd.kdz3-qx35#c">
    <rdf:type rdf:resource="http://www.w3.org/2004/02/skos/core#Concept"/>
    <skos:inScheme rdf:resource="https://doi.org/10.6069/uwlswd.kdz3-qx35"/>
    <skos:prefLabel xml:lang="en">filmstrip cartridge</skos:prefLabel>
    <skos:definition xml:lang="en">A filmstrip which is encased in a cartridge and which has the
         ends joined to form a loop. A cartridge denotes a permanently encased single reel of film
         or tape that has the ends joined together to form a loop that provides playback without
         rewinding.</skos:definition>
    <skos:notation xml:lang="en">c</skos:notation>
  </rdf:Description>
  <rdf:Description rdf:about="https://doi.org/10.6069/uwlswd.kdz3-qx35#n">
    <rdf:type rdf:resource="http://www.w3.org/2004/02/skos/core#Concept"/>
    <skos:inScheme rdf:resource="https://doi.org/10.6069/uwlswd.kdz3-qx35"/>
    <skos:prefLabel xml:lang="en">not applicable [obsolete]</skos:prefLabel>
    <skos:notation xml:lang="en">n</skos:notation>
  </rdf:Description>
  <rdf:Description rdf:about="https://doi.org/10.6069/uwlswd.kdz3-qx35#f">
    <rdf:type rdf:resource="http://www.w3.org/2004/02/skos/core#Concept"/>
    <skos:inScheme rdf:resource="https://doi.org/10.6069/uwlswd.kdz3-qx35"/>
    <skos:prefLabel xml:lang="en">other filmstrip type</skos:prefLabel>
    <skos:definition xml:lang="en">A filmstrip other than a filmstrip cartridge, filmslip or
         filmstrip roll or is an unspecified type of filmstrip.</skos:definition>
    <skos:notation xml:lang="en">f</skos:notation>
  </rdf:Description>
</rdf:RDF>
