@prefix dc: <http://purl.org/dc/elements/1.1/> .
@prefix dct: <http://purl.org/dc/terms/> .
@prefix schema: <https://schema.org/> .
@prefix skos: <http://www.w3.org/2004/02/skos/core#> .

<https://doi.org/10.6069/uwlswd.kb0p-ta35#a> a skos:Concept ;
    skos:definition """Moon type, which is an abstraction of the
         print."""@en ;
    skos:inScheme <https://doi.org/10.6069/uwlswd.kb0p-ta35> ;
    skos:notation "a" ;
    skos:prefLabel "moon"@en .

<https://doi.org/10.6069/uwlswd.kb0p-ta35#b> a skos:Concept ;
    skos:definition """A system of writing for the blind in which letters, numerals,
         and punctuation are made of raised dots distinguishable by the fingers."""@en ;
    skos:inScheme <https://doi.org/10.6069/uwlswd.kb0p-ta35> ;
    skos:notation "b" ;
    skos:prefLabel "braille"@en .

<https://doi.org/10.6069/uwlswd.kb0p-ta35#c> a skos:Concept ;
    skos:definition "Combination of two or more types."@en ;
    skos:inScheme <https://doi.org/10.6069/uwlswd.kb0p-ta35> ;
    skos:notation "c" ;
    skos:prefLabel "combination"@en .

<https://doi.org/10.6069/uwlswd.kb0p-ta35#d> a skos:Concept ;
    skos:definition """No text and only communicated as graphic, i.e. a raised line
         diagram or drawing."""@en ;
    skos:inScheme <https://doi.org/10.6069/uwlswd.kb0p-ta35> ;
    skos:notation "d" ;
    skos:prefLabel "tactile, with no writing system"@en .

<https://doi.org/10.6069/uwlswd.kb0p-ta35#u> a skos:Concept ;
    skos:definition """Special material designation for the tactile material is not
         specified."""@en ;
    skos:inScheme <https://doi.org/10.6069/uwlswd.kb0p-ta35> ;
    skos:notation "u" ;
    skos:prefLabel "unspecified"@en .

<https://doi.org/10.6069/uwlswd.kb0p-ta35#z> a skos:Concept ;
    skos:definition """Specific material designation other than moon; braille;
         combination; or tactile, with no writing system."""@en ;
    skos:inScheme <https://doi.org/10.6069/uwlswd.kb0p-ta35> ;
    skos:notation "z" ;
    skos:prefLabel "other"@en .

<https://doi.org/10.6069/uwlswd.kb0p-ta35> a skos:ConceptScheme ;
    dc:contributor "Metadata Management Associates"@en ;
    dc:language "en" ;
    dct:alternative """MARC21 007/01 values for tactile material expressed using
         RDF"""@en ;
    dct:contributor <http://viaf.org/viaf/151962300> ;
    dct:creator <http://viaf.org/viaf/139541794> ;
    dct:description """Special class of tactile material to which the item
         belongs."""@en ;
    dct:format <http://www.w3.org/ns/formats/Turtle> ;
    dct:hasFormat <https://uwlib-cams.github.io/uwlswd_vocabs_marc_007/tactile_material_specific_material_designation/tactile_material_specific_material_designation.html>,
        <https://uwlib-cams.github.io/uwlswd_vocabs_marc_007/tactile_material_specific_material_designation/tactile_material_specific_material_designation.jsonld>,
        <https://uwlib-cams.github.io/uwlswd_vocabs_marc_007/tactile_material_specific_material_designation/tactile_material_specific_material_designation.nt>,
        <https://uwlib-cams.github.io/uwlswd_vocabs_marc_007/tactile_material_specific_material_designation/tactile_material_specific_material_designation.rdf> ;
    dct:issued "2024" ;
    dct:license <http://creativecommons.org/publicdomain/zero/1.0> ;
    dct:provenance <https://doi.org/10.6069/uwlswd.2e2b-y833#marc00Xvalues> ;
    dct:publisher <http://viaf.org/viaf/139541794> ;
    dct:source <http://marc21rdf.info>,
        <https://www.loc.gov/marc/bibliographic/bd007.html> ;
    dct:title "Tactile material: specific material designation"@en ;
    dct:type <http://purl.org/dc/dcmitype/Dataset> ;
    schema:disambiguatingDescription """SKOS Concept Scheme for MARC 00X
         Values"""@en ;
    schema:version "1-0-0" .

