<?xml version="1.0" encoding="utf-8"?>
<rdf:RDF
   xmlns:dc="http://purl.org/dc/elements/1.1/"
   xmlns:dct="http://purl.org/dc/terms/"
   xmlns:rdf="http://www.w3.org/1999/02/22-rdf-syntax-ns#"
   xmlns:schema="https://schema.org/"
   xmlns:skos="http://www.w3.org/2004/02/skos/core#"
>
  <rdf:Description rdf:about="https://doi.org/10.6069/uwlswd.kb0p-ta35">
    <rdf:type rdf:resource="http://www.w3.org/2004/02/skos/core#ConceptScheme"/>
    <dct:type rdf:resource="http://purl.org/dc/dcmitype/Dataset"/>
    <dct:title xml:lang="en">Tactile material: specific material designation</dct:title>
    <dct:alternative xml:lang="en">MARC21 007/01 values for tactile material expressed using
         RDF</dct:alternative>
    <dct:description xml:lang="en">Special class of tactile material to which the item
         belongs.</dct:description>
    <schema:disambiguatingDescription>SKOS Concept Scheme for MARC 00X
         Values</schema:disambiguatingDescription>
    <dct:publisher rdf:resource="http://viaf.org/viaf/139541794"/>
    <dct:source rdf:resource="https://www.loc.gov/marc/bibliographic/bd007.html"/>
    <dct:source rdf:resource="http://marc21rdf.info"/>
    <dct:provenance rdf:resource="https://doi.org/10.6069/uwlswd.2e2b-y833"/>
    <dct:creator rdf:resource="http://viaf.org/viaf/139541794"/>
    <dct:contributor rdf:resource="http://viaf.org/viaf/151962300"/>
    <dct:issued>2024</dct:issued>
    <dc:contributor xml:lang="en">Metadata Management Associates</dc:contributor>
    <dc:language>en</dc:language>
    <dct:license rdf:resource="http://creativecommons.org/publicdomain/zero/1.0"/>
    <schema:version>1-0-0</schema:version>
    <dct:format rdf:resource="http://www.w3.org/ns/formats/RDF_XML"/>
  </rdf:Description>
  <rdf:Description rdf:about="https://doi.org/10.6069/uwlswd.kb0p-ta35#u">
    <rdf:type rdf:resource="http://www.w3.org/2004/02/skos/core#Concept"/>
    <skos:inScheme rdf:resource="https://doi.org/10.6069/uwlswd.kb0p-ta35"/>
    <skos:prefLabel xml:lang="en">unspecified</skos:prefLabel>
    <skos:definition xml:lang="en">Special material designation for the tactile material is not
         specified.</skos:definition>
    <skos:notation xml:lang="en">u</skos:notation>
  </rdf:Description>
  <rdf:Description rdf:about="https://doi.org/10.6069/uwlswd.kb0p-ta35#b">
    <rdf:type rdf:resource="http://www.w3.org/2004/02/skos/core#Concept"/>
    <skos:inScheme rdf:resource="https://doi.org/10.6069/uwlswd.kb0p-ta35"/>
    <skos:prefLabel xml:lang="en">braille</skos:prefLabel>
    <skos:definition xml:lang="en">A system of writing for the blind in which letters, numerals,
         and punctuation are made of raised dots distinguishable by the fingers.</skos:definition>
    <skos:notation xml:lang="en">b</skos:notation>
  </rdf:Description>
  <rdf:Description rdf:about="https://doi.org/10.6069/uwlswd.kb0p-ta35#d">
    <rdf:type rdf:resource="http://www.w3.org/2004/02/skos/core#Concept"/>
    <skos:inScheme rdf:resource="https://doi.org/10.6069/uwlswd.kb0p-ta35"/>
    <skos:prefLabel xml:lang="en">tactile, with no writing system</skos:prefLabel>
    <skos:definition xml:lang="en">No text and only communicated as graphic, i.e. a raised line
         diagram or drawing.</skos:definition>
    <skos:notation xml:lang="en">d</skos:notation>
  </rdf:Description>
  <rdf:Description rdf:about="https://doi.org/10.6069/uwlswd.kb0p-ta35#c">
    <rdf:type rdf:resource="http://www.w3.org/2004/02/skos/core#Concept"/>
    <skos:inScheme rdf:resource="https://doi.org/10.6069/uwlswd.kb0p-ta35"/>
    <skos:prefLabel xml:lang="en">combination</skos:prefLabel>
    <skos:definition xml:lang="en">Combination of two or more types.</skos:definition>
    <skos:notation xml:lang="en">c</skos:notation>
  </rdf:Description>
  <rdf:Description rdf:about="https://doi.org/10.6069/uwlswd.kb0p-ta35#a">
    <rdf:type rdf:resource="http://www.w3.org/2004/02/skos/core#Concept"/>
    <skos:inScheme rdf:resource="https://doi.org/10.6069/uwlswd.kb0p-ta35"/>
    <skos:prefLabel xml:lang="en">moon</skos:prefLabel>
    <skos:definition xml:lang="en">Moon type, which is an abstraction of the
         print.</skos:definition>
    <skos:notation xml:lang="en">a</skos:notation>
  </rdf:Description>
  <rdf:Description rdf:about="https://doi.org/10.6069/uwlswd.kb0p-ta35#z">
    <rdf:type rdf:resource="http://www.w3.org/2004/02/skos/core#Concept"/>
    <skos:inScheme rdf:resource="https://doi.org/10.6069/uwlswd.kb0p-ta35"/>
    <skos:prefLabel xml:lang="en">other</skos:prefLabel>
    <skos:definition xml:lang="en">Specific material designation other than moon; braille;
         combination; or tactile, with no writing system.</skos:definition>
    <skos:notation xml:lang="en">z</skos:notation>
  </rdf:Description>
</rdf:RDF>
