<?xml version="1.0" encoding="utf-8"?>
<rdf:RDF
   xmlns:dc="http://purl.org/dc/elements/1.1/"
   xmlns:dct="http://purl.org/dc/terms/"
   xmlns:rdf="http://www.w3.org/1999/02/22-rdf-syntax-ns#"
   xmlns:schema="https://schema.org/"
   xmlns:skos="http://www.w3.org/2004/02/skos/core#"
>
  <rdf:Description rdf:about="https://doi.org/10.6069/uwlswd.c9kk-6x09#d">
    <rdf:type rdf:resource="http://www.w3.org/2004/02/skos/core#Concept"/>
    <skos:inScheme rdf:resource="https://doi.org/10.6069/uwlswd.c9kk-6x09"/>
    <skos:prefLabel xml:lang="en">anamorphic (wide-screen)</skos:prefLabel>
    <skos:definition xml:lang="en">Films which achieve the wide-screen effect through the use of
         an image which is optically compressed or squeezed horizontally. It is then expanded to the
         correct proportions by projection on a wide screen with the use of special lenses that give
         greater magnification laterally than vertically.</skos:definition>
    <skos:scopeNote xml:lang="en">Introduced and adopted for commercial use in 1953 under the name
         of Cinemascope, followed by Techniscope (1963), Naturama, Panavision, etc. Also used for 16
         mm. film which employs this process.</skos:scopeNote>
    <skos:notation>d</skos:notation>
  </rdf:Description>
  <rdf:Description rdf:about="https://doi.org/10.6069/uwlswd.c9kk-6x09">
    <rdf:type rdf:resource="http://www.w3.org/2004/02/skos/core#ConceptScheme"/>
    <dct:type rdf:resource="http://purl.org/dc/dcmitype/Dataset"/>
    <dct:title xml:lang="en">Motion picture: presentation format</dct:title>
    <dct:alternative xml:lang="en">MARC21 007/04 values for motion pictures expressed using
         RDF</dct:alternative>
    <dct:description xml:lang="en">Presentation format for motion pictures.</dct:description>
    <schema:disambiguatingDescription xml:lang="en">SKOS Concept Scheme for MARC 00X
         Values</schema:disambiguatingDescription>
    <dct:publisher rdf:resource="http://viaf.org/viaf/139541794"/>
    <dct:source rdf:resource="https://www.loc.gov/marc/bibliographic/bd007.html"/>
    <dct:source rdf:resource="http://marc21rdf.info"/>
    <dct:provenance rdf:resource="https://doi.org/10.6069/uwlswd.2e2b-y833#marc00Xvalues"/>
    <dct:creator rdf:resource="http://viaf.org/viaf/139541794"/>
    <dct:contributor rdf:resource="http://viaf.org/viaf/151962300"/>
    <dct:issued>2024</dct:issued>
    <dc:contributor xml:lang="en">Metadata Management Associates</dc:contributor>
    <dc:language>en</dc:language>
    <dct:license rdf:resource="http://creativecommons.org/publicdomain/zero/1.0"/>
    <schema:version>1-0-0</schema:version>
    <dct:format rdf:resource="http://www.w3.org/ns/formats/RDF_XML"/>
    <dct:hasFormat rdf:resource="https://uwlib-cams.github.io/uwlswd_vocabs_marc_007/motion_picture_presentation_format/motion_picture_presentation_format.ttl"/>
    <dct:hasFormat rdf:resource="https://uwlib-cams.github.io/uwlswd_vocabs_marc_007/motion_picture_presentation_format/motion_picture_presentation_format.nt"/>
    <dct:hasFormat rdf:resource="https://uwlib-cams.github.io/uwlswd_vocabs_marc_007/motion_picture_presentation_format/motion_picture_presentation_format.jsonld"/>
    <dct:hasFormat rdf:resource="https://uwlib-cams.github.io/uwlswd_vocabs_marc_007/motion_picture_presentation_format/motion_picture_presentation_format.html"/>
  </rdf:Description>
  <rdf:Description rdf:about="https://doi.org/10.6069/uwlswd.c9kk-6x09#e">
    <rdf:type rdf:resource="http://www.w3.org/2004/02/skos/core#Concept"/>
    <skos:inScheme rdf:resource="https://doi.org/10.6069/uwlswd.c9kk-6x09"/>
    <skos:prefLabel xml:lang="en">other wide-screen format</skos:prefLabel>
    <skos:definition xml:lang="en">Any other wide-screen process not covered by other
         codes.</skos:definition>
    <skos:scopeNote xml:lang="en">Includes Cinerama, Viterama, Cinemiracle, Circarama and other
         formats that achieve a wide-screen effect though the use of simultaneous projection of
         separate prints on very large, sometimes deeply curved screens through the use of
         multiprojectors that build up the projected picture by a series of images, generally
         side-by-side.</skos:scopeNote>
    <skos:notation>e</skos:notation>
  </rdf:Description>
  <rdf:Description rdf:about="https://doi.org/10.6069/uwlswd.c9kk-6x09#n">
    <rdf:type rdf:resource="http://www.w3.org/2004/02/skos/core#Concept"/>
    <skos:inScheme rdf:resource="https://doi.org/10.6069/uwlswd.c9kk-6x09"/>
    <skos:prefLabel xml:lang="en">not applicable [obsolete]</skos:prefLabel>
    <skos:notation>n</skos:notation>
  </rdf:Description>
  <rdf:Description rdf:about="https://doi.org/10.6069/uwlswd.c9kk-6x09#z">
    <rdf:type rdf:resource="http://www.w3.org/2004/02/skos/core#Concept"/>
    <skos:inScheme rdf:resource="https://doi.org/10.6069/uwlswd.c9kk-6x09"/>
    <skos:prefLabel xml:lang="en">other</skos:prefLabel>
    <skos:definition xml:lang="en">Motion picture presentation format other than standard sound
         aperture (reduced frame), nonanamorphic (wide-screen), 3d, anamorphic (wide-screen), other
         wide-screen format, or standard silent aperture (full frame).</skos:definition>
    <skos:scopeNote xml:lang="en">An example of this is the 70 mm. Imax format which is a
         non-rectangular, circular 180 degree limited use format that is not standardized. Imax may
         not technically be considered a wide-screen format because it does not have an aspect
         ratio, but it does achieve a wide-screen effect.</skos:scopeNote>
    <skos:notation>z</skos:notation>
  </rdf:Description>
  <rdf:Description rdf:about="https://doi.org/10.6069/uwlswd.c9kk-6x09#c">
    <rdf:type rdf:resource="http://www.w3.org/2004/02/skos/core#Concept"/>
    <skos:inScheme rdf:resource="https://doi.org/10.6069/uwlswd.c9kk-6x09"/>
    <skos:prefLabel xml:lang="en">3D</skos:prefLabel>
    <skos:definition xml:lang="en">Films which achieve a three-dimensional effect originally
         through the use of two projectors which superimpose two images of the film on the screen
         (usually a wide screen). It is usually associated with 35 mm. film. Polarized lenses worn
         by viewers help to create the impression of depth and dimension.</skos:definition>
    <skos:notation>c</skos:notation>
  </rdf:Description>
  <rdf:Description rdf:about="https://doi.org/10.6069/uwlswd.c9kk-6x09#ex">
    <rdf:type rdf:resource="http://www.w3.org/2004/02/skos/core#Concept"/>
    <skos:inScheme rdf:resource="https://doi.org/10.6069/uwlswd.c9kk-6x09"/>
    <skos:prefLabel xml:lang="en">other [obsolete]</skos:prefLabel>
    <skos:notation>e</skos:notation>
  </rdf:Description>
  <rdf:Description rdf:about="https://doi.org/10.6069/uwlswd.c9kk-6x09#f">
    <rdf:type rdf:resource="http://www.w3.org/2004/02/skos/core#Concept"/>
    <skos:inScheme rdf:resource="https://doi.org/10.6069/uwlswd.c9kk-6x09"/>
    <skos:prefLabel xml:lang="en">standard silent aperture (full frame)</skos:prefLabel>
    <skos:definition xml:lang="en">35 mm. film on which the exposed picture is approximately the
         width of the space between the perforation holes of the frame.</skos:definition>
    <skos:scopeNote xml:lang="en">Standard format for silent film from about 1899 until the late
         1920s when sound film was introduced and the frame size decreased to make room for the
         sound track.</skos:scopeNote>
    <skos:notation>f</skos:notation>
  </rdf:Description>
  <rdf:Description rdf:about="https://doi.org/10.6069/uwlswd.c9kk-6x09#b">
    <rdf:type rdf:resource="http://www.w3.org/2004/02/skos/core#Concept"/>
    <skos:inScheme rdf:resource="https://doi.org/10.6069/uwlswd.c9kk-6x09"/>
    <skos:prefLabel xml:lang="en">nonanamorphic (wide-screen)</skos:prefLabel>
    <skos:definition xml:lang="en">Wide-screen effect without optically compressing the image or
         requiring the use of special projection techniques.</skos:definition>
    <skos:scopeNote xml:lang="en">Nonanamorphic wide-screen process is primarily associated with
         35 mm. and larger film gauges where the image on the film is natural (not optically
         compressed) and of smaller frame height, which is expanded by projection on a wide screen
         through the use of normal lenses and the appropriate aperture plate to give the required
         aspect ratio.</skos:scopeNote>
    <skos:notation>b</skos:notation>
  </rdf:Description>
  <rdf:Description rdf:about="https://doi.org/10.6069/uwlswd.c9kk-6x09#a">
    <rdf:type rdf:resource="http://www.w3.org/2004/02/skos/core#Concept"/>
    <skos:inScheme rdf:resource="https://doi.org/10.6069/uwlswd.c9kk-6x09"/>
    <skos:prefLabel xml:lang="en">standard sound aperture (reduced frame)</skos:prefLabel>
    <skos:definition xml:lang="en">Standard sound aperture (reduced frame).</skos:definition>
    <skos:scopeNote xml:lang="en">Used for non-wide-screen formats. Includes all standard sound 35
         mm., 16 mm., and super 8 mm. film. Should be used even for silent films in which a space
         has been left for the inclusion of a sound track, i.e., where a full frame silent picture
         has been cropped to allow space for a sound track.</skos:scopeNote>
    <skos:notation>a</skos:notation>
  </rdf:Description>
  <rdf:Description rdf:about="https://doi.org/10.6069/uwlswd.c9kk-6x09#u">
    <rdf:type rdf:resource="http://www.w3.org/2004/02/skos/core#Concept"/>
    <skos:inScheme rdf:resource="https://doi.org/10.6069/uwlswd.c9kk-6x09"/>
    <skos:prefLabel xml:lang="en">unknown</skos:prefLabel>
    <skos:definition xml:lang="en">Presentation format of the motion picture is not
         known.</skos:definition>
    <skos:notation>u</skos:notation>
  </rdf:Description>
</rdf:RDF>
