@prefix dc: <http://purl.org/dc/elements/1.1/> .
@prefix dct: <http://purl.org/dc/terms/> .
@prefix schema: <https://schema.org/> .
@prefix skos: <http://www.w3.org/2004/02/skos/core#> .

<https://doi.org/10.6069/uwlswd.er3s-pg07#k> a skos:Concept ;
    skos:definition """More than one configuration of playback channels is available
         on a single motion picture."""@en ;
    skos:inScheme <https://doi.org/10.6069/uwlswd.er3s-pg07> ;
    skos:notation "k" ;
    skos:prefLabel "mixed"@en ;
    skos:scopeNote """An example would be a film with both monaural optical and
         stereophonic magnetic sound tracks."""@en .

<https://doi.org/10.6069/uwlswd.er3s-pg07#m> a skos:Concept ;
    skos:definition "Configured to be played back on one channel."@en ;
    skos:inScheme <https://doi.org/10.6069/uwlswd.er3s-pg07> ;
    skos:notation "m" ;
    skos:prefLabel "monaural"@en .

<https://doi.org/10.6069/uwlswd.er3s-pg07#n> a skos:Concept ;
    skos:definition """Film is silent, has no sound or sound is on separate
         medium."""@en ;
    skos:inScheme <https://doi.org/10.6069/uwlswd.er3s-pg07> ;
    skos:notation "n" ;
    skos:prefLabel "not applicable"@en ;
    skos:scopeNote """Also used when describing an item with separate
         sound."""@en .

<https://doi.org/10.6069/uwlswd.er3s-pg07#q> a skos:Concept ;
    skos:definition """Configured to be played back or more than two
         channels."""@en ;
    skos:inScheme <https://doi.org/10.6069/uwlswd.er3s-pg07> ;
    skos:notation "q" ;
    skos:prefLabel "quadraphonic, multichannel, or surround"@en ;
    skos:scopeNote """Used for Dolby surround sound tracks and other multichannel
         techniques."""@en .

<https://doi.org/10.6069/uwlswd.er3s-pg07#s> a skos:Concept ;
    skos:definition """Configured to be played back on two separate
         channels."""@en ;
    skos:inScheme <https://doi.org/10.6069/uwlswd.er3s-pg07> ;
    skos:notation "s" ;
    skos:prefLabel "stereophonic"@en ;
    skos:scopeNote """Use when the medium is not monaural and when it is not possible
         to ascertain that multiple playback sources are available or intended."""@en .

<https://doi.org/10.6069/uwlswd.er3s-pg07#u> a skos:Concept ;
    skos:definition """Configuration of sound playback channels is not
         known."""@en ;
    skos:inScheme <https://doi.org/10.6069/uwlswd.er3s-pg07> ;
    skos:notation "u" ;
    skos:prefLabel "unknown"@en .

<https://doi.org/10.6069/uwlswd.er3s-pg07#z> a skos:Concept ;
    skos:definition """Configuration of playback channels other than mixed; monaural;
         quadraphonic, multichannel, or surround; or stereophonic."""@en ;
    skos:inScheme <https://doi.org/10.6069/uwlswd.er3s-pg07> ;
    skos:notation "z" ;
    skos:prefLabel "other"@en .

<https://doi.org/10.6069/uwlswd.er3s-pg07> a skos:ConceptScheme ;
    dc:contributor "Metadata Management Associates"@en ;
    dc:language "en" ;
    dct:alternative """MARC21 007/08 values for motion pictures expressed using
         RDF"""@en ;
    dct:contributor <http://viaf.org/viaf/151962300> ;
    dct:creator <http://viaf.org/viaf/139541794> ;
    dct:description """Configuration of playback channels for the sound portion of a
         motion picture."""@en ;
    dct:format <http://www.w3.org/ns/formats/Turtle> ;
    dct:hasFormat <https://uwlib-cams.github.io/uwlswd_vocabs_marc_007/motion_picture_configuration_of_playback_channels/motion_picture_configuration_of_playback_channels.html>,
        <https://uwlib-cams.github.io/uwlswd_vocabs_marc_007/motion_picture_configuration_of_playback_channels/motion_picture_configuration_of_playback_channels.jsonld>,
        <https://uwlib-cams.github.io/uwlswd_vocabs_marc_007/motion_picture_configuration_of_playback_channels/motion_picture_configuration_of_playback_channels.nt>,
        <https://uwlib-cams.github.io/uwlswd_vocabs_marc_007/motion_picture_configuration_of_playback_channels/motion_picture_configuration_of_playback_channels.rdf> ;
    dct:issued "2024" ;
    dct:license <http://creativecommons.org/publicdomain/zero/1.0> ;
    dct:provenance <https://doi.org/10.6069/uwlswd.2e2b-y833#marc00Xvalues> ;
    dct:publisher <http://viaf.org/viaf/139541794> ;
    dct:source <http://marc21rdf.info>,
        <https://www.loc.gov/marc/bibliographic/bd007.html> ;
    dct:title "Motion picture: configuration of playback channels"@en ;
    dct:type <http://purl.org/dc/dcmitype/Dataset> ;
    schema:disambiguatingDescription """SKOS Concept Scheme for MARC 00X
         Values"""@en ;
    schema:version "1-0-0" .

