<?xml version="1.0" encoding="utf-8"?>
<rdf:RDF
   xmlns:dc="http://purl.org/dc/elements/1.1/"
   xmlns:dct="http://purl.org/dc/terms/"
   xmlns:rdf="http://www.w3.org/1999/02/22-rdf-syntax-ns#"
   xmlns:schema="https://schema.org/"
   xmlns:skos="http://www.w3.org/2004/02/skos/core#"
>
  <rdf:Description rdf:about="https://doi.org/10.6069/uwlswd.4ehm-fa55#u">
    <rdf:type rdf:resource="http://www.w3.org/2004/02/skos/core#Concept"/>
    <skos:inScheme rdf:resource="https://doi.org/10.6069/uwlswd.4ehm-fa55"/>
    <skos:prefLabel xml:lang="en">unknown</skos:prefLabel>
    <skos:definition xml:lang="en">Generation stage of the film is not known.</skos:definition>
    <skos:notation>u</skos:notation>
  </rdf:Description>
  <rdf:Description rdf:about="https://doi.org/10.6069/uwlswd.4ehm-fa55#o">
    <rdf:type rdf:resource="http://www.w3.org/2004/02/skos/core#Concept"/>
    <skos:inScheme rdf:resource="https://doi.org/10.6069/uwlswd.4ehm-fa55"/>
    <skos:prefLabel xml:lang="en">original</skos:prefLabel>
    <skos:definition xml:lang="en">Original that is usually negative. It is film exposed in a
         camera and thus of better quality than any subsequent generation or
         derivative.</skos:definition>
    <skos:scopeNote xml:lang="en">When referring to older film, an original is almost always a
         negative. However, the original film may also be a reversal positive.</skos:scopeNote>
    <skos:notation>o</skos:notation>
  </rdf:Description>
  <rdf:Description rdf:about="https://doi.org/10.6069/uwlswd.4ehm-fa55">
    <rdf:type rdf:resource="http://www.w3.org/2004/02/skos/core#ConceptScheme"/>
    <dct:type rdf:resource="http://purl.org/dc/dcmitype/Dataset"/>
    <dct:title xml:lang="en">Motion picture: generation</dct:title>
    <dct:alternative xml:lang="en">MARC21 007/11 values for motion pictures expressed using
         RDF</dct:alternative>
    <dct:description xml:lang="en">How far away from the original material the item is (e.g., the
         actual negative film or original videotape in the camera).</dct:description>
    <schema:disambiguatingDescription xml:lang="en">SKOS Concept Scheme for MARC 00X
         Values</schema:disambiguatingDescription>
    <dct:publisher rdf:resource="http://viaf.org/viaf/139541794"/>
    <dct:source rdf:resource="https://www.loc.gov/marc/bibliographic/bd007.html"/>
    <dct:source rdf:resource="http://marc21rdf.info"/>
    <dct:provenance rdf:resource="https://doi.org/10.6069/uwlswd.2e2b-y833#marc00Xvalues"/>
    <dct:creator rdf:resource="http://viaf.org/viaf/139541794"/>
    <dct:contributor rdf:resource="http://viaf.org/viaf/151962300"/>
    <dct:issued>2024</dct:issued>
    <dc:contributor xml:lang="en">Metadata Management Associates</dc:contributor>
    <dc:language>en</dc:language>
    <dct:license rdf:resource="http://creativecommons.org/publicdomain/zero/1.0"/>
    <schema:version>1-0-0</schema:version>
    <dct:format rdf:resource="http://www.w3.org/ns/formats/RDF_XML"/>
    <dct:hasFormat rdf:resource="https://uwlib-cams.github.io/uwlswd_vocabs_marc_007/motion_picture_generation/motion_picture_generation.ttl"/>
    <dct:hasFormat rdf:resource="https://uwlib-cams.github.io/uwlswd_vocabs_marc_007/motion_picture_generation/motion_picture_generation.nt"/>
    <dct:hasFormat rdf:resource="https://uwlib-cams.github.io/uwlswd_vocabs_marc_007/motion_picture_generation/motion_picture_generation.jsonld"/>
    <dct:hasFormat rdf:resource="https://uwlib-cams.github.io/uwlswd_vocabs_marc_007/motion_picture_generation/motion_picture_generation.html"/>
  </rdf:Description>
  <rdf:Description rdf:about="https://doi.org/10.6069/uwlswd.4ehm-fa55#z">
    <rdf:type rdf:resource="http://www.w3.org/2004/02/skos/core#Concept"/>
    <skos:inScheme rdf:resource="https://doi.org/10.6069/uwlswd.4ehm-fa55"/>
    <skos:prefLabel xml:lang="en">other</skos:prefLabel>
    <skos:definition xml:lang="en">Generation other than duplicate, master original, reference
         print/viewing copy.</skos:definition>
    <skos:notation>z</skos:notation>
  </rdf:Description>
  <rdf:Description rdf:about="https://doi.org/10.6069/uwlswd.4ehm-fa55#e">
    <rdf:type rdf:resource="http://www.w3.org/2004/02/skos/core#Concept"/>
    <skos:inScheme rdf:resource="https://doi.org/10.6069/uwlswd.4ehm-fa55"/>
    <skos:prefLabel xml:lang="en">master</skos:prefLabel>
    <skos:definition xml:lang="en">Master that is usually positive and referred to as a master
         positive. It is a specially prepared positive print made from an earlier generation
         negative film and used for the preparation of duplicate negatives rather than for
         projection.</skos:definition>
    <skos:scopeNote xml:lang="en">The master is normally considered second generation
         material.</skos:scopeNote>
    <skos:notation>e</skos:notation>
  </rdf:Description>
  <rdf:Description rdf:about="https://doi.org/10.6069/uwlswd.4ehm-fa55#r">
    <rdf:type rdf:resource="http://www.w3.org/2004/02/skos/core#Concept"/>
    <skos:inScheme rdf:resource="https://doi.org/10.6069/uwlswd.4ehm-fa55"/>
    <skos:prefLabel xml:lang="en">reference print/viewing copy</skos:prefLabel>
    <skos:definition xml:lang="en">Reference print (ref print) that is defined technically as a
         release print which has been approved by the producer and director of a film. A reference
         print may also mean a print kept as a reference print to evaluate the quality of subsequent
         prints. In film archives, the term is used to indicate that a film may be viewed by
         researchers.</skos:definition>
    <skos:scopeNote xml:lang="en">It is not original, master, or duplicate
         material.</skos:scopeNote>
    <skos:notation>r</skos:notation>
  </rdf:Description>
  <rdf:Description rdf:about="https://doi.org/10.6069/uwlswd.4ehm-fa55#d">
    <rdf:type rdf:resource="http://www.w3.org/2004/02/skos/core#Concept"/>
    <skos:inScheme rdf:resource="https://doi.org/10.6069/uwlswd.4ehm-fa55"/>
    <skos:prefLabel xml:lang="en">duplicate</skos:prefLabel>
    <skos:definition xml:lang="en">Duplicate that is usually negative, referred to as a dupe neg,
         and is a reproduction of the original picture or sound track. A duplicate negative is made
         from a master positive, which in turn was made from an earlier negative.</skos:definition>
    <skos:scopeNote xml:lang="en">A duplicate is at least three generations from the original.
         Duplicate negatives may be prepared either to obtain characteristics not present in the
         original image, as in special effects work, or to protect and extend the production
         availability of the assembled original negative as when duplicate negatives are prepared
         for release printing simultaneously at different labs.</skos:scopeNote>
    <skos:notation>d</skos:notation>
  </rdf:Description>
</rdf:RDF>
