@prefix dc: <http://purl.org/dc/elements/1.1/> .
@prefix dct: <http://purl.org/dc/terms/> .
@prefix schema: <https://schema.org/> .
@prefix skos: <http://www.w3.org/2004/02/skos/core#> .

<https://doi.org/10.6069/uwlswd.4ehm-fa55#d> a skos:Concept ;
    skos:definition """Duplicate that is usually negative, referred to as a dupe neg,
         and is a reproduction of the original picture or sound track. A duplicate negative is made
         from a master positive, which in turn was made from an earlier negative."""@en ;
    skos:inScheme <https://doi.org/10.6069/uwlswd.4ehm-fa55> ;
    skos:notation "d" ;
    skos:prefLabel "duplicate"@en ;
    skos:scopeNote """A duplicate is at least three generations from the original.
         Duplicate negatives may be prepared either to obtain characteristics not present in the
         original image, as in special effects work, or to protect and extend the production
         availability of the assembled original negative as when duplicate negatives are prepared
         for release printing simultaneously at different labs."""@en .

<https://doi.org/10.6069/uwlswd.4ehm-fa55#e> a skos:Concept ;
    skos:definition """Master that is usually positive and referred to as a master
         positive. It is a specially prepared positive print made from an earlier generation
         negative film and used for the preparation of duplicate negatives rather than for
         projection."""@en ;
    skos:inScheme <https://doi.org/10.6069/uwlswd.4ehm-fa55> ;
    skos:notation "e" ;
    skos:prefLabel "master"@en ;
    skos:scopeNote """The master is normally considered second generation
         material."""@en .

<https://doi.org/10.6069/uwlswd.4ehm-fa55#o> a skos:Concept ;
    skos:definition """Original that is usually negative. It is film exposed in a
         camera and thus of better quality than any subsequent generation or
         derivative."""@en ;
    skos:inScheme <https://doi.org/10.6069/uwlswd.4ehm-fa55> ;
    skos:notation "o" ;
    skos:prefLabel "original"@en ;
    skos:scopeNote """When referring to older film, an original is almost always a
         negative. However, the original film may also be a reversal positive."""@en .

<https://doi.org/10.6069/uwlswd.4ehm-fa55#r> a skos:Concept ;
    skos:definition """Reference print (ref print) that is defined technically as a
         release print which has been approved by the producer and director of a film. A reference
         print may also mean a print kept as a reference print to evaluate the quality of subsequent
         prints. In film archives, the term is used to indicate that a film may be viewed by
         researchers."""@en ;
    skos:inScheme <https://doi.org/10.6069/uwlswd.4ehm-fa55> ;
    skos:notation "r" ;
    skos:prefLabel "reference print/viewing copy"@en ;
    skos:scopeNote """It is not original, master, or duplicate
         material."""@en .

<https://doi.org/10.6069/uwlswd.4ehm-fa55#u> a skos:Concept ;
    skos:definition "Generation stage of the film is not known."@en ;
    skos:inScheme <https://doi.org/10.6069/uwlswd.4ehm-fa55> ;
    skos:notation "u" ;
    skos:prefLabel "unknown"@en .

<https://doi.org/10.6069/uwlswd.4ehm-fa55#z> a skos:Concept ;
    skos:definition """Generation other than duplicate, master original, reference
         print/viewing copy."""@en ;
    skos:inScheme <https://doi.org/10.6069/uwlswd.4ehm-fa55> ;
    skos:notation "z" ;
    skos:prefLabel "other"@en .

<https://doi.org/10.6069/uwlswd.4ehm-fa55> a skos:ConceptScheme ;
    dc:contributor "Metadata Management Associates"@en ;
    dc:language "en" ;
    dct:alternative """MARC21 007/11 values for motion pictures expressed using
         RDF"""@en ;
    dct:contributor <http://viaf.org/viaf/151962300> ;
    dct:creator <http://viaf.org/viaf/139541794> ;
    dct:description """How far away from the original material the item is (e.g., the
         actual negative film or original videotape in the camera)."""@en ;
    dct:format <http://www.w3.org/ns/formats/Turtle> ;
    dct:hasFormat <https://uwlib-cams.github.io/uwlswd_vocabs_marc_007/motion_picture_generation/motion_picture_generation.html>,
        <https://uwlib-cams.github.io/uwlswd_vocabs_marc_007/motion_picture_generation/motion_picture_generation.jsonld>,
        <https://uwlib-cams.github.io/uwlswd_vocabs_marc_007/motion_picture_generation/motion_picture_generation.nt>,
        <https://uwlib-cams.github.io/uwlswd_vocabs_marc_007/motion_picture_generation/motion_picture_generation.rdf> ;
    dct:issued "2024" ;
    dct:license <http://creativecommons.org/publicdomain/zero/1.0> ;
    dct:provenance <https://doi.org/10.6069/uwlswd.2e2b-y833#marc00Xvalues> ;
    dct:publisher <http://viaf.org/viaf/139541794> ;
    dct:source <http://marc21rdf.info>,
        <https://www.loc.gov/marc/bibliographic/bd007.html> ;
    dct:title "Motion picture: generation"@en ;
    dct:type <http://purl.org/dc/dcmitype/Dataset> ;
    schema:disambiguatingDescription """SKOS Concept Scheme for MARC 00X
         Values"""@en ;
    schema:version "1-0-0" .

