@prefix dc: <http://purl.org/dc/elements/1.1/> .
@prefix dct: <http://purl.org/dc/terms/> .
@prefix schema: <https://schema.org/> .
@prefix skos: <http://www.w3.org/2004/02/skos/core#> .

<https://doi.org/10.6069/uwlswd.a3v4-v844#a> a skos:Concept ;
    skos:definition """National Association of Broadcasters (NAB) standard was used
         for the transcription of the recording and NAB playback equalization is
         required."""@en ;
    skos:inScheme <https://doi.org/10.6069/uwlswd.a3v4-v844> ;
    skos:notation "a" ;
    skos:prefLabel "NAB standard"@en .

<https://doi.org/10.6069/uwlswd.a3v4-v844#b> a skos:Concept ;
    skos:definition """Comit√© consultatif de la radiodiffusion (CCIR) standard was
         used for the transcription of the recording and CCIR playback equalization is
         required."""@en ;
    skos:inScheme <https://doi.org/10.6069/uwlswd.a3v4-v844> ;
    skos:notation "b" ;
    skos:prefLabel "CCIR standard"@en .

<https://doi.org/10.6069/uwlswd.a3v4-v844#c> a skos:Concept ;
    skos:definition "Requires Dolby-B decoding playback equipment."@en ;
    skos:inScheme <https://doi.org/10.6069/uwlswd.a3v4-v844> ;
    skos:notation "c" ;
    skos:prefLabel "Dolby-B encoded"@en ;
    skos:scopeNote """Indicated on commercial recordings by the double D insignia
         (without indication of Dolby-C encoding). If Dolby is used on a tape recording without
         other indication, Dolby-B may be assumed. Despite the presence of the double-D or "Dolby"
         on a disc recording, this code is never used for commercial discs."""@en .

<https://doi.org/10.6069/uwlswd.a3v4-v844#d> a skos:Concept ;
    skos:definition """Used for disc or tape recordings which indicate on the label or
         package that dbx decoding is required."""@en ;
    skos:inScheme <https://doi.org/10.6069/uwlswd.a3v4-v844> ;
    skos:notation "d" ;
    skos:prefLabel "dbx encoded"@en ;
    skos:scopeNote """Not used if descriptive material indicates that dbx was used
         during recording but that standard playback equipment may be used."""@en .

<https://doi.org/10.6069/uwlswd.a3v4-v844#e> a skos:Concept ;
    skos:definition """Requires digital playback equipment, such as Phillips/Sony
         Compact Discs or Sony PCM tape recordings."""@en ;
    skos:inScheme <https://doi.org/10.6069/uwlswd.a3v4-v844> ;
    skos:notation "e" ;
    skos:prefLabel "digital recording"@en ;
    skos:scopeNote """Not used when there is indication that digital equipment was
         used during recording, but that analog playback equipment may be used. No commercial
         recordings prior to 1982, and no analog disc or tape recordings use digitial equipment
         during recording."""@en .

<https://doi.org/10.6069/uwlswd.a3v4-v844#f> a skos:Concept ;
    skos:definition "Requires Dolby-A playback equipment."@en ;
    skos:inScheme <https://doi.org/10.6069/uwlswd.a3v4-v844> ;
    skos:notation "f" ;
    skos:prefLabel "Dolby-A encoded"@en ;
    skos:scopeNote """Used only for master tapes and other tape recordings where clear
         indication is given that the professional Dolby-A encoding was applied, and that Dolby-A
         decoding is required. Dolby-A encoding is never used for commercial tape or discs.
         (Instantaneous tape recordings labelled "Dolby" without other indication are normally
         Dolby-B, particularly cassette recordings.)"""@en .

<https://doi.org/10.6069/uwlswd.a3v4-v844#g> a skos:Concept ;
    skos:definition "Requires Dolby-C playback equipment."@en ;
    skos:inScheme <https://doi.org/10.6069/uwlswd.a3v4-v844> ;
    skos:notation "g" ;
    skos:prefLabel "Dolby-C encoded"@en ;
    skos:scopeNote """Used for tape recordings where the label or packaging clearly
         indicates that Dolby-C is required. "Dolby" or the double-D symbol without specific
         explanation normally indicates Dolby-B."""@en .

<https://doi.org/10.6069/uwlswd.a3v4-v844#h> a skos:Concept ;
    skos:definition "Requires CX encoded playback equipment."@en ;
    skos:inScheme <https://doi.org/10.6069/uwlswd.a3v4-v844> ;
    skos:notation "h" ;
    skos:prefLabel "CX encoded"@en ;
    skos:scopeNote """Used for recordings where the symbol or mark CX appears. Such
         recordings may be labelled as compatible with standard playback equipment. No CX recordings
         will appear with pressing dates prior to 1981."""@en .

<https://doi.org/10.6069/uwlswd.a3v4-v844#n> a skos:Concept ;
    skos:definition """Item does not have special playback
         characteristics."""@en ;
    skos:inScheme <https://doi.org/10.6069/uwlswd.a3v4-v844> ;
    skos:notation "n" ;
    skos:prefLabel "not applicable"@en .

<https://doi.org/10.6069/uwlswd.a3v4-v844#u> a skos:Concept ;
    skos:definition """Playback characteristics of the item are not
         known."""@en ;
    skos:inScheme <https://doi.org/10.6069/uwlswd.a3v4-v844> ;
    skos:notation "u" ;
    skos:prefLabel "unknown"@en .

<https://doi.org/10.6069/uwlswd.a3v4-v844#z> a skos:Concept ;
    skos:definition """Playback characteristics other than NAB standard, CCIR
         standard, Dolby-B encoded, dbx encoded, digital recording, Dolby-A encoded, Dolby-C
         encoded, or CX encoded."""@en ;
    skos:inScheme <https://doi.org/10.6069/uwlswd.a3v4-v844> ;
    skos:notation "z" ;
    skos:prefLabel "other"@en .

<https://doi.org/10.6069/uwlswd.a3v4-v844> a skos:ConceptScheme ;
    dc:contributor "Metadata Management Associates"@en ;
    dc:language "en" ;
    dct:alternative """MARC21 007/12 values for sound recordings expressed using
         RDF"""@en ;
    dct:contributor <http://viaf.org/viaf/151962300> ;
    dct:creator <http://viaf.org/viaf/139541794> ;
    dct:description """Playback characteristics for sound recordings, including
         special equipment or equalization necessary for proper playback. Not used to indicate
         special processes used during recording unless those processes must be applied during
         playback."""@en ;
    dct:format <http://www.w3.org/ns/formats/Turtle> ;
    dct:hasFormat <https://uwlib-cams.github.io/uwlswd_vocabs_marc_007/sound_recording_special_playback_characteristics/sound_recording_special_playback_characteristics.html>,
        <https://uwlib-cams.github.io/uwlswd_vocabs_marc_007/sound_recording_special_playback_characteristics/sound_recording_special_playback_characteristics.jsonld>,
        <https://uwlib-cams.github.io/uwlswd_vocabs_marc_007/sound_recording_special_playback_characteristics/sound_recording_special_playback_characteristics.nt>,
        <https://uwlib-cams.github.io/uwlswd_vocabs_marc_007/sound_recording_special_playback_characteristics/sound_recording_special_playback_characteristics.rdf> ;
    dct:issued "2024" ;
    dct:license <http://creativecommons.org/publicdomain/zero/1.0> ;
    dct:provenance <https://doi.org/10.6069/uwlswd.2e2b-y833#marc00Xvalues> ;
    dct:publisher <http://viaf.org/viaf/139541794> ;
    dct:source <http://marc21rdf.info>,
        <https://www.loc.gov/marc/bibliographic/bd007.html> ;
    dct:title "Sound recording: special playback characteristics"@en ;
    dct:type <http://purl.org/dc/dcmitype/Dataset> ;
    schema:disambiguatingDescription """SKOS Concept Scheme for MARC 00X
         Values"""@en ;
    schema:version "1-0-0" .

