<?xml version="1.0" encoding="utf-8"?>
<rdf:RDF
   xmlns:dc="http://purl.org/dc/elements/1.1/"
   xmlns:dct="http://purl.org/dc/terms/"
   xmlns:rdf="http://www.w3.org/1999/02/22-rdf-syntax-ns#"
   xmlns:schema="https://schema.org/"
   xmlns:skos="http://www.w3.org/2004/02/skos/core#"
>
  <rdf:Description rdf:about="http://fakeIRI.edu/terms/projectedbas#d">
    <rdf:type rdf:resource="http://www.w3.org/2004/02/skos/core#Concept"/>
    <skos:inScheme rdf:resource="http://fakeIRI.edu/terms/projectedbas"/>
    <skos:prefLabel xml:lang="en">glass</skos:prefLabel>
    <skos:definition xml:lang="en">Glass.</skos:definition>
    <skos:notation xml:lang="en">d</skos:notation>
  </rdf:Description>
  <rdf:Description rdf:about="http://fakeIRI.edu/terms/projectedbas">
    <rdf:type rdf:resource="http://www.w3.org/2004/02/skos/core#ConceptScheme"/>
    <dct:type rdf:resource="http://purl.org/dc/dcmitype/Dataset"/>
    <dct:title xml:lang="en">Projected graphic: Base of emulsion</dct:title>
    <dct:alternative xml:lang="en">MARC21 007/04 values for projected graphics expressed using
         RDF</dct:alternative>
    <dct:description xml:lang="en">Type of material for the base of the emulsion of a
         photonegative, filmstrip, slide, or transparency.</dct:description>
    <schema:disambiguatingDescription>SKOS Concept Scheme for MARC 00X
         Values</schema:disambiguatingDescription>
    <dct:publisher rdf:resource="http://viaf.org/viaf/139541794"/>
    <dct:source rdf:resource="https://www.loc.gov/marc/bibliographic/bd007.html"/>
    <dct:source rdf:resource="http://marc21rdf.info"/>
    <dct:provenance rdf:resource="https://doi.org/10.6069/uwlswd.2e2b-y833"/>
    <dct:creator rdf:resource="http://viaf.org/viaf/139541794"/>
    <dct:contributor rdf:resource="http://viaf.org/viaf/151962300"/>
    <dct:issued>2024</dct:issued>
    <dc:contributor xml:lang="en">Metadata Management Associates</dc:contributor>
    <dc:language>en</dc:language>
    <dct:license rdf:resource="http://creativecommons.org/publicdomain/zero/1.0"/>
    <schema:version>1-0-0</schema:version>
    <dct:format rdf:resource="http://www.w3.org/ns/formats/RDF_XML"/>
  </rdf:Description>
  <rdf:Description rdf:about="http://fakeIRI.edu/terms/projectedbas#z">
    <rdf:type rdf:resource="http://www.w3.org/2004/02/skos/core#Concept"/>
    <skos:inScheme rdf:resource="http://fakeIRI.edu/terms/projectedbas"/>
    <skos:prefLabel xml:lang="en">other</skos:prefLabel>
    <skos:definition xml:lang="en">Base of emulsion other than glass; synthetic; safety film; film
         base, other than safety film; mixed collection; or paper.</skos:definition>
    <skos:notation xml:lang="en">z</skos:notation>
  </rdf:Description>
  <rdf:Description rdf:about="http://fakeIRI.edu/terms/projectedbas#e">
    <rdf:type rdf:resource="http://www.w3.org/2004/02/skos/core#Concept"/>
    <skos:inScheme rdf:resource="http://fakeIRI.edu/terms/projectedbas"/>
    <skos:prefLabel xml:lang="en">synthetic</skos:prefLabel>
    <skos:definition xml:lang="en">Synthetic material.</skos:definition>
    <skos:scopeNote xml:lang="en">E.g., plastics, vinyl, etc. Most commercially issued overhead
         transparency sets have a synthetic primary support material, unless known to be
         otherwise.</skos:scopeNote>
    <skos:notation xml:lang="en">e</skos:notation>
  </rdf:Description>
  <rdf:Description rdf:about="http://fakeIRI.edu/terms/projectedbas#pound">
    <rdf:type rdf:resource="http://www.w3.org/2004/02/skos/core#Concept"/>
    <skos:inScheme rdf:resource="http://fakeIRI.edu/terms/projectedbas"/>
    <skos:prefLabel xml:lang="en">not applicable or no attempt to code [obsolete]</skos:prefLabel>
    <skos:notation xml:lang="en">#</skos:notation>
  </rdf:Description>
  <rdf:Description rdf:about="http://fakeIRI.edu/terms/projectedbas#u">
    <rdf:type rdf:resource="http://www.w3.org/2004/02/skos/core#Concept"/>
    <skos:inScheme rdf:resource="http://fakeIRI.edu/terms/projectedbas"/>
    <skos:prefLabel xml:lang="en">unknown</skos:prefLabel>
    <skos:definition xml:lang="en">Material varies for different items in a
         collection.</skos:definition>
    <skos:notation xml:lang="en">u</skos:notation>
  </rdf:Description>
  <rdf:Description rdf:about="http://fakeIRI.edu/terms/projectedbas#j">
    <rdf:type rdf:resource="http://www.w3.org/2004/02/skos/core#Concept"/>
    <skos:inScheme rdf:resource="http://fakeIRI.edu/terms/projectedbas"/>
    <skos:prefLabel xml:lang="en">safety film</skos:prefLabel>
    <skos:definition xml:lang="en">Safety (i.e., not nitrate) film.</skos:definition>
    <skos:scopeNote xml:lang="en">For all commercially issued filmstrips and slide sets, assume
         that the base of the emulsion is safety film unless known to be otherwise.</skos:scopeNote>
    <skos:notation xml:lang="en">j</skos:notation>
  </rdf:Description>
  <rdf:Description rdf:about="http://fakeIRI.edu/terms/projectedbas#m">
    <rdf:type rdf:resource="http://www.w3.org/2004/02/skos/core#Concept"/>
    <skos:inScheme rdf:resource="http://fakeIRI.edu/terms/projectedbas"/>
    <skos:prefLabel xml:lang="en">mixed collection</skos:prefLabel>
    <skos:definition xml:lang="en">Material varies for different items in a
         collection.</skos:definition>
    <skos:scopeNote xml:lang="en">Typically this would be used for groups of projected graphics on
         various bases.</skos:scopeNote>
    <skos:notation xml:lang="en">m</skos:notation>
  </rdf:Description>
  <rdf:Description rdf:about="http://fakeIRI.edu/terms/projectedbas#o">
    <rdf:type rdf:resource="http://www.w3.org/2004/02/skos/core#Concept"/>
    <skos:inScheme rdf:resource="http://fakeIRI.edu/terms/projectedbas"/>
    <skos:prefLabel xml:lang="en">paper</skos:prefLabel>
    <skos:definition xml:lang="en">Any kind of cellulose-based paper.</skos:definition>
    <skos:notation xml:lang="en">o</skos:notation>
  </rdf:Description>
  <rdf:Description rdf:about="http://fakeIRI.edu/terms/projectedbas#k">
    <rdf:type rdf:resource="http://www.w3.org/2004/02/skos/core#Concept"/>
    <skos:inScheme rdf:resource="http://fakeIRI.edu/terms/projectedbas"/>
    <skos:prefLabel xml:lang="en">film base, other than safety film</skos:prefLabel>
    <skos:definition xml:lang="en">Not safety film.</skos:definition>
    <skos:notation xml:lang="en">k</skos:notation>
  </rdf:Description>
  <rdf:Description rdf:about="http://fakeIRI.edu/terms/projectedbas#n">
    <rdf:type rdf:resource="http://www.w3.org/2004/02/skos/core#Concept"/>
    <skos:inScheme rdf:resource="http://fakeIRI.edu/terms/projectedbas"/>
    <skos:prefLabel xml:lang="en">not applicable [obsolete]</skos:prefLabel>
    <skos:notation xml:lang="en">n</skos:notation>
  </rdf:Description>
</rdf:RDF>
