@prefix dc: <http://purl.org/dc/elements/1.1/> .
@prefix dct: <http://purl.org/dc/terms/> .
@prefix schema: <https://schema.org/> .
@prefix skos: <http://www.w3.org/2004/02/skos/core#> .

<https://doi.org/10.6069/uwlswd.q8qv-nz89#a> a skos:Concept ;
    skos:definition """Removable module containing secondary storage medium such as
         magnetic tape or magnetic disks."""@en ;
    skos:inScheme <https://doi.org/10.6069/uwlswd.q8qv-nz89> ;
    skos:notation "a" ;
    skos:prefLabel "tape cartridge"@en .

<https://doi.org/10.6069/uwlswd.q8qv-nz89#b> a skos:Concept ;
    skos:definition """Removable module containing a miniaturized electronic circuit,
         mass-produced on a tiny chip or wafer of silicon, designed to provide additional processing
         or memory capacity to a computer."""@en ;
    skos:inScheme <https://doi.org/10.6069/uwlswd.q8qv-nz89> ;
    skos:notation "b" ;
    skos:prefLabel "chip cartridge"@en ;
    skos:scopeNote """Includes several types of solid-state, memory/storage devices
         such as non-rewritable ROM-chip cartridges and rewritable flash drives (e.g. USB
         keys)."""@en .

<https://doi.org/10.6069/uwlswd.q8qv-nz89#c> a skos:Concept ;
    skos:definition """Removable module containing one or more nonmagnetic discs used
         to store digital information."""@en ;
    skos:inScheme <https://doi.org/10.6069/uwlswd.q8qv-nz89> ;
    skos:notation "c" ;
    skos:prefLabel "computer optical disc cartridge"@en .

<https://doi.org/10.6069/uwlswd.q8qv-nz89#d> a skos:Concept ;
    skos:definition "A disc whose type is not specified."@en ;
    skos:inScheme <https://doi.org/10.6069/uwlswd.q8qv-nz89> ;
    skos:notation "d" ;
    skos:prefLabel "computer disc, type unspecified"@en .

<https://doi.org/10.6069/uwlswd.q8qv-nz89#e> a skos:Concept ;
    skos:definition "A disc cartridge whose type is not specified."@en ;
    skos:inScheme <https://doi.org/10.6069/uwlswd.q8qv-nz89> ;
    skos:notation "e" ;
    skos:prefLabel "computer disc cartridge, type unspecified"@en .

<https://doi.org/10.6069/uwlswd.q8qv-nz89#f> a skos:Concept ;
    skos:definition """Removable module, somewhat like an audio cassette, that
         contains magnetic tape that can be written on and read from by a tape
         drive."""@en ;
    skos:inScheme <https://doi.org/10.6069/uwlswd.q8qv-nz89> ;
    skos:notation "f" ;
    skos:prefLabel "tape cassette"@en .

<https://doi.org/10.6069/uwlswd.q8qv-nz89#h> a skos:Concept ;
    skos:definition """Removable spool containing magnetic tape that can be written to
         and read from by a tape drive."""@en ;
    skos:inScheme <https://doi.org/10.6069/uwlswd.q8qv-nz89> ;
    skos:notation "h" ;
    skos:prefLabel "tape reel"@en .

<https://doi.org/10.6069/uwlswd.q8qv-nz89#j> a skos:Concept ;
    skos:definition """Digital information storage medium usually consisting of a thin
         Mylar disk coated with a magnetic material that permits the recording of data. Magnetic
         disks come in various sizes. They are also known as floppy disks, stiffy disks, computer
         diskettes, or floppy diskettes."""@en ;
    skos:inScheme <https://doi.org/10.6069/uwlswd.q8qv-nz89> ;
    skos:notation "j" ;
    skos:prefLabel "magnetic disk"@en .

<https://doi.org/10.6069/uwlswd.q8qv-nz89#k> a skos:Concept ;
    skos:definition "Computer card."@en ;
    skos:inScheme <https://doi.org/10.6069/uwlswd.q8qv-nz89> ;
    skos:notation "k" ;
    skos:prefLabel "computer card"@en .

<https://doi.org/10.6069/uwlswd.q8qv-nz89#m> a skos:Concept ;
    skos:definition """Erasable or semi-erasable storage medium, similar to a CD-ROM
         disc, capable of storing data at a very high density. The disc is written to and read from
         using a laser beam used to heat the recording surface to a point at which regions of the
         surface of the disk become magnetically aligned to store bits of data."""@en ;
    skos:inScheme <https://doi.org/10.6069/uwlswd.q8qv-nz89> ;
    skos:notation "m" ;
    skos:prefLabel "magneto-optical disc"@en .

<https://doi.org/10.6069/uwlswd.q8qv-nz89#o> a skos:Concept ;
    skos:definition """Medium that uses a series of laser-burned micron-sized holes
         (pits) on a special recording surface to store data. Recorded data is read optically. These
         discs are usually a read-only medium."""@en ;
    skos:inScheme <https://doi.org/10.6069/uwlswd.q8qv-nz89> ;
    skos:notation "o" ;
    skos:prefLabel "optical disc"@en ;
    skos:scopeNote """Commonly found computer optical disc formats include: CD-A,
         CD-I, CD-R, CD-ROM, CD-ROM-XA, DVD-ROM and Photo CD."""@en .

<https://doi.org/10.6069/uwlswd.q8qv-nz89#r> a skos:Concept ;
    skos:definition """Electronic resource that is accessed, processed, executed, etc.
         remotely. In this case the electronic resource is used via input/output devices connected
         electronically to a computer. Frequently this involves connection through a computer
         network."""@en ;
    skos:inScheme <https://doi.org/10.6069/uwlswd.q8qv-nz89> ;
    skos:notation "r" ;
    skos:prefLabel "remote"@en .

<https://doi.org/10.6069/uwlswd.q8qv-nz89#s> a skos:Concept ;
    skos:definition """Consists of storage and reader components as an integrated
         standalone device. The data storage medium cannot be removed from the playback device with
         which it is issued. The data carried on the medium can only be read using the integrated
         special-purpose device."""@en ;
    skos:inScheme <https://doi.org/10.6069/uwlswd.q8qv-nz89> ;
    skos:notation "s" ;
    skos:prefLabel "standalone device"@en .

<https://doi.org/10.6069/uwlswd.q8qv-nz89#u> a skos:Concept ;
    skos:definition """Special material designation for the electronic resource is not
         specified."""@en ;
    skos:inScheme <https://doi.org/10.6069/uwlswd.q8qv-nz89> ;
    skos:notation "u" ;
    skos:prefLabel "unspecified"@en ;
    skos:scopeNote """E.g., it may be an electronic resource that changes its medium
         over time."""@en .

<https://doi.org/10.6069/uwlswd.q8qv-nz89#z> a skos:Concept ;
    skos:definition """Specific material designation other than tape cartridge, chip
         cartridge, computer optical disc cartridge, computer disc, type unspecified, computer disc
         cartridge, type unspecified, tape cassette, tape reel, magnetic disk, computer card,
         magneto-optical disc, optical disc, remote, or standalone device."""@en ;
    skos:inScheme <https://doi.org/10.6069/uwlswd.q8qv-nz89> ;
    skos:notation "z" ;
    skos:prefLabel "other"@en .

<https://doi.org/10.6069/uwlswd.q8qv-nz89> a skos:ConceptScheme ;
    dc:contributor "Metadata Management Associates"@en ;
    dc:language "en" ;
    dct:alternative """MARC21 007/01 values for electronic resources expressed using
         RDF"""@en ;
    dct:contributor <http://viaf.org/viaf/151962300> ;
    dct:creator <http://viaf.org/viaf/139541794> ;
    dct:description """Special class of material (usually the class of physical
         object) to which an item belongs (e.g., a magnetic disk)."""@en ;
    dct:format <http://www.w3.org/ns/formats/Turtle> ;
    dct:hasFormat <https://uwlib-cams.github.io/uwlswd_vocabs_marc_007/electronic_resource_specific_material_designation/electronic_resource_specific_material_designation.html>,
        <https://uwlib-cams.github.io/uwlswd_vocabs_marc_007/electronic_resource_specific_material_designation/electronic_resource_specific_material_designation.jsonld>,
        <https://uwlib-cams.github.io/uwlswd_vocabs_marc_007/electronic_resource_specific_material_designation/electronic_resource_specific_material_designation.nt>,
        <https://uwlib-cams.github.io/uwlswd_vocabs_marc_007/electronic_resource_specific_material_designation/electronic_resource_specific_material_designation.rdf> ;
    dct:issued "2024" ;
    dct:license <http://creativecommons.org/publicdomain/zero/1.0> ;
    dct:provenance <https://doi.org/10.6069/uwlswd.2e2b-y833#marc00Xvalues> ;
    dct:publisher <http://viaf.org/viaf/139541794> ;
    dct:source <http://marc21rdf.info>,
        <https://www.loc.gov/marc/bibliographic/bd007.html> ;
    dct:title "Electronic resource: specific material designation"@en ;
    dct:type <http://purl.org/dc/dcmitype/Dataset> ;
    schema:disambiguatingDescription """SKOS Concept Scheme for MARC 00X
         Values"""@en ;
    schema:version "1-0-0" .

