<?xml version="1.0" encoding="UTF-8"?>
<rdf:RDF xmlns:dc="http://purl.org/dc/elements/1.1/" xmlns:dct="http://purl.org/dc/terms/"
   xmlns:rdf="http://www.w3.org/1999/02/22-rdf-syntax-ns#"
   xmlns:rdfs="http://www.w3.org/2000/01/rdf-schema#" xmlns:schema="https://schema.org/"
   xmlns:skos="http://www.w3.org/2004/02/skos/core#"
   xmlns:uw="https://www.lib.washington.edu/static/public/cams/data/localResources/properties_local.html"
   xmlns:uwp="https://doi.org/10.6069/uwlib.55.d.3#">


   <rdf:Description rdf:about="http://fakeIRI.edu/terms/electrosmd">
      <rdf:type rdf:resource="http://www.w3.org/2004/02/skos/core#ConceptScheme"/>
      <dct:type rdf:resource="http://purl.org/dc/dcmitype/Dataset"/>
      <dct:title xml:lang="en">Electronic resource: specific material designation</dct:title>
      <dct:alternative xml:lang="en">MARC21 007/01 values for electronic resources expressed using
         RDF</dct:alternative>
      <dct:description xml:lang="en">Special class of material (usually the class of physical
         object) to which an item belongs (e.g., a magnetic disk).</dct:description>
      <schema:disambiguatingDescription>SKOS Concept Scheme for MARC 00X
         Values</schema:disambiguatingDescription>
      <dct:publisher rdf:resource="http://viaf.org/viaf/139541794"/>
      <dct:source rdf:resource="https://www.loc.gov/marc/bibliographic/bd007.html"/>
      <dct:source rdf:resource="http://marc21rdf.info"/>
      <dct:provenance rdf:resource="https://doi.org/10.6069/uwlswd.2e2b-y833"/>
      <dct:creator rdf:resource="http://viaf.org/viaf/139541794"/>
      <dct:contributor rdf:resource="http://viaf.org/viaf/151962300"/>
      <dct:issued>2024</dct:issued>
      <dc:contributor xml:lang="en">Metadata Management Associates</dc:contributor>
      <dc:language>en</dc:language>
      <dct:license rdf:resource="http://creativecommons.org/publicdomain/zero/1.0"/>
      <schema:version>1-0-0</schema:version>
      <dct:issued>2024</dct:issued>
      <dct:format rdf:resource="http://www.w3.org/ns/formats/RDF_XML"/>
   </rdf:Description>

   <rdf:Description rdf:about="http://fakeIRI.edu/terms/electrosmd#b">
      <rdf:type rdf:resource="http://www.w3.org/2004/02/skos/core#Concept"/>
      <skos:inScheme rdf:resource="http://fakeIRI.edu/terms/electrosmd"/>
      <skos:prefLabel xml:lang="en">chip cartridge</skos:prefLabel>
      <skos:definition xml:lang="en">Removable module containing a miniaturized electronic circuit,
         mass-produced on a tiny chip or wafer of silicon, designed to provide additional processing
         or memory capacity to a computer.</skos:definition>
      <skos:scopeNote xml:lang="en">Includes several types of solid-state, memory/storage devices
         such as non-rewritable ROM-chip cartridges and rewritable flash drives (e.g. USB
         keys).</skos:scopeNote>
      <skos:notation xml:lang="en">b</skos:notation>
   </rdf:Description>

   <rdf:Description rdf:about="http://fakeIRI.edu/terms/electrosmd#k">
      <rdf:type rdf:resource="http://www.w3.org/2004/02/skos/core#Concept"/>
      <skos:inScheme rdf:resource="http://fakeIRI.edu/terms/electrosmd"/>
      <skos:prefLabel xml:lang="en">computer card</skos:prefLabel>
      <skos:definition xml:lang="en">Computer card.</skos:definition>
      <skos:notation xml:lang="en">k</skos:notation>
   </rdf:Description>

   <rdf:Description rdf:about="http://fakeIRI.edu/terms/electrosmd#e">
      <rdf:type rdf:resource="http://www.w3.org/2004/02/skos/core#Concept"/>
      <skos:inScheme rdf:resource="http://fakeIRI.edu/terms/electrosmd"/>
      <skos:prefLabel xml:lang="en">computer disc cartridge, type unspecified</skos:prefLabel>
      <skos:definition xml:lang="en">A disc cartridge whose type is not specified.</skos:definition>
      <skos:notation xml:lang="en">e</skos:notation>
   </rdf:Description>

   <rdf:Description rdf:about="http://fakeIRI.edu/terms/electrosmd#d">
      <rdf:type rdf:resource="http://www.w3.org/2004/02/skos/core#Concept"/>
      <skos:inScheme rdf:resource="http://fakeIRI.edu/terms/electrosmd"/>
      <skos:prefLabel xml:lang="en">computer disc, type unspecified</skos:prefLabel>
      <skos:definition xml:lang="en">A disc whose type is not specified.</skos:definition>
      <skos:notation xml:lang="en">d</skos:notation>
   </rdf:Description>

   <rdf:Description rdf:about="http://fakeIRI.edu/terms/electrosmd#c">
      <rdf:type rdf:resource="http://www.w3.org/2004/02/skos/core#Concept"/>
      <skos:inScheme rdf:resource="http://fakeIRI.edu/terms/electrosmd"/>
      <skos:prefLabel xml:lang="en">computer optical disc cartridge</skos:prefLabel>
      <skos:definition xml:lang="en">Removable module containing one or more nonmagnetic discs used
         to store digital information.</skos:definition>
      <skos:notation xml:lang="en">c</skos:notation>
   </rdf:Description>

   <rdf:Description rdf:about="http://fakeIRI.edu/terms/electrosmd#j">
      <rdf:type rdf:resource="http://www.w3.org/2004/02/skos/core#Concept"/>
      <skos:inScheme rdf:resource="http://fakeIRI.edu/terms/electrosmd"/>
      <skos:prefLabel xml:lang="en">magnetic disk</skos:prefLabel>
      <skos:definition xml:lang="en">Digital information storage medium usually consisting of a thin
         Mylar disk coated with a magnetic material that permits the recording of data. Magnetic
         disks come in various sizes. They are also known as floppy disks, stiffy disks, computer
         diskettes, or floppy diskettes.</skos:definition>
      <skos:notation xml:lang="en">j</skos:notation>
   </rdf:Description>

   <rdf:Description rdf:about="http://fakeIRI.edu/terms/electrosmd#m">
      <rdf:type rdf:resource="http://www.w3.org/2004/02/skos/core#Concept"/>
      <skos:inScheme rdf:resource="http://fakeIRI.edu/terms/electrosmd"/>
      <skos:prefLabel xml:lang="en">magneto-optical disc</skos:prefLabel>
      <skos:definition xml:lang="en">Erasable or semi-erasable storage medium, similar to a CD-ROM
         disc, capable of storing data at a very high density. The disc is written to and read from
         using a laser beam used to heat the recording surface to a point at which regions of the
         surface of the disk become magnetically aligned to store bits of data.</skos:definition>
      <skos:notation xml:lang="en">m</skos:notation>
   </rdf:Description>

   <rdf:Description rdf:about="http://fakeIRI.edu/terms/electrosmd#o">
      <rdf:type rdf:resource="http://www.w3.org/2004/02/skos/core#Concept"/>
      <skos:inScheme rdf:resource="http://fakeIRI.edu/terms/electrosmd"/>
      <skos:prefLabel xml:lang="en">optical disc</skos:prefLabel>
      <skos:definition xml:lang="en">Medium that uses a series of laser-burned micron-sized holes
         (pits) on a special recording surface to store data. Recorded data is read optically. These
         discs are usually a read-only medium.</skos:definition>
      <skos:scopeNote xml:lang="en">Commonly found computer optical disc formats include: CD-A,
         CD-I, CD-R, CD-ROM, CD-ROM-XA, DVD-ROM and Photo CD.</skos:scopeNote>
      <skos:notation xml:lang="en">o</skos:notation>
   </rdf:Description>

   <rdf:Description rdf:about="http://fakeIRI.edu/terms/electrosmd#z">
      <rdf:type rdf:resource="http://www.w3.org/2004/02/skos/core#Concept"/>
      <skos:inScheme rdf:resource="http://fakeIRI.edu/terms/electrosmd"/>
      <skos:prefLabel xml:lang="en">other</skos:prefLabel>
      <skos:definition xml:lang="en">Specific material designation other than tape cartridge, chip
         cartridge, computer optical disc cartridge, computer disc, type unspecified, computer disc
         cartridge, type unspecified, tape cassette, tape reel, magnetic disk, computer card,
         magneto-optical disc, optical disc, remote, or standalone device.</skos:definition>
      <skos:notation xml:lang="en">z</skos:notation>
   </rdf:Description>

   <rdf:Description rdf:about="http://fakeIRI.edu/terms/electrosmd#r">
      <rdf:type rdf:resource="http://www.w3.org/2004/02/skos/core#Concept"/>
      <skos:inScheme rdf:resource="http://fakeIRI.edu/terms/electrosmd"/>
      <skos:prefLabel xml:lang="en">remote</skos:prefLabel>
      <skos:definition xml:lang="en">Electronic resource that is accessed, processed, executed, etc.
         remotely. In this case the electronic resource is used via input/output devices connected
         electronically to a computer. Frequently this involves connection through a computer
         network.</skos:definition>
      <skos:notation xml:lang="en">r</skos:notation>
   </rdf:Description>

   <rdf:Description rdf:about="http://fakeIRI.edu/terms/electrosmd#s">
      <rdf:type rdf:resource="http://www.w3.org/2004/02/skos/core#Concept"/>
      <skos:inScheme rdf:resource="http://fakeIRI.edu/terms/electrosmd"/>
      <skos:prefLabel xml:lang="en">standalone device</skos:prefLabel>
      <skos:definition xml:lang="en">Consists of storage and reader components as an integrated
         standalone device. The data storage medium cannot be removed from the playback device with
         which it is issued. The data carried on the medium can only be read using the integrated
         special-purpose device.</skos:definition>
      <skos:notation xml:lang="en">s</skos:notation>
   </rdf:Description>

   <rdf:Description rdf:about="http://fakeIRI.edu/terms/electrosmd#a">
      <rdf:type rdf:resource="http://www.w3.org/2004/02/skos/core#Concept"/>
      <skos:inScheme rdf:resource="http://fakeIRI.edu/terms/electrosmd"/>
      <skos:prefLabel xml:lang="en">tape cartridge</skos:prefLabel>
      <skos:definition xml:lang="en">Removable module containing secondary storage medium such as
         magnetic tape or magnetic disks.</skos:definition>
      <skos:notation xml:lang="en">a</skos:notation>
   </rdf:Description>

   <rdf:Description rdf:about="http://fakeIRI.edu/terms/electrosmd#f">
      <rdf:type rdf:resource="http://www.w3.org/2004/02/skos/core#Concept"/>
      <skos:inScheme rdf:resource="http://fakeIRI.edu/terms/electrosmd"/>
      <skos:prefLabel xml:lang="en">tape cassette</skos:prefLabel>
      <skos:definition xml:lang="en">Removable module, somewhat like an audio cassette, that
         contains magnetic tape that can be written on and read from by a tape
         drive.</skos:definition>
      <skos:notation xml:lang="en">f</skos:notation>
   </rdf:Description>

   <rdf:Description rdf:about="http://fakeIRI.edu/terms/electrosmd#h">
      <rdf:type rdf:resource="http://www.w3.org/2004/02/skos/core#Concept"/>
      <skos:inScheme rdf:resource="http://fakeIRI.edu/terms/electrosmd"/>
      <skos:prefLabel xml:lang="en">tape reel</skos:prefLabel>
      <skos:definition xml:lang="en">Removable spool containing magnetic tape that can be written to
         and read from by a tape drive.</skos:definition>
      <skos:notation xml:lang="en">h</skos:notation>
   </rdf:Description>

   <rdf:Description rdf:about="http://fakeIRI.edu/terms/electrosmd#u">
      <rdf:type rdf:resource="http://www.w3.org/2004/02/skos/core#Concept"/>
      <skos:inScheme rdf:resource="http://fakeIRI.edu/terms/electrosmd"/>
      <skos:prefLabel xml:lang="en">unspecified</skos:prefLabel>
      <skos:definition xml:lang="en">Special material designation for the electronic resource is not
         specified.</skos:definition>
      <skos:scopeNote xml:lang="en">E.g., it may be an electronic resource that changes its medium
         over time.</skos:scopeNote>
      <skos:notation xml:lang="en">u</skos:notation>
   </rdf:Description>
</rdf:RDF>
