@prefix dc: <http://purl.org/dc/elements/1.1/> .
@prefix dct: <http://purl.org/dc/terms/> .
@prefix schema: <https://schema.org/> .
@prefix skos: <http://www.w3.org/2004/02/skos/core#> .

<https://doi.org/10.6069/uwlswd.x654-gd54#b> a skos:Concept ;
    skos:definition """Image is in black-and-white (usually
         black-and-transparent)."""@en ;
    skos:inScheme <https://doi.org/10.6069/uwlswd.x654-gd54> ;
    skos:notation "b" ;
    skos:prefLabel "black-and-white"@en ;
    skos:scopeNote """Includes only one color or hue other than black, for example,
         blue-and-white (blue-and-transparent). Always used for microopaques."""@en .

<https://doi.org/10.6069/uwlswd.x654-gd54#c> a skos:Concept ;
    skos:definition "Has more than one color."@en ;
    skos:inScheme <https://doi.org/10.6069/uwlswd.x654-gd54> ;
    skos:notation "c" ;
    skos:prefLabel "multicolored"@en .

<https://doi.org/10.6069/uwlswd.x654-gd54#m> a skos:Concept ;
    skos:definition """Combination of one-color and multicolored
         images."""@en ;
    skos:inScheme <https://doi.org/10.6069/uwlswd.x654-gd54> ;
    skos:notation "m" ;
    skos:prefLabel "mixed"@en .

<https://doi.org/10.6069/uwlswd.x654-gd54#u> a skos:Concept ;
    skos:definition "Color of the microform is not known."@en ;
    skos:inScheme <https://doi.org/10.6069/uwlswd.x654-gd54> ;
    skos:notation "u" ;
    skos:prefLabel "unknown"@en .

<https://doi.org/10.6069/uwlswd.x654-gd54#z> a skos:Concept ;
    skos:definition """Color other than black-and-white, multicolored, or
         mixed."""@en ;
    skos:inScheme <https://doi.org/10.6069/uwlswd.x654-gd54> ;
    skos:notation "z" ;
    skos:prefLabel "other"@en .

<https://doi.org/10.6069/uwlswd.x654-gd54> a skos:ConceptScheme ;
    dc:contributor "Metadata Management Associates"@en ;
    dc:language "en" ;
    dct:alternative """MARC21 007/09 values for microform expressed using
         RDF"""@en ;
    dct:contributor <http://viaf.org/viaf/151962300> ;
    dct:creator <http://viaf.org/viaf/139541794> ;
    dct:description "Color of the image for microforms."@en ;
    dct:format <http://www.w3.org/ns/formats/Turtle> ;
    dct:hasFormat <https://uwlib-cams.github.io/uwlswd_vocabs_marc_007/microform_color/microform_color.html>,
        <https://uwlib-cams.github.io/uwlswd_vocabs_marc_007/microform_color/microform_color.jsonld>,
        <https://uwlib-cams.github.io/uwlswd_vocabs_marc_007/microform_color/microform_color.nt>,
        <https://uwlib-cams.github.io/uwlswd_vocabs_marc_007/microform_color/microform_color.rdf> ;
    dct:issued "2024" ;
    dct:license <http://creativecommons.org/publicdomain/zero/1.0> ;
    dct:provenance <https://doi.org/10.6069/uwlswd.2e2b-y833#marc00Xvalues> ;
    dct:publisher <http://viaf.org/viaf/139541794> ;
    dct:source <http://marc21rdf.info>,
        <https://www.loc.gov/marc/bibliographic/bd007.html> ;
    dct:title "Microform: color"@en ;
    dct:type <http://purl.org/dc/dcmitype/Dataset> ;
    schema:disambiguatingDescription """SKOS Concept Scheme for MARC 00X
         Values"""@en ;
    schema:version "1-0-0" .

