<?xml version="1.0" encoding="utf-8"?>
<rdf:RDF
   xmlns:dc="http://purl.org/dc/elements/1.1/"
   xmlns:dct="http://purl.org/dc/terms/"
   xmlns:rdf="http://www.w3.org/1999/02/22-rdf-syntax-ns#"
   xmlns:schema="https://schema.org/"
   xmlns:skos="http://www.w3.org/2004/02/skos/core#"
>
  <rdf:Description rdf:about="http://fakeIRI.edu/terms/tactilecla#e">
    <rdf:type rdf:resource="http://www.w3.org/2004/02/skos/core#Concept"/>
    <skos:inScheme rdf:resource="http://fakeIRI.edu/terms/tactilecla"/>
    <skos:prefLabel xml:lang="en">music braille</skos:prefLabel>
    <skos:definition xml:lang="en">Braille representations for symbols used in notated
         music.</skos:definition>
    <skos:notation xml:lang="en">e</skos:notation>
  </rdf:Description>
  <rdf:Description rdf:about="http://fakeIRI.edu/terms/tactilecla#c">
    <rdf:type rdf:resource="http://www.w3.org/2004/02/skos/core#Concept"/>
    <skos:inScheme rdf:resource="http://fakeIRI.edu/terms/tactilecla"/>
    <skos:prefLabel xml:lang="en">mathematics and scientific braille</skos:prefLabel>
    <skos:definition xml:lang="en">Braille representations for symbols employed in mathematics and
         scientific writing.</skos:definition>
    <skos:notation xml:lang="en">c</skos:notation>
  </rdf:Description>
  <rdf:Description rdf:about="http://fakeIRI.edu/terms/tactilecla#u">
    <rdf:type rdf:resource="http://www.w3.org/2004/02/skos/core#Concept"/>
    <skos:inScheme rdf:resource="http://fakeIRI.edu/terms/tactilecla"/>
    <skos:prefLabel xml:lang="en">unknown</skos:prefLabel>
    <skos:definition xml:lang="en">Class of braille writing is not known.</skos:definition>
    <skos:notation xml:lang="en">u</skos:notation>
  </rdf:Description>
  <rdf:Description rdf:about="http://fakeIRI.edu/terms/tactilecla">
    <rdf:type rdf:resource="http://www.w3.org/2004/02/skos/core#ConceptScheme"/>
    <dct:type rdf:resource="http://purl.org/dc/dcmitype/Dataset"/>
    <dct:title xml:lang="en">Tactile material: class of braille writing</dct:title>
    <dct:alternative xml:lang="en">MARC21 007/03-04 values for tactile material expressed using
         RDF</dct:alternative>
    <dct:description xml:lang="en">Family of braille to which the item belongs. This is not the
         particular braille code, but the type of braille code used, representing different types of
         written symbols.</dct:description>
    <schema:disambiguatingDescription>SKOS Concept Scheme for MARC 00X
         Values</schema:disambiguatingDescription>
    <dct:publisher rdf:resource="http://viaf.org/viaf/139541794"/>
    <dct:source rdf:resource="https://www.loc.gov/marc/bibliographic/bd007.html"/>
    <dct:source rdf:resource="http://marc21rdf.info"/>
    <dct:provenance rdf:resource="https://doi.org/10.6069/uwlswd.2e2b-y833"/>
    <dct:creator rdf:resource="http://viaf.org/viaf/139541794"/>
    <dct:contributor rdf:resource="http://viaf.org/viaf/151962300"/>
    <dct:issued>2024</dct:issued>
    <dc:contributor xml:lang="en">Metadata Management Associates</dc:contributor>
    <dc:language>en</dc:language>
    <dct:license rdf:resource="http://creativecommons.org/publicdomain/zero/1.0"/>
    <schema:version>1-0-0</schema:version>
    <dct:format rdf:resource="http://www.w3.org/ns/formats/RDF_XML"/>
  </rdf:Description>
  <rdf:Description rdf:about="http://fakeIRI.edu/terms/tactilecla#z">
    <rdf:type rdf:resource="http://www.w3.org/2004/02/skos/core#Concept"/>
    <skos:inScheme rdf:resource="http://fakeIRI.edu/terms/tactilecla"/>
    <skos:prefLabel xml:lang="en">other</skos:prefLabel>
    <skos:definition xml:lang="en">Class of braille writing other than no specified class of
         braille writing, literary braille, format code braille, mathematics and scientific braille,
         computer braille, music braille, or multiple braille types.</skos:definition>
    <skos:notation xml:lang="en">z</skos:notation>
  </rdf:Description>
  <rdf:Description rdf:about="http://fakeIRI.edu/terms/tactilecla#m">
    <rdf:type rdf:resource="http://www.w3.org/2004/02/skos/core#Concept"/>
    <skos:inScheme rdf:resource="http://fakeIRI.edu/terms/tactilecla"/>
    <skos:prefLabel xml:lang="en">multiple braille types</skos:prefLabel>
    <skos:definition xml:lang="en">Multiple braille types exist and no one type
         predominates.</skos:definition>
    <skos:notation xml:lang="en">m</skos:notation>
  </rdf:Description>
  <rdf:Description rdf:about="http://fakeIRI.edu/terms/tactilecla#a">
    <rdf:type rdf:resource="http://www.w3.org/2004/02/skos/core#Concept"/>
    <skos:inScheme rdf:resource="http://fakeIRI.edu/terms/tactilecla"/>
    <skos:prefLabel xml:lang="en">literary braille</skos:prefLabel>
    <skos:definition xml:lang="en">Braille representation for the alphabet, numbers, and
         punctuation marks commonly used in general writing.</skos:definition>
    <skos:notation xml:lang="en">a</skos:notation>
  </rdf:Description>
  <rdf:Description rdf:about="http://fakeIRI.edu/terms/tactilecla#d">
    <rdf:type rdf:resource="http://www.w3.org/2004/02/skos/core#Concept"/>
    <skos:inScheme rdf:resource="http://fakeIRI.edu/terms/tactilecla"/>
    <skos:prefLabel xml:lang="en">computer braille</skos:prefLabel>
    <skos:definition xml:lang="en">Braille representations for symbols used in computer programs,
         texts, and other computer related materials.</skos:definition>
    <skos:notation xml:lang="en">d</skos:notation>
  </rdf:Description>
  <rdf:Description rdf:about="http://fakeIRI.edu/terms/tactilecla#b">
    <rdf:type rdf:resource="http://www.w3.org/2004/02/skos/core#Concept"/>
    <skos:inScheme rdf:resource="http://fakeIRI.edu/terms/tactilecla"/>
    <skos:prefLabel xml:lang="en">format code braille</skos:prefLabel>
    <skos:definition xml:lang="en">Braille formatting rules for textbooks and related
         materials.</skos:definition>
    <skos:notation xml:lang="en">b</skos:notation>
  </rdf:Description>
  <rdf:Description rdf:about="http://fakeIRI.edu/terms/tactilecla##">
    <rdf:type rdf:resource="http://www.w3.org/2004/02/skos/core#Concept"/>
    <skos:inScheme rdf:resource="http://fakeIRI.edu/terms/tactilecla"/>
    <skos:prefLabel xml:lang="en">no specified class of braille writing</skos:prefLabel>
    <skos:definition xml:lang="en">Item consists of fewer than two specified classes of braille
         writing.</skos:definition>
    <skos:notation xml:lang="en">#</skos:notation>
  </rdf:Description>
  <rdf:Description rdf:about="http://fakeIRI.edu/terms/tactilecla#n">
    <rdf:type rdf:resource="http://www.w3.org/2004/02/skos/core#Concept"/>
    <skos:inScheme rdf:resource="http://fakeIRI.edu/terms/tactilecla"/>
    <skos:prefLabel xml:lang="en">not applicable</skos:prefLabel>
    <skos:definition xml:lang="en">Item is not braille.</skos:definition>
    <skos:notation xml:lang="en">n</skos:notation>
  </rdf:Description>
</rdf:RDF>
