<?xml version="1.0" encoding="UTF-8"?><rdf:RDF xmlns:dc="http://purl.org/dc/elements/1.1/" xmlns:dct="http://purl.org/dc/terms/" xmlns:rdf="http://www.w3.org/1999/02/22-rdf-syntax-ns#" xmlns:rdfs="http://www.w3.org/2000/01/rdf-schema#" xmlns:schema="https://schema.org/" xmlns:skos="http://www.w3.org/2004/02/skos/core#" xmlns:uw="https://www.lib.washington.edu/static/public/cams/data/localResources/properties_local.html" xmlns:uwp="https://doi.org/10.6069/uwlib.55.d.3#">


   <rdf:Description rdf:about="http://fakeIRI.edu/terms/mapmed"><rdf:type rdf:resource="http://www.w3.org/2004/02/skos/core#ConceptScheme"/><dct:type rdf:resource="http://purl.org/dc/dcmitype/Dataset"/><dct:title xml:lang="en">Map: physical medium</dct:title><dct:alternative xml:lang="en">MARC21 007/04 values for maps expressed using RDF</dct:alternative><dct:description xml:lang="en">Material out of which the cartographic item is made.</dct:description><schema:disambiguatingDescription>SKOS Concept Scheme for MARC 00X Values</schema:disambiguatingDescription><dct:publisher rdf:resource="http://viaf.org/viaf/139541794"/><dct:source rdf:resource="https://www.loc.gov/marc/bibliographic/bd007.html"/><dct:source rdf:resource="http://marc21rdf.info"/><dct:provenance rdf:resource="https://doi.org/10.6069/uwlswd.2e2b-y833"/><dct:creator rdf:resource="http://viaf.org/viaf/139541794"/><dct:contributor rdf:resource="http://viaf.org/viaf/151962300"/><dct:issued>2024</dct:issued><dc:contributor xml:lang="en">Metadata Management Associates</dc:contributor><dc:language>en</dc:language><dct:license rdf:resource="http://creativecommons.org/publicdomain/zero/1.0"/><schema:version>1-0-0</schema:version><dct:issued>2024</dct:issued><dct:format rdf:resource="http://www.w3.org/ns/formats/RDF_XML"/></rdf:Description>
   
   <rdf:Description rdf:about="http://fakeIRI.edu/terms/mapmed#r"><rdf:type rdf:resource="http://www.w3.org/2004/02/skos/core#Concept"/><skos:inScheme rdf:resource="http://fakeIRI.edu/terms/mapmed"/><skos:prefLabel xml:lang="en">flexible base photographic, negative</skos:prefLabel><skos:definition xml:lang="en">Flexible base photographic medium designed to render a negative image.</skos:definition><skos:notation xml:lang="en">r</skos:notation></rdf:Description>
   
   <rdf:Description rdf:about="http://fakeIRI.edu/terms/mapmed#q"><rdf:type rdf:resource="http://www.w3.org/2004/02/skos/core#Concept"/><skos:inScheme rdf:resource="http://fakeIRI.edu/terms/mapmed"/><skos:prefLabel xml:lang="en">flexible base photographic, positive</skos:prefLabel><skos:definition xml:lang="en">Flexible base photographic medium designed to render a positive image.</skos:definition><skos:notation xml:lang="en">q</skos:notation></rdf:Description>
   
   <rdf:Description rdf:about="http://fakeIRI.edu/terms/mapmed#j"><rdf:type rdf:resource="http://www.w3.org/2004/02/skos/core#Concept"/><skos:inScheme rdf:resource="http://fakeIRI.edu/terms/mapmed"/><skos:prefLabel xml:lang="en">glass</skos:prefLabel><skos:definition xml:lang="en">Glass.</skos:definition><skos:notation xml:lang="en">j</skos:notation></rdf:Description>
   
   <rdf:Description rdf:about="http://fakeIRI.edu/terms/mapmed#v"><rdf:type rdf:resource="http://www.w3.org/2004/02/skos/core#Concept"/><skos:inScheme rdf:resource="http://fakeIRI.edu/terms/mapmed"/><skos:prefLabel xml:lang="en">leather</skos:prefLabel><skos:definition xml:lang="en">Animal skin dressed for use.</skos:definition><skos:notation xml:lang="en">v</skos:notation></rdf:Description>
   
   <rdf:Description rdf:about="http://fakeIRI.edu/terms/mapmed#d"><rdf:type rdf:resource="http://www.w3.org/2004/02/skos/core#Concept"/><skos:inScheme rdf:resource="http://fakeIRI.edu/terms/mapmed"/><skos:prefLabel xml:lang="en">metal</skos:prefLabel><skos:definition xml:lang="en">Metal.</skos:definition><skos:notation xml:lang="en">d</skos:notation></rdf:Description>
   
   <rdf:Description rdf:about="http://fakeIRI.edu/terms/mapmed#t"><rdf:type rdf:resource="http://www.w3.org/2004/02/skos/core#Concept"/><skos:inScheme rdf:resource="http://fakeIRI.edu/terms/mapmed"/><skos:prefLabel xml:lang="en">non-flexible base photographic, negative</skos:prefLabel><skos:definition xml:lang="en">Non-flexible base photographic medium designed to render a negative image.</skos:definition><skos:notation xml:lang="en">t</skos:notation></rdf:Description>
   
   <rdf:Description rdf:about="http://fakeIRI.edu/terms/mapmed#s"><rdf:type rdf:resource="http://www.w3.org/2004/02/skos/core#Concept"/><skos:inScheme rdf:resource="http://fakeIRI.edu/terms/mapmed"/><skos:prefLabel xml:lang="en">non-flexible base photographic, positive</skos:prefLabel><skos:definition xml:lang="en">Non-flexible base photographic medium designed to render a positive image.</skos:definition><skos:notation xml:lang="en">s</skos:notation></rdf:Description>
   
   <rdf:Description rdf:about="http://fakeIRI.edu/terms/mapmed#z"><rdf:type rdf:resource="http://www.w3.org/2004/02/skos/core#Concept"/><skos:inScheme rdf:resource="http://fakeIRI.edu/terms/mapmed"/><skos:prefLabel xml:lang="en">other</skos:prefLabel><skos:definition xml:lang="en">Physical medium other than paper; wood; stone; metal; synthetic; skin; textile; plastic; glass; vinyl; vellum; plaster; flexible base photographic, positive; flexible base photographic, negative; non-flexible base photographic, positive; non-flexible base photographic, negative; leather; parchment; or other photographic medium.</skos:definition><skos:notation xml:lang="en">z</skos:notation></rdf:Description>
   
   <rdf:Description rdf:about="http://fakeIRI.edu/terms/mapmed#y"><rdf:type rdf:resource="http://www.w3.org/2004/02/skos/core#Concept"/><skos:inScheme rdf:resource="http://fakeIRI.edu/terms/mapmed"/><skos:prefLabel xml:lang="en">other photographic medium</skos:prefLabel><skos:definition xml:lang="en">Photographic medium other than flexible base photographic, positive; flexible base photographic, negative; non-flexible base photographic, positive; or non-flexible base photographic, negative.</skos:definition><skos:notation xml:lang="en">y</skos:notation></rdf:Description>
   
   <rdf:Description rdf:about="http://fakeIRI.edu/terms/mapmed#a"><rdf:type rdf:resource="http://www.w3.org/2004/02/skos/core#Concept"/><skos:inScheme rdf:resource="http://fakeIRI.edu/terms/mapmed"/><skos:prefLabel xml:lang="en">paper</skos:prefLabel><skos:definition xml:lang="en">Any kind of cellulose-based paper.</skos:definition><skos:notation xml:lang="en">a</skos:notation></rdf:Description>
   
   <rdf:Description rdf:about="http://fakeIRI.edu/terms/mapmed#w"><rdf:type rdf:resource="http://www.w3.org/2004/02/skos/core#Concept"/><skos:inScheme rdf:resource="http://fakeIRI.edu/terms/mapmed"/><skos:prefLabel xml:lang="en">parchment</skos:prefLabel><skos:definition xml:lang="en">Skin of a sheep or goat prepared for writing on.</skos:definition><skos:notation xml:lang="en">w</skos:notation></rdf:Description>
   
   <rdf:Description rdf:about="http://fakeIRI.edu/terms/mapmed#x"><rdf:type rdf:resource="http://www.w3.org/2004/02/skos/core#Concept"/><skos:inScheme rdf:resource="http://fakeIRI.edu/terms/mapmed"/><skos:prefLabel xml:lang="en">not applicable</skos:prefLabel><skos:definition xml:lang="en">Physical medium is not applicable to remote digital cartographic resources because it pertains to characteristics specific to physical aspects of carriers.</skos:definition><skos:notation xml:lang="en">x</skos:notation></rdf:Description>
   
   <rdf:Description rdf:about="http://fakeIRI.edu/terms/mapmed#p"><rdf:type rdf:resource="http://www.w3.org/2004/02/skos/core#Concept"/><skos:inScheme rdf:resource="http://fakeIRI.edu/terms/mapmed"/><skos:prefLabel xml:lang="en">plaster</skos:prefLabel><skos:definition xml:lang="en">Plaster.</skos:definition><skos:scopeNote xml:lang="en">Includes mixtures of ground solids and plaster.</skos:scopeNote><skos:notation xml:lang="en">p</skos:notation></rdf:Description>
   
   <rdf:Description rdf:about="http://fakeIRI.edu/terms/mapmed#i"><rdf:type rdf:resource="http://www.w3.org/2004/02/skos/core#Concept"/><skos:inScheme rdf:resource="http://fakeIRI.edu/terms/mapmed"/><skos:prefLabel xml:lang="en">plastic</skos:prefLabel><skos:definition xml:lang="en">Plastic.</skos:definition><skos:notation xml:lang="en">i</skos:notation></rdf:Description>
   
   <rdf:Description rdf:about="http://fakeIRI.edu/terms/mapmed#f"><rdf:type rdf:resource="http://www.w3.org/2004/02/skos/core#Concept"/><skos:inScheme rdf:resource="http://fakeIRI.edu/terms/mapmed"/><skos:prefLabel xml:lang="en">skin</skos:prefLabel><skos:definition xml:lang="en">Skin.</skos:definition><skos:scopeNote xml:lang="en">Excludes leather, parchment, and vellum.</skos:scopeNote><skos:scopeNote xml:lang="en">Synthetic materials that are made to resemble animal skin are coded as synthetic.</skos:scopeNote><skos:notation xml:lang="en">f</skos:notation></rdf:Description>
   
   <rdf:Description rdf:about="http://fakeIRI.edu/terms/mapmed#c"><rdf:type rdf:resource="http://www.w3.org/2004/02/skos/core#Concept"/><skos:inScheme rdf:resource="http://fakeIRI.edu/terms/mapmed"/><skos:prefLabel xml:lang="en">stone</skos:prefLabel><skos:definition xml:lang="en">Stone.</skos:definition><skos:notation xml:lang="en">c</skos:notation></rdf:Description>
   
   <rdf:Description rdf:about="http://fakeIRI.edu/terms/mapmed#e"><rdf:type rdf:resource="http://www.w3.org/2004/02/skos/core#Concept"/><skos:inScheme rdf:resource="http://fakeIRI.edu/terms/mapmed"/><skos:prefLabel xml:lang="en">synthetic</skos:prefLabel><skos:definition xml:lang="en">Man-made substances other than textiles, plastic, and vinyl.</skos:definition><skos:notation xml:lang="en">e</skos:notation></rdf:Description>
   
   <rdf:Description rdf:about="http://fakeIRI.edu/terms/mapmed#g"><rdf:type rdf:resource="http://www.w3.org/2004/02/skos/core#Concept"/><skos:inScheme rdf:resource="http://fakeIRI.edu/terms/mapmed"/><skos:prefLabel xml:lang="en">textile</skos:prefLabel><skos:definition xml:lang="en">Textile.</skos:definition><skos:scopeNote xml:lang="en">Used for all fabrics, whether made from natural or synthetic fibers.</skos:scopeNote><skos:notation xml:lang="en">g</skos:notation></rdf:Description>
   
   <rdf:Description rdf:about="http://fakeIRI.edu/terms/mapmed#u"><rdf:type rdf:resource="http://www.w3.org/2004/02/skos/core#Concept"/><skos:inScheme rdf:resource="http://fakeIRI.edu/terms/mapmed"/><skos:prefLabel xml:lang="en">unknown</skos:prefLabel><skos:definition xml:lang="en">Unknown.</skos:definition><skos:notation xml:lang="en">u</skos:notation></rdf:Description>
   
   <rdf:Description rdf:about="http://fakeIRI.edu/terms/mapmed#n"><rdf:type rdf:resource="http://www.w3.org/2004/02/skos/core#Concept"/><skos:inScheme rdf:resource="http://fakeIRI.edu/terms/mapmed"/><skos:prefLabel xml:lang="en">vellum</skos:prefLabel><skos:definition xml:lang="en">Fine-grained unsplit lambskin, kidskin, or calfskin prepared especially for writing or drawing on.</skos:definition><skos:notation xml:lang="en">n</skos:notation></rdf:Description>
   
   <rdf:Description rdf:about="http://fakeIRI.edu/terms/mapmed#l"><rdf:type rdf:resource="http://www.w3.org/2004/02/skos/core#Concept"/><skos:inScheme rdf:resource="http://fakeIRI.edu/terms/mapmed"/><skos:prefLabel xml:lang="en">vinyl</skos:prefLabel><skos:definition xml:lang="en">Vinyl.</skos:definition><skos:notation xml:lang="en">l</skos:notation></rdf:Description>
   
   <rdf:Description rdf:about="http://fakeIRI.edu/terms/mapmed#b"><rdf:type rdf:resource="http://www.w3.org/2004/02/skos/core#Concept"/><skos:inScheme rdf:resource="http://fakeIRI.edu/terms/mapmed"/><skos:prefLabel xml:lang="en">wood</skos:prefLabel><skos:scopeNote xml:lang="en">Material which is based on wood particles or fibers may or may not be considered wood. Consider particle board to be wood.</skos:scopeNote><skos:notation xml:lang="en">b</skos:notation></rdf:Description>
</rdf:RDF>