@prefix dc: <http://purl.org/dc/elements/1.1/> .
@prefix dct: <http://purl.org/dc/terms/> .
@prefix schema: <https://schema.org/> .
@prefix skos: <http://www.w3.org/2004/02/skos/core#> .

<https://doi.org/10.6069/uwlswd.s0ms-4p29#a> a skos:Concept ;
    skos:definition """File(s) which comprise(s)the electronic resource are of the
         same format or type."""@en ;
    skos:inScheme <https://doi.org/10.6069/uwlswd.s0ms-4p29> ;
    skos:notation "a" ;
    skos:prefLabel "one file format"@en ;
    skos:scopeNote """E.g., all .jpg; all .tif; all .txt; all .wav; all .mpg;
         etc."""@en .

<https://doi.org/10.6069/uwlswd.s0ms-4p29#m> a skos:Concept ;
    skos:definition """Files which comprise the electronic resource are of at least 2
         different formats."""@en ;
    skos:inScheme <https://doi.org/10.6069/uwlswd.s0ms-4p29> ;
    skos:notation "m" ;
    skos:prefLabel "multiple file formats"@en ;
    skos:scopeNote """E.g., .jpg and .tif; .tif and .txt; .sgml and .wav;
         etc."""@en .

<https://doi.org/10.6069/uwlswd.s0ms-4p29#u> a skos:Concept ;
    skos:definition """Format(s) of the file(s) which comprise(s) the electronic
         resource are not known."""@en ;
    skos:inScheme <https://doi.org/10.6069/uwlswd.s0ms-4p29> ;
    skos:notation "u" ;
    skos:prefLabel "unknown"@en .

<https://doi.org/10.6069/uwlswd.s0ms-4p29> a skos:ConceptScheme ;
    dc:contributor "Metadata Management Associates"@en ;
    dc:language "en" ;
    dct:alternative """MARC21 007/09 values for electronic resources expressed using
         RDF"""@en ;
    dct:contributor <http://viaf.org/viaf/151962300> ;
    dct:creator <http://viaf.org/viaf/139541794> ;
    dct:description """Whether the file(s) which comprise the electronic resource are
         of the same format or type for digitally reformatted materials."""@en ;
    dct:format <http://www.w3.org/ns/formats/Turtle> ;
    dct:hasFormat <https://uwlib-cams.github.io/uwlswd_vocabs_marc_007/electronic_resource_file_formats/electronic_resource_file_formats.html>,
        <https://uwlib-cams.github.io/uwlswd_vocabs_marc_007/electronic_resource_file_formats/electronic_resource_file_formats.jsonld>,
        <https://uwlib-cams.github.io/uwlswd_vocabs_marc_007/electronic_resource_file_formats/electronic_resource_file_formats.nt>,
        <https://uwlib-cams.github.io/uwlswd_vocabs_marc_007/electronic_resource_file_formats/electronic_resource_file_formats.rdf> ;
    dct:issued "2024" ;
    dct:license <http://creativecommons.org/publicdomain/zero/1.0> ;
    dct:provenance <https://doi.org/10.6069/uwlswd.2e2b-y833#marc00Xvalues> ;
    dct:publisher <http://viaf.org/viaf/139541794> ;
    dct:source <http://marc21rdf.info>,
        <https://www.loc.gov/marc/bibliographic/bd007.html> ;
    dct:title "Electronic resouce: file formats"@en ;
    dct:type <http://purl.org/dc/dcmitype/Dataset> ;
    schema:disambiguatingDescription """SKOS Concept Scheme for MARC 00X
         Values"""@en ;
    schema:version "1-0-0" .

