<?xml version="1.0" encoding="utf-8"?>
<rdf:RDF
   xmlns:dc="http://purl.org/dc/elements/1.1/"
   xmlns:dct="http://purl.org/dc/terms/"
   xmlns:rdf="http://www.w3.org/1999/02/22-rdf-syntax-ns#"
   xmlns:schema="https://schema.org/"
   xmlns:skos="http://www.w3.org/2004/02/skos/core#"
>
  <rdf:Description rdf:about="https://doi.org/10.6069/uwlswd.s0ms-4p29">
    <rdf:type rdf:resource="http://www.w3.org/2004/02/skos/core#ConceptScheme"/>
    <dct:type rdf:resource="http://purl.org/dc/dcmitype/Dataset"/>
    <dct:title xml:lang="en">Electronic resouce: file formats</dct:title>
    <dct:alternative xml:lang="en">MARC21 007/09 values for electronic resources expressed using
         RDF</dct:alternative>
    <dct:description xml:lang="en">Whether the file(s) which comprise the electronic resource are
         of the same format or type for digitally reformatted materials.</dct:description>
    <schema:disambiguatingDescription>SKOS Concept Scheme for MARC 00X
         Values</schema:disambiguatingDescription>
    <dct:publisher rdf:resource="http://viaf.org/viaf/139541794"/>
    <dct:source rdf:resource="https://www.loc.gov/marc/bibliographic/bd007.html"/>
    <dct:source rdf:resource="http://marc21rdf.info"/>
    <dct:provenance rdf:resource="https://doi.org/10.6069/uwlswd.2e2b-y833"/>
    <dct:creator rdf:resource="http://viaf.org/viaf/139541794"/>
    <dct:contributor rdf:resource="http://viaf.org/viaf/151962300"/>
    <dct:issued>2024</dct:issued>
    <dc:contributor xml:lang="en">Metadata Management Associates</dc:contributor>
    <dc:language>en</dc:language>
    <dct:license rdf:resource="http://creativecommons.org/publicdomain/zero/1.0"/>
    <schema:version>1-0-0</schema:version>
    <dct:format rdf:resource="http://www.w3.org/ns/formats/RDF_XML"/>
  </rdf:Description>
  <rdf:Description rdf:about="https://doi.org/10.6069/uwlswd.s0ms-4p29#a">
    <rdf:type rdf:resource="http://www.w3.org/2004/02/skos/core#Concept"/>
    <skos:inScheme rdf:resource="https://doi.org/10.6069/uwlswd.s0ms-4p29"/>
    <skos:prefLabel xml:lang="en">one file format</skos:prefLabel>
    <skos:definition xml:lang="en">File(s) which comprise(s)the electronic resource are of the
         same format or type.</skos:definition>
    <skos:scopeNote xml:lang="en">E.g., all .jpg; all .tif; all .txt; all .wav; all .mpg;
         etc.</skos:scopeNote>
    <skos:notation xml:lang="en">a</skos:notation>
  </rdf:Description>
  <rdf:Description rdf:about="https://doi.org/10.6069/uwlswd.s0ms-4p29#m">
    <rdf:type rdf:resource="http://www.w3.org/2004/02/skos/core#Concept"/>
    <skos:inScheme rdf:resource="https://doi.org/10.6069/uwlswd.s0ms-4p29"/>
    <skos:prefLabel xml:lang="en">multiple file formats</skos:prefLabel>
    <skos:definition xml:lang="en">Files which comprise the electronic resource are of at least 2
         different formats.</skos:definition>
    <skos:scopeNote xml:lang="en">E.g., .jpg and .tif; .tif and .txt; .sgml and .wav;
         etc.</skos:scopeNote>
    <skos:notation xml:lang="en">m</skos:notation>
  </rdf:Description>
  <rdf:Description rdf:about="https://doi.org/10.6069/uwlswd.s0ms-4p29#u">
    <rdf:type rdf:resource="http://www.w3.org/2004/02/skos/core#Concept"/>
    <skos:inScheme rdf:resource="https://doi.org/10.6069/uwlswd.s0ms-4p29"/>
    <skos:prefLabel xml:lang="en">unknown</skos:prefLabel>
    <skos:definition xml:lang="en">Format(s) of the file(s) which comprise(s) the electronic
         resource are not known.</skos:definition>
    <skos:notation xml:lang="en">u</skos:notation>
  </rdf:Description>
</rdf:RDF>
