@prefix dc: <http://purl.org/dc/elements/1.1/> .
@prefix dct: <http://purl.org/dc/terms/> .
@prefix schema: <https://schema.org/> .
@prefix skos: <http://www.w3.org/2004/02/skos/core#> .

<https://doi.org/10.6069/uwlswd.xrxa-qa70#a> a skos:Concept ;
    skos:definition """Model relating to the sky of visible heavens (sun, stars, etc.)
         depicted on the surface of a sphere."""@en ;
    skos:inScheme <https://doi.org/10.6069/uwlswd.xrxa-qa70> ;
    skos:notation "a" ;
    skos:prefLabel "celestial globe"@en .

<https://doi.org/10.6069/uwlswd.xrxa-qa70#b> a skos:Concept ;
    skos:definition """Lunar globe (other than Earth's moon) or a moon depicted on the
         surface of a sphere."""@en ;
    skos:inScheme <https://doi.org/10.6069/uwlswd.xrxa-qa70> ;
    skos:notation "b" ;
    skos:prefLabel "planetary or lunar globe"@en .

<https://doi.org/10.6069/uwlswd.xrxa-qa70#c> a skos:Concept ;
    skos:definition """Model of the Earth depicted on the surface of a
         sphere."""@en ;
    skos:inScheme <https://doi.org/10.6069/uwlswd.xrxa-qa70> ;
    skos:notation "c" ;
    skos:prefLabel "terrestrial globe"@en .

<https://doi.org/10.6069/uwlswd.xrxa-qa70#d> a skos:Concept ;
    skos:inScheme <https://doi.org/10.6069/uwlswd.xrxa-qa70> ;
    skos:notation "d" ;
    skos:prefLabel """satellite globe (of our solar system), excluding the earth moon
         [obsolete]"""@en .

<https://doi.org/10.6069/uwlswd.xrxa-qa70#e> a skos:Concept ;
    skos:definition """Model of the Earth's moon depicted on the surface of a
         sphere."""@en ;
    skos:inScheme <https://doi.org/10.6069/uwlswd.xrxa-qa70> ;
    skos:notation "e" ;
    skos:prefLabel "earth moon globe"@en .

<https://doi.org/10.6069/uwlswd.xrxa-qa70#u> a skos:Concept ;
    skos:inScheme <https://doi.org/10.6069/uwlswd.xrxa-qa70> ;
    skos:notation "u" ;
    skos:prefLabel "unspecified"@en .

<https://doi.org/10.6069/uwlswd.xrxa-qa70#z> a skos:Concept ;
    skos:definition """Specific material designation other than celestial globe,
         planetary or lunar globe, terrestrial globe, Earth moon globe."""@en ;
    skos:inScheme <https://doi.org/10.6069/uwlswd.xrxa-qa70> ;
    skos:notation "z" ;
    skos:prefLabel "other"@en .

<https://doi.org/10.6069/uwlswd.xrxa-qa70> a skos:ConceptScheme ;
    dc:contributor "Metadata Management Associates"@en ;
    dc:language "en" ;
    dct:alternative """MARC21 007/01 values for globes expressed using
         RDF"""@en ;
    dct:contributor <http://viaf.org/viaf/151962300> ;
    dct:creator <http://viaf.org/viaf/139541794> ;
    dct:description """Special class of material (usually the class of physical
         object) to which an item belongs, e.g., a celestial globe."""@en ;
    dct:format <http://www.w3.org/ns/formats/Turtle> ;
    dct:hasFormat <https://uwlib-cams.github.io/uwlswd_vocabs_marc_007/globe_specific_material_designation/globe_specific_material_designation.html>,
        <https://uwlib-cams.github.io/uwlswd_vocabs_marc_007/globe_specific_material_designation/globe_specific_material_designation.jsonld>,
        <https://uwlib-cams.github.io/uwlswd_vocabs_marc_007/globe_specific_material_designation/globe_specific_material_designation.nt>,
        <https://uwlib-cams.github.io/uwlswd_vocabs_marc_007/globe_specific_material_designation/globe_specific_material_designation.rdf> ;
    dct:issued "2024" ;
    dct:license <http://creativecommons.org/publicdomain/zero/1.0> ;
    dct:provenance <https://doi.org/10.6069/uwlswd.2e2b-y833#marc00Xvalues> ;
    dct:publisher <http://viaf.org/viaf/139541794> ;
    dct:source <http://marc21rdf.info>,
        <https://www.loc.gov/marc/bibliographic/bd007.html> ;
    dct:title "Globe: specific material designation"@en ;
    dct:type <http://purl.org/dc/dcmitype/Dataset> ;
    schema:disambiguatingDescription """SKOS Concept Scheme for MARC 00X
         Values"""@en ;
    schema:version "1-0-0" .

