<?xml version="1.0" encoding="UTF-8"?><rdf:RDF xmlns:dc="http://purl.org/dc/elements/1.1/" xmlns:dct="http://purl.org/dc/terms/" xmlns:rdf="http://www.w3.org/1999/02/22-rdf-syntax-ns#" xmlns:rdfs="http://www.w3.org/2000/01/rdf-schema#" xmlns:schema="https://schema.org/" xmlns:skos="http://www.w3.org/2004/02/skos/core#" xmlns:uw="https://www.lib.washington.edu/static/public/cams/data/localResources/properties_local.html" xmlns:uwp="https://doi.org/10.6069/uwlib.55.d.3#">


   <rdf:Description rdf:about="http://fakeIRI.edu/terms/soundrecordingtap"><rdf:type rdf:resource="http://www.w3.org/2004/02/skos/core#ConceptScheme"/><dct:type rdf:resource="http://purl.org/dc/dcmitype/Dataset"/><dct:title xml:lang="en">Sound recording: tape configuration</dct:title><dct:alternative xml:lang="en">MARC21 007/08 values for sound recordings expressed using RDF</dct:alternative><dct:description xml:lang="en">Number of tracks on a tape.</dct:description><schema:disambiguatingDescription>SKOS Concept Scheme for MARC 00X Values</schema:disambiguatingDescription><dct:publisher rdf:resource="http://viaf.org/viaf/139541794"/><dct:source rdf:resource="https://www.loc.gov/marc/bibliographic/bd007.html"/><dct:source rdf:resource="http://marc21rdf.info"/><dct:provenance rdf:resource="https://doi.org/10.6069/uwlswd.2e2b-y833"/><dct:creator rdf:resource="http://viaf.org/viaf/139541794"/><dct:contributor rdf:resource="http://viaf.org/viaf/151962300"/><dct:issued>2024</dct:issued><dc:contributor xml:lang="en">Metadata Management Associates</dc:contributor><dc:language>en</dc:language><dct:license rdf:resource="http://creativecommons.org/publicdomain/zero/1.0"/><schema:version>1-0-0</schema:version><dct:issued>2024</dct:issued><dct:format rdf:resource="http://www.w3.org/ns/formats/RDF_XML"/></rdf:Description>
   
   <rdf:Description rdf:about="http://fakeIRI.edu/terms/soundrecordingtap#d"><rdf:type rdf:resource="http://www.w3.org/2004/02/skos/core#Concept"/><skos:inScheme rdf:resource="http://fakeIRI.edu/terms/soundrecordingtap"/><skos:prefLabel xml:lang="en">eight track</skos:prefLabel><skos:definition xml:lang="en">Eight track configuration is used with monaural, stereophonic, and quadraphonic recordings.</skos:definition><skos:scopeNote xml:lang="en">Commercial eight track cartridges customarily include four pairs of stereophonic (two track) recordings.</skos:scopeNote><skos:notation xml:lang="en">d</skos:notation></rdf:Description>
   
   <rdf:Description rdf:about="http://fakeIRI.edu/terms/soundrecordingtap#a"><rdf:type rdf:resource="http://www.w3.org/2004/02/skos/core#Concept"/><skos:inScheme rdf:resource="http://fakeIRI.edu/terms/soundrecordingtap"/><skos:prefLabel xml:lang="en">full (1) track</skos:prefLabel><skos:definition xml:lang="en">Full or single track.</skos:definition><skos:notation xml:lang="en">a</skos:notation></rdf:Description>
   
   <rdf:Description rdf:about="http://fakeIRI.edu/terms/soundrecordingtap#b"><rdf:type rdf:resource="http://www.w3.org/2004/02/skos/core#Concept"/><skos:inScheme rdf:resource="http://fakeIRI.edu/terms/soundrecordingtap"/><skos:prefLabel xml:lang="en">half (2) track</skos:prefLabel><skos:definition xml:lang="en">Half track configuration is used to permit two tracks (channels) to be recorded on one tape.</skos:definition><skos:scopeNote xml:lang="en">It is used with audio cassettes to permit monoaural recordings in two directions and with stereophonic recordings in one direction.</skos:scopeNote><skos:notation xml:lang="en">b</skos:notation></rdf:Description>
   
   <rdf:Description rdf:about="http://fakeIRI.edu/terms/soundrecordingtap#n"><rdf:type rdf:resource="http://www.w3.org/2004/02/skos/core#Concept"/><skos:inScheme rdf:resource="http://fakeIRI.edu/terms/soundrecordingtap"/><skos:prefLabel xml:lang="en">not applicable</skos:prefLabel><skos:definition xml:lang="en">Item is not a tape or does not include a tape.</skos:definition><skos:scopeNote xml:lang="en">For example, the item is a disc.</skos:scopeNote><skos:notation xml:lang="en">n</skos:notation></rdf:Description>
   
   <rdf:Description rdf:about="http://fakeIRI.edu/terms/soundrecordingtap#z"><rdf:type rdf:resource="http://www.w3.org/2004/02/skos/core#Concept"/><skos:inScheme rdf:resource="http://fakeIRI.edu/terms/soundrecordingtap"/><skos:prefLabel xml:lang="en">other</skos:prefLabel><skos:definition xml:lang="en">Tape configuration other than half (2) track, quarter (4) track, eight track, twelve track, or sixteen track.</skos:definition><skos:notation xml:lang="en">z</skos:notation></rdf:Description>
   
   <rdf:Description rdf:about="http://fakeIRI.edu/terms/soundrecordingtap#c"><rdf:type rdf:resource="http://www.w3.org/2004/02/skos/core#Concept"/><skos:inScheme rdf:resource="http://fakeIRI.edu/terms/soundrecordingtap"/><skos:prefLabel xml:lang="en">quarter (4) track</skos:prefLabel><skos:definition xml:lang="en">Quarter track configuration is used to permit four tracks (channels) to be recorded on one tape.</skos:definition><skos:scopeNote xml:lang="en">It is used with standard audio cassettes to permit stereophonic recordings in two directions, and with quadraphonic recordings in one direction.</skos:scopeNote><skos:notation xml:lang="en">c</skos:notation></rdf:Description>
   
   <rdf:Description rdf:about="http://fakeIRI.edu/terms/soundrecordingtap#f"><rdf:type rdf:resource="http://www.w3.org/2004/02/skos/core#Concept"/><skos:inScheme rdf:resource="http://fakeIRI.edu/terms/soundrecordingtap"/><skos:prefLabel xml:lang="en">sixteen track</skos:prefLabel><skos:definition xml:lang="en">Sixteen track configuration is used in professional recording studios to permit separate control of various tracks which are later mixed to produce a stereophonic or quadraphonic recording.</skos:definition><skos:notation xml:lang="en">f</skos:notation></rdf:Description>
   
   <rdf:Description rdf:about="http://fakeIRI.edu/terms/soundrecordingtap#e"><rdf:type rdf:resource="http://www.w3.org/2004/02/skos/core#Concept"/><skos:inScheme rdf:resource="http://fakeIRI.edu/terms/soundrecordingtap"/><skos:prefLabel xml:lang="en">twelve track</skos:prefLabel><skos:definition xml:lang="en">Twelve track configuration is used in professional recording studios to permit separate control of various tracks which are later mixed to produce a stereophonic or quadraphonic recording.</skos:definition><skos:notation xml:lang="en">e</skos:notation></rdf:Description>
   
   <rdf:Description rdf:about="http://fakeIRI.edu/terms/soundrecordingtap#u"><rdf:type rdf:resource="http://www.w3.org/2004/02/skos/core#Concept"/><skos:inScheme rdf:resource="http://fakeIRI.edu/terms/soundrecordingtap"/><skos:prefLabel xml:lang="en">unknown</skos:prefLabel><skos:definition xml:lang="en">Tape configuration is not known.</skos:definition><skos:notation xml:lang="en">u</skos:notation></rdf:Description>
</rdf:RDF>