<?xml version="1.0" encoding="utf-8"?>
<rdf:RDF
   xmlns:dc="http://purl.org/dc/elements/1.1/"
   xmlns:dct="http://purl.org/dc/terms/"
   xmlns:rdf="http://www.w3.org/1999/02/22-rdf-syntax-ns#"
   xmlns:schema="https://schema.org/"
   xmlns:skos="http://www.w3.org/2004/02/skos/core#"
>
  <rdf:Description rdf:about="https://doi.org/10.6069/uwlswd.fh0k-hk62">
    <rdf:type rdf:resource="http://www.w3.org/2004/02/skos/core#ConceptScheme"/>
    <dct:type rdf:resource="http://purl.org/dc/dcmitype/Dataset"/>
    <dct:title xml:lang="en">Sound recording: tape configuration</dct:title>
    <dct:alternative xml:lang="en">MARC21 007/08 values for sound recordings expressed using
         RDF</dct:alternative>
    <dct:description xml:lang="en">Number of tracks on a tape.</dct:description>
    <schema:disambiguatingDescription>SKOS Concept Scheme for MARC 00X
         Values</schema:disambiguatingDescription>
    <dct:publisher rdf:resource="http://viaf.org/viaf/139541794"/>
    <dct:source rdf:resource="https://www.loc.gov/marc/bibliographic/bd007.html"/>
    <dct:source rdf:resource="http://marc21rdf.info"/>
    <dct:provenance rdf:resource="https://doi.org/10.6069/uwlswd.2e2b-y833"/>
    <dct:creator rdf:resource="http://viaf.org/viaf/139541794"/>
    <dct:contributor rdf:resource="http://viaf.org/viaf/151962300"/>
    <dct:issued>2024</dct:issued>
    <dc:contributor xml:lang="en">Metadata Management Associates</dc:contributor>
    <dc:language>en</dc:language>
    <dct:license rdf:resource="http://creativecommons.org/publicdomain/zero/1.0"/>
    <schema:version>1-0-0</schema:version>
    <dct:format rdf:resource="http://www.w3.org/ns/formats/RDF_XML"/>
  </rdf:Description>
  <rdf:Description rdf:about="https://doi.org/10.6069/uwlswd.fh0k-hk62#e">
    <rdf:type rdf:resource="http://www.w3.org/2004/02/skos/core#Concept"/>
    <skos:inScheme rdf:resource="https://doi.org/10.6069/uwlswd.fh0k-hk62"/>
    <skos:prefLabel xml:lang="en">twelve track</skos:prefLabel>
    <skos:definition xml:lang="en">Twelve track configuration is used in professional recording
         studios to permit separate control of various tracks which are later mixed to produce a
         stereophonic or quadraphonic recording.</skos:definition>
    <skos:notation xml:lang="en">e</skos:notation>
  </rdf:Description>
  <rdf:Description rdf:about="https://doi.org/10.6069/uwlswd.fh0k-hk62#z">
    <rdf:type rdf:resource="http://www.w3.org/2004/02/skos/core#Concept"/>
    <skos:inScheme rdf:resource="https://doi.org/10.6069/uwlswd.fh0k-hk62"/>
    <skos:prefLabel xml:lang="en">other</skos:prefLabel>
    <skos:definition xml:lang="en">Tape configuration other than half (2) track, quarter (4)
         track, eight track, twelve track, or sixteen track.</skos:definition>
    <skos:notation xml:lang="en">z</skos:notation>
  </rdf:Description>
  <rdf:Description rdf:about="https://doi.org/10.6069/uwlswd.fh0k-hk62#d">
    <rdf:type rdf:resource="http://www.w3.org/2004/02/skos/core#Concept"/>
    <skos:inScheme rdf:resource="https://doi.org/10.6069/uwlswd.fh0k-hk62"/>
    <skos:prefLabel xml:lang="en">eight track</skos:prefLabel>
    <skos:definition xml:lang="en">Eight track configuration is used with monaural, stereophonic,
         and quadraphonic recordings.</skos:definition>
    <skos:scopeNote xml:lang="en">Commercial eight track cartridges customarily include four pairs
         of stereophonic (two track) recordings.</skos:scopeNote>
    <skos:notation xml:lang="en">d</skos:notation>
  </rdf:Description>
  <rdf:Description rdf:about="https://doi.org/10.6069/uwlswd.fh0k-hk62#b">
    <rdf:type rdf:resource="http://www.w3.org/2004/02/skos/core#Concept"/>
    <skos:inScheme rdf:resource="https://doi.org/10.6069/uwlswd.fh0k-hk62"/>
    <skos:prefLabel xml:lang="en">half (2) track</skos:prefLabel>
    <skos:definition xml:lang="en">Half track configuration is used to permit two tracks
         (channels) to be recorded on one tape.</skos:definition>
    <skos:scopeNote xml:lang="en">It is used with audio cassettes to permit monoaural recordings
         in two directions and with stereophonic recordings in one direction.</skos:scopeNote>
    <skos:notation xml:lang="en">b</skos:notation>
  </rdf:Description>
  <rdf:Description rdf:about="https://doi.org/10.6069/uwlswd.fh0k-hk62#c">
    <rdf:type rdf:resource="http://www.w3.org/2004/02/skos/core#Concept"/>
    <skos:inScheme rdf:resource="https://doi.org/10.6069/uwlswd.fh0k-hk62"/>
    <skos:prefLabel xml:lang="en">quarter (4) track</skos:prefLabel>
    <skos:definition xml:lang="en">Quarter track configuration is used to permit four tracks
         (channels) to be recorded on one tape.</skos:definition>
    <skos:scopeNote xml:lang="en">It is used with standard audio cassettes to permit stereophonic
         recordings in two directions, and with quadraphonic recordings in one
         direction.</skos:scopeNote>
    <skos:notation xml:lang="en">c</skos:notation>
  </rdf:Description>
  <rdf:Description rdf:about="https://doi.org/10.6069/uwlswd.fh0k-hk62#a">
    <rdf:type rdf:resource="http://www.w3.org/2004/02/skos/core#Concept"/>
    <skos:inScheme rdf:resource="https://doi.org/10.6069/uwlswd.fh0k-hk62"/>
    <skos:prefLabel xml:lang="en">full (1) track</skos:prefLabel>
    <skos:definition xml:lang="en">Full or single track.</skos:definition>
    <skos:notation xml:lang="en">a</skos:notation>
  </rdf:Description>
  <rdf:Description rdf:about="https://doi.org/10.6069/uwlswd.fh0k-hk62#n">
    <rdf:type rdf:resource="http://www.w3.org/2004/02/skos/core#Concept"/>
    <skos:inScheme rdf:resource="https://doi.org/10.6069/uwlswd.fh0k-hk62"/>
    <skos:prefLabel xml:lang="en">not applicable</skos:prefLabel>
    <skos:definition xml:lang="en">Item is not a tape or does not include a
         tape.</skos:definition>
    <skos:scopeNote xml:lang="en">For example, the item is a disc.</skos:scopeNote>
    <skos:notation xml:lang="en">n</skos:notation>
  </rdf:Description>
  <rdf:Description rdf:about="https://doi.org/10.6069/uwlswd.fh0k-hk62#u">
    <rdf:type rdf:resource="http://www.w3.org/2004/02/skos/core#Concept"/>
    <skos:inScheme rdf:resource="https://doi.org/10.6069/uwlswd.fh0k-hk62"/>
    <skos:prefLabel xml:lang="en">unknown</skos:prefLabel>
    <skos:definition xml:lang="en">Tape configuration is not known.</skos:definition>
    <skos:notation xml:lang="en">u</skos:notation>
  </rdf:Description>
  <rdf:Description rdf:about="https://doi.org/10.6069/uwlswd.fh0k-hk62#f">
    <rdf:type rdf:resource="http://www.w3.org/2004/02/skos/core#Concept"/>
    <skos:inScheme rdf:resource="https://doi.org/10.6069/uwlswd.fh0k-hk62"/>
    <skos:prefLabel xml:lang="en">sixteen track</skos:prefLabel>
    <skos:definition xml:lang="en">Sixteen track configuration is used in professional recording
         studios to permit separate control of various tracks which are later mixed to produce a
         stereophonic or quadraphonic recording.</skos:definition>
    <skos:notation xml:lang="en">f</skos:notation>
  </rdf:Description>
</rdf:RDF>
