@prefix dc: <http://purl.org/dc/elements/1.1/> .
@prefix dct: <http://purl.org/dc/terms/> .
@prefix schema: <https://schema.org/> .
@prefix skos: <http://www.w3.org/2004/02/skos/core#> .

<https://doi.org/10.6069/uwlswd.84qn-zz83#a> a skos:Concept ;
    skos:definition "Canvas."@en ;
    skos:inScheme <https://doi.org/10.6069/uwlswd.84qn-zz83> ;
    skos:notation "a" ;
    skos:prefLabel "canvas"@en .

<https://doi.org/10.6069/uwlswd.84qn-zz83#b> a skos:Concept ;
    skos:definition """Fine, smooth pasteboard used by artists and
         painters."""@en ;
    skos:inScheme <https://doi.org/10.6069/uwlswd.84qn-zz83> ;
    skos:notation "b" ;
    skos:prefLabel "Bristol board"@en .

<https://doi.org/10.6069/uwlswd.84qn-zz83#c> a skos:Concept ;
    skos:definition "Cardboard/illustration board."@en ;
    skos:inScheme <https://doi.org/10.6069/uwlswd.84qn-zz83> ;
    skos:notation "c" ;
    skos:prefLabel "cardboard/illustration board"@en .

<https://doi.org/10.6069/uwlswd.84qn-zz83#d> a skos:Concept ;
    skos:definition "Glass."@en ;
    skos:inScheme <https://doi.org/10.6069/uwlswd.84qn-zz83> ;
    skos:notation "d" ;
    skos:prefLabel "glass"@en .

<https://doi.org/10.6069/uwlswd.84qn-zz83#e> a skos:Concept ;
    skos:definition """Man-made substances other than textiles, plastic, and
         vinyl."""@en ;
    skos:inScheme <https://doi.org/10.6069/uwlswd.84qn-zz83> ;
    skos:notation "e" ;
    skos:prefLabel "synthetic"@en .

<https://doi.org/10.6069/uwlswd.84qn-zz83#f> a skos:Concept ;
    skos:definition "Skin."@en ;
    skos:inScheme <https://doi.org/10.6069/uwlswd.84qn-zz83> ;
    skos:notation "f" ;
    skos:prefLabel "skin"@en ;
    skos:scopeNote """Excludes leather, parchment, and vellum. Synthetic materials
         that are made to resemble animal skin are coded as synthetic."""@en .

<https://doi.org/10.6069/uwlswd.84qn-zz83#g> a skos:Concept ;
    skos:definition "Textile."@en ;
    skos:inScheme <https://doi.org/10.6069/uwlswd.84qn-zz83> ;
    skos:notation "g" ;
    skos:prefLabel "textile"@en ;
    skos:scopeNote """Includes all natural or synthetic fibre fabrics except canvas.
         Synthetic materials formed to resemble a fabric are considered textiles."""@en .

<https://doi.org/10.6069/uwlswd.84qn-zz83#h> a skos:Concept ;
    skos:definition "Metal."@en ;
    skos:inScheme <https://doi.org/10.6069/uwlswd.84qn-zz83> ;
    skos:notation "h" ;
    skos:prefLabel "metal"@en .

<https://doi.org/10.6069/uwlswd.84qn-zz83#i> a skos:Concept ;
    skos:definition "Plastic."@en ;
    skos:inScheme <https://doi.org/10.6069/uwlswd.84qn-zz83> ;
    skos:notation "i" ;
    skos:prefLabel "plastic"@en .

<https://doi.org/10.6069/uwlswd.84qn-zz83#l> a skos:Concept ;
    skos:definition "Vinyl."@en ;
    skos:inScheme <https://doi.org/10.6069/uwlswd.84qn-zz83> ;
    skos:notation "l" ;
    skos:prefLabel "vinyl"@en .

<https://doi.org/10.6069/uwlswd.84qn-zz83#m> a skos:Concept ;
    skos:definition """Primary support material varies for different items in a
         collection."""@en ;
    skos:inScheme <https://doi.org/10.6069/uwlswd.84qn-zz83> ;
    skos:notation "m" ;
    skos:prefLabel "mixed collection"@en ;
    skos:scopeNote """Typically this would be used for groups of nonprojected graphics
         on various bases."""@en .

<https://doi.org/10.6069/uwlswd.84qn-zz83#n> a skos:Concept ;
    skos:definition """Fine-grained unsplit lambskin, kidskin, or calfskin prepared
         especially for writing or drawing on."""@en ;
    skos:inScheme <https://doi.org/10.6069/uwlswd.84qn-zz83> ;
    skos:notation "n" ;
    skos:prefLabel "vellum"@en .

<https://doi.org/10.6069/uwlswd.84qn-zz83#o> a skos:Concept ;
    skos:definition "Any kind of cellulose-based paper."@en ;
    skos:inScheme <https://doi.org/10.6069/uwlswd.84qn-zz83> ;
    skos:notation "o" ;
    skos:prefLabel "paper"@en .

<https://doi.org/10.6069/uwlswd.84qn-zz83#p> a skos:Concept ;
    skos:definition "Plaster."@en ;
    skos:inScheme <https://doi.org/10.6069/uwlswd.84qn-zz83> ;
    skos:notation "p" ;
    skos:prefLabel "plaster"@en ;
    skos:scopeNote "Includes mixtures of ground solids and plaster."@en .

<https://doi.org/10.6069/uwlswd.84qn-zz83#q> a skos:Concept ;
    skos:definition "Hardboard."@en ;
    skos:inScheme <https://doi.org/10.6069/uwlswd.84qn-zz83> ;
    skos:notation "q" ;
    skos:prefLabel "hardboard"@en .

<https://doi.org/10.6069/uwlswd.84qn-zz83#r> a skos:Concept ;
    skos:definition "Porcelain."@en ;
    skos:inScheme <https://doi.org/10.6069/uwlswd.84qn-zz83> ;
    skos:notation "r" ;
    skos:prefLabel "porcelain"@en ;
    skos:scopeNote """Used only for clay-based porcelain. Porcelain-like synthetic
         materials are coded as synthetic."""@en .

<https://doi.org/10.6069/uwlswd.84qn-zz83#s> a skos:Concept ;
    skos:definition "Stone."@en ;
    skos:inScheme <https://doi.org/10.6069/uwlswd.84qn-zz83> ;
    skos:notation "s" ;
    skos:prefLabel "stone"@en .

<https://doi.org/10.6069/uwlswd.84qn-zz83#t> a skos:Concept ;
    skos:definition """Material that is based on wood particles or fibers may or may
         not be considered wood."""@en ;
    skos:inScheme <https://doi.org/10.6069/uwlswd.84qn-zz83> ;
    skos:notation "t" ;
    skos:prefLabel "wood"@en ;
    skos:scopeNote "Consider particle board to be wood."@en .

<https://doi.org/10.6069/uwlswd.84qn-zz83#u> a skos:Concept ;
    skos:definition "Primary support material is not known."@en ;
    skos:inScheme <https://doi.org/10.6069/uwlswd.84qn-zz83> ;
    skos:notation "u" ;
    skos:prefLabel "unknown"@en .

<https://doi.org/10.6069/uwlswd.84qn-zz83#v> a skos:Concept ;
    skos:definition "Animal skin dressed for use."@en ;
    skos:inScheme <https://doi.org/10.6069/uwlswd.84qn-zz83> ;
    skos:notation "v" ;
    skos:prefLabel "leather"@en .

<https://doi.org/10.6069/uwlswd.84qn-zz83#w> a skos:Concept ;
    skos:definition """Skin of a sheep or goat prepared for writing
         on."""@en ;
    skos:inScheme <https://doi.org/10.6069/uwlswd.84qn-zz83> ;
    skos:notation "w" ;
    skos:prefLabel "parchment"@en .

<https://doi.org/10.6069/uwlswd.84qn-zz83#z> a skos:Concept ;
    skos:definition """Primary support material other than canvas, bristol board,
         cardboard/illustration board, glass, synthetic, skin, textile, metal, plastic, vinyl, mixed
         collection, vellum, paper, plaster, hardboard, porcelain, stone, wood, leather, or
         parchment."""@en ;
    skos:inScheme <https://doi.org/10.6069/uwlswd.84qn-zz83> ;
    skos:notation "z" ;
    skos:prefLabel "other"@en .

<https://doi.org/10.6069/uwlswd.84qn-zz83> a skos:ConceptScheme ;
    dc:contributor "Metadata Management Associates"@en ;
    dc:language "en" ;
    dct:alternative """MARC21 007/04 values for nonprojected graphics expressed using
         RDF"""@en ;
    dct:contributor <http://viaf.org/viaf/151962300> ;
    dct:creator <http://viaf.org/viaf/139541794> ;
    dct:description """Type of material used for the support or base on which an image
         is printed or executed."""@en ;
    dct:format <http://www.w3.org/ns/formats/Turtle> ;
    dct:hasFormat <https://uwlib-cams.github.io/uwlswd_vocabs_marc_007/nonprojected_graphic_primary_support_material/nonprojected_graphic_primary_support_material.html>,
        <https://uwlib-cams.github.io/uwlswd_vocabs_marc_007/nonprojected_graphic_primary_support_material/nonprojected_graphic_primary_support_material.jsonld>,
        <https://uwlib-cams.github.io/uwlswd_vocabs_marc_007/nonprojected_graphic_primary_support_material/nonprojected_graphic_primary_support_material.nt>,
        <https://uwlib-cams.github.io/uwlswd_vocabs_marc_007/nonprojected_graphic_primary_support_material/nonprojected_graphic_primary_support_material.rdf> ;
    dct:issued "2024" ;
    dct:license <http://creativecommons.org/publicdomain/zero/1.0> ;
    dct:provenance <https://doi.org/10.6069/uwlswd.2e2b-y833#marc00Xvalues> ;
    dct:publisher <http://viaf.org/viaf/139541794> ;
    dct:source <http://marc21rdf.info>,
        <https://www.loc.gov/marc/bibliographic/bd007.html> ;
    dct:title "Nonprojected graphic: primary support material"@en ;
    dct:type <http://purl.org/dc/dcmitype/Dataset> ;
    schema:disambiguatingDescription """SKOS Concept Scheme for MARC 00X
         Values"""@en ;
    schema:version "1-0-0" .

