<?xml version="1.0" encoding="UTF-8"?><rdf:RDF xmlns:dc="http://purl.org/dc/elements/1.1/" xmlns:dct="http://purl.org/dc/terms/" xmlns:rdf="http://www.w3.org/1999/02/22-rdf-syntax-ns#" xmlns:rdfs="http://www.w3.org/2000/01/rdf-schema#" xmlns:schema="https://schema.org/" xmlns:skos="http://www.w3.org/2004/02/skos/core#" xmlns:uw="https://www.lib.washington.edu/static/public/cams/data/localResources/properties_local.html" xmlns:uwp="https://doi.org/10.6069/uwlib.55.d.3#">


   <rdf:Description rdf:about="http://fakeIRI.edu/terms/microformgen"><rdf:type rdf:resource="http://www.w3.org/2004/02/skos/core#ConceptScheme"/><dct:type rdf:resource="http://purl.org/dc/dcmitype/Dataset"/><dct:title xml:lang="en">Microform: generation</dct:title><dct:alternative xml:lang="en">MARC21 007/11 values for microform expressed using RDF</dct:alternative><dct:description xml:lang="en">Generation aspect of a microform.</dct:description><schema:disambiguatingDescription>SKOS Concept Scheme for MARC 00X Values</schema:disambiguatingDescription><dct:publisher rdf:resource="http://viaf.org/viaf/139541794"/><dct:source rdf:resource="https://www.loc.gov/marc/bibliographic/bd007.html"/><dct:source rdf:resource="http://marc21rdf.info"/><dct:provenance rdf:resource="https://doi.org/10.6069/uwlswd.2e2b-y833"/><dct:creator rdf:resource="http://viaf.org/viaf/139541794"/><dct:contributor rdf:resource="http://viaf.org/viaf/151962300"/><dct:issued>2024</dct:issued><dc:contributor xml:lang="en">Metadata Management Associates</dc:contributor><dc:language>en</dc:language><dct:license rdf:resource="http://creativecommons.org/publicdomain/zero/1.0"/><schema:version>1-0-0</schema:version><dct:issued>2024</dct:issued><dct:format rdf:resource="http://www.w3.org/ns/formats/RDF_XML"/></rdf:Description>
   
   <rdf:Description rdf:about="http://fakeIRI.edu/terms/microformgen#a"><rdf:type rdf:resource="http://www.w3.org/2004/02/skos/core#Concept"/><skos:inScheme rdf:resource="http://fakeIRI.edu/terms/microformgen"/><skos:prefLabel xml:lang="en">first generation (master)</skos:prefLabel><skos:definition xml:lang="en">Camera master or COM recorder master.</skos:definition><skos:scopeNote xml:lang="en">Used for all master films that are made on archival stock in accordance with archival productions standards and that are given archival storage under relevant ISO standards.</skos:scopeNote><skos:notation xml:lang="en">a</skos:notation></rdf:Description>
   
   <rdf:Description rdf:about="http://fakeIRI.edu/terms/microformgen#m"><rdf:type rdf:resource="http://www.w3.org/2004/02/skos/core#Concept"/><skos:inScheme rdf:resource="http://fakeIRI.edu/terms/microformgen"/><skos:prefLabel xml:lang="en">mixed generation</skos:prefLabel><skos:definition xml:lang="en">A combination of generations of film.</skos:definition><skos:notation xml:lang="en">m</skos:notation></rdf:Description>
   
   <rdf:Description rdf:about="http://fakeIRI.edu/terms/microformgen#b"><rdf:type rdf:resource="http://www.w3.org/2004/02/skos/core#Concept"/><skos:inScheme rdf:resource="http://fakeIRI.edu/terms/microformgen"/><skos:prefLabel xml:lang="en">printing master</skos:prefLabel><skos:definition xml:lang="en">Any generation employed mainly for the production of other microforms.</skos:definition><skos:scopeNote xml:lang="en">Used for all masters that are not manufactured, produced, and stored in accordance with archival standards.</skos:scopeNote><skos:notation xml:lang="en">b</skos:notation></rdf:Description>
   
   <rdf:Description rdf:about="http://fakeIRI.edu/terms/microformgen#c"><rdf:type rdf:resource="http://www.w3.org/2004/02/skos/core#Concept"/><skos:inScheme rdf:resource="http://fakeIRI.edu/terms/microformgen"/><skos:prefLabel xml:lang="en">service copy</skos:prefLabel><skos:definition xml:lang="en">Microform made from another microform that is intended primarily for use rather than for production of other microforms.</skos:definition><skos:scopeNote xml:lang="en">Always used for microopaques.</skos:scopeNote><skos:notation xml:lang="en">c</skos:notation></rdf:Description>
   
   <rdf:Description rdf:about="http://fakeIRI.edu/terms/microformgen#u"><rdf:type rdf:resource="http://www.w3.org/2004/02/skos/core#Concept"/><skos:inScheme rdf:resource="http://fakeIRI.edu/terms/microformgen"/><skos:prefLabel xml:lang="en">unknown</skos:prefLabel><skos:definition xml:lang="en">Generation aspect is not known.</skos:definition><skos:notation xml:lang="en">u</skos:notation></rdf:Description>
</rdf:RDF>