@prefix dc: <http://purl.org/dc/elements/1.1/> .
@prefix dct: <http://purl.org/dc/terms/> .
@prefix schema: <https://schema.org/> .
@prefix skos: <http://www.w3.org/2004/02/skos/core#> .

<https://doi.org/10.6069/uwlswd.043f-gn39#c> a skos:Concept ;
    skos:definition """Encased in a cartridge that has the ends joined together to
         form a loop that provides playback without rewinding."""@en ;
    skos:inScheme <https://doi.org/10.6069/uwlswd.043f-gn39> ;
    skos:notation "c" ;
    skos:prefLabel "film cartridge"@en .

<https://doi.org/10.6069/uwlswd.043f-gn39#f> a skos:Concept ;
    skos:definition """Encased in a cassette that winds and rewinds
         reel-to-reel."""@en ;
    skos:inScheme <https://doi.org/10.6069/uwlswd.043f-gn39> ;
    skos:notation "f" ;
    skos:prefLabel "film cassette"@en .

<https://doi.org/10.6069/uwlswd.043f-gn39#o> a skos:Concept ;
    skos:definition """A wound length of film not in a reel, cartridge,
         etc."""@en ;
    skos:inScheme <https://doi.org/10.6069/uwlswd.043f-gn39> ;
    skos:notation "o" ;
    skos:prefLabel "film roll"@en .

<https://doi.org/10.6069/uwlswd.043f-gn39#r> a skos:Concept ;
    skos:definition """Open reel of motion picture film designed for use with a
         projector having its own take-up reel."""@en ;
    skos:inScheme <https://doi.org/10.6069/uwlswd.043f-gn39> ;
    skos:notation "r" ;
    skos:prefLabel "film reel"@en ;
    skos:scopeNote """Includes sound track film intended to accompany visual images
         actually not present."""@en .

<https://doi.org/10.6069/uwlswd.043f-gn39#u> a skos:Concept ;
    skos:definition """Special material designation for the motion picture is not
         specified."""@en ;
    skos:inScheme <https://doi.org/10.6069/uwlswd.043f-gn39> ;
    skos:notation "u" ;
    skos:prefLabel "unspecified"@en .

<https://doi.org/10.6069/uwlswd.043f-gn39#z> a skos:Concept ;
    skos:definition """Specific material designation other than film cartridge, film
         cassette, film roll, or film reel."""@en ;
    skos:inScheme <https://doi.org/10.6069/uwlswd.043f-gn39> ;
    skos:notation "z" ;
    skos:prefLabel "other"@en .

<https://doi.org/10.6069/uwlswd.043f-gn39> a skos:ConceptScheme ;
    dc:contributor "Metadata Management Associates"@en ;
    dc:language "en" ;
    dct:alternative """MARC21 007/01 values for motion pictures expressed using
         RDF"""@en ;
    dct:contributor <http://viaf.org/viaf/151962300> ;
    dct:creator <http://viaf.org/viaf/139541794> ;
    dct:description """Special class of motion picture to which the item belongs.,
         e.g., a film reel."""@en ;
    dct:format <http://www.w3.org/ns/formats/Turtle> ;
    dct:hasFormat <https://uwlib-cams.github.io/uwlswd_vocabs_marc_007/motion_picture_specific_material_designation/motion_picture_specific_material_designation.html>,
        <https://uwlib-cams.github.io/uwlswd_vocabs_marc_007/motion_picture_specific_material_designation/motion_picture_specific_material_designation.jsonld>,
        <https://uwlib-cams.github.io/uwlswd_vocabs_marc_007/motion_picture_specific_material_designation/motion_picture_specific_material_designation.nt>,
        <https://uwlib-cams.github.io/uwlswd_vocabs_marc_007/motion_picture_specific_material_designation/motion_picture_specific_material_designation.rdf> ;
    dct:issued "2024" ;
    dct:license <http://creativecommons.org/publicdomain/zero/1.0> ;
    dct:provenance <https://doi.org/10.6069/uwlswd.2e2b-y833#marc00Xvalues> ;
    dct:publisher <http://viaf.org/viaf/139541794> ;
    dct:source <http://marc21rdf.info>,
        <https://www.loc.gov/marc/bibliographic/bd007.html> ;
    dct:title "Motion picture: specific material designation"@en ;
    dct:type <http://purl.org/dc/dcmitype/Dataset> ;
    schema:disambiguatingDescription """SKOS Concept Scheme for MARC 00X
         Values"""@en ;
    schema:version "1-0-0" .

