<?xml version="1.0" encoding="utf-8"?>
<rdf:RDF
   xmlns:dc="http://purl.org/dc/elements/1.1/"
   xmlns:dct="http://purl.org/dc/terms/"
   xmlns:rdf="http://www.w3.org/1999/02/22-rdf-syntax-ns#"
   xmlns:schema="https://schema.org/"
   xmlns:skos="http://www.w3.org/2004/02/skos/core#"
>
  <rdf:Description rdf:about="https://doi.org/10.6069/uwlswd.z7rs-y926">
    <rdf:type rdf:resource="http://www.w3.org/2004/02/skos/core#ConceptScheme"/>
    <dct:type rdf:resource="http://purl.org/dc/dcmitype/Dataset"/>
    <dct:title xml:lang="en">Motion picture: production elements</dct:title>
    <dct:alternative xml:lang="en">MARC21 007/09 values for motion pictures expressed using
         RDF</dct:alternative>
    <dct:description xml:lang="en">Whether the film is part of a complete production or is a
         preliminary or post-production element.</dct:description>
    <schema:disambiguatingDescription>SKOS Concept Scheme for MARC 00X
         Values</schema:disambiguatingDescription>
    <dct:publisher rdf:resource="http://viaf.org/viaf/139541794"/>
    <dct:source rdf:resource="https://www.loc.gov/marc/bibliographic/bd007.html"/>
    <dct:source rdf:resource="http://marc21rdf.info"/>
    <dct:provenance rdf:resource="https://doi.org/10.6069/uwlswd.2e2b-y833"/>
    <dct:creator rdf:resource="http://viaf.org/viaf/139541794"/>
    <dct:contributor rdf:resource="http://viaf.org/viaf/151962300"/>
    <dct:issued>2024</dct:issued>
    <dc:contributor xml:lang="en">Metadata Management Associates</dc:contributor>
    <dc:language>en</dc:language>
    <dct:license rdf:resource="http://creativecommons.org/publicdomain/zero/1.0"/>
    <schema:version>1-0-0</schema:version>
    <dct:format rdf:resource="http://www.w3.org/ns/formats/RDF_XML"/>
  </rdf:Description>
  <rdf:Description rdf:about="https://doi.org/10.6069/uwlswd.z7rs-y926#g">
    <rdf:type rdf:resource="http://www.w3.org/2004/02/skos/core#Concept"/>
    <skos:inScheme rdf:resource="https://doi.org/10.6069/uwlswd.z7rs-y926"/>
    <skos:prefLabel xml:lang="en">production rolls</skos:prefLabel>
    <skos:definition xml:lang="en">Various types of production elements (film usually wound on
         cores) before they are cut and assembled into reels.</skos:definition>
    <skos:notation xml:lang="en">g</skos:notation>
  </rdf:Description>
  <rdf:Description rdf:about="https://doi.org/10.6069/uwlswd.z7rs-y926#a">
    <rdf:type rdf:resource="http://www.w3.org/2004/02/skos/core#Concept"/>
    <skos:inScheme rdf:resource="https://doi.org/10.6069/uwlswd.z7rs-y926"/>
    <skos:prefLabel xml:lang="en">workprint</skos:prefLabel>
    <skos:definition xml:lang="en">Print from the original camera footage which is edited to a
         fine degree to achieve the final version.</skos:definition>
    <skos:notation xml:lang="en">a</skos:notation>
  </rdf:Description>
  <rdf:Description rdf:about="https://doi.org/10.6069/uwlswd.z7rs-y926#n">
    <rdf:type rdf:resource="http://www.w3.org/2004/02/skos/core#Concept"/>
    <skos:inScheme rdf:resource="https://doi.org/10.6069/uwlswd.z7rs-y926"/>
    <skos:prefLabel xml:lang="en">not applicable</skos:prefLabel>
    <skos:definition xml:lang="en">Item is not a production element.</skos:definition>
    <skos:notation xml:lang="en">n</skos:notation>
  </rdf:Description>
  <rdf:Description rdf:about="https://doi.org/10.6069/uwlswd.z7rs-y926#b">
    <rdf:type rdf:resource="http://www.w3.org/2004/02/skos/core#Concept"/>
    <skos:inScheme rdf:resource="https://doi.org/10.6069/uwlswd.z7rs-y926"/>
    <skos:prefLabel xml:lang="en">trims</skos:prefLabel>
    <skos:definition xml:lang="en">Sections of shots remaining after the desired portions have
         been incorporated into the workprint.</skos:definition>
    <skos:notation xml:lang="en">b</skos:notation>
  </rdf:Description>
  <rdf:Description rdf:about="https://doi.org/10.6069/uwlswd.z7rs-y926#f">
    <rdf:type rdf:resource="http://www.w3.org/2004/02/skos/core#Concept"/>
    <skos:inScheme rdf:resource="https://doi.org/10.6069/uwlswd.z7rs-y926"/>
    <skos:prefLabel xml:lang="en">title bands/intertitle rolls</skos:prefLabel>
    <skos:definition xml:lang="en">Printed captions or titles separated from their corresponding
         picture.</skos:definition>
    <skos:notation xml:lang="en">f</skos:notation>
  </rdf:Description>
  <rdf:Description rdf:about="https://doi.org/10.6069/uwlswd.z7rs-y926#h">
    <rdf:type rdf:resource="http://www.w3.org/2004/02/skos/core#Concept"/>
    <skos:inScheme rdf:resource="https://doi.org/10.6069/uwlswd.z7rs-y926"/>
    <skos:prefLabel xml:lang="en">other [obsolete]</skos:prefLabel>
    <skos:notation xml:lang="en">h</skos:notation>
  </rdf:Description>
  <rdf:Description rdf:about="https://doi.org/10.6069/uwlswd.z7rs-y926#e">
    <rdf:type rdf:resource="http://www.w3.org/2004/02/skos/core#Concept"/>
    <skos:inScheme rdf:resource="https://doi.org/10.6069/uwlswd.z7rs-y926"/>
    <skos:prefLabel xml:lang="en">mixing tracks</skos:prefLabel>
    <skos:definition xml:lang="en">Separate sound tracks that are combined for the final film
         sound track.</skos:definition>
    <skos:scopeNote xml:lang="en">Mixing tracks may include music, sound effects, and dialog
         tracks.</skos:scopeNote>
    <skos:notation xml:lang="en">e</skos:notation>
  </rdf:Description>
  <rdf:Description rdf:about="https://doi.org/10.6069/uwlswd.z7rs-y926#d">
    <rdf:type rdf:resource="http://www.w3.org/2004/02/skos/core#Concept"/>
    <skos:inScheme rdf:resource="https://doi.org/10.6069/uwlswd.z7rs-y926"/>
    <skos:prefLabel xml:lang="en">rushes</skos:prefLabel>
    <skos:definition xml:lang="en">First positive prints from the laboratory of the previous day's
         shooting.</skos:definition>
    <skos:scopeNote xml:lang="en">Also called dailies.</skos:scopeNote>
    <skos:notation xml:lang="en">d</skos:notation>
  </rdf:Description>
  <rdf:Description rdf:about="https://doi.org/10.6069/uwlswd.z7rs-y926#c">
    <rdf:type rdf:resource="http://www.w3.org/2004/02/skos/core#Concept"/>
    <skos:inScheme rdf:resource="https://doi.org/10.6069/uwlswd.z7rs-y926"/>
    <skos:prefLabel xml:lang="en">outtakes</skos:prefLabel>
    <skos:definition xml:lang="en">Shots discarded in the editing of a film.</skos:definition>
    <skos:notation xml:lang="en">c</skos:notation>
  </rdf:Description>
  <rdf:Description rdf:about="https://doi.org/10.6069/uwlswd.z7rs-y926#z">
    <rdf:type rdf:resource="http://www.w3.org/2004/02/skos/core#Concept"/>
    <skos:inScheme rdf:resource="https://doi.org/10.6069/uwlswd.z7rs-y926"/>
    <skos:prefLabel xml:lang="en">other</skos:prefLabel>
    <skos:definition xml:lang="en">Production elements other than workprint, trims, outtakes,
         rushes, mixing tracks, title bands/intertitle rolls, or production rolls.</skos:definition>
    <skos:notation xml:lang="en">z</skos:notation>
  </rdf:Description>
</rdf:RDF>
