@prefix dc: <http://purl.org/dc/elements/1.1/> .
@prefix dct: <http://purl.org/dc/terms/> .
@prefix schema: <https://schema.org/> .
@prefix skos: <http://www.w3.org/2004/02/skos/core#> .

<https://doi.org/10.6069/uwlswd.6h5g-mr73#a> a skos:Concept ;
    skos:definition """Film color prints created by the transfer of two or more
         differently colored dye images to a single strip of blank film. The dye transfer process
         was used only to produce prints. Imbibition dye transfer prints can be produced from film
         originally shot on either multi-strip or multi-layer film."""@en ;
    skos:inScheme <https://doi.org/10.6069/uwlswd.6h5g-mr73> ;
    skos:notation "a" ;
    skos:prefLabel "imbibition dye transfer prints"@en ;
    skos:scopeNote """The process was used only by the Technicolor Company from ca.
         1928 to ca. 1975. The patents were sold to the People's Republic of China, and since ca.
         1980, the process has been available only in China."""@en .

<https://doi.org/10.6069/uwlswd.6h5g-mr73#b> a skos:Concept ;
    skos:definition """Color film stock with three layers of emulsion: cyan, magenta
         and yellow. Each layer is sensitive to its own primary color."""@en ;
    skos:inScheme <https://doi.org/10.6069/uwlswd.6h5g-mr73> ;
    skos:notation "b" ;
    skos:prefLabel "three layer stock"@en ;
    skos:scopeNote """Since the early 1950s, most color films have been both shot and
         printed on this stock. It is also called multilayer film stock."""@en .

<https://doi.org/10.6069/uwlswd.6h5g-mr73#c> a skos:Concept ;
    skos:definition """Color film stock with three layers of emulsion: cyan, magenta
         and yellow. Each layer is sensitive to its own primary color and stabilized to reduce color
         fading as much as possible."""@en ;
    skos:inScheme <https://doi.org/10.6069/uwlswd.6h5g-mr73> ;
    skos:notation "c" ;
    skos:prefLabel "three layer stock, low fade"@en ;
    skos:scopeNote "It has been available since ca. 1983."@en .

<https://doi.org/10.6069/uwlswd.6h5g-mr73#d> a skos:Concept ;
    skos:definition """Color print stock with emulsion on both sides. Usually one side
         is dyed red, and the other side is dyed or toned blue."""@en ;
    skos:inScheme <https://doi.org/10.6069/uwlswd.6h5g-mr73> ;
    skos:notation "d" ;
    skos:prefLabel "duplitized stock"@en .

<https://doi.org/10.6069/uwlswd.6h5g-mr73#n> a skos:Concept ;
    skos:definition "Item is not a color film."@en ;
    skos:inScheme <https://doi.org/10.6069/uwlswd.6h5g-mr73> ;
    skos:notation "n" ;
    skos:prefLabel "not applicable"@en .

<https://doi.org/10.6069/uwlswd.6h5g-mr73#u> a skos:Concept ;
    skos:definition "Type of color film stock is not known."@en ;
    skos:inScheme <https://doi.org/10.6069/uwlswd.6h5g-mr73> ;
    skos:notation "u" ;
    skos:prefLabel "unknown"@en .

<https://doi.org/10.6069/uwlswd.6h5g-mr73#z> a skos:Concept ;
    skos:definition """Kind of color stock or print other than imbibition dye transfer
         prints, three layer stock, three layer stock, low fade, or duplitized
         stock."""@en ;
    skos:inScheme <https://doi.org/10.6069/uwlswd.6h5g-mr73> ;
    skos:notation "z" ;
    skos:prefLabel "other"@en .

<https://doi.org/10.6069/uwlswd.6h5g-mr73> a skos:ConceptScheme ;
    dc:contributor "Metadata Management Associates"@en ;
    dc:language "en" ;
    dct:alternative """MARC21 007/14 values for motion pictures expressed using
         RDF"""@en ;
    dct:contributor <http://viaf.org/viaf/151962300> ;
    dct:creator <http://viaf.org/viaf/139541794> ;
    dct:description """Type of color film stock or color print the item
         represents."""@en ;
    dct:format <http://www.w3.org/ns/formats/Turtle> ;
    dct:hasFormat <https://uwlib-cams.github.io/uwlswd_vocabs_marc_007/motion_picture_kind_of_color_stock_or_print/motion_picture_kind_of_color_stock_or_print.html>,
        <https://uwlib-cams.github.io/uwlswd_vocabs_marc_007/motion_picture_kind_of_color_stock_or_print/motion_picture_kind_of_color_stock_or_print.jsonld>,
        <https://uwlib-cams.github.io/uwlswd_vocabs_marc_007/motion_picture_kind_of_color_stock_or_print/motion_picture_kind_of_color_stock_or_print.nt>,
        <https://uwlib-cams.github.io/uwlswd_vocabs_marc_007/motion_picture_kind_of_color_stock_or_print/motion_picture_kind_of_color_stock_or_print.rdf> ;
    dct:issued "2024" ;
    dct:license <http://creativecommons.org/publicdomain/zero/1.0> ;
    dct:provenance <https://doi.org/10.6069/uwlswd.2e2b-y833#marc00Xvalues> ;
    dct:publisher <http://viaf.org/viaf/139541794> ;
    dct:source <http://marc21rdf.info>,
        <https://www.loc.gov/marc/bibliographic/bd007.html> ;
    dct:title "Motion picture: kind of color stock or print"@en ;
    dct:type <http://purl.org/dc/dcmitype/Dataset> ;
    schema:disambiguatingDescription """SKOS Concept Scheme for MARC 00X
         Values"""@en ;
    schema:version "1-0-0" .

