<?xml version="1.0" encoding="UTF-8"?>
<rdf:RDF xmlns:dc="http://purl.org/dc/elements/1.1/" xmlns:dct="http://purl.org/dc/terms/"
   xmlns:rdf="http://www.w3.org/1999/02/22-rdf-syntax-ns#"
   xmlns:rdfs="http://www.w3.org/2000/01/rdf-schema#" xmlns:schema="https://schema.org/"
   xmlns:skos="http://www.w3.org/2004/02/skos/core#"
   xmlns:uw="https://www.lib.washington.edu/static/public/cams/data/localResources/properties_local.html"
   xmlns:uwp="https://doi.org/10.6069/uwlib.55.d.3#">


   <rdf:Description rdf:about="http://fakeIRI.edu/terms/motionpicturecsp">
      <rdf:type rdf:resource="http://www.w3.org/2004/02/skos/core#ConceptScheme"/>
      <dct:type rdf:resource="http://purl.org/dc/dcmitype/Dataset"/>
      <dct:title xml:lang="en">Motion picture: kind of color stock or print</dct:title>
      <dct:alternative xml:lang="en">MARC21 007/14 values for motion pictures expressed using
         RDF</dct:alternative>
      <dct:description xml:lang="en">Type of color film stock or color print the item
         represents.</dct:description>
      <schema:disambiguatingDescription>SKOS Concept Scheme for MARC 00X
         Values</schema:disambiguatingDescription>
      <dct:publisher rdf:resource="http://viaf.org/viaf/139541794"/>
      <dct:source rdf:resource="https://www.loc.gov/marc/bibliographic/bd007.html"/>
      <dct:source rdf:resource="http://marc21rdf.info"/>
      <dct:provenance rdf:resource="https://doi.org/10.6069/uwlswd.2e2b-y833"/>
      <dct:creator rdf:resource="http://viaf.org/viaf/139541794"/>
      <dct:contributor rdf:resource="http://viaf.org/viaf/151962300"/>
      <dct:issued>2024</dct:issued>
      <dc:contributor xml:lang="en">Metadata Management Associates</dc:contributor>
      <dc:language>en</dc:language>
      <dct:license rdf:resource="http://creativecommons.org/publicdomain/zero/1.0"/>
      <schema:version>1-0-0</schema:version>
      <dct:issued>2024</dct:issued>
      <dct:format rdf:resource="http://www.w3.org/ns/formats/RDF_XML"/>
   </rdf:Description>

   <rdf:Description rdf:about="http://fakeIRI.edu/terms/motionpicturecsp#d">
      <rdf:type rdf:resource="http://www.w3.org/2004/02/skos/core#Concept"/>
      <skos:inScheme rdf:resource="http://fakeIRI.edu/terms/motionpicturecsp"/>
      <skos:prefLabel xml:lang="en">duplitized stock</skos:prefLabel>
      <skos:definition xml:lang="en">Color print stock with emulsion on both sides. Usually one side
         is dyed red, and the other side is dyed or toned blue.</skos:definition>
      <skos:notation xml:lang="en">d</skos:notation>
   </rdf:Description>

   <rdf:Description rdf:about="http://fakeIRI.edu/terms/motionpicturecsp#a">
      <rdf:type rdf:resource="http://www.w3.org/2004/02/skos/core#Concept"/>
      <skos:inScheme rdf:resource="http://fakeIRI.edu/terms/motionpicturecsp"/>
      <skos:prefLabel xml:lang="en">imbibition dye transfer prints</skos:prefLabel>
      <skos:definition xml:lang="en">Film color prints created by the transfer of two or more
         differently colored dye images to a single strip of blank film. The dye transfer process
         was used only to produce prints. Imbibition dye transfer prints can be produced from film
         originally shot on either multi-strip or multi-layer film.</skos:definition>
      <skos:scopeNote xml:lang="en">The process was used only by the Technicolor Company from ca.
         1928 to ca. 1975. The patents were sold to the People's Republic of China, and since ca.
         1980, the process has been available only in China.</skos:scopeNote>
      <skos:notation xml:lang="en">a</skos:notation>
   </rdf:Description>

   <rdf:Description rdf:about="http://fakeIRI.edu/terms/motionpicturecsp#n">
      <rdf:type rdf:resource="http://www.w3.org/2004/02/skos/core#Concept"/>
      <skos:inScheme rdf:resource="http://fakeIRI.edu/terms/motionpicturecsp"/>
      <skos:prefLabel xml:lang="en">not applicable</skos:prefLabel>
      <skos:definition xml:lang="en">Item is not a color film.</skos:definition>
      <skos:notation xml:lang="en">n</skos:notation>
   </rdf:Description>

   <rdf:Description rdf:about="http://fakeIRI.edu/terms/motionpicturecsp#z">
      <rdf:type rdf:resource="http://www.w3.org/2004/02/skos/core#Concept"/>
      <skos:inScheme rdf:resource="http://fakeIRI.edu/terms/motionpicturecsp"/>
      <skos:prefLabel xml:lang="en">other</skos:prefLabel>
      <skos:definition xml:lang="en">Kind of color stock or print other than imbibition dye transfer
         prints, three layer stock, three layer stock, low fade, or duplitized
         stock.</skos:definition>
      <skos:notation xml:lang="en">z</skos:notation>
   </rdf:Description>

   <rdf:Description rdf:about="http://fakeIRI.edu/terms/motionpicturecsp#b">
      <rdf:type rdf:resource="http://www.w3.org/2004/02/skos/core#Concept"/>
      <skos:inScheme rdf:resource="http://fakeIRI.edu/terms/motionpicturecsp"/>
      <skos:prefLabel xml:lang="en">three layer stock</skos:prefLabel>
      <skos:definition xml:lang="en">Color film stock with three layers of emulsion: cyan, magenta
         and yellow. Each layer is sensitive to its own primary color.</skos:definition>
      <skos:scopeNote xml:lang="en">Since the early 1950s, most color films have been both shot and
         printed on this stock. It is also called multilayer film stock.</skos:scopeNote>
      <skos:notation xml:lang="en">b</skos:notation>
   </rdf:Description>

   <rdf:Description rdf:about="http://fakeIRI.edu/terms/motionpicturecsp#c">
      <rdf:type rdf:resource="http://www.w3.org/2004/02/skos/core#Concept"/>
      <skos:inScheme rdf:resource="http://fakeIRI.edu/terms/motionpicturecsp"/>
      <skos:prefLabel xml:lang="en">three layer stock, low fade</skos:prefLabel>
      <skos:definition xml:lang="en">Color film stock with three layers of emulsion: cyan, magenta
         and yellow. Each layer is sensitive to its own primary color and stabilized to reduce color
         fading as much as possible.</skos:definition>
      <skos:scopeNote xml:lang="en">It has been available since ca. 1983.</skos:scopeNote>
      <skos:notation xml:lang="en">c</skos:notation>
   </rdf:Description>

   <rdf:Description rdf:about="http://fakeIRI.edu/terms/motionpicturecsp#u">
      <rdf:type rdf:resource="http://www.w3.org/2004/02/skos/core#Concept"/>
      <skos:inScheme rdf:resource="http://fakeIRI.edu/terms/motionpicturecsp"/>
      <skos:prefLabel xml:lang="en">unknown</skos:prefLabel>
      <skos:definition xml:lang="en">Type of color film stock is not known.</skos:definition>
      <skos:notation xml:lang="en">u</skos:notation>
   </rdf:Description>
</rdf:RDF>
