<?xml version='1.0' encoding='UTF-8'?>
<rdf:RDF xmlns:dc="http://purl.org/dc/elements/1.1/" xmlns:dct="http://purl.org/dc/terms/" xmlns:rdf="http://www.w3.org/1999/02/22-rdf-syntax-ns#" xmlns:schema="https://schema.org/" xmlns:skos="http://www.w3.org/2004/02/skos/core#">
  <rdf:Description rdf:about="https://doi.org/10.6069/uwlswd.n3ew-mc60#j">
    <rdf:type rdf:resource="http://www.w3.org/2004/02/skos/core#Concept"/>
    <skos:inScheme rdf:resource="https://doi.org/10.6069/uwlswd.n3ew-mc60"/>
    <skos:prefLabel xml:lang="en">metal and glass</skos:prefLabel>
    <skos:definition xml:lang="en">Metal portion is usually a frame that holds one or two pieces
         of glass to support the film base. Glass should not be the primary support for the film
         emulsion.</skos:definition>
    <skos:notation>j</skos:notation>
  </rdf:Description>
  <rdf:Description rdf:about="https://doi.org/10.6069/uwlswd.n3ew-mc60">
    <rdf:type rdf:resource="http://www.w3.org/2004/02/skos/core#ConceptScheme"/>
    <dct:type rdf:resource="http://purl.org/dc/dcmitype/Dataset"/>
    <dct:title xml:lang="en">Projected graphic: secondary support material</dct:title>
    <dct:alternative xml:lang="en">MARC21 007/08 values for projected graphics expressed using
         RDF</dct:alternative>
    <dct:description xml:lang="en">Type of material of the mount of a slide or transparency for a
         projected graphic.</dct:description>
    <schema:disambiguatingDescription xml:lang="en">SKOS Concept Scheme for MARC 00X
         Values</schema:disambiguatingDescription>
    <dct:publisher rdf:resource="http://viaf.org/viaf/139541794"/>
    <dct:source rdf:resource="https://www.loc.gov/marc/bibliographic/bd007.html"/>
    <dct:source rdf:resource="http://marc21rdf.info"/>
    <dct:provenance rdf:resource="https://doi.org/10.6069/uwlswd.2e2b-y833#marc00Xvalues"/>
    <dct:creator rdf:resource="http://viaf.org/viaf/139541794"/>
    <dct:contributor rdf:resource="http://viaf.org/viaf/151962300"/>
    <dct:issued>2024</dct:issued>
    <dc:contributor xml:lang="en">Metadata Management Associates</dc:contributor>
    <dc:language>en</dc:language>
    <dct:license rdf:resource="http://creativecommons.org/publicdomain/zero/1.0"/>
    <schema:version>1-0-0</schema:version>
    <dct:format rdf:resource="http://www.w3.org/ns/formats/RDF_XML"/>
  </rdf:Description>
  <rdf:Description rdf:about="https://doi.org/10.6069/uwlswd.n3ew-mc60#k">
    <rdf:type rdf:resource="http://www.w3.org/2004/02/skos/core#Concept"/>
    <skos:inScheme rdf:resource="https://doi.org/10.6069/uwlswd.n3ew-mc60"/>
    <skos:prefLabel xml:lang="en">synthetic and glass</skos:prefLabel>
    <skos:definition xml:lang="en">Synthetic material is usually used as a frame to hold one or
         two pieces of glass to support the film base. Glass should not be the primary support for
         the film emulsion.</skos:definition>
    <skos:scopeNote xml:lang="en">E.g. plastics, vinyl, etc.</skos:scopeNote>
    <skos:notation>k</skos:notation>
  </rdf:Description>
  <rdf:Description rdf:about="https://doi.org/10.6069/uwlswd.n3ew-mc60#c">
    <rdf:type rdf:resource="http://www.w3.org/2004/02/skos/core#Concept"/>
    <skos:inScheme rdf:resource="https://doi.org/10.6069/uwlswd.n3ew-mc60"/>
    <skos:prefLabel xml:lang="en">cardboard</skos:prefLabel>
    <skos:definition xml:lang="en">Cardboard mount.</skos:definition>
    <skos:scopeNote xml:lang="en">Slides and transparencies cataloged from data sheets are assumed
         to have cardboard mounts unless otherwise known.</skos:scopeNote>
    <skos:notation>c</skos:notation>
  </rdf:Description>
  <rdf:Description rdf:about="https://doi.org/10.6069/uwlswd.n3ew-mc60#pound">
    <rdf:type rdf:resource="http://www.w3.org/2004/02/skos/core#Concept"/>
    <skos:inScheme rdf:resource="https://doi.org/10.6069/uwlswd.n3ew-mc60"/>
    <skos:prefLabel xml:lang="en">no secondary support</skos:prefLabel>
    <skos:definition xml:lang="en">No secondary support.</skos:definition>
    <skos:scopeNote xml:lang="en">Includes all filmstrips.</skos:scopeNote>
    <skos:notation>#</skos:notation>
  </rdf:Description>
  <rdf:Description rdf:about="https://doi.org/10.6069/uwlswd.n3ew-mc60#h">
    <rdf:type rdf:resource="http://www.w3.org/2004/02/skos/core#Concept"/>
    <skos:inScheme rdf:resource="https://doi.org/10.6069/uwlswd.n3ew-mc60"/>
    <skos:prefLabel xml:lang="en">metal</skos:prefLabel>
    <skos:definition xml:lang="en">Metal.</skos:definition>
    <skos:scopeNote xml:lang="en">Usually used to frame larger projected graphics which need
         better support.</skos:scopeNote>
    <skos:notation>h</skos:notation>
  </rdf:Description>
  <rdf:Description rdf:about="https://doi.org/10.6069/uwlswd.n3ew-mc60#u">
    <rdf:type rdf:resource="http://www.w3.org/2004/02/skos/core#Concept"/>
    <skos:inScheme rdf:resource="https://doi.org/10.6069/uwlswd.n3ew-mc60"/>
    <skos:prefLabel xml:lang="en">unknown</skos:prefLabel>
    <skos:definition xml:lang="en">Secondary support material is not known.</skos:definition>
    <skos:notation>u</skos:notation>
  </rdf:Description>
  <rdf:Description rdf:about="https://doi.org/10.6069/uwlswd.n3ew-mc60#m">
    <rdf:type rdf:resource="http://www.w3.org/2004/02/skos/core#Concept"/>
    <skos:inScheme rdf:resource="https://doi.org/10.6069/uwlswd.n3ew-mc60"/>
    <skos:prefLabel xml:lang="en">mixed collection</skos:prefLabel>
    <skos:definition xml:lang="en">Secondary support material varies for different items in a
         collection.</skos:definition>
    <skos:scopeNote xml:lang="en">Typically this is used for groups of projected graphics on
         various secondary support materials.</skos:scopeNote>
    <skos:notation>m</skos:notation>
  </rdf:Description>
  <rdf:Description rdf:about="https://doi.org/10.6069/uwlswd.n3ew-mc60#d">
    <rdf:type rdf:resource="http://www.w3.org/2004/02/skos/core#Concept"/>
    <skos:inScheme rdf:resource="https://doi.org/10.6069/uwlswd.n3ew-mc60"/>
    <skos:prefLabel xml:lang="en">glass</skos:prefLabel>
    <skos:definition xml:lang="en">Glass mount that usually covers the film base but should not be
         the primary support for the film emulsion.</skos:definition>
    <skos:notation>d</skos:notation>
  </rdf:Description>
  <rdf:Description rdf:about="https://doi.org/10.6069/uwlswd.n3ew-mc60#e">
    <rdf:type rdf:resource="http://www.w3.org/2004/02/skos/core#Concept"/>
    <skos:inScheme rdf:resource="https://doi.org/10.6069/uwlswd.n3ew-mc60"/>
    <skos:prefLabel xml:lang="en">synthetic</skos:prefLabel>
    <skos:definition xml:lang="en">Synthetic material.</skos:definition>
    <skos:scopeNote xml:lang="en">E.g. plastics, vinyl, etc.</skos:scopeNote>
    <skos:notation>e</skos:notation>
  </rdf:Description>
  <rdf:Description rdf:about="https://doi.org/10.6069/uwlswd.n3ew-mc60#z">
    <rdf:type rdf:resource="http://www.w3.org/2004/02/skos/core#Concept"/>
    <skos:inScheme rdf:resource="https://doi.org/10.6069/uwlswd.n3ew-mc60"/>
    <skos:prefLabel xml:lang="en">other</skos:prefLabel>
    <skos:definition xml:lang="en">Secondary support material other than cardboard, glass,
         synthetic, metal, metal and glass, synthetic and glass, or mixed
         collection.</skos:definition>
    <skos:notation>z</skos:notation>
  </rdf:Description>
</rdf:RDF>