@prefix dc: <http://purl.org/dc/elements/1.1/> .
@prefix dct: <http://purl.org/dc/terms/> .
@prefix schema: <https://schema.org/> .
@prefix skos: <http://www.w3.org/2004/02/skos/core#> .

<https://doi.org/10.6069/uwlswd.9t5f-qz73#a> a skos:Concept ;
    skos:definition """Measures are displayed in units called parallels and the
         beginning of each part's measure is vertically aligned with the beginning of the same
         measure for the other part(s)."""@en ;
    skos:inScheme <https://doi.org/10.6069/uwlswd.9t5f-qz73> ;
    skos:notation "a" ;
    skos:prefLabel "bar over bar"@en ;
    skos:scopeNote "Used chiefly for keyboard music."@en .

<https://doi.org/10.6069/uwlswd.9t5f-qz73#b> a skos:Concept ;
    skos:definition """Music is displayed in indented paragraphs with all of the parts
         for each measure written consecutively."""@en ;
    skos:inScheme <https://doi.org/10.6069/uwlswd.9t5f-qz73> ;
    skos:notation "b" ;
    skos:prefLabel "bar by bar"@en .

<https://doi.org/10.6069/uwlswd.9t5f-qz73#c> a skos:Concept ;
    skos:definition """Measures are displayed in parallels, but the measures are not
         necessarily aligned."""@en ;
    skos:inScheme <https://doi.org/10.6069/uwlswd.9t5f-qz73> ;
    skos:notation "c" ;
    skos:prefLabel "line over line"@en .

<https://doi.org/10.6069/uwlswd.9t5f-qz73#d> a skos:Concept ;
    skos:definition """Music is displayed in paragraphs with one part per
         paragraph."""@en ;
    skos:inScheme <https://doi.org/10.6069/uwlswd.9t5f-qz73> ;
    skos:notation "d" ;
    skos:prefLabel "paragraph"@en .

<https://doi.org/10.6069/uwlswd.9t5f-qz73#e> a skos:Concept ;
    skos:definition """Music is presented in segments of two to five lines, the
         initial line displaying a measure number or rehearsal designation."""@en ;
    skos:inScheme <https://doi.org/10.6069/uwlswd.9t5f-qz73> ;
    skos:notation "e" ;
    skos:prefLabel "single line"@en ;
    skos:scopeNote """Used for single instrumental parts or solos. It is also called
         solo instrumental format."""@en .

<https://doi.org/10.6069/uwlswd.9t5f-qz73#f> a skos:Concept ;
    skos:definition """Hand or part signs are prominent in the left
         margin."""@en ;
    skos:inScheme <https://doi.org/10.6069/uwlswd.9t5f-qz73> ;
    skos:notation "f" ;
    skos:prefLabel "section by section"@en .

<https://doi.org/10.6069/uwlswd.9t5f-qz73#g> a skos:Concept ;
    skos:definition """Lines of text alternate with lines of music for the preceding
         text."""@en ;
    skos:inScheme <https://doi.org/10.6069/uwlswd.9t5f-qz73> ;
    skos:notation "g" ;
    skos:prefLabel "line by line"@en .

<https://doi.org/10.6069/uwlswd.9t5f-qz73#h> a skos:Concept ;
    skos:definition """Music is presented in parallels. Open score is similar to bar
         over bar, but used for ensemble scores."""@en ;
    skos:inScheme <https://doi.org/10.6069/uwlswd.9t5f-qz73> ;
    skos:notation "h" ;
    skos:prefLabel "open score"@en .

<https://doi.org/10.6069/uwlswd.9t5f-qz73#i> a skos:Concept ;
    skos:definition """Chord symbols and melody are presented in
         paragraphs."""@en ;
    skos:inScheme <https://doi.org/10.6069/uwlswd.9t5f-qz73> ;
    skos:notation "i" ;
    skos:prefLabel "spanner short form scoring"@en ;
    skos:scopeNote """Used chiefly for popular and folk music, but music braille is
         used for the chord symbols. Also used to indicate that the music is in the Canadian melody
         chord system."""@en .

<https://doi.org/10.6069/uwlswd.9t5f-qz73#j> a skos:Concept ;
    skos:definition """Words, chord symbols, and melody are presented in parallels,
         and literary braille is used for the chord symbols."""@en ;
    skos:inScheme <https://doi.org/10.6069/uwlswd.9t5f-qz73> ;
    skos:notation "j" ;
    skos:prefLabel "short form scoring"@en ;
    skos:scopeNote """Used chiefly for popular and folk music. This format is also
         referred to as the American or BANA short form scoring format."""@en .

<https://doi.org/10.6069/uwlswd.9t5f-qz73#k> a skos:Concept ;
    skos:definition "Music is in the outline format."@en ;
    skos:inScheme <https://doi.org/10.6069/uwlswd.9t5f-qz73> ;
    skos:notation "k" ;
    skos:prefLabel "outline"@en .

<https://doi.org/10.6069/uwlswd.9t5f-qz73#l> a skos:Concept ;
    skos:definition "Parts are combined and written as chords."@en ;
    skos:inScheme <https://doi.org/10.6069/uwlswd.9t5f-qz73> ;
    skos:notation "l" ;
    skos:prefLabel "vertical score"@en .

<https://doi.org/10.6069/uwlswd.9t5f-qz73#n> a skos:Concept ;
    skos:definition "Not braille music."@en ;
    skos:inScheme <https://doi.org/10.6069/uwlswd.9t5f-qz73> ;
    skos:notation "n" ;
    skos:prefLabel "not applicable"@en .

<https://doi.org/10.6069/uwlswd.9t5f-qz73#pound> a skos:Concept ;
    skos:definition """Item uses fewer than three specified braille writing
         formats."""@en ;
    skos:inScheme <https://doi.org/10.6069/uwlswd.9t5f-qz73> ;
    skos:notation "#" ;
    skos:prefLabel "no specified braille music format"@en .

<https://doi.org/10.6069/uwlswd.9t5f-qz73#u> a skos:Concept ;
    skos:definition "Braille music format is not known."@en ;
    skos:inScheme <https://doi.org/10.6069/uwlswd.9t5f-qz73> ;
    skos:notation "u" ;
    skos:prefLabel "unknown"@en .

<https://doi.org/10.6069/uwlswd.9t5f-qz73#z> a skos:Concept ;
    skos:definition """Braille music format other than no specified braille music
         format, bar over bar, bar by bar, line over line, paragraph, single line, section by
         section, line by line, open score, spanner short form scoring, short form scoring, outline,
         or vertical score."""@en ;
    skos:inScheme <https://doi.org/10.6069/uwlswd.9t5f-qz73> ;
    skos:notation "z" ;
    skos:prefLabel "other"@en .

<https://doi.org/10.6069/uwlswd.9t5f-qz73> a skos:ConceptScheme ;
    dc:contributor "Metadata Management Associates"@en ;
    dc:language "en" ;
    dct:alternative """MARC21 007/06-08 values for tactile material expressed using
         RDF"""@en ;
    dct:contributor <http://viaf.org/viaf/151962300> ;
    dct:creator <http://viaf.org/viaf/139541794> ;
    dct:description """Indicates the braille music format of the item. The music
         formats are the way measures, sections, parts, and related information, such as words, are
         presented in relation to each other."""@en ;
    dct:format <http://www.w3.org/ns/formats/Turtle> ;
    dct:hasFormat <https://uwlib-cams.github.io/uwlswd_vocabs_marc_007/tactile_material_braille_music_format/tactile_material_braille_music_format.html>,
        <https://uwlib-cams.github.io/uwlswd_vocabs_marc_007/tactile_material_braille_music_format/tactile_material_braille_music_format.jsonld>,
        <https://uwlib-cams.github.io/uwlswd_vocabs_marc_007/tactile_material_braille_music_format/tactile_material_braille_music_format.nt>,
        <https://uwlib-cams.github.io/uwlswd_vocabs_marc_007/tactile_material_braille_music_format/tactile_material_braille_music_format.rdf> ;
    dct:issued "2024" ;
    dct:license <http://creativecommons.org/publicdomain/zero/1.0> ;
    dct:provenance <https://doi.org/10.6069/uwlswd.2e2b-y833#marc00Xvalues> ;
    dct:publisher <http://viaf.org/viaf/139541794> ;
    dct:source <http://marc21rdf.info>,
        <https://www.loc.gov/marc/bibliographic/bd007.html> ;
    dct:title "Tactile material: braille music format"@en ;
    dct:type <http://purl.org/dc/dcmitype/Dataset> ;
    schema:disambiguatingDescription """SKOS Concept Scheme for MARC 00X
         Values"""@en ;
    schema:version "1-0-0" .

