<?xml version="1.0" encoding="UTF-8"?><rdf:RDF xmlns:dc="http://purl.org/dc/elements/1.1/" xmlns:dct="http://purl.org/dc/terms/" xmlns:rdf="http://www.w3.org/1999/02/22-rdf-syntax-ns#" xmlns:rdfs="http://www.w3.org/2000/01/rdf-schema#" xmlns:schema="https://schema.org/" xmlns:skos="http://www.w3.org/2004/02/skos/core#" xmlns:uw="https://www.lib.washington.edu/static/public/cams/data/localResources/properties_local.html" xmlns:uwp="https://doi.org/10.6069/uwlib.55.d.3#">


   <rdf:Description rdf:about="http://fakeIRI.edu/terms/tactilebmf"><rdf:type rdf:resource="http://www.w3.org/2004/02/skos/core#ConceptScheme"/><dct:type rdf:resource="http://purl.org/dc/dcmitype/Dataset"/><dct:title xml:lang="en">Tactile material: braille music format</dct:title><dct:alternative xml:lang="en">MARC21 007/06-08 values for tactile material expressed using RDF</dct:alternative><dct:description xml:lang="en">Indicates the braille music format of the item. The music formats are the way measures, sections, parts, and related information, such as words, are presented in relation to each other.</dct:description><schema:disambiguatingDescription>SKOS Concept Scheme for MARC 00X Values</schema:disambiguatingDescription><dct:publisher rdf:resource="http://viaf.org/viaf/139541794"/><dct:source rdf:resource="https://www.loc.gov/marc/bibliographic/bd007.html"/><dct:source rdf:resource="http://marc21rdf.info"/><dct:provenance rdf:resource="https://doi.org/10.6069/uwlswd.2e2b-y833"/><dct:creator rdf:resource="http://viaf.org/viaf/139541794"/><dct:contributor rdf:resource="http://viaf.org/viaf/151962300"/><dct:issued>2024</dct:issued><dc:contributor xml:lang="en">Metadata Management Associates</dc:contributor><dc:language>en</dc:language><dct:license rdf:resource="http://creativecommons.org/publicdomain/zero/1.0"/><schema:version>1-0-0</schema:version><dct:issued>2024</dct:issued><dct:format rdf:resource="http://www.w3.org/ns/formats/RDF_XML"/></rdf:Description>
   
   <rdf:Description rdf:about="http://fakeIRI.edu/terms/tactilebmf#b"><rdf:type rdf:resource="http://www.w3.org/2004/02/skos/core#Concept"/><skos:inScheme rdf:resource="http://fakeIRI.edu/terms/tactilebmf"/><skos:prefLabel xml:lang="en">bar by bar</skos:prefLabel><skos:definition xml:lang="en">Music is displayed in indented paragraphs with all of the parts for each measure written consecutively.</skos:definition><skos:notation xml:lang="en">b</skos:notation></rdf:Description>
   
   <rdf:Description rdf:about="http://fakeIRI.edu/terms/tactilebmf#a"><rdf:type rdf:resource="http://www.w3.org/2004/02/skos/core#Concept"/><skos:inScheme rdf:resource="http://fakeIRI.edu/terms/tactilebmf"/><skos:prefLabel xml:lang="en">bar over bar</skos:prefLabel><skos:definition xml:lang="en">Measures are displayed in units called parallels and the beginning of each part's measure is vertically aligned with the beginning of the same measure for the other part(s).</skos:definition><skos:scopeNote xml:lang="en">Used chiefly for keyboard music.</skos:scopeNote><skos:notation xml:lang="en">a</skos:notation></rdf:Description>
   
   <rdf:Description rdf:about="http://fakeIRI.edu/terms/tactilebmf#g"><rdf:type rdf:resource="http://www.w3.org/2004/02/skos/core#Concept"/><skos:inScheme rdf:resource="http://fakeIRI.edu/terms/tactilebmf"/><skos:prefLabel xml:lang="en">line by line</skos:prefLabel><skos:definition xml:lang="en">Lines of text alternate with lines of music for the preceding text.</skos:definition><skos:notation xml:lang="en">g</skos:notation></rdf:Description>
   
   <rdf:Description rdf:about="http://fakeIRI.edu/terms/tactilebmf#c"><rdf:type rdf:resource="http://www.w3.org/2004/02/skos/core#Concept"/><skos:inScheme rdf:resource="http://fakeIRI.edu/terms/tactilebmf"/><skos:prefLabel xml:lang="en">line over line</skos:prefLabel><skos:definition xml:lang="en">Measures are displayed in parallels, but the measures are not necessarily aligned.</skos:definition><skos:notation xml:lang="en">c</skos:notation></rdf:Description>
   
   <rdf:Description rdf:about="http://fakeIRI.edu/terms/tactilebmf#pound"><rdf:type rdf:resource="http://www.w3.org/2004/02/skos/core#Concept"/><skos:inScheme rdf:resource="http://fakeIRI.edu/terms/tactilebmf"/><skos:prefLabel xml:lang="en">no specified braille music format</skos:prefLabel><skos:definition xml:lang="en">Item uses fewer than three specified braille writing formats.</skos:definition><skos:notation xml:lang="en">#</skos:notation></rdf:Description>
   
   <rdf:Description rdf:about="http://fakeIRI.edu/terms/tactilebmf#n"><rdf:type rdf:resource="http://www.w3.org/2004/02/skos/core#Concept"/><skos:inScheme rdf:resource="http://fakeIRI.edu/terms/tactilebmf"/><skos:prefLabel xml:lang="en">not applicable</skos:prefLabel><skos:definition xml:lang="en">Not braille music.</skos:definition><skos:notation xml:lang="en">n</skos:notation></rdf:Description>
   
   <rdf:Description rdf:about="http://fakeIRI.edu/terms/tactilebmf#h"><rdf:type rdf:resource="http://www.w3.org/2004/02/skos/core#Concept"/><skos:inScheme rdf:resource="http://fakeIRI.edu/terms/tactilebmf"/><skos:prefLabel xml:lang="en">open score</skos:prefLabel><skos:definition xml:lang="en">Music is presented in parallels. Open score is similar to bar over bar, but used for ensemble scores.</skos:definition><skos:notation xml:lang="en">h</skos:notation></rdf:Description>
   
   <rdf:Description rdf:about="http://fakeIRI.edu/terms/tactilebmf#z"><rdf:type rdf:resource="http://www.w3.org/2004/02/skos/core#Concept"/><skos:inScheme rdf:resource="http://fakeIRI.edu/terms/tactilebmf"/><skos:prefLabel xml:lang="en">other</skos:prefLabel><skos:definition xml:lang="en">Braille music format other than no specified braille music format, bar over bar, bar by bar, line over line, paragraph, single line, section by section, line by line, open score, spanner short form scoring, short form scoring, outline, or vertical score.</skos:definition><skos:notation xml:lang="en">z</skos:notation></rdf:Description>
   
   <rdf:Description rdf:about="http://fakeIRI.edu/terms/tactilebmf#k"><rdf:type rdf:resource="http://www.w3.org/2004/02/skos/core#Concept"/><skos:inScheme rdf:resource="http://fakeIRI.edu/terms/tactilebmf"/><skos:prefLabel xml:lang="en">outline</skos:prefLabel><skos:definition xml:lang="en">Music is in the outline format.</skos:definition><skos:notation xml:lang="en">k</skos:notation></rdf:Description>
   
   <rdf:Description rdf:about="http://fakeIRI.edu/terms/tactilebmf#d"><rdf:type rdf:resource="http://www.w3.org/2004/02/skos/core#Concept"/><skos:inScheme rdf:resource="http://fakeIRI.edu/terms/tactilebmf"/><skos:prefLabel xml:lang="en">paragraph</skos:prefLabel><skos:definition xml:lang="en">Music is displayed in paragraphs with one part per paragraph.</skos:definition><skos:notation xml:lang="en">d</skos:notation></rdf:Description>
   
   <rdf:Description rdf:about="http://fakeIRI.edu/terms/tactilebmf#f"><rdf:type rdf:resource="http://www.w3.org/2004/02/skos/core#Concept"/><skos:inScheme rdf:resource="http://fakeIRI.edu/terms/tactilebmf"/><skos:prefLabel xml:lang="en">section by section</skos:prefLabel><skos:definition xml:lang="en">Hand or part signs are prominent in the left margin.</skos:definition><skos:notation xml:lang="en">f</skos:notation></rdf:Description>
   
   <rdf:Description rdf:about="http://fakeIRI.edu/terms/tactilebmf#j"><rdf:type rdf:resource="http://www.w3.org/2004/02/skos/core#Concept"/><skos:inScheme rdf:resource="http://fakeIRI.edu/terms/tactilebmf"/><skos:prefLabel xml:lang="en">short form scoring</skos:prefLabel><skos:definition xml:lang="en">Words, chord symbols, and melody are presented in parallels, and literary braille is used for the chord symbols.</skos:definition><skos:scopeNote xml:lang="en">Used chiefly for popular and folk music. This format is also referred to as the American or BANA short form scoring format.</skos:scopeNote><skos:notation xml:lang="en">j</skos:notation></rdf:Description>
   
   <rdf:Description rdf:about="http://fakeIRI.edu/terms/tactilebmf#e"><rdf:type rdf:resource="http://www.w3.org/2004/02/skos/core#Concept"/><skos:inScheme rdf:resource="http://fakeIRI.edu/terms/tactilebmf"/><skos:prefLabel xml:lang="en">single line</skos:prefLabel><skos:definition xml:lang="en">Music is presented in segments of two to five lines, the initial line displaying a measure number or rehearsal designation.</skos:definition><skos:scopeNote xml:lang="en">Used for single instrumental parts or solos. It is also called solo instrumental format.</skos:scopeNote><skos:notation xml:lang="en">e</skos:notation></rdf:Description>
   
   <rdf:Description rdf:about="http://fakeIRI.edu/terms/tactilebmf#i"><rdf:type rdf:resource="http://www.w3.org/2004/02/skos/core#Concept"/><skos:inScheme rdf:resource="http://fakeIRI.edu/terms/tactilebmf"/><skos:prefLabel xml:lang="en">spanner short form scoring</skos:prefLabel><skos:definition xml:lang="en">Chord symbols and melody are presented in paragraphs.</skos:definition><skos:scopeNote xml:lang="en">Used chiefly for popular and folk music, but music braille is used for the chord symbols. Also used to indicate that the music is in the Canadian melody chord system.</skos:scopeNote><skos:notation xml:lang="en">i</skos:notation></rdf:Description>
   
   <rdf:Description rdf:about="http://fakeIRI.edu/terms/tactilebmf#u"><rdf:type rdf:resource="http://www.w3.org/2004/02/skos/core#Concept"/><skos:inScheme rdf:resource="http://fakeIRI.edu/terms/tactilebmf"/><skos:prefLabel xml:lang="en">unknown</skos:prefLabel><skos:definition xml:lang="en">Braille music format is not known.</skos:definition><skos:notation xml:lang="en">u</skos:notation></rdf:Description>
   
   <rdf:Description rdf:about="http://fakeIRI.edu/terms/tactilebmf#l"><rdf:type rdf:resource="http://www.w3.org/2004/02/skos/core#Concept"/><skos:inScheme rdf:resource="http://fakeIRI.edu/terms/tactilebmf"/><skos:prefLabel xml:lang="en">vertical score</skos:prefLabel><skos:definition xml:lang="en">Parts are combined and written as chords.</skos:definition><skos:notation xml:lang="en">l</skos:notation></rdf:Description>
</rdf:RDF>