<?xml version="1.0" encoding="utf-8"?>
<rdf:RDF
   xmlns:dc="http://purl.org/dc/elements/1.1/"
   xmlns:dct="http://purl.org/dc/terms/"
   xmlns:rdf="http://www.w3.org/1999/02/22-rdf-syntax-ns#"
   xmlns:schema="https://schema.org/"
   xmlns:skos="http://www.w3.org/2004/02/skos/core#"
>
  <rdf:Description rdf:about="https://doi.org/10.6069/uwlswd.h5tb-zk94#a">
    <rdf:type rdf:resource="http://www.w3.org/2004/02/skos/core#Concept"/>
    <skos:inScheme rdf:resource="https://doi.org/10.6069/uwlswd.h5tb-zk94"/>
    <skos:prefLabel xml:lang="en">map</skos:prefLabel>
    <skos:definition xml:lang="en">Map</skos:definition>
    <skos:scopeNote xml:lang="en">Used for all cartographic materials except
         globes.</skos:scopeNote>
    <skos:notation xml:lang="en">a</skos:notation>
  </rdf:Description>
  <rdf:Description rdf:about="https://doi.org/10.6069/uwlswd.h5tb-zk94#h">
    <rdf:type rdf:resource="http://www.w3.org/2004/02/skos/core#Concept"/>
    <skos:inScheme rdf:resource="https://doi.org/10.6069/uwlswd.h5tb-zk94"/>
    <skos:prefLabel xml:lang="en">microform</skos:prefLabel>
    <skos:definition xml:lang="en">A generic term for any medium, transparent or opaque bearing
         microimages. A microimage is a unit (e.g., a page) of textual, graphic, or
         computer-generated material that is contained on aperture cards, microfiche, microfilm,
         micro-opaques, or other microformats and that is too small to be read without
         magnification.</skos:definition>
    <skos:scopeNote xml:lang="en">Microforms may be reproductions of existing textual or graphic
         materials or they may be original publications.</skos:scopeNote>
    <skos:notation xml:lang="en">h</skos:notation>
  </rdf:Description>
  <rdf:Description rdf:about="https://doi.org/10.6069/uwlswd.h5tb-zk94">
    <rdf:type rdf:resource="http://www.w3.org/2004/02/skos/core#ConceptScheme"/>
    <dct:type rdf:resource="http://purl.org/dc/dcmitype/Dataset"/>
    <dct:title xml:lang="en">All: category of material</dct:title>
    <dct:alternative xml:lang="en">MARC21 007/00 values for all material types expressed using
         RDF</dct:alternative>
    <dct:description xml:lang="en">Identifies the category of material.</dct:description>
    <schema:disambiguatingDescription>SKOS Concept Scheme for MARC 00X
         Values</schema:disambiguatingDescription>
    <dct:publisher rdf:resource="http://viaf.org/viaf/139541794"/>
    <dct:source rdf:resource="https://www.loc.gov/marc/bibliographic/bd007.html"/>
    <dct:source rdf:resource="http://marc21rdf.info"/>
    <dct:provenance rdf:resource="https://doi.org/10.6069/uwlswd.2e2b-y833"/>
    <dct:creator rdf:resource="http://viaf.org/viaf/139541794"/>
    <dct:contributor rdf:resource="http://viaf.org/viaf/151962300"/>
    <dct:issued>2024</dct:issued>
    <dc:contributor xml:lang="en">Metadata Management Associates</dc:contributor>
    <dc:language>en</dc:language>
    <dct:license rdf:resource="http://creativecommons.org/publicdomain/zero/1.0"/>
    <schema:version>1-0-0</schema:version>
    <dct:format rdf:resource="http://www.w3.org/ns/formats/RDF_XML"/>
    <dct:hasFormat rdf:resource="https://uwlib-cams.github.io/uwlswd_vocabs_marc_007/all_category_of_material/all_category_of_material.ttl"/>
    <dct:hasFormat rdf:resource="https://uwlib-cams.github.io/uwlswd_vocabs_marc_007/all_category_of_material/all_category_of_material.nt"/>
    <dct:hasFormat rdf:resource="https://uwlib-cams.github.io/uwlswd_vocabs_marc_007/all_category_of_material/all_category_of_material.jsonld"/>
    <dct:hasFormat rdf:resource="https://uwlib-cams.github.io/uwlswd_vocabs_marc_007/all_category_of_material/all_category_of_material.html"/>
  </rdf:Description>
  <rdf:Description rdf:about="https://doi.org/10.6069/uwlswd.h5tb-zk94#c">
    <rdf:type rdf:resource="http://www.w3.org/2004/02/skos/core#Concept"/>
    <skos:inScheme rdf:resource="https://doi.org/10.6069/uwlswd.h5tb-zk94"/>
    <skos:prefLabel xml:lang="en">electronic resource</skos:prefLabel>
    <skos:definition xml:lang="en">Involves a medium (usually digitized machine-readable data,
         program code, etc.) intended to be accessed, processed, or executed by a
         computer.</skos:definition>
    <skos:scopeNote xml:lang="en">Examples are programs, data files, image files, digitized audio
         and video tapes, etc.</skos:scopeNote>
    <skos:notation xml:lang="en">c</skos:notation>
  </rdf:Description>
  <rdf:Description rdf:about="https://doi.org/10.6069/uwlswd.h5tb-zk94#g">
    <rdf:type rdf:resource="http://www.w3.org/2004/02/skos/core#Concept"/>
    <skos:inScheme rdf:resource="https://doi.org/10.6069/uwlswd.h5tb-zk94"/>
    <skos:prefLabel xml:lang="en">projected graphic</skos:prefLabel>
    <skos:definition xml:lang="en">A two-dimensional representation intended to be projected
         without motion by means of an optical device.</skos:definition>
    <skos:scopeNote xml:lang="en">For example, a filmstrip, slide, or transparency (includes
         x-rays).</skos:scopeNote>
    <skos:notation xml:lang="en">g</skos:notation>
  </rdf:Description>
  <rdf:Description rdf:about="https://doi.org/10.6069/uwlswd.h5tb-zk94#v">
    <rdf:type rdf:resource="http://www.w3.org/2004/02/skos/core#Concept"/>
    <skos:inScheme rdf:resource="https://doi.org/10.6069/uwlswd.h5tb-zk94"/>
    <skos:prefLabel xml:lang="en">videorecording</skos:prefLabel>
    <skos:definition xml:lang="en">A recording on which visual images, usually in motion and
         accompanied by sound, have been registered.</skos:definition>
    <skos:scopeNote xml:lang="en">Designed for playback by means of a television receiver, or
         video monitor.</skos:scopeNote>
    <skos:notation xml:lang="en">v</skos:notation>
  </rdf:Description>
  <rdf:Description rdf:about="https://doi.org/10.6069/uwlswd.h5tb-zk94#d">
    <rdf:type rdf:resource="http://www.w3.org/2004/02/skos/core#Concept"/>
    <skos:inScheme rdf:resource="https://doi.org/10.6069/uwlswd.h5tb-zk94"/>
    <skos:prefLabel xml:lang="en">globe</skos:prefLabel>
    <skos:definition xml:lang="en">The model of a celestial body, usually the earth or the
         celestial sphere, depicted on the surface of a sphere.</skos:definition>
    <skos:notation xml:lang="en">d</skos:notation>
  </rdf:Description>
  <rdf:Description rdf:about="https://doi.org/10.6069/uwlswd.h5tb-zk94#t">
    <rdf:type rdf:resource="http://www.w3.org/2004/02/skos/core#Concept"/>
    <skos:inScheme rdf:resource="https://doi.org/10.6069/uwlswd.h5tb-zk94"/>
    <skos:prefLabel xml:lang="en">text</skos:prefLabel>
    <skos:definition xml:lang="en">Printed or manuscript language material that is accessible to
         the naked eye.</skos:definition>
    <skos:scopeNote xml:lang="en">E.g., a book, a pamphlet, a broadside.</skos:scopeNote>
    <skos:notation xml:lang="en">t</skos:notation>
  </rdf:Description>
  <rdf:Description rdf:about="https://doi.org/10.6069/uwlswd.h5tb-zk94#m">
    <rdf:type rdf:resource="http://www.w3.org/2004/02/skos/core#Concept"/>
    <skos:inScheme rdf:resource="https://doi.org/10.6069/uwlswd.h5tb-zk94"/>
    <skos:prefLabel xml:lang="en">motion picture</skos:prefLabel>
    <skos:definition xml:lang="en">A series of still pictures on film, with or without sound,
         designed to be projected in rapid succession to produce the optical effect of
         motion.</skos:definition>
    <skos:notation xml:lang="en">m</skos:notation>
  </rdf:Description>
  <rdf:Description rdf:about="https://doi.org/10.6069/uwlswd.h5tb-zk94#z">
    <rdf:type rdf:resource="http://www.w3.org/2004/02/skos/core#Concept"/>
    <skos:inScheme rdf:resource="https://doi.org/10.6069/uwlswd.h5tb-zk94"/>
    <skos:prefLabel xml:lang="en">unspecified</skos:prefLabel>
    <skos:definition xml:lang="en">Item is not identified by one of the other values or that its
         multiple physical forms are not being specifically denoted.</skos:definition>
    <skos:notation xml:lang="en">z</skos:notation>
  </rdf:Description>
  <rdf:Description rdf:about="https://doi.org/10.6069/uwlswd.h5tb-zk94#f">
    <rdf:type rdf:resource="http://www.w3.org/2004/02/skos/core#Concept"/>
    <skos:inScheme rdf:resource="https://doi.org/10.6069/uwlswd.h5tb-zk94"/>
    <skos:prefLabel xml:lang="en">tactile material</skos:prefLabel>
    <skos:definition xml:lang="en">Material intended to be read or interpreted by
         touch.</skos:definition>
    <skos:notation xml:lang="en">f</skos:notation>
  </rdf:Description>
  <rdf:Description rdf:about="https://doi.org/10.6069/uwlswd.h5tb-zk94#o">
    <rdf:type rdf:resource="http://www.w3.org/2004/02/skos/core#Concept"/>
    <skos:inScheme rdf:resource="https://doi.org/10.6069/uwlswd.h5tb-zk94"/>
    <skos:prefLabel xml:lang="en">kit</skos:prefLabel>
    <skos:definition xml:lang="en">A mixture of various components issued as a unit and intended
         primarily for instructional purposes. No one component is identifiable as the predominant
         component of the item.</skos:definition>
    <skos:scopeNote xml:lang="en">Examples are packages of assorted materials, such as a set of
         K-12 social studies curriculum material (books, workbooks, guides, activities, etc.), or
         packages of educational test materials (tests, answer sheets, scoring guides, score charts,
         interpretative manuals, etc.).</skos:scopeNote>
    <skos:notation xml:lang="en">o</skos:notation>
  </rdf:Description>
  <rdf:Description rdf:about="https://doi.org/10.6069/uwlswd.h5tb-zk94#k">
    <rdf:type rdf:resource="http://www.w3.org/2004/02/skos/core#Concept"/>
    <skos:inScheme rdf:resource="https://doi.org/10.6069/uwlswd.h5tb-zk94"/>
    <skos:prefLabel xml:lang="en">nonprojected graphic</skos:prefLabel>
    <skos:definition xml:lang="en">A two-dimensional pictorial representation whether opaque
         (e.g., print, photoprint, drawing) or transparent, but not intended to be projected for
         viewing (e.g., a photographic negative).</skos:definition>
    <skos:notation xml:lang="en">k</skos:notation>
  </rdf:Description>
  <rdf:Description rdf:about="https://doi.org/10.6069/uwlswd.h5tb-zk94#r">
    <rdf:type rdf:resource="http://www.w3.org/2004/02/skos/core#Concept"/>
    <skos:inScheme rdf:resource="https://doi.org/10.6069/uwlswd.h5tb-zk94"/>
    <skos:prefLabel xml:lang="en">remote-sensing image</skos:prefLabel>
    <skos:definition xml:lang="en">An image produced by a recording device that is not in physical
         or intimate contact with the object under study.</skos:definition>
    <skos:scopeNote xml:lang="en">This may be a map or other image that is obtained through
         various remote sensing devices such as cameras, computers, lasers, radio frequency
         receivers, radar systems, sonar, seismographs, gravimeters, magnetometers, and
         scintillation counters. When the image has cartographic or bibliographic information added,
         it is referred to as a remote-sensing map.</skos:scopeNote>
    <skos:notation xml:lang="en">r</skos:notation>
  </rdf:Description>
  <rdf:Description rdf:about="https://doi.org/10.6069/uwlswd.h5tb-zk94#q">
    <rdf:type rdf:resource="http://www.w3.org/2004/02/skos/core#Concept"/>
    <skos:inScheme rdf:resource="https://doi.org/10.6069/uwlswd.h5tb-zk94"/>
    <skos:prefLabel xml:lang="en">notated music</skos:prefLabel>
    <skos:definition xml:lang="en">Graphic, non-realized representations of musical works, both in
         printed and digitized manifestations.</skos:definition>
    <skos:scopeNote xml:lang="en">Includes musical scores and/or parts, diagrammatic
         representations, tablature, instructions for chance compositions, pictures or paintings
         intended as musical compositions, square note notation, klavirskribo, chant notation,
         neumes, braille, and other ways of representing the four components of musical sound:
         pitch, duration, timbre, and loudness. Notated music is often the means for communicating
         to the performer(s) how the musical work notated therein is to be realized in
         sound.</skos:scopeNote>
    <skos:notation xml:lang="en">q</skos:notation>
  </rdf:Description>
  <rdf:Description rdf:about="https://doi.org/10.6069/uwlswd.h5tb-zk94#s">
    <rdf:type rdf:resource="http://www.w3.org/2004/02/skos/core#Concept"/>
    <skos:inScheme rdf:resource="https://doi.org/10.6069/uwlswd.h5tb-zk94"/>
    <skos:prefLabel xml:lang="en">sound recording</skos:prefLabel>
    <skos:definition xml:lang="en">A storage medium containing recorded sound or a representation
         of a musical composition from which sound can be mechanically reproduced, such as a piano
         roll.</skos:definition>
    <skos:notation xml:lang="en">s</skos:notation>
  </rdf:Description>
</rdf:RDF>
