@prefix dc: <http://purl.org/dc/elements/1.1/> .
@prefix dct: <http://purl.org/dc/terms/> .
@prefix schema: <https://schema.org/> .
@prefix skos: <http://www.w3.org/2004/02/skos/core#> .

<https://doi.org/10.6069/uwlswd.h5tb-zk94#a> a skos:Concept ;
    skos:definition "Map"@en ;
    skos:inScheme <https://doi.org/10.6069/uwlswd.h5tb-zk94> ;
    skos:notation "a" ;
    skos:prefLabel "map"@en ;
    skos:scopeNote """Used for all cartographic materials except
         globes."""@en .

<https://doi.org/10.6069/uwlswd.h5tb-zk94#c> a skos:Concept ;
    skos:definition """Involves a medium (usually digitized machine-readable data,
         program code, etc.) intended to be accessed, processed, or executed by a
         computer."""@en ;
    skos:inScheme <https://doi.org/10.6069/uwlswd.h5tb-zk94> ;
    skos:notation "c" ;
    skos:prefLabel "electronic resource"@en ;
    skos:scopeNote """Examples are programs, data files, image files, digitized audio
         and video tapes, etc."""@en .

<https://doi.org/10.6069/uwlswd.h5tb-zk94#d> a skos:Concept ;
    skos:definition """The model of a celestial body, usually the earth or the
         celestial sphere, depicted on the surface of a sphere."""@en ;
    skos:inScheme <https://doi.org/10.6069/uwlswd.h5tb-zk94> ;
    skos:notation "d" ;
    skos:prefLabel "globe"@en .

<https://doi.org/10.6069/uwlswd.h5tb-zk94#f> a skos:Concept ;
    skos:definition """Material intended to be read or interpreted by
         touch."""@en ;
    skos:inScheme <https://doi.org/10.6069/uwlswd.h5tb-zk94> ;
    skos:notation "f" ;
    skos:prefLabel "tactile material"@en .

<https://doi.org/10.6069/uwlswd.h5tb-zk94#g> a skos:Concept ;
    skos:definition """A two-dimensional representation intended to be projected
         without motion by means of an optical device."""@en ;
    skos:inScheme <https://doi.org/10.6069/uwlswd.h5tb-zk94> ;
    skos:notation "g" ;
    skos:prefLabel "projected graphic"@en ;
    skos:scopeNote """For example, a filmstrip, slide, or transparency (includes
         x-rays)."""@en .

<https://doi.org/10.6069/uwlswd.h5tb-zk94#h> a skos:Concept ;
    skos:definition """A generic term for any medium, transparent or opaque bearing
         microimages. A microimage is a unit (e.g., a page) of textual, graphic, or
         computer-generated material that is contained on aperture cards, microfiche, microfilm,
         micro-opaques, or other microformats and that is too small to be read without
         magnification."""@en ;
    skos:inScheme <https://doi.org/10.6069/uwlswd.h5tb-zk94> ;
    skos:notation "h" ;
    skos:prefLabel "microform"@en ;
    skos:scopeNote """Microforms may be reproductions of existing textual or graphic
         materials or they may be original publications."""@en .

<https://doi.org/10.6069/uwlswd.h5tb-zk94#k> a skos:Concept ;
    skos:definition """A two-dimensional pictorial representation whether opaque
         (e.g., print, photoprint, drawing) or transparent, but not intended to be projected for
         viewing (e.g., a photographic negative)."""@en ;
    skos:inScheme <https://doi.org/10.6069/uwlswd.h5tb-zk94> ;
    skos:notation "k" ;
    skos:prefLabel "nonprojected graphic"@en .

<https://doi.org/10.6069/uwlswd.h5tb-zk94#m> a skos:Concept ;
    skos:definition """A series of still pictures on film, with or without sound,
         designed to be projected in rapid succession to produce the optical effect of
         motion."""@en ;
    skos:inScheme <https://doi.org/10.6069/uwlswd.h5tb-zk94> ;
    skos:notation "m" ;
    skos:prefLabel "motion picture"@en .

<https://doi.org/10.6069/uwlswd.h5tb-zk94#o> a skos:Concept ;
    skos:definition """A mixture of various components issued as a unit and intended
         primarily for instructional purposes. No one component is identifiable as the predominant
         component of the item."""@en ;
    skos:inScheme <https://doi.org/10.6069/uwlswd.h5tb-zk94> ;
    skos:notation "o" ;
    skos:prefLabel "kit"@en ;
    skos:scopeNote """Examples are packages of assorted materials, such as a set of
         K-12 social studies curriculum material (books, workbooks, guides, activities, etc.), or
         packages of educational test materials (tests, answer sheets, scoring guides, score charts,
         interpretative manuals, etc.)."""@en .

<https://doi.org/10.6069/uwlswd.h5tb-zk94#q> a skos:Concept ;
    skos:definition """Graphic, non-realized representations of musical works, both in
         printed and digitized manifestations."""@en ;
    skos:inScheme <https://doi.org/10.6069/uwlswd.h5tb-zk94> ;
    skos:notation "q" ;
    skos:prefLabel "notated music"@en ;
    skos:scopeNote """Includes musical scores and/or parts, diagrammatic
         representations, tablature, instructions for chance compositions, pictures or paintings
         intended as musical compositions, square note notation, klavirskribo, chant notation,
         neumes, braille, and other ways of representing the four components of musical sound:
         pitch, duration, timbre, and loudness. Notated music is often the means for communicating
         to the performer(s) how the musical work notated therein is to be realized in
         sound."""@en .

<https://doi.org/10.6069/uwlswd.h5tb-zk94#r> a skos:Concept ;
    skos:definition """An image produced by a recording device that is not in physical
         or intimate contact with the object under study."""@en ;
    skos:inScheme <https://doi.org/10.6069/uwlswd.h5tb-zk94> ;
    skos:notation "r" ;
    skos:prefLabel "remote-sensing image"@en ;
    skos:scopeNote """This may be a map or other image that is obtained through
         various remote sensing devices such as cameras, computers, lasers, radio frequency
         receivers, radar systems, sonar, seismographs, gravimeters, magnetometers, and
         scintillation counters. When the image has cartographic or bibliographic information added,
         it is referred to as a remote-sensing map."""@en .

<https://doi.org/10.6069/uwlswd.h5tb-zk94#s> a skos:Concept ;
    skos:definition """A storage medium containing recorded sound or a representation
         of a musical composition from which sound can be mechanically reproduced, such as a piano
         roll."""@en ;
    skos:inScheme <https://doi.org/10.6069/uwlswd.h5tb-zk94> ;
    skos:notation "s" ;
    skos:prefLabel "sound recording"@en .

<https://doi.org/10.6069/uwlswd.h5tb-zk94#t> a skos:Concept ;
    skos:definition """Printed or manuscript language material that is accessible to
         the naked eye."""@en ;
    skos:inScheme <https://doi.org/10.6069/uwlswd.h5tb-zk94> ;
    skos:notation "t" ;
    skos:prefLabel "text"@en ;
    skos:scopeNote "E.g., a book, a pamphlet, a broadside."@en .

<https://doi.org/10.6069/uwlswd.h5tb-zk94#v> a skos:Concept ;
    skos:definition """A recording on which visual images, usually in motion and
         accompanied by sound, have been registered."""@en ;
    skos:inScheme <https://doi.org/10.6069/uwlswd.h5tb-zk94> ;
    skos:notation "v" ;
    skos:prefLabel "videorecording"@en ;
    skos:scopeNote """Designed for playback by means of a television receiver, or
         video monitor."""@en .

<https://doi.org/10.6069/uwlswd.h5tb-zk94#z> a skos:Concept ;
    skos:definition """Item is not identified by one of the other values or that its
         multiple physical forms are not being specifically denoted."""@en ;
    skos:inScheme <https://doi.org/10.6069/uwlswd.h5tb-zk94> ;
    skos:notation "z" ;
    skos:prefLabel "unspecified"@en .

<https://doi.org/10.6069/uwlswd.h5tb-zk94> a skos:ConceptScheme ;
    dc:contributor "Metadata Management Associates"@en ;
    dc:language "en" ;
    dct:alternative """MARC21 007/00 values for all material types expressed using
         RDF"""@en ;
    dct:contributor <http://viaf.org/viaf/151962300> ;
    dct:creator <http://viaf.org/viaf/139541794> ;
    dct:description "Identifies the category of material."@en ;
    dct:format <http://www.w3.org/ns/formats/Turtle> ;
    dct:hasFormat <https://uwlib-cams.github.io/uwlswd_vocabs_marc_007/all_category_of_material/all_category_of_material.html>,
        <https://uwlib-cams.github.io/uwlswd_vocabs_marc_007/all_category_of_material/all_category_of_material.jsonld>,
        <https://uwlib-cams.github.io/uwlswd_vocabs_marc_007/all_category_of_material/all_category_of_material.nt>,
        <https://uwlib-cams.github.io/uwlswd_vocabs_marc_007/all_category_of_material/all_category_of_material.rdf> ;
    dct:issued "2024" ;
    dct:license <http://creativecommons.org/publicdomain/zero/1.0> ;
    dct:provenance <https://doi.org/10.6069/uwlswd.2e2b-y833#marc00Xvalues> ;
    dct:publisher <http://viaf.org/viaf/139541794> ;
    dct:source <http://marc21rdf.info>,
        <https://www.loc.gov/marc/bibliographic/bd007.html> ;
    dct:title "All: category of material"@en ;
    dct:type <http://purl.org/dc/dcmitype/Dataset> ;
    schema:disambiguatingDescription """SKOS Concept Scheme for MARC 00X
         Values"""@en ;
    schema:version "1-0-0" .

